<?xml version="1.0" encoding="UTF-8"?>
<rdf:RDF xml:base="http://inspire-registry.jrc.ec.europa.eu/registers/FCD/" xmlns:dct="http://purl.org/dc/terms/" xmlns:inspire="http://inspire-registry.jrc.ec.europa.eu/rdfschema/inspire-schema.rdf#" xmlns:rdf="http://www.w3.org/1999/02/22-rdf-syntax-ns#" xmlns:skos="http://www.w3.org/2004/02/skos/core#" xmlns:owl="http://www.w3.org/2002/07/owl#" xml:lang="en">
	<owl:Ontology rdf:about="http://inspire-registry.jrc.ec.europa.eu/registers/FCD/">
		<owl:imports rdf:resource="http://inspire-registry.jrc.ec.europa.eu/rdfschema/inspire-schema.rdf"/>
	</owl:Ontology>

    <skos:ConceptScheme rdf:about="http://inspire-registry.jrc.ec.europa.eu/registers/Themes/items">
		<!-- <owl:sameIndividualAs rdf:resource="http://www.eionet.europa.eu/gemet/inspire_themes" /> -->
        <skos:prefLabel>GEMET - INSPIRE themes, version 1.0</skos:prefLabel>
        <dct:title>GEMET - INSPIRE themes, version 1.0</dct:title>
        <dct:issued>2008-06-01</dct:issued>
    </skos:ConceptScheme>
	
	<!-- TODO verify version and publication date -->
	<skos:ConceptScheme rdf:about="http://inspire-registry.jrc.ec.europa.eu/registers/FCD/items">
		<skos:definition>The INSPIRE Feature Concept Dictionary (IFCD) acts as a common feature concept dictionary for all INSPIRE data specifications. The common feature concept dictionary contains terms and definitions required for specifying thematic spatial object types and it is main role is in particular to support the harmonisation effort and to identify conflicts between the specifications of the spatial object types in the different themes.</skos:definition>
		<dct:creator>European Commission, Joint Research Centre</dct:creator>
        <dct:issued>2010-01-19</dct:issued>
		<skos:prefLabel>INSPIRE - Feature Concept Dictionary, version 3</skos:prefLabel>
        <dct:title>INSPIRE - Feature Concept Dictionary, version 3</dct:title>
	</skos:ConceptScheme>
	
	<inspire:Theme rdf:about="http://inspire-registry.jrc.ec.europa.eu/registers/FCD/items/1">
		<!-- <owl:sameIndividualAs rdf:resource="http://www.eionet.europa.eu/gemet/theme_concepts?th=1&ns=5" /> -->
		<inspire:itemStatus>valid</inspire:itemStatus>
		<inspire:dateAccepted>2008-12-05T17:00:29.077+01:00</inspire:dateAccepted>
		<skos:prefLabel xml:lang="en">Coordinate reference systems</skos:prefLabel>
		<skos:definition xml:lang="en">Systems for uniquely referencing spatial information in space as a set of coordinates (x, y, z) and/or latitude and longitude and height, based on a geodetic horizontal and vertical datum.</skos:definition>
		<dct:description xml:lang="en">The theme establishes a structure for spatial referencing of features by coordinates. This topic shall link to appropriate standards for information technology and data where possible, and provide a framework for the development of sector-specific applications using geographic data.

ISO 19111 describes the conceptual schema and defines the description for a minimum data to two cases for which 1-, 2- and 3- dimensional coordinates reference system information shall be given. The first case is given by a coordinate reference system to which a set of coordinates is related. The second case consists of a coordinate operation (coordinate transformation, coordinate conversion, concatenated coordinate operation) to change coordinate values from one coordinate reference system to another.

There are no explicit accuracy numbers given in ISO 19111. We must consider that it has been developed for geographic information in general, but not for precise positioning. Spatial information may be referenced to the earth surface with an improving accuracy on the global scale for the future. Such high accuracy level may be required for some themes of the Directive, e.g., the trans-European railway transport network. Spatial referencing could no longer be considered as constant in time, if we reach the sub-centimetre level. We need additional parameters compared to ISO 19111 in that case, because that document considers changes in time of the coordinate reference only system through the “date of realisation”. This model is not suitable to describe continuous movements of the spatial reference. Kinematic models or so-called “loading models” are examples to incorporate such dynamics. A re-iteration of accuracy aspects may be needed, if specifications for Annex I and II are ready.

The spatial referencing is usually referred to selected points of the earth surface. Such point are, e.g., given by geodetic markers, stations performing permanent satellite observations, levelling benchmarks, or tide gauges. As soon as the marker coordinates are given, they provide a direct access to the realisation of the coordinate reference system.</dct:description>
		<skos:prefLabel xml:lang="bg">Координатни справочни системи</skos:prefLabel>
		<skos:definition xml:lang="bg">Системи за пространствена информация, предназначена изключително за справочни цели, представена в пространството с координати (x, y, z) и/или ширина, дължина и височина, на базата на геодезични хоризонтални и вертикални данни.</skos:definition>
		<skos:prefLabel xml:lang="cs">Souřadnicové referenční systémy</skos:prefLabel>
		<skos:definition xml:lang="cs">Systémy umožňující jednoznačné přiřazení polohy prostorovým informacím pomocí souboru souřadnic (x, y, z) nebo zeměpisné šířky, zeměpisné délky a výšky, vycházející z údajů polohových a výškových geodetických systémů.</skos:definition>
		<skos:prefLabel xml:lang="da">Koordinatsystemer</skos:prefLabel>
		<skos:definition xml:lang="da">Systemer for entydig rumlig stedfæstelse af geografiske informationer ved hjælp af et sæt koordinater (x, y, z) og/eller længde, bredde og højde, baseret på et horisontalt og vertikalt geodætisk datum.</skos:definition>
		<skos:prefLabel xml:lang="de">Koordinatenreferenzsysteme</skos:prefLabel>
		<skos:definition xml:lang="de">Systeme zur eindeutigen räumlichen Referenzierung von Geodaten anhand eines Koordinatensatzes (x, y, z) und/oder Angaben zu Breite, Länge und Höhe auf der Grundlage eines geodätischen horizontalen und vertikalen Datums.</skos:definition>
		<skos:prefLabel xml:lang="el">Συστήματα συντεταγμένων</skos:prefLabel>
		<skos:definition xml:lang="el">Συστήματα για μονοσήμαντη αναφορά χωρικών πληροφοριών στον χώρο, ως σύνολο συντεταγμένων (x,y,z) ή/και γεωγραφικό πλάτος και μήκος και ύψος, με βάση γεωδαιτικό οριζόντιο και κατακόρυφο σύστημα αναφοράς (datum).</skos:definition>
		<skos:prefLabel xml:lang="es">Sistemas de coordenadas de referencia</skos:prefLabel>
		<skos:definition xml:lang="es">Sistemas para referenciar de forma unívoca la información espacial en el espacio como una serie de coordenadas (x, y, z) y/o latitud y longitud y altura, basándose en un punto de referencia geodésico horizontal y vertical.</skos:definition>
		<skos:prefLabel xml:lang="et">Koordinaatsüsteemid</skos:prefLabel>
		<skos:definition xml:lang="et">Süsteemid, milles ruumiandmete asukoht ruumis määratakse üheselt koordinaatide hulgaga (x, y, z) ja/või geodeetilisel referents- ja kõrgussüsteemil põhineva laiuse, pikkuse ja kõrgusega.</skos:definition>
		<skos:prefLabel xml:lang="fi">Koordinaattijärjestelmät</skos:prefLabel>
		<skos:definition xml:lang="fi">Järjestelmät, joissa paikkatietoihin liittyvä sijainti esitetään yksikäsitteisesti koordinaattien (x, y, z) ja/tai maantieteellisten pituus- ja leveysasteiden sekä korkeuden avulla ja jotka perustuvat horisontaalisiin ja vertikaalisiin geodeettisiin vertausjärjestelmiin.</skos:definition>
		<skos:prefLabel xml:lang="fr">Référentiels de coordonnées</skos:prefLabel>
		<skos:definition xml:lang="fr">Systèmes de référencement unique des informations géographiques dans l'espace sous forme d'une série de coordonnées (x, y, z) et/ou la latitude et la longitude et l'altitude, en se fondant sur un point géodésique horizontal et vertical.</skos:definition>
		<skos:prefLabel xml:lang="hu">Koordinátarendszerek</skos:prefLabel>
		<skos:definition xml:lang="hu">Olyan rendszerek, amelyek a térinformáció térbeli helyzetét koordinátákkal (x, y, z) és/vagy vízszintes és függőleges geodéziai adatokon alapuló földrajzi szélességgel, hosszúsággal és magassággal adják meg.</skos:definition>
		<skos:prefLabel xml:lang="it">Sistemi di coordinate</skos:prefLabel>
		<skos:definition xml:lang="it">Sistemi per referenziare in maniera univoca le informazioni territoriali nello spazio mediante un sistema di coordinate (x, y, z) e/o latitudine e longitudine e quota, sulla base di un dato geodetico orizzontale e verticale.</skos:definition>
		<skos:prefLabel xml:lang="lt">Koordinačių atskaitos sistemos</skos:prefLabel>
		<skos:definition xml:lang="lt">Vienareikšmio erdvinės informacijos nurodymo erdvėje naudojant koordinačių (x, y, z) derinį ir (arba) platumą, ilgumą bei aukštį sistemos, pagrįstos geodezinės horizontaliosios ir vertikaliosios atskaitos duomenimis.</skos:definition>
		<skos:prefLabel xml:lang="lv">Koordinātu atskaites sistēmas</skos:prefLabel>
		<skos:definition xml:lang="lv">Sistēmas viennozīmīgai telpiskās informācijas atskaišu norādīšanai telpā ar koordinātu kopu (x, y, z) un/vai platumu, garumu un augstumu, izmantojot ģeodēziskos horizontālos un vertikālos datus.</skos:definition>
		
		<skos:prefLabel xml:lang="mt">Sistemi ta' referenza ta' koordinati</skos:prefLabel>
		<skos:definition xml:lang="mt">Sistemi biex issir referenza unika ta' informazzjoni ġeografika fl-ispazju bħala sett ta' koordinati (x,y,z) u/jew latitudni u lonġitudni u altitudni, ibbażati fuq datum ġeodetiku orizzontali u vertikali.</skos:definition>		
		
		<skos:prefLabel xml:lang="nl">Systemen voor verwijzing door middel van coördinaten</skos:prefLabel>
		<skos:definition xml:lang="nl">Systemen om aan ruimtelijke informatie een unieke reeks coördinaten (x, y,z) en/of breedte, lengte en hoogte toe te kennen, gebaseerd op een horizontaal en verticaal geodetische datum.</skos:definition>
		<skos:prefLabel xml:lang="pl">Systemy odniesienia za pomocą współrzędnych</skos:prefLabel>
		<skos:definition xml:lang="pl">Systemy dla jednoznacznego przestrzennego odnoszenia informacji przestrzennej za pomocą współrzędnych x, y, z lub za pomocą szerokości, długości lub wysokości na podstawie geodezyjnego poziomego i pionowego układu odniesienia.</skos:definition>
		<skos:prefLabel xml:lang="pt">Sistemas de referencia</skos:prefLabel>
		<skos:definition xml:lang="pt">Sistemas para referenciar de forma única a informação geográfica no espaço sob a forma de um conjunto de coordenadas (x, y, z) e/ou latitude e longitude e altitude, com base num datum geodésico horizontal e vertical.</skos:definition>
		<skos:prefLabel xml:lang="ro">Sisteme de coordonate de referinţă</skos:prefLabel>
		<skos:definition xml:lang="ro">Sisteme de referinţă unică în spaţiu a informaţiilor spaţiale, alcătuite dintr-un set de coordonate (x, y, z) şi/sau latitudine şi longitudine şi altitudine, bazate pe un datum orizontal şi pe unul vertical.</skos:definition>
		<skos:prefLabel xml:lang="sk">Súradnicové referenčné systémy</skos:prefLabel>
		<skos:definition xml:lang="sk">Systémy pre jednotne referenčné priestorové informácie v priestore v podobe množiny súradníc (x, y, z) a/alebo zemepisnej šírky, dĺžky a výšky založených na geodetickom horizontálnom a vertikálnom východzom bode.</skos:definition>
		<skos:prefLabel xml:lang="sl">Referenčni koordinatni sistemi</skos:prefLabel>
		<skos:definition xml:lang="sl">Sistemi za izključno navajanje prostorskih informacij v prostoru v obliki niza koordinat (x, y, z) in/ali širine in dolžine ter višine, ki temeljijo na horizontalnem in vertikalnem geodetskem podatku.</skos:definition>
		<skos:prefLabel xml:lang="sv">Referenskoordinatsystem</skos:prefLabel>
		<skos:definition xml:lang="sv">System för att entydigt lägesbestämma rumslig information i rummet som en uppsättning koordinater (x, y, z) och/ eller som latitud, longitud och höjd, på grundval av ett geodetiskt horisontellt och vertikalt datum.</skos:definition>
		<!--
		<skos:prefLabel xml:lang="el">SAMPLE ALTERNATIVE EXPRESSION - αναφορά</skos:prefLabel>
		<skos:definition xml:lang="el">Συστήματα συντεταγμένων</skos:definition>
		<dct:description xml:lang="el">Συστήματα για μονοσήμαντη αναφορά χωρικών πληροφοριών στον χώρο, ως σύνολο συντεταγμένων (x,y,z) ή/και γεωγραφικό πλάτος και μήκος και ύψος, με βάση γεωδαιτικό οριζόντιο και κατακόρυφο σύστημα αναφοράς (datum).</dct:description>
		-->
		<skos:inScheme rdf:resource="http://inspire-registry.jrc.ec.europa.eu/registers/Themes/items"/>
	</inspire:Theme>
	<inspire:Theme rdf:about="http://inspire-registry.jrc.ec.europa.eu/registers/FCD/items/2">
		<!-- <owl:sameIndividualAs rdf:resource="http://www.eionet.europa.eu/gemet/theme_concepts?th=2&ns=5" /> -->
		<inspire:itemStatus>valid</inspire:itemStatus>
		<inspire:dateAccepted>2008-12-05T17:00:29.141+01:00</inspire:dateAccepted>
		<skos:prefLabel xml:lang="en">Geographical grid systems</skos:prefLabel>
		<skos:definition xml:lang="en">Harmonised multi-resolution grid with a common point of origin and standardised location and size of grid cells.</skos:definition>
		<dct:description xml:lang="en">Geographical grids are an agreed, defined and harmonised grid net for Pan-Europe with standardised location and size of grid cells. Examples of cell sizes could be 10x10 m, 100x100 m, 1x1 km, 16x16 km. A good candidate for the INSPIRE-focused Pan-European grid has been proposed as a result of the Workshop on “European Reference Grids”.

The grid – proposed as Pan_European standard – is based on the ETRS89 Lambert Azimuthal Equal Area coordinate reference system with the centre of the projection at the point N 52o, E 10o. The grid is defined as hierarchical one in metric coordinates in power of 10.

The detail description of the proposed grid is available at the Proceedings of the Workshop on the European Reference Grids, EUR Report 21494 EN, 2005. The Proposal for a European Grid System is presented from page 39 to 46 of that document.

Other grids could be also used, however they need a lot of harmonisation work, as well as a number of conversion tools. Some international organisations, like WMO, perform their operations, using their own and purpose-oriented grid construction.</dct:description>
		<skos:prefLabel xml:lang="bg">Географски координатни системи</skos:prefLabel>
		<skos:definition xml:lang="bg">Хармонизирана сложна координатна система с обща начална точка и стандартизирано разположение и размер на квадрантите на координатната система.</skos:definition>
		<skos:prefLabel xml:lang="cs">Zeměpisné soustavy souřadnicových sítí</skos:prefLabel>
		<skos:definition xml:lang="cs">Harmonizovaná souřadnicová síť s víceúrovňovým rozlišením, normalizovanou polohou a velikostí buněk souřadnicové sítě, a společným vztažným bodem.</skos:definition>
		<skos:prefLabel xml:lang="da">Geografiske kvadratnetsystemer</skos:prefLabel>
		<skos:definition xml:lang="da">Et harmoniseret kvadratnet med flere cellestørrelser samt fælles nulpunkt og standardiseret cellelokalisering og -størrelse.</skos:definition>
		<skos:prefLabel xml:lang="de">Geografische Gittersysteme</skos:prefLabel>
		<skos:definition xml:lang="de">Harmonisiertes Gittersystem mit Mehrfachauflösung, gemeinsamem Ursprungspunkt und standardisierter Lokalisierung und Größe der Gitterzellen.</skos:definition>
		<skos:prefLabel xml:lang="el">Συστήματα γεωγραφικού καννάβου</skos:prefLabel>
		<skos:definition xml:lang="el">Εναρμονισμένος κάνναβος πολλαπλής ανάλυσης με ενιαίο σημείο αφετηρίας και τυποποιημένη θέση και μέγεθος των φατνίων του καννάβου.</skos:definition>
		<skos:prefLabel xml:lang="es">Sistema de cuadrículas geográficas</skos:prefLabel>
		<skos:definition xml:lang="es">Cuadrículas armonizadas multirresolución con un punto de origen común y con ubicación y tamaños de cuadrícula normalizados.</skos:definition>
		<skos:prefLabel xml:lang="et">Geograafilised ruutvõrgud</skos:prefLabel>
		<skos:definition xml:lang="et">Ühtlustatud, ühise lähtepunktiga ning võrguruutude standardse paigutuse ja suurusega mitmetasandiline ruutvõrk.</skos:definition>
		<skos:prefLabel xml:lang="fi">Paikannusruudustot</skos:prefLabel>
		<skos:definition xml:lang="fi">Yhdenmukaistettu monitasoinen ruudukko, jossa on yhteinen lähtöpiste ja standardoitu yksittäisen ruudun sijainti ja koko.</skos:definition>
		<skos:prefLabel xml:lang="fr">Systèmes de maillage géographique</skos:prefLabel>
		<skos:definition xml:lang="fr">Grille multi-résolution harmonisée avec un point d'origine commun et une localisation ainsi qu'une taille des cellules harmonisées.</skos:definition>
		<skos:prefLabel xml:lang="hu">Földrajzi rácsrendszerek</skos:prefLabel>
		<skos:definition xml:lang="hu">Harmonizált több felbontású rács közös kiindulóponttal és egységesített rácscella-helymeghatározással és -mérettel.</skos:definition>
		<skos:prefLabel xml:lang="it">Sistemi di griglie geografiche</skos:prefLabel>
		<skos:definition xml:lang="it">Griglia multi-risoluzione armonizzata con un punto di origine comune e un posizionamento e una dimensione standard delle celle.</skos:definition>
		<skos:prefLabel xml:lang="lt">Geografinio tinklelio sistemos</skos:prefLabel>
		<skos:definition xml:lang="lt">Suderintas kintamos skiriamosios gebos tinklelis su bendru atskaitos tašku ir standartizuota tinklelio langelių lokacija bei dydžiu.</skos:definition>
		<skos:prefLabel xml:lang="lv">Ģeogrāfisko koordinātu tīklu sistēmas</skos:prefLabel>
		<skos:definition xml:lang="lv">Saskaņots daudzpakāpju izšķiršanas koordinātu tīkls ar kopēju sākumpunktu un standartizētu tīkla šūnu atrašanās vietu un izmēru.</skos:definition>
		
		<skos:prefLabel xml:lang="mt">Sistemi ta' grilji ġeografiċi</skos:prefLabel>
		<skos:definition xml:lang="mt">Grilja multi-risoluzzjoni armonizzata b'punt ta' oriġini komuni u pożizzjoni u daqs taċ-ċelluli tal-grilja standardizzati.</skos:definition>		
		
		<skos:prefLabel xml:lang="nl">Geografisch rastersysteem</skos:prefLabel>
		<skos:definition xml:lang="nl">Geharmoniseerde multiresolutieraster met een gemeenschappelijk beginpunt en gestandaardiseerde plaats en grootte van de gridcellen.</skos:definition>
		<skos:prefLabel xml:lang="pl">Systemy siatek geograficznych</skos:prefLabel>
		<skos:definition xml:lang="pl">Zharmonizowana wielorozdzielcza siatka o wspólnym punkcie początkowym i znormalizowanym położeniu oraz wielkości pól siatki.</skos:definition>
		<skos:prefLabel xml:lang="pt">Sistemas de quadrículas geográficas</skos:prefLabel>
		<skos:definition xml:lang="pt">Quadrícula harmonizada multi-resolução com um ponto de origem comum e localização e dimensão normalizadas das células.</skos:definition>
		<skos:prefLabel xml:lang="ro">Sisteme de caroiaj geografic</skos:prefLabel>
		<skos:definition xml:lang="ro">Caroiaj multirezoluţie armonizat, având un punct de origine comun, precum şi localizare şi mărime standardizate ale celulelor.</skos:definition>
		<skos:prefLabel xml:lang="sk">Geografické systémy sietí</skos:prefLabel>
		<skos:definition xml:lang="sk">Harmonizovaná sieť s viacúrovňovým rozlíšením so spoločným počiatočným bodom a štandardizovanou polohou a veľkosťou buniek siete.</skos:definition>
		<skos:prefLabel xml:lang="sl">Geografska koordinatna mreža</skos:prefLabel>
		<skos:definition xml:lang="sl">Usklajena večločljivostna mreža s skupno točko izvora in standardizirano lokacijo ter velikostjo mrežnih celic.</skos:definition>
		<skos:prefLabel xml:lang="sv">Geografiska rutnätssystem</skos:prefLabel>
		<skos:definition xml:lang="sv">Harmoniserade rutnät med flera upplösningar, gemensam utgångspunkt och standardiserad placering och storlek på rutorna.</skos:definition>
		<!--
		<skos:prefLabel xml:lang="el">SAMPLE ALTERNATIVE EXPRESSION - αναφορά</skos:prefLabel>
		<skos:definition xml:lang="el">Συστήματα συντεταγμένων</skos:definition>
		<dct:description xml:lang="el">Συστήματα για μονοσήμαντη αναφορά χωρικών πληροφοριών στον χώρο, ως σύνολο συντεταγμένων (x,y,z) ή/και γεωγραφικό πλάτος και μήκος και ύψος, με βάση γεωδαιτικό οριζόντιο και κατακόρυφο σύστημα αναφοράς (datum).</dct:description>
		-->
		<skos:inScheme rdf:resource="http://inspire-registry.jrc.ec.europa.eu/registers/Themes/items"/>
	</inspire:Theme>
	<inspire:Theme rdf:about="http://inspire-registry.jrc.ec.europa.eu/registers/FCD/items/10">
		<!-- <owl:sameIndividualAs rdf:resource="http://www.eionet.europa.eu/gemet/theme_concepts?th=10&ns=5" /> -->
		<inspire:itemStatus>valid</inspire:itemStatus>
		<inspire:dateAccepted>2008-12-05T17:00:29.621+01:00</inspire:dateAccepted>
		<skos:prefLabel xml:lang="en">Elevation</skos:prefLabel>
		<skos:definition xml:lang="en">Digital elevation models for land, ice and ocean surface. Includes terrestrial elevation, bathymetry and shoreline.</skos:definition>
		<dct:description xml:lang="en">The theme includes:
• Terrestrial elevation, generally represented as
   - the terrain data, ground surface topography, called Digital Terrain Model describing the threedimensional shape of the Earth's surface
   - the surface data, named Digital Elevation Model, including the three dimensional shape of every feature placed on the soil (buildings, bridges, trees, ...).
• Bathymetry, e.g. a gridded bottom model

The height will be according to a common vertical coordinate reference system. The current one is European Vertical Reference System 2000 (EVRS), ) but EVRS 2007 is under development and might be taken into account or mentioned (cf. resolutions of the EUREF Symposium in London, 06-09 June 2007)</dct:description>
		<skos:prefLabel xml:lang="bg">Релеф</skos:prefLabel>
		<skos:definition xml:lang="bg">Цифрови релефни модели за земната, ледената и океанската повърхност. Включва земен релеф, батиметрия и брегова линия.</skos:definition>
		<skos:prefLabel xml:lang="cs">Nadmořská výška</skos:prefLabel>
		<skos:definition xml:lang="cs">Digitální výškový model pevniny, povrchu ledovců a oceánů. Zahrnuje nadmořské výšky pevnin, vodní hloubky a pobřežní čáru.</skos:definition>
		<skos:prefLabel xml:lang="da">Højde</skos:prefLabel>
		<skos:definition xml:lang="da">Digitale højdemodeller for land, is og havoverflade. Omfatter landhøjder, havdybder og kystlinje.</skos:definition>
		<skos:prefLabel xml:lang="de">Höhe</skos:prefLabel>
		<skos:definition xml:lang="de">Digitale Höhenmodelle für Land-, Eis- und Meeresflächen. Dazu gehören Geländemodell, Tiefenmessung und Küstenlinie.</skos:definition>
		<skos:prefLabel xml:lang="el">Υψομετρία</skos:prefLabel>
		<skos:definition xml:lang="el">Ψηφιακά υψομετρικά μοντέλα για χερσαίες εκτάσεις, εκτάσεις καλυπτόμενες από πάγους και ωκεανούς. Περιλαμβάνονται, εν προκειμένω, η χερσαία υψομετρία, η βαθυμετρία και οι ακτογραμμές.</skos:definition>
		<skos:prefLabel xml:lang="es">Elevaciones</skos:prefLabel>
		<skos:definition xml:lang="es">Modelos digitales de elevaciones para las superficies de tierra, hielo y mar. Se incluirán la altimetría, la batimetría y la línea de costa.</skos:definition>
		<skos:prefLabel xml:lang="et">Kõrgused</skos:prefLabel>
		<skos:definition xml:lang="et">Maa- ja jääpinna ning ookeani põhja digitaalsed reljeefimudelid. Hõlmab maapinna ja veekogude põhja reljeefi ning kaldajooni.</skos:definition>
		<skos:prefLabel xml:lang="fi">Korkeus</skos:prefLabel>
		<skos:definition xml:lang="fi">Digitaaliset maan-, jään- ja merenpintaa kuvaavat korkeusmallit. Sisältää maanpinnan korkeussuhteet, syvyystiedot ja rantaviivan.</skos:definition>
		<skos:prefLabel xml:lang="fr">Altitude</skos:prefLabel>
		<skos:definition xml:lang="fr">Modèles numériques pour l'altitude des surfaces terrestres, glaciaires et océaniques. Comprend l'altitude terrestre, la bathymétrie et la ligne de rivage.</skos:definition>
		<skos:prefLabel xml:lang="hu">Domborzat</skos:prefLabel>
		<skos:definition xml:lang="hu">Digitális domborzati modellek a szárazföldi, jéggel borított és óceáni felszínre. Ide tartozik a felszíni és víz alatti domborzat és a partvonal.</skos:definition>
		<skos:prefLabel xml:lang="it">Elevazione</skos:prefLabel>
		<skos:definition xml:lang="it">Modelli digitali di elevazione per superfici emerse, ghiacci e superfici oceaniche. La voce comprende l’altitudine terrestre, la batimetria e la linea di costa.</skos:definition>
		<skos:prefLabel xml:lang="lt">Aukštis</skos:prefLabel>
		<skos:definition xml:lang="lt">Sausumos, ledo ir vandenyno paviršių skaitmeniniai aukščio modeliai. Tai apima sausumos aukštį, batimetriją ir pakrantės liniją.</skos:definition>
		<skos:prefLabel xml:lang="lv">Augstums</skos:prefLabel>
		<skos:definition xml:lang="lv">Digitāli augstuma modeļi zemes, ledus un jūras virsmai. Tie ietver arī sauszemes reljefu, dziļumu un krasta līniju.</skos:definition>
		
		<skos:prefLabel xml:lang="mt">Elevazzjoni</skos:prefLabel>
		<skos:definition xml:lang="mt">Mudelli ta' elevazzjoni diġitali għall-art, is-silġ u l-wiċċ ta' l-oċean. Tinkludi l-elevazzjoni ta' l-art, il-batimetrija u l-linja tal-kosta.</skos:definition>		
		
		<skos:prefLabel xml:lang="nl">Hoogte</skos:prefLabel>
		<skos:definition xml:lang="nl">Digitale hoogtemodellen voor land-, ijs- en oceaanoppervlakken, inclusief landhoogte, bathymetrie en kustlijn.</skos:definition>
		<skos:prefLabel xml:lang="pl">Ukształtowanie terenu</skos:prefLabel>
		<skos:definition xml:lang="pl">Cyfrowe modele wysokościowe powierzchni lądu, lodu i oceanu. Obejmuje również wysokość topograficzną terenu, batymetrię oraz linię brzegową.</skos:definition>
		<skos:prefLabel xml:lang="pt">Altitude</skos:prefLabel>
		<skos:definition xml:lang="pt">Modelos digitais de terreno aplicáveis às superfícies terrestre, gelada e oceânica. Inclui a elevação terrestre, a batimetria e a linha costeira.</skos:definition>
		<skos:prefLabel xml:lang="ro">Elevaţie</skos:prefLabel>
		<skos:definition xml:lang="ro">Modele digitale de elevaţii ale suprafeţelor terestre, de gheaţă sau oceanice. Include altimetria, batimetria şi linia de coastă.</skos:definition>
		<skos:prefLabel xml:lang="sk">Výška</skos:prefLabel>
		<skos:definition xml:lang="sk">Digitálne výškové modely zemského povrchu, ľadovcov a hladín oceánov. Patria sem pevninové vyvýšeniny, batymetria a pobrežná čiara.</skos:definition>
		<skos:prefLabel xml:lang="sl">Digitalni model višin</skos:prefLabel>
		<skos:definition xml:lang="sl">Digitalni model višin za kopensko, zaledenelo in oceansko površino. Vključuje nadmorske višine, batimetrijo in obalne mreže.</skos:definition>
		<skos:prefLabel xml:lang="sv">Höjd</skos:prefLabel>
		<skos:definition xml:lang="sv">Digitala höjdmodeller för mark-, is- och havsyta. Inbegriper höjdförhållanden på land, batymetri samt kustlinje.</skos:definition>
		<!--
		<skos:prefLabel xml:lang="el">SAMPLE ALTERNATIVE EXPRESSION - αναφορά</skos:prefLabel>
		<skos:definition xml:lang="el">Συστήματα συντεταγμένων</skos:definition>
		<dct:description xml:lang="el">Συστήματα για μονοσήμαντη αναφορά χωρικών πληροφοριών στον χώρο, ως σύνολο συντεταγμένων (x,y,z) ή/και γεωγραφικό πλάτος και μήκος και ύψος, με βάση γεωδαιτικό οριζόντιο και κατακόρυφο σύστημα αναφοράς (datum).</dct:description>
		-->
		<skos:inScheme rdf:resource="http://inspire-registry.jrc.ec.europa.eu/registers/Themes/items"/>
	</inspire:Theme>
	<inspire:Theme rdf:about="http://inspire-registry.jrc.ec.europa.eu/registers/FCD/items/11">
		<!-- <owl:sameIndividualAs rdf:resource="http://www.eionet.europa.eu/gemet/theme_concepts?th=11&ns=5" /> -->
		<inspire:itemStatus>valid</inspire:itemStatus>
		<inspire:dateAccepted>2008-12-05T17:00:29.675+01:00</inspire:dateAccepted>
		<skos:prefLabel xml:lang="en">Land cover</skos:prefLabel>
		<skos:definition xml:lang="en">Physical and biological cover of the earth's surface including artificial surfaces, agricultural areas, forests, (semi-)natural areas, wetlands, water bodies.</skos:definition>
		<dct:description xml:lang="en">Land cover data is a physical or biological description of the earth surface. In this way it is different from the land use data (Annex III, theme number 4), dedicated to the description of the use of the Earth surface.
Land cover information has to be homogenous and comparable between different locations in Europe, based on the infrastructures for Land Cover information created by the Member States (if existing), and made available and maintained at the most appropriate level.

DG ENV among other DGs, together with 37 participating countries are financing and implementing the European multi-annual land cover database, within the framework of the GMES precursor Fast Track Service on Land Management and as the result of the users’ requirements at national and European levels.</dct:description>
		<skos:prefLabel xml:lang="bg">Земна покривка</skos:prefLabel>
		<skos:definition xml:lang="bg">Физическа или биологична покривка на земната повърхност, включително изкуствени повърхности, селскостопански райони, гори, (полу-) естествени райони, влажни зони, водни маси.</skos:definition>
		<skos:prefLabel xml:lang="cs">Krajinný pokryv</skos:prefLabel>
		<skos:definition xml:lang="cs">Fyzický a biologický pokryv zemského povrchu, včetně uměle vytvořených ploch, zemědělských oblastí, lesů, přirozených a částečně přirozených oblastí, mokřadů, vodních těles.</skos:definition>
		<skos:prefLabel xml:lang="da">Arealdække</skos:prefLabel>
		<skos:definition xml:lang="da">Jordens fysiske og biologiske overflade, herunder kunstige overflader, landbrugsarealer, skove, (halv-)naturlige områder, vådområder, vandområder.</skos:definition>
		<skos:prefLabel xml:lang="de">Bodenbedeckung</skos:prefLabel>
		<skos:definition xml:lang="de">Physische und biologische Bedeckung der Erdoberfläche, einschließlich künstlicher Flächen, landwirtschaftlicher Flächen, Wäldern, natürlicher (naturnaher) Gebiete, Feuchtgebieten und Wasserkörpern.</skos:definition>
		<skos:prefLabel xml:lang="el">Κάλυψη γης</skos:prefLabel>
		<skos:definition xml:lang="el">Φυσική και βιολογική κάλυψη της γήινης επιφάνειας, όπου συμπεριλαμβάνονται τεχνητές εκτάσεις, γεωργικές εκτάσεις, δάση, (ημι-)φυσικές εκτάσεις, υγρότοποι, υδατικά συστήματα.</skos:definition>
		<skos:prefLabel xml:lang="es">Cubierta terrestre</skos:prefLabel>
		<skos:definition xml:lang="es">Cubierta física y biológica de la superficie de la tierra, incluidas las superficies artificiales, las zonas agrarias, los bosques, las zonas naturales o seminaturales, los humedales, las láminas de agua.</skos:definition>
		<skos:prefLabel xml:lang="et">Maakate</skos:prefLabel>
		<skos:definition xml:lang="et">Maapinna elutust või elusainest kate, sealhulgas tehislikud pinnakatted, põllumajandusalad, metsad, (pool-)looduslikud alad, märgalad ning veekogud.</skos:definition>
		<skos:prefLabel xml:lang="fi">Maanpeite</skos:prefLabel>
		<skos:definition xml:lang="fi">Maapallon pinnan fysikaalinen ja biologinen peite, mukaan luettuina keinotekoiset peitteet, maatalousalueet, metsät, (osaksi) luonnontilassa olevat alueet, kosteikot ja vesistöt.</skos:definition>
		<skos:prefLabel xml:lang="fr">Occupation des terres</skos:prefLabel>
		<skos:definition xml:lang="fr">Couverture physique et biologique de la surface terrestre, y compris les surfaces artificielles, les zones agricoles, les forêts, les zones (semi-)naturelles, les zones humides et les masses d'eau.</skos:definition>
		<skos:prefLabel xml:lang="hu">A felszín borítása</skos:prefLabel>
		<skos:definition xml:lang="hu">A Föld felszínének fizikai és biológiai borítása, beleértve a mesterséges felszínt, a mezőgazdasági területeket, erdőket, a (félig) természetes területeket, a vizes élőhelyeket és a víztesteket.</skos:definition>
		<skos:prefLabel xml:lang="it">Copertura del suolo</skos:prefLabel>
		<skos:definition xml:lang="it">Copertura fisica e biologica della superficie terrestre comprese le superfici artificiali, le zone agricole, i boschi e le foreste, le aree (semi)naturali, le zone umide, i corpi idrici.</skos:definition>
		<skos:prefLabel xml:lang="lt">Žemės danga</skos:prefLabel>
		<skos:definition xml:lang="lt">Fizinė ir biologinė žemės paviršiaus danga, įskaitant dirbtinius paviršius, žemės ūkio plotus, miškus, (pusiau) natūralius plotus, šlapžemes, vandens telkinius.</skos:definition>
		<skos:prefLabel xml:lang="lv">Zemes virsma</skos:prefLabel>
		<skos:definition xml:lang="lv">Zemes virsmas fiziskais un bioloģiskais segums, tostarp mākslīgu virsmu, lauksaimniecības teritoriju, mežu, (daļēji) dabisku platību, mitrzemju, ūdenstilpņu fiziskais un bioloģiskais segums.</skos:definition>
		
		<skos:prefLabel xml:lang="mt">Kopertura ta' l-art</skos:prefLabel>
		<skos:definition xml:lang="mt">Kopertura fiżika u bijoloġika tal-wiċċ tad-dinja inklużi superfiċji artifiċjali, żoni agrikoli, foresti, żoni (semi-)naturali, artijiet mistagħdra, u korpi ta' ilma.</skos:definition>		
		
		<skos:prefLabel xml:lang="nl">Bodemgebruik</skos:prefLabel>
		<skos:definition xml:lang="nl">Fysieke en biologische bedekking van het aardoppervlak, met inbegrip van kunstmatige oppervlakken, landbouwgebieden, bossen, halfnatuurlijke gebieden, moeraslanden en wateroppervlakken.</skos:definition>
		<skos:prefLabel xml:lang="pl">Użytkowanie terenu</skos:prefLabel>
		<skos:definition xml:lang="pl">Fizyczne i biologiczne użytkowanie powierzchni Ziemi, włączając w to powierzchnie sztuczne, obszary rolnicze, lasy, obszary (pół-)naturalne, tereny podmokłe, akweny.</skos:definition>
		<skos:prefLabel xml:lang="pt">Ocupação do solo</skos:prefLabel>
		<skos:definition xml:lang="pt">Cobertura física e biológica da superfície terrestre, incluindo superfícies artificiais, zonas agrícolas, florestas, zonas naturais ou semi-naturais, zonas húmidas, massas de água.</skos:definition>
		<skos:prefLabel xml:lang="ro">Acoperire terestră</skos:prefLabel>
		<skos:definition xml:lang="ro">Acoperirea fizică şi biologică a suprafeţei terestre, inclusiv suprafeţele artificiale, zonele agricole, pădurile, zonele (semi)naturale, zonele umede şi corpurile de apă.</skos:definition>
		<skos:prefLabel xml:lang="sk">Krajinná pokrývka</skos:prefLabel>
		<skos:definition xml:lang="sk">Fyzikálna a biologická pokrývka zemského povrchu vrátane umelých povrchov, poľnohospodárskych oblastí, lesov, (polo)prírodných oblastí, mokradí, vodných útvarov.</skos:definition>
		<skos:prefLabel xml:lang="sl">Pokrovnost tal</skos:prefLabel>
		<skos:definition xml:lang="sl">Fizični in biološki pojavi na zemeljski površini, vključno z umetnimi površinami, kmetijskimi območji, gozdovi, (pol-) naravnimi območji, mokrišči, vodnimi telesi.</skos:definition>
		<skos:prefLabel xml:lang="sv">Landtäcke</skos:prefLabel>
		<skos:definition xml:lang="sv">Fysiskt och biologiskt landtäcke på jordytan, inbegripet artificiella ytor, jordbruksmark, skogar, (delvis) naturliga områden, våtmarker, vattenförekomster.</skos:definition>
		<!--
		<skos:prefLabel xml:lang="el">SAMPLE ALTERNATIVE EXPRESSION - αναφορά</skos:prefLabel>
		<skos:definition xml:lang="el">Συστήματα συντεταγμένων</skos:definition>
		<dct:description xml:lang="el">Συστήματα για μονοσήμαντη αναφορά χωρικών πληροφοριών στον χώρο, ως σύνολο συντεταγμένων (x,y,z) ή/και γεωγραφικό πλάτος και μήκος και ύψος, με βάση γεωδαιτικό οριζόντιο και κατακόρυφο σύστημα αναφοράς (datum).</dct:description>
		-->
		<skos:inScheme rdf:resource="http://inspire-registry.jrc.ec.europa.eu/registers/Themes/items"/>
	</inspire:Theme>
	<inspire:Theme rdf:about="http://inspire-registry.jrc.ec.europa.eu/registers/FCD/items/12">
		<!-- <owl:sameIndividualAs rdf:resource="http://www.eionet.europa.eu/gemet/theme_concepts?th=12&ns=5" /> -->
		<inspire:itemStatus>valid</inspire:itemStatus>
		<inspire:dateAccepted>2008-12-05T17:00:29.734+01:00</inspire:dateAccepted>
		<skos:prefLabel xml:lang="en">Orthoimagery</skos:prefLabel>
		<skos:definition xml:lang="en">Geo-referenced image data of the Earth's surface, from either satellite or airborne sensors.</skos:definition>
		<dct:description xml:lang="en">An orthoimage is a raster image that has been geometrically corrected ("orthorectified") to remove distortion caused by camera optics, camera tilt, and differences in elevation. Source is either satellite or air-borne sensors. Data is orthorectified to achieve an accuracy commensurate with a given topographic map equivalent.</dct:description>
		<skos:prefLabel xml:lang="bg">Ортоизображение</skos:prefLabel>
		<skos:definition xml:lang="bg">Данни от геоизображение на земната повърхност, направено от сателит или въздушни сензори.</skos:definition>
		<skos:prefLabel xml:lang="cs">Ortofotosnímky</skos:prefLabel>
		<skos:definition xml:lang="cs">Obrazová data pořízená satelitními nebo leteckými čidly vztažená k zemskému povrchu pomocí zeměpisné soustavy souřadnic.</skos:definition>
		<skos:prefLabel xml:lang="da">Ortofoto</skos:prefLabel>
		<skos:definition xml:lang="da">Georefererede billeddata om Jordens overflade optaget fra enten satellit- eller flybaserede sensorer.</skos:definition>
		<skos:prefLabel xml:lang="de">Orthofotografie</skos:prefLabel>
		<skos:definition xml:lang="de">Georeferenzierte Bilddaten der Erdoberfläche von satelliten- oder luftfahrzeuggestützten Sensoren.</skos:definition>
		<skos:prefLabel xml:lang="el">Ορθοφωτογραφία</skos:prefLabel>
		<skos:definition xml:lang="el">Γεωαναφερόμενα δεδομένα από εικόνες της επιφάνειας της γης, από δορυφόρους ή αερομεταφερόμενους αισθητήρες.</skos:definition>
		<skos:prefLabel xml:lang="es">Ortoimágenes</skos:prefLabel>
		<skos:definition xml:lang="es">Imágenes georreferenciadas de la superficie de la tierra, obtenidas por satélite o por sensores aerotransportados.</skos:definition>
		<skos:prefLabel xml:lang="et">Ortokujutised</skos:prefLabel>
		<skos:definition xml:lang="et">Maapinna georefereeritud kujutised, mis on talletatud satelliitidel või lennuvahenditel asuvate sensorite abil.</skos:definition>
		<skos:prefLabel xml:lang="fi">Ortoilmakuvat</skos:prefLabel>
		<skos:definition xml:lang="fi">Joko satelliittien tai lentokäyttöisten sensorien toimittamia maantieteelliseen koordinaatistoon sidottuja kuvatietoja maapallon pinnasta.</skos:definition>
		<skos:prefLabel xml:lang="fr">Ortho-imagerie</skos:prefLabel>
		<skos:definition xml:lang="fr">Images géoréférencées de la surface terrestre, provenant de satellites ou de capteurs aéroportés.</skos:definition>
		<skos:prefLabel xml:lang="hu">Ortofotók</skos:prefLabel>
		<skos:definition xml:lang="hu">A Föld felszínének földrajzi hivatkozással ellátott, műhold vagy légi adatgyűjtők által készített képi adatai.</skos:definition>
		<skos:prefLabel xml:lang="it">Orto immagini</skos:prefLabel>
		<skos:definition xml:lang="it">Immagini georeferenziate della superficie terrestre prese da satellite o da telesensori.</skos:definition>
		<skos:prefLabel xml:lang="lt">Ortofotografinis vaizdavimas</skos:prefLabel>
		<skos:definition xml:lang="lt">Georeferencinis žemės paviršiaus atvaizdas, gaunamas iš palydove arba orlaivyje esančių jutiklių.</skos:definition>
		<skos:prefLabel xml:lang="lv">Ortofotogrāfija</skos:prefLabel>
		<skos:definition xml:lang="lv">Zemes virsmas attēli ar piekārtotu norādi par ģeogrāfisko novietojumu telpā, kas saņemti no satelīta vai gaisā esošiem sensoriem.</skos:definition>
		
		<skos:prefLabel xml:lang="mt">Orthoimagery</skos:prefLabel>
		<skos:definition xml:lang="mt">Data fil-forma ta' stampa ġeo-referenzjata tal-wiċċ tad-dinja, minn satellita jew minn sensuri fl-ajru.</skos:definition>		
		
		<skos:prefLabel xml:lang="nl">Orthobeeldvorming</skos:prefLabel>
		<skos:definition xml:lang="nl">Geogerefereerde beeldgegevens van het aardoppervlak, afkomstig van sensoren op satellieten of vliegtuigen.</skos:definition>
		<skos:prefLabel xml:lang="pl">Sporządzanie ortoobrazów</skos:prefLabel>
		<skos:definition xml:lang="pl">Dane obrazowe powierzchni Ziemi posiadające odniesienie geograficzne, pochodzące z rejestracji z pokładu satelity lub samolotu.</skos:definition>
		<skos:prefLabel xml:lang="pt">Ortoimagens</skos:prefLabel>
		<skos:definition xml:lang="pt">Imagens georeferenciadas da superfície terrestre recolhidas por satélite ou sensores aéreos.</skos:definition>
		<skos:prefLabel xml:lang="ro">Ortoimagini</skos:prefLabel>
		<skos:definition xml:lang="ro">Imagini georeferenţiate ale suprafeţei terestre, înregistrate cu senzori plasaţi pe sateliţi sau aeropurtaţi.</skos:definition>
		<skos:prefLabel xml:lang="sk">Ortometria</skos:prefLabel>
		<skos:definition xml:lang="sk">Georeferencované obrazové údaje o zemskom povrchu buď zo satelitu alebo z leteckých snímačov.</skos:definition>
		<skos:prefLabel xml:lang="sl">Ortofoto</skos:prefLabel>
		<skos:definition xml:lang="sl">Geolocirani slikovni podatki zemeljske površine iz satelita ali senzorjev v zraku.</skos:definition>
		<skos:prefLabel xml:lang="sv">Ortofoto</skos:prefLabel>
		<skos:definition xml:lang="sv">Georefererade bilddata över jordytan, antingen från satelliter eller från flygburna sensorer.</skos:definition>
		<!--
		<skos:prefLabel xml:lang="el">SAMPLE ALTERNATIVE EXPRESSION - αναφορά</skos:prefLabel>
		<skos:definition xml:lang="el">Συστήματα συντεταγμένων</skos:definition>
		<dct:description xml:lang="el">Συστήματα για μονοσήμαντη αναφορά χωρικών πληροφοριών στον χώρο, ως σύνολο συντεταγμένων (x,y,z) ή/και γεωγραφικό πλάτος και μήκος και ύψος, με βάση γεωδαιτικό οριζόντιο και κατακόρυφο σύστημα αναφοράς (datum).</dct:description>
		-->
		<skos:inScheme rdf:resource="http://inspire-registry.jrc.ec.europa.eu/registers/Themes/items"/>
	</inspire:Theme>
	<inspire:Theme rdf:about="http://inspire-registry.jrc.ec.europa.eu/registers/FCD/items/13">
		<!-- <owl:sameIndividualAs rdf:resource="http://www.eionet.europa.eu/gemet/theme_concepts?th=13&ns=5" /> -->
		<inspire:itemStatus>valid</inspire:itemStatus>
		<inspire:dateAccepted>2008-12-05T17:00:29.792+01:00</inspire:dateAccepted>
		<skos:prefLabel xml:lang="en">Geology</skos:prefLabel>
		<skos:definition xml:lang="en">Geology characterised according to composition and structure. Includes bedrock, aquifers and geomorphology.</skos:definition>
		<dct:description xml:lang="en">Geological information provides basic knowledge about the physical and chemical composition and the genesis of the underground, in particular on the properties of the rocks and sediments (age, petrography, genesis and tectonic elements, ....) and their structure.
NOTE: Experts from EuroGeosurveys will provide an improved version of the Description for the theme ‘Geology’ in 2008.</dct:description>
		<skos:prefLabel xml:lang="bg">Геология</skos:prefLabel>
		<skos:definition xml:lang="bg">Геология, определена според състава и структурата. Включва земен слой, воден слой и геоморфология.</skos:definition>
		<skos:prefLabel xml:lang="cs">Geologie</skos:prefLabel>
		<skos:definition xml:lang="cs">Geologie charakterizovaná podle složení a struktury. Zahrnuje skalní podloží, zvodně a geomorfologii.</skos:definition>
		<skos:prefLabel xml:lang="da">Geologi</skos:prefLabel>
		<skos:definition xml:lang="da">Geologi karakteriseret ved sammensætning og struktur. Omfatter grundfjeld, grundvandsmagasiner og geomorfologi.</skos:definition>
		<skos:prefLabel xml:lang="de">Geologie</skos:prefLabel>
		<skos:definition xml:lang="de">Geologische Beschreibung anhand von Zusammensetzung und Struktur. Dies umfasst auch Grundgestein, Grundwasserleiter und Geomorphologie.</skos:definition>
		<skos:prefLabel xml:lang="el">Γεωλογία</skos:prefLabel>
		<skos:definition xml:lang="el">Γεωλογικός χαρακτηρισμός με βάση τη σύσταση και τη δομή. Περιλαμβάνονται το μητρικό πέτρωμα, οι υδροφόροι ορίζοντες και η γεωμορφολογία.</skos:definition>
		<skos:prefLabel xml:lang="es">Geología</skos:prefLabel>
		<skos:definition xml:lang="es">Características geológicas según la composición y la estructura. Se incluirán la plataforma de roca firme, los acuíferos y la geomorfología.</skos:definition>
		<skos:prefLabel xml:lang="et">Geoloogia</skos:prefLabel>
		<skos:definition xml:lang="et">Maapinna geoloogiline iseloom vastavalt koostisele ja struktuurile. Hõlmab aluskivimeid, põhjaveekihte ja geomorfoloogiat.</skos:definition>
		<skos:prefLabel xml:lang="fi">Geologia</skos:prefLabel>
		<skos:definition xml:lang="fi">Geologia kuvattuna koostumuksen ja rakenteen mukaan. Sisältää kallioperän, akviferit ja pinnanmuodot.</skos:definition>
		<skos:prefLabel xml:lang="fr">Géologie</skos:prefLabel>
		<skos:definition xml:lang="fr">Géologie caractérisée en fonction de la composition et de la structure. Englobe le substratum rocheux, les aquifères et la géomorphologie.</skos:definition>
		<skos:prefLabel xml:lang="hu">Földtan</skos:prefLabel>
		<skos:definition xml:lang="hu">Az összetétel és szerkezet alapján jellemzett földtan. Ide tartozik az alapkőzet, a víztartó rétegek és a geomorfológia is.</skos:definition>
		<skos:prefLabel xml:lang="it">Geologia</skos:prefLabel>
		<skos:definition xml:lang="it">Classificazione geologica in base alla composizione e alla struttura. Questa voce comprende il basamento roccioso, gli acquiferi e la geomorfologia.</skos:definition>
		<skos:prefLabel xml:lang="lt">Geologija</skos:prefLabel>
		<skos:definition xml:lang="lt">Geologija apibūdinama pagal sudėtį ir struktūrą. Tai apima pamatinę uolieną, vandeninguosius sluoksnius ir geomorfologiją.</skos:definition>
		<skos:prefLabel xml:lang="lv">Ģeoloģija</skos:prefLabel>
		<skos:definition xml:lang="lv">Ģeoloģiskais stāvoklis, ko raksturo uzbūve un struktūra. Tostarp informācija par pamatiežiem, ūdens nesējslāņiem un ģeomorfoloģiju.</skos:definition>
		
		<skos:prefLabel xml:lang="mt">Ġeologija</skos:prefLabel>
		<skos:definition xml:lang="mt">Ġeoloġija kkaratterizzata skond il-kompożizzjoni u l-istruttura. Tinkludi s-sodda tal-blat, l-akwiferi u lġeomorfoloġija.</skos:definition>		
		
		<skos:prefLabel xml:lang="nl">Geologie</skos:prefLabel>
		<skos:definition xml:lang="nl">Geologie, gekenmerkt volgens samenstelling en structuur, inclusief vast gesteente, waterhoudende grondlagen en geomorfologie.</skos:definition>
		<skos:prefLabel xml:lang="pl">Geologia</skos:prefLabel>
		<skos:definition xml:lang="pl">Geologia charakteryzowana na podstawie składu i struktury. Obejmuje podłoże skalne, warstwy wodonośne i geomorfologię.</skos:definition>
		<skos:prefLabel xml:lang="pt">Geologia</skos:prefLabel>
		<skos:definition xml:lang="pt">Geologia caracterizada de acordo com a composição e a estrutura. Inclui a base rochosa, os aquíferos e a geomorfologia.</skos:definition>
		<skos:prefLabel xml:lang="ro">Geologie</skos:prefLabel>
		<skos:definition xml:lang="ro">Geologie caracterizată în funcţie de compoziţie şi structură. Include roca de bază, straturile acvifere şi geomorfologia.</skos:definition>
		<skos:prefLabel xml:lang="sk">Geológia</skos:prefLabel>
		<skos:definition xml:lang="sk">Geológia charakterizovaná na základe zloženia a štruktúry. Zahŕňa skalné podložie, zvodnené vrstvy a geomorfológiu.</skos:definition>
		<skos:prefLabel xml:lang="sl">Geologija</skos:prefLabel>
		<skos:definition xml:lang="sl">Geologija je določena v skladu s sestavo in strukturo. Vključuje živo skalo, vodonosnike in geomorfologijo.</skos:definition>
		<skos:prefLabel xml:lang="sv">Geologi</skos:prefLabel>
		<skos:definition xml:lang="sv">Geologiska förhållanden indelade efter sammansättning och struktur. Innefattar berggrund, akviferer och geomorfologi.</skos:definition>
		<!--
		<skos:prefLabel xml:lang="el">SAMPLE ALTERNATIVE EXPRESSION - αναφορά</skos:prefLabel>
		<skos:definition xml:lang="el">Συστήματα συντεταγμένων</skos:definition>
		<dct:description xml:lang="el">Συστήματα για μονοσήμαντη αναφορά χωρικών πληροφοριών στον χώρο, ως σύνολο συντεταγμένων (x,y,z) ή/και γεωγραφικό πλάτος και μήκος και ύψος, με βάση γεωδαιτικό οριζόντιο και κατακόρυφο σύστημα αναφοράς (datum).</dct:description>
		-->
		<skos:inScheme rdf:resource="http://inspire-registry.jrc.ec.europa.eu/registers/Themes/items"/>
	</inspire:Theme>
	<inspire:Theme rdf:about="http://inspire-registry.jrc.ec.europa.eu/registers/FCD/items/14">
		<!-- <owl:sameIndividualAs rdf:resource="http://www.eionet.europa.eu/gemet/theme_concepts?th=14&ns=5" /> -->
		<inspire:itemStatus>valid</inspire:itemStatus>
		<inspire:dateAccepted>2008-12-05T17:00:29.850+01:00</inspire:dateAccepted>
		<skos:prefLabel xml:lang="en">Statistical units</skos:prefLabel>
		<skos:definition xml:lang="en">Units for dissemination or use of statistical information.</skos:definition>
		<dct:description xml:lang="en">The theme statistical units must be seen as one of several thematic groups of administrative units, but may also include other area units (e.g. grids or watersheds) or points in point-based statistics (e.g. statistics on address level). The IMS paper (INSPIRE IMS, 2003) describes the following sub-grouping of administrative units
  - official administrative units
  - government management zones
  - blocks, census and statistical districts
  - civil security units
  - environmental reporting and management units
  - postal codes/ regions

Units for dissemination of statistical information can be viewed as spatial units; areas, lines or point objects used in reporting of information, in geographical analysis and in distribution systems for environmental and socio-economic information. "Use" can be interpreted as something else than "dissemination", as the words is connected with the word "or". The use may represent any use in the full cycle of establishment, aggregation, assessment and display of "statistical information". Statistical information can be defined as "any numerical representation of a phenomenon".</dct:description>
		<skos:prefLabel xml:lang="bg">Статистически единици</skos:prefLabel>
		<skos:definition xml:lang="bg">Единици, разпространяващи или ползващи статистическа информация.</skos:definition>
		<skos:prefLabel xml:lang="cs">Statistické jednotky</skos:prefLabel>
		<skos:definition xml:lang="cs">Jednotky pro šíření nebo používání statistických informací.</skos:definition>
		<skos:prefLabel xml:lang="da">Statistiske enheder</skos:prefLabel>
		<skos:definition xml:lang="da">Enheder for formidling eller anvendelse af statistiske oplysninger.</skos:definition>
		<skos:prefLabel xml:lang="de">Statistische Einheiten</skos:prefLabel>
		<skos:definition xml:lang="de">Einheiten für die Verbreitung oder Verwendung statistischer Daten.</skos:definition>
		<skos:prefLabel xml:lang="el">Στατιστικές μονάδες</skos:prefLabel>
		<skos:definition xml:lang="el">Μονάδες διάδοσης ή χρήσης στατιστικών πληροφοριών.</skos:definition>
		<skos:prefLabel xml:lang="es">Unidades estadísticas</skos:prefLabel>
		<skos:definition xml:lang="es">Unidades para la difusión o el uso de información estadística.</skos:definition>
		<skos:prefLabel xml:lang="et">Statistilised üksused</skos:prefLabel>
		<skos:definition xml:lang="et">Statistilise teabe levitamise või kasutamise üksused.</skos:definition>
		<skos:prefLabel xml:lang="fi">Tilastoyksiköt</skos:prefLabel>
		<skos:definition xml:lang="fi">Tilastotietojen levittämis- tai käyttöyksiköt.</skos:definition>
		<skos:prefLabel xml:lang="fr">Unités statistiques</skos:prefLabel>
		<skos:definition xml:lang="fr">Unités de diffusion ou d'utilisation d'autres informations statistiques.</skos:definition>
		<skos:prefLabel xml:lang="hu">Statisztikai egységek</skos:prefLabel>
		<skos:definition xml:lang="hu">Statisztikai információk terjesztésére vagy felhasználására szolgáló egységek.</skos:definition>
		<skos:prefLabel xml:lang="it">Unità statistiche</skos:prefLabel>
		<skos:definition xml:lang="it">Unità per la divulgazione o l'utilizzo di dati statistici.</skos:definition>
		<skos:prefLabel xml:lang="lt">Statistiniai vienetai</skos:prefLabel>
		<skos:definition xml:lang="lt">Vienetai, skirti statistinės informacijos platinimui ar panaudojimui.</skos:definition>
		<skos:prefLabel xml:lang="lv">Statistikas vienības</skos:prefLabel>
		<skos:definition xml:lang="lv">Vienības, kuras izmanto statistikas informācijas izplatīšanā vai izmantošanā.</skos:definition>
		
		<skos:prefLabel xml:lang="mt">Unitajiet statistiċi</skos:prefLabel>
		<skos:definition xml:lang="mt">Unitajiet biex issir disseminazzjoni jew użu ta' informazzjoni ta' l-istatistika.</skos:definition>		
		
		<skos:prefLabel xml:lang="nl">Statistische eenheden</skos:prefLabel>
		<skos:definition xml:lang="nl">Eenheden voor verspreiding en gebruik van statistische informatie.</skos:definition>
		<skos:prefLabel xml:lang="pl">Jednostki statystyczne</skos:prefLabel>
		<skos:definition xml:lang="pl">Jednostki służące do rozpowszechniania lub wykorzystywania informacji statystycznych.</skos:definition>
		<skos:prefLabel xml:lang="pt">Unidades estatísticas</skos:prefLabel>
		<skos:definition xml:lang="pt">Unidades para fins de divulgação ou utilização da informação estatística.</skos:definition>
		<skos:prefLabel xml:lang="ro">Unităţi statistice</skos:prefLabel>
		<skos:definition xml:lang="ro">Unităţi de difuzare sau de utilizare a informaţiilor statistice.</skos:definition>
		<skos:prefLabel xml:lang="sk">Štatistické jednotky</skos:prefLabel>
		<skos:definition xml:lang="sk">Jednotky pre šírenie alebo využívanie štatistických informácií.</skos:definition>
		<skos:prefLabel xml:lang="sl">Statistični okoliši</skos:prefLabel>
		<skos:definition xml:lang="sl">Enote za širjenje ali uporabo statističnih podatkov.</skos:definition>
		<skos:prefLabel xml:lang="sv">Statistiska enheter</skos:prefLabel>
		<skos:definition xml:lang="sv">Enheter för spridning och användning av statistisk information.</skos:definition>
		<!--
		<skos:prefLabel xml:lang="el">SAMPLE ALTERNATIVE EXPRESSION - αναφορά</skos:prefLabel>
		<skos:definition xml:lang="el">Συστήματα συντεταγμένων</skos:definition>
		<dct:description xml:lang="el">Συστήματα για μονοσήμαντη αναφορά χωρικών πληροφοριών στον χώρο, ως σύνολο συντεταγμένων (x,y,z) ή/και γεωγραφικό πλάτος και μήκος και ύψος, με βάση γεωδαιτικό οριζόντιο και κατακόρυφο σύστημα αναφοράς (datum).</dct:description>
		-->
		<skos:inScheme rdf:resource="http://inspire-registry.jrc.ec.europa.eu/registers/Themes/items"/>
	</inspire:Theme>
	<inspire:Theme rdf:about="http://inspire-registry.jrc.ec.europa.eu/registers/FCD/items/15">
		<!-- <owl:sameIndividualAs rdf:resource="http://www.eionet.europa.eu/gemet/theme_concepts?th=15&ns=5" /> -->
		<inspire:itemStatus>valid</inspire:itemStatus>
		<inspire:dateAccepted>2008-12-05T17:00:29.913+01:00</inspire:dateAccepted>
		<skos:prefLabel xml:lang="en">Buildings</skos:prefLabel>
		<skos:definition xml:lang="en">Geographical location of buildings.</skos:definition>
		<dct:description xml:lang="en">A building is a covered facility, usable for the protection of humans, animals, things or the production of economic goods. A building refers to any structure permanently constructed or erected on its site.
Information on location of buildings may be supplied as points or with the actual basic form of the building.
Usually buildings are part of cadastre. On the local level buildings are available within the large scale cadastral maps or cadastral data sets and are geometrically represented as surfaces.
Most buildings can be identified (geocoded) by address (separate theme in INSPIRE).</dct:description>
		<skos:prefLabel xml:lang="bg">Сгради</skos:prefLabel>
		<skos:definition xml:lang="bg">Географско разположение на сградите.</skos:definition>
		<skos:prefLabel xml:lang="cs">Budovy</skos:prefLabel>
		<skos:definition xml:lang="cs">Zeměpisná poloha budov.</skos:definition>
		<skos:prefLabel xml:lang="da">Bygninger</skos:prefLabel>
		<skos:definition xml:lang="da">Geografisk stedfæstelse af bygninger.</skos:definition>
		<skos:prefLabel xml:lang="de">Gebäude</skos:prefLabel>
		<skos:definition xml:lang="de">Geografischer Standort von Gebäuden.</skos:definition>
		<skos:prefLabel xml:lang="el">Κτίρια</skos:prefLabel>
		<skos:definition xml:lang="el">Γεωγραφική θέση κτιρίων.</skos:definition>
		<skos:prefLabel xml:lang="es">Edificios</skos:prefLabel>
		<skos:definition xml:lang="es">Localización geográfica de los edificios.</skos:definition>
		<skos:prefLabel xml:lang="et">Ehitised</skos:prefLabel>
		<skos:definition xml:lang="et">Ehitiste geograafiline asukoht.</skos:definition>
		<skos:prefLabel xml:lang="fi">Rakennukset</skos:prefLabel>
		<skos:definition xml:lang="fi">Rakennusten maantieteellinen sijainti.</skos:definition>
		<skos:prefLabel xml:lang="fr">Bâtiments</skos:prefLabel>
		<skos:definition xml:lang="fr">Situation géographique des bâtiments.</skos:definition>
		<skos:prefLabel xml:lang="hu">Épületek</skos:prefLabel>
		<skos:definition xml:lang="hu">Az épületek földrajzi helye.</skos:definition>
		<skos:prefLabel xml:lang="it">Edifici</skos:prefLabel>
		<skos:definition xml:lang="it">Localizzazione geografica degli edifici.</skos:definition>
		<skos:prefLabel xml:lang="lt">Pastatai</skos:prefLabel>
		<skos:definition xml:lang="lt">Geografinė pastatų buvimo vieta.</skos:definition>
		<skos:prefLabel xml:lang="lv">Ēkas</skos:prefLabel>
		<skos:definition xml:lang="lv">Ēku ģeogrāfiskā atrašanās vieta.</skos:definition>
		
		<skos:prefLabel xml:lang="mt">Bini</skos:prefLabel>
		<skos:definition xml:lang="mt">Posizzjoni ġeografika ta' bini.</skos:definition>		
		
		<skos:prefLabel xml:lang="nl">Gebouwen</skos:prefLabel>
		<skos:definition xml:lang="nl">Geografische locatie van gebouwen.</skos:definition>
		<skos:prefLabel xml:lang="pl">Budynki</skos:prefLabel>
		<skos:definition xml:lang="pl">Położenie geograficzne budynków.</skos:definition>
		<skos:prefLabel xml:lang="pt">Edifícios</skos:prefLabel>
		<skos:definition xml:lang="pt">Localização geográfica dos edifícios.</skos:definition>
		<skos:prefLabel xml:lang="ro">Clădiri</skos:prefLabel>
		<skos:definition xml:lang="ro">Localizarea geografică a clădirilor.</skos:definition>
		<skos:prefLabel xml:lang="sk">Stavby</skos:prefLabel>
		<skos:definition xml:lang="sk">Zemepisná poloha stavieb.</skos:definition>
		<skos:prefLabel xml:lang="sl">Stavbe</skos:prefLabel>
		<skos:definition xml:lang="sl">Prostorska lega stavb.</skos:definition>
		<skos:prefLabel xml:lang="sv">Byggnader</skos:prefLabel>
		<skos:definition xml:lang="sv">Geografiskt läge för byggnader.</skos:definition>
		<!--
		<skos:prefLabel xml:lang="el">SAMPLE ALTERNATIVE EXPRESSION - αναφορά</skos:prefLabel>
		<skos:definition xml:lang="el">Συστήματα συντεταγμένων</skos:definition>
		<dct:description xml:lang="el">Συστήματα για μονοσήμαντη αναφορά χωρικών πληροφοριών στον χώρο, ως σύνολο συντεταγμένων (x,y,z) ή/και γεωγραφικό πλάτος και μήκος και ύψος, με βάση γεωδαιτικό οριζόντιο και κατακόρυφο σύστημα αναφοράς (datum).</dct:description>
		-->
		<skos:inScheme rdf:resource="http://inspire-registry.jrc.ec.europa.eu/registers/Themes/items"/>
	</inspire:Theme>
	<inspire:Theme rdf:about="http://inspire-registry.jrc.ec.europa.eu/registers/FCD/items/16">
		<!-- <owl:sameIndividualAs rdf:resource="http://www.eionet.europa.eu/gemet/theme_concepts?th=16&ns=5" /> -->
		<inspire:itemStatus>valid</inspire:itemStatus>
		<inspire:dateAccepted>2008-12-05T17:00:29.974+01:00</inspire:dateAccepted>
		<skos:prefLabel xml:lang="en">Soil</skos:prefLabel>
		<skos:definition xml:lang="en">Soils and subsoil characterised according to depth, texture, structure and content of particles and organic material, stoniness, erosion, where appropriate mean slope and anticipated water storage capacity.</skos:definition>
		<dct:description xml:lang="en">The proposed Soil Framework Directive (COM(2006) 232 final), which aims at the establishment of a framework for the protection of soil, specifies in Article 1 that soil is “the top layer of the earth’s crust situated between the bedrock and the surface, excluding groundwater as defined in Article 2(2) of Directive 2000/60/EC of the European Parliament and of the Council”. In the Communication from the Commission regarding the Thematic Strategy for Soil Protection (COM(2006)231 final), it is mentioned that “soil is generally defined as the top layer of the earth’s crust, formed by mineral particles, organic matter, water, air and living organisms. It is the interface between earth, air and water and hosts most of the biosphere”.

As soil formation is an extremely slow process, soil can be considered essentially as a non-renewable resource. Soil provides us with food, biomass and raw materials. It serves as a platform for human activities and landscape and as an archive of heritage and plays a central role as a habitat and gene pool. It stores, filters and transforms many substances, including water, nutrients and carbon. In fact, it is the biggest carbon store in the world. These functions must be protected because of both their socio-economic and environmental importance.

Soil is an extremely complex and variable medium. Over 320 major soil types have been identified in Europe and within each there are enormous variations in physical, chemical and biological properties. Soil’s structure plays a major role in determining its ability to perform its functions. Any damage to its structure also damages other environmental media and ecosystems.

Soil is subject to a series of degradation processes or threats. These include erosion, decline in organic matter, local and diffuse contamination, sealing, compaction, decline in biodiversity, salinisation, floods and landslides. A combination of some of these threats can ultimately lead arid or sub-arid climatic conditions to desertification.”

Typically, soil is characterized on the basis of soil profile descriptions, analysed by taking samples from genetic horizons or depth classes, and classified according to national or international nomenclature. Soil maps contain the borders of typical combinations of soil development factors of the target mapping scale. There is no internationally defined aggregation scheme between the various map scales.

The collection of soil information can be broadly classified into three categories:
  a) Soil mapping, enabling to identify areas of land for management purposes.
  b) Soil inventories, providing a one-off assessment of soil conditions and/or properties at a point in time, and soil monitoring, providing a series of assessments showing how soil conditions and/or properties change over time.
  c) Soil thematic mapping

(a) Soil maps
The general aim of soil mapping is to provide a spatial representation and description of the soils of continents, countries, regions, farms, or any area of land of interest. It involves identifying the different types of soils that occur, collecting data on their nature, properties and potential use, and recording this information on maps and in geographic information systems and derived media.

(b) Soil inventories and soil monitoring
Soil inventories (predominantly based on “soil profiles”) provide information on the soil condition. It can be introduced to soil maps as attribute (semantic) data describing soil properties. Soil monitoring in national or Europe-wide grid systems, or in stratified sampling regimes, is designed to provide information about how soils are changing with time (see also INSPIRE Theme ‘Environmental Monitoring Facilities’). Geochemical surveys also gather soil information and are specifically targeted to provide information on natural background values and on overimposed anthropic pollution.

(c) Thematic data/risk maps in soil protection and environmental reporting
The general adoption of GIS technology and the creation of databases of georeferenced soil information have allowed a number of new types of assessments producing more policy relevant information than the basic soil maps. For example, modelling approaches using the existing soil inventories allow deriving information like soil erosion risk, organic matter content, diffuse contamination, soil compaction, salinisation, etc.</dct:description>
		<skos:prefLabel xml:lang="bg">Почва</skos:prefLabel>
		<skos:definition xml:lang="bg">Почви и подпочви, определени според дълбочина, строеж, структура, механичен състав и съдържание на органични материали, каменливост, ерозия и, по целесъобразност, среден наклон и предполагаема водопопиваемост.</skos:definition>
		<skos:prefLabel xml:lang="cs">Půda</skos:prefLabel>
		<skos:definition xml:lang="cs">Půda a její podloží popsané podle hloubky, zrnitosti, struktury a obsahu částic a organického materiálu, podílu skeletu, erozí, případně průměrného sklonu svahu a očekávané kapacity jímavosti vody.</skos:definition>
		<skos:prefLabel xml:lang="da">Jord</skos:prefLabel>
		<skos:definition xml:lang="da">Jordbund og underjord karakteriseret efter dybde, tekstur, struktur og indhold af partikler og organisk materiale, stenindhold, erosion, i givet fald gennemsnitlig hældning og forventet vandlagringskapacitet.</skos:definition>
		<skos:prefLabel xml:lang="de">Boden</skos:prefLabel>
		<skos:definition xml:lang="de">Beschreibung von Boden und Unterboden anhand von Tiefe, Textur, Struktur und Gehalt an Teilchen sowie organischem Material, Steinigkeit, Erosion, gegebenenfalls durchschnittliches Gefälle und erwartete Wasserspeicherkapazität.</skos:definition>
		<skos:prefLabel xml:lang="el">Έδαφος</skos:prefLabel>
		<skos:definition xml:lang="el">Χαρακτηρισμός εδάφους και υπεδάφους ανάλογα με το βάθος, την υφή, τη δομή και την περιεκτικότητα σε σωματίδια και οργανικά υλικά, το πετρώδες, τη διάβρωση και, κατά περίπτωση, τη μέση κλίση και την προβλεπόμενη χωρητικότητα αποθήκευσης νερού.</skos:definition>
		<skos:prefLabel xml:lang="es">Suelo</skos:prefLabel>
		<skos:definition xml:lang="es">Suelo y subsuelo, caracterizados según su profundidad, textura, estructura y contenido de partículas y material orgánico, pedregosidad, erosión y, cuando proceda, pendiente media y capacidad estimada de almacenamiento de agua.</skos:definition>
		<skos:prefLabel xml:lang="et">Pinnas</skos:prefLabel>
		<skos:definition xml:lang="et">Pinnas ja aluspinnas, mida iseloomustatakse sügavuse, tekstuuri, struktuuri, osakeste ja orgaanilise materjali sisalduse, kivimisisalduse, erosiooni, vajadusel keskmise kalde ja eeldatava veemahutavuse järgi.</skos:definition>
		<skos:prefLabel xml:lang="fi">Maaperä</skos:prefLabel>
		<skos:definition xml:lang="fi">Maannoksen ja muuttumattoman pohjamaalajin kuvaaminen syvyyden, raekoostumuksen, rakenteen sekä hiukkasten ja orgaanisen aineksen sisällön, kivisyyden, eroosion ja tarvittaessa keskimääräisen kaltevuuden ja arvioidun veden varastointikapasiteetin mukaan.</skos:definition>
		<skos:prefLabel xml:lang="fr">Sols</skos:prefLabel>
		<skos:definition xml:lang="fr">Sols et sous-sol caractérisés selon leur profondeur, texture, structure et teneur en particules et en matières organiques, pierrosité, érosion, le cas échéant pente moyenne et capacité anticipée de stockage de l'eau.</skos:definition>
		<skos:prefLabel xml:lang="hu">Talaj</skos:prefLabel>
		<skos:definition xml:lang="hu">A mélység, állag, szerkezet, a részecskék és szerves anyagok jelenléte, a köves jelleg, az erózió, valamint adott esetben az átlagos lejtés és a becsült víztartó képesség alapján jellemzett talajok és altalaj.</skos:definition>
		<skos:prefLabel xml:lang="it">Suolo</skos:prefLabel>
		<skos:definition xml:lang="it">Caratterizzazione del suolo e del sottosuolo in base a profondità, tessitura (texture), struttura e contenuto delle particelle e della materia organica, pietrosità, erosione, eventualmente pendenza media e capacità prevista di ritenzione dell’acqua.</skos:definition>
		<skos:prefLabel xml:lang="lt">Dirvožemis</skos:prefLabel>
		<skos:definition xml:lang="lt">Dirvožemio ir podirvio charakteristikos: gylis, granuliometrinė sudėtis, dalelių ir organinių medžiagų struktūra ir sudėtis, akmeningumas, erozija ir tam tikrais atvejais vidutinis nuolydis bei numatomas vandens sulaikymo pajėgumas.</skos:definition>
		<skos:prefLabel xml:lang="lv">Augsne</skos:prefLabel>
		<skos:definition xml:lang="lv">Augsnes un tās apakškārtas stāvoklis, ko raksturo dziļums, faktūra, struktūra un daļiņu un organisko vielu saturs, akmeņainība, erozija un, attiecīgā gadījumā, vidējais slīpums un prognozējamā ūdens uzkrāšanas spēja.</skos:definition>
		
		<skos:prefLabel xml:lang="mt">Ħamrija</skos:prefLabel>
		<skos:definition xml:lang="mt">Tipi ta' ħamrija u sub-ħamrija kkaratterizzati skond il-fond, it-tessut, l-istruttura u l-kontenut ta' partiċelli u materjal organiku, il-kontenut ta' ġebel, it-tgħawwir, fejn xieraq il-medja tax-xaqlib ta' l-art u l-kapaċità antiċipata għall-ħażna ta' l-ilma.</skos:definition>		
		
		<skos:prefLabel xml:lang="nl">Bodem</skos:prefLabel>
		<skos:definition xml:lang="nl">Bodem en ondergrond, gekenmerkt volgens diepte, textuur, structuur en inhoud van deeltjes en organisch materiaal, steenachtigheid, erosie en, waar passend, gemiddelde hellingsgraad en verwachte wateropslagcapaciteit.</skos:definition>
		<skos:prefLabel xml:lang="pl">Gleba</skos:prefLabel>
		<skos:definition xml:lang="pl">Gleby i podglebie charakteryzowane na podstawie głębokości, tekstury, struktury i zawartości cząstek oraz materiału organicznego, kamienistości, erozji, a w odpowiednich przypadkach na podstawie przeciętnego nachylenia oraz przewidywanej zdolności zatrzymywania wody.</skos:definition>
		<skos:prefLabel xml:lang="pt">Solo</skos:prefLabel>
		<skos:definition xml:lang="pt">Solo e subsolo caracterizado de acordo com a profundidade, textura, estrutura e conteúdo das partículas e material orgânico, carácter pedregoso, erosão, eventualmente declive médio e capacidade estimada de armazenamento de água.</skos:definition>
		<skos:prefLabel xml:lang="ro">Soluri</skos:prefLabel>
		<skos:definition xml:lang="ro">Soluri şi subsoluri, caracterizate în funcţie de adâncime, textură, structură şi conţinut al particulelor şi materialului organic, schelet, eroziune, înclinaţie medie şi capacitate anticipată de stocare a apei, după caz.</skos:definition>
		<skos:prefLabel xml:lang="sk">Pôda</skos:prefLabel>
		<skos:definition xml:lang="sk">Pôdy a podložia charakterizované podľa hĺbky, textúry, štruktúry a obsahu častíc a organického materiálu, kamenitosti, erózie, prípadne priemerným sklonom a predpokladanou schopnosťou zadržiavať vodu.</skos:definition>
		<skos:prefLabel xml:lang="sl">Tla</skos:prefLabel>
		<skos:definition xml:lang="sl">Tla in sloji prsti pod površjem, določeni po debelini, teksturi, zgradbi in vsebnosti delcev in organskih snovi, kamnitosti, eroziji, po potrebi povprečni nagib in predvidene zmogljivosti vodnih zalog.</skos:definition>
		<skos:prefLabel xml:lang="sv">Mark</skos:prefLabel>
		<skos:definition xml:lang="sv">Jordmåner och jordarter klassificerade efter djup, textur, struktur och innehåll av partiklar och organiskt material, stenighet, erosion, vid behov genomsnittlig lutning och beräknad vattenhållande förmåga.</skos:definition>
		<!--
		<skos:prefLabel xml:lang="el">SAMPLE ALTERNATIVE EXPRESSION - αναφορά</skos:prefLabel>
		<skos:definition xml:lang="el">Συστήματα συντεταγμένων</skos:definition>
		<dct:description xml:lang="el">Συστήματα για μονοσήμαντη αναφορά χωρικών πληροφοριών στον χώρο, ως σύνολο συντεταγμένων (x,y,z) ή/και γεωγραφικό πλάτος και μήκος και ύψος, με βάση γεωδαιτικό οριζόντιο και κατακόρυφο σύστημα αναφοράς (datum).</dct:description>
		-->
		<skos:inScheme rdf:resource="http://inspire-registry.jrc.ec.europa.eu/registers/Themes/items"/>
	</inspire:Theme>
	<inspire:Theme rdf:about="http://inspire-registry.jrc.ec.europa.eu/registers/FCD/items/17">
		<!-- <owl:sameIndividualAs rdf:resource="http://www.eionet.europa.eu/gemet/theme_concepts?th=17&ns=5" /> -->
		<inspire:itemStatus>valid</inspire:itemStatus>
		<inspire:dateAccepted>2008-12-05T17:00:30.052+01:00</inspire:dateAccepted>
		<skos:prefLabel xml:lang="en">Land use</skos:prefLabel>
		<skos:definition xml:lang="en">Territory characterised according to its current and future planned functional dimension or socio-economic purpose (e.g. residential, industrial, commercial, agricultural, forestry, recreational).</skos:definition>
		<dct:description xml:lang="en">Land regulation is the general spatial planning tool at regional and local levels. Land use may be characterised as ordinary mapping of existing functions as an objective picture of the use and functions of a territory, but may also be plans characterising how land may be utilised at present and in the future.

There are two main land use definitions, a functional one and sequential one (Duhamel, 1998). The first of them defines land use as the description of land in terms or its socio-economic purpose (agricultural, residential, forestry etc.). The second one describes land use as a series of operations on land, carried out by humans, with the intention to obtain products and/or benefits through using land resources.

Land use plans/ land user regulation
The land use plans regulate actual and future use of areas. The land use plans commonly have significant textual regulations to each area/ land category or specific areas. The land use plans are of varying detail; Municipal land use plans, detailed regulation plans for blocks or smaller areas within urban areas.
  • Land use may be seen as divisions at a high level, e.g. distinguishing between private and state owned land. , e.g. at scale 1: 1 mill.
  • Land use plans is commonly made at regional levels as kinds of master plans, e.g. covering the full extent of municipalities and being at the scale 1: 50.000
  • Land regulation plans at detailed low level may cover populated areas or areas of specific economic or social interest. The plans may direct utilization level, the % of building coverage within areas, height regulations or functional regulations, and maps produced may have a detailed scale, e.g. 1: 5000.

It is a very diverse situation concerning land regulation/ land use plans as these spatial data commonly are based on national or regional legislation or other kinds of regulation. The documents/maps are frequently seen as legal documents, and the categories remain for decades as rights directing use land and property. Categories of land use follow such regulations. Furthermore, operational plans may for some areas be old and based on older legislation, and the nomenclature may have changed through time. Operational land use plans may be as old as 100 years or more. Also plans being proposed and being in a process or public/sectoral hearing can be relevant for dissemination in the infrastructure.

A common strategy to activate land use plans in a GIS is through the production of raster versions of land use plans. This is by some seen as a very good strategy, as the rasterisation makes a "copy" of the visual content, thus locking the content and accuracy for changes and misleading interpretation of the legal map documents. Some organisations have a strategy of first supplying raster versions of existing plans, and with a long term plan for establishment of vector versions.

Functional land use – according to socio-economic purpose
Functional areas within urban or rural areas may be mapped through fieldwork, register information or through modelling using socio-economic input data in a GIS.

The recommended classification of the land use phenomenon is based on the ISIC Rev.3 (International Standard Classification of All Economic Activities) classification drawn up by the United Nations (approved by the Statistical Commission in 1989) and recommended for use throughout the world. This classification is integrated in the sense that it ensures a full harmonization with another main branches of economic classifications: the classifications of products ICPC Central Product Classification) which are fundamental for foreign trade statistics, statistics of production and consumption, energy statistics, etc. The ISIC Rev. 3, it is important to state, is fully compatible with the EU NACE Rev. 1 (Nomenclature des Activités de la Communauté Européenne) system for the first two levels. (System replaced by 1.1.2008, see references).

The ISIC system is made of four levels of breakdown: 17 sections, 60 divisions, 159 groups and 292 classes. The 17 sections of the first level are characterizing main economic activities. These categories are:
SECTION A Agriculture, Hunting and Forestry
SECTION B Fishing
SECTION C Mining and Quarrying
SECTION D Manufacturing
SECTION E Electricity, Gas and Water Supply
SECTION F Construction
SECTION G Wholesale and Retail Trade, Repair of motor vehicles, motorcycles and Personal and household goods
SECTION H Hotels and Restaurants
SECTION I Transport, Storage and Communication
SECTION J Financial intermediation
SECTION K Real estate, Renting and Business activities
SECTION L Public Administration and Defence, Compulsory social security
SECTION M Education
SECTION N Health and Social work
SECTION O Other Community, Social and Personal Service Activities
SECTION P Private Households with Employed Persons
SECTION Q Extra-territorial Organizations and Bodies</dct:description>
		<skos:prefLabel xml:lang="bg">Ползване на земята</skos:prefLabel>
		<skos:definition xml:lang="bg">Територия, определена според настоящите и бъдещите ѝ планирани функционални параметри или социално- икономическо предназначение (например жилищна, промишлена, търговска, селскостопанска, горска, почивна).</skos:definition>
		<skos:prefLabel xml:lang="cs">Využití území</skos:prefLabel>
		<skos:definition xml:lang="cs">Území popsané podle své současné a plánované funkce nebo společensko-hospodářských účelů (např. obytné, průmyslové, obchodní, zemědělské, lesnické, rekreační).</skos:definition>
		<skos:prefLabel xml:lang="da">Arealanvendelse</skos:prefLabel>
		<skos:definition xml:lang="da">Området karakteriseret ved dets nuværende og fremtidige planlagte funktion eller samfundsøkonomiske formål (f.eks. beboelse, industri, handel, landbrug, skovbrug, rekreation).</skos:definition>
		<skos:prefLabel xml:lang="de">Bodennutzung</skos:prefLabel>
		<skos:definition xml:lang="de">Beschreibung von Gebieten anhand ihrer derzeitigen und geplanten künftigen Funktion oder ihres sozioökonomischen Zwecks (z. B. Wohn-, Industrie- oder Gewerbegebiete, land- oder forstwirtschaftliche Flächen, Freizeitgebiete).</skos:definition>
		<skos:prefLabel xml:lang="el">Χρήσεις γης</skos:prefLabel>
		<skos:definition xml:lang="el">Χαρακτηρισμός περιοχών ανάλογα με τη σημερινή και τη μελλοντική σχεδιαζόμενη λειτουργία τους ή τον κοινωνικοοικονομικό σκοπό τους (π.χ. αμιγώς οικιστική, βιομηχανική, εμπορική, γεωργική, δασική, αναψυχής).</skos:definition>
		<skos:prefLabel xml:lang="es">Uso del suelo</skos:prefLabel>
		<skos:definition xml:lang="es">Caracterización del territorio, de acuerdo con su dimensión funcional o su dedicación socioeconómica actual o futura planificadas (por ejemplo, residencial, industrial, comercial, agrario, forestal, recreativo).</skos:definition>
		<skos:prefLabel xml:lang="et">Maakasutus</skos:prefLabel>
		<skos:definition xml:lang="et">Maa-ala iseloomustus olemasolevate ja tulevaste kavandatud kasutusaspektide või sotsiaalmajandusliku sihtotstarbe järgi (nt elamu- tööstus-, äri-, põllumajandus-, metsa- või puhkemaa).</skos:definition>
		<skos:prefLabel xml:lang="fi">Maankäyttö</skos:prefLabel>
		<skos:definition xml:lang="fi">Alueen kuvaaminen sen nykyisen ja tulevan suunnitellun käyttötarkoituksen tai sosioekonomisen tarkoituksen (esimerkiksi asuin- tai teollisuusalue, liikekeskus, maa- tai metsätalousalue tai virkistysalue) mukaan.</skos:definition>
		<skos:prefLabel xml:lang="fr">Usage des sols</skos:prefLabel>
		<skos:definition xml:lang="fr">Territoire caractérisé selon sa dimension fonctionnelle prévue ou son objet socioéconomique actuel et futur (par exemple, résidentiel, industriel, commercial, agricole, forestier, récréatif).</skos:definition>
		<skos:prefLabel xml:lang="hu">Földhasználat</skos:prefLabel>
		<skos:definition xml:lang="hu">A jelenlegi és a jövőbeli tervezett funkcionális szempontok vagy a társadalmigazdasági rendeltetés (például lakó-, ipari, kereskedelmi, mezőgazdasági, erdő- vagy pihenőövezet) szerint jellemzett területek.</skos:definition>
		<skos:prefLabel xml:lang="it">Utilizzo del territorio</skos:prefLabel>
		<skos:definition xml:lang="it">Classificazione del territorio in base alla dimensione funzionale o alla destinazione socioeconomica presenti e programmate per il futuro (ad esempio ad uso residenziale, industriale, commerciale, agricolo, silvicolo, ricreativo).</skos:definition>
		<skos:prefLabel xml:lang="lt">Žemės naudojimas</skos:prefLabel>
		<skos:definition xml:lang="lt">Teritorija apibūdinama pagal jos esamą ir būsimą planuojamą funkcinę arba socialinę ir ekonominę paskirtį (pvz., gyvenamoji, pramoninė, komercinė, žemės ūkio, miškų, rekreacinė).</skos:definition>
		<skos:prefLabel xml:lang="lv">Zemes izmantošana</skos:prefLabel>
		<skos:definition xml:lang="lv">Teritorijas stāvoklis, ko raksturo tās pašreizējās un nākotnē plānotās funkcionālās izmantošanas dimensija vai sociāli ekonomiskais izmantošanas nolūks (piemēram, zeme dzīvojamiem namiem, rūpnieciskiem, komerciāliem, lauksaimniecības, mežniecības, atpūtas mērķiem).</skos:definition>
		
		<skos:prefLabel xml:lang="mt">Użu ta' l-art</skos:prefLabel>
		<skos:definition xml:lang="mt">Territorju kkaratterizzat skond id-dimensjoni funzjonali tiegħu ppjanata attwali u futura jew l-iskop soċjo-ekonomiku tiegħu (eż. residenzjali, industrijali, kummerċjali, agrikolu, forestali, rikreazzjonali).</skos:definition>		
		
		<skos:prefLabel xml:lang="nl">Landgebruik</skos:prefLabel>
		<skos:definition xml:lang="nl">Het grondgebied, gekenmerkt volgens zijn huidige en geplande toekomstige functionele dimensie of sociaaleconomische bestemming (bv. wonen, industrieel, commercieel, landbouw, bosbouw, recreatie).</skos:definition>
		<skos:prefLabel xml:lang="pl">Zagospodarowanie przestrzenne</skos:prefLabel>
		<skos:definition xml:lang="pl">Terytorium charakteryzowane ze względu na jego obecny lub przyszły wymiar funkcjonalny lub przeznaczenie społeczno-gospodarcze (np. mieszkaniowe, przemysłowe, handlowe, rolnicze, leśne, wypoczynkowe).</skos:definition>
		<skos:prefLabel xml:lang="pt">Uso do solo</skos:prefLabel>
		<skos:definition xml:lang="pt">Caracterização do território de acordo com a dimensão funcional ou finalidade socioeconómica planeada, presente e futura (por exemplo, residencial, industrial, comercial, agrícola, silvícola, recreativa).</skos:definition>
		<skos:prefLabel xml:lang="ro">Utilizarea terenului</skos:prefLabel>
		<skos:definition xml:lang="ro">Teritoriu caracterizat în funcţie de dimensiunea funcţională actuală sau viitoare planificată sau de scopul socioeconomic (de exemplu rezidenţial, industrial, comercial, agricol, forestier, de recreaţie).</skos:definition>
		<skos:prefLabel xml:lang="sk">Využitie územia</skos:prefLabel>
		<skos:definition xml:lang="sk">Územie charakterizované podľa jeho súčasného a budúceho plánovaného funkčného rozmeru alebo socioekonomického účelu (napr. obytný, priemyselný, obchodný, poľnohospodársky, lesnícky, rekreačný).</skos:definition>
		<skos:prefLabel xml:lang="sl">Namenska raba tal</skos:prefLabel>
		<skos:definition xml:lang="sl">Ozemlje, opredeljeno glede na svojo sedanjo in v prihodnje načrtovano funkcionalno razsežnost ali socialnoekonomski namen (npr. stanovanjski, industrijski, trgovinski, kmetijski, gozdni, rekreacijski).</skos:definition>
		<skos:prefLabel xml:lang="sv">Markanvändning</skos:prefLabel>
		<skos:definition xml:lang="sv">Territorium indelat efter nuvarande och framtida planerade funktion eller socioekonomisk användning (t.ex. bostadsmark, industrimark, handel, jordbruk, skogsbruk, friluftsliv).</skos:definition>
		<!--
		<skos:prefLabel xml:lang="el">SAMPLE ALTERNATIVE EXPRESSION - αναφορά</skos:prefLabel>
		<skos:definition xml:lang="el">Συστήματα συντεταγμένων</skos:definition>
		<dct:description xml:lang="el">Συστήματα για μονοσήμαντη αναφορά χωρικών πληροφοριών στον χώρο, ως σύνολο συντεταγμένων (x,y,z) ή/και γεωγραφικό πλάτος και μήκος και ύψος, με βάση γεωδαιτικό οριζόντιο και κατακόρυφο σύστημα αναφοράς (datum).</dct:description>
		-->
		<skos:inScheme rdf:resource="http://inspire-registry.jrc.ec.europa.eu/registers/Themes/items"/>
	</inspire:Theme>
	<inspire:Theme rdf:about="http://inspire-registry.jrc.ec.europa.eu/registers/FCD/items/18">
		<!-- <owl:sameIndividualAs rdf:resource="http://www.eionet.europa.eu/gemet/theme_concepts?th=18&ns=5" /> -->
		<inspire:itemStatus>valid</inspire:itemStatus>
		<inspire:dateAccepted>2008-12-05T17:00:30.124+01:00</inspire:dateAccepted>
		<skos:prefLabel xml:lang="en">Human health and safety</skos:prefLabel>
		<skos:definition xml:lang="en">Geographical distribution of dominance of pathologies (allergies, cancers, respiratory diseases, etc.), information indicating the effect on health (biomarkers, decline of fertility, epidemics) or well-being of humans (fatigue, stress, etc.) linked directly (air pollution, chemicals, depletion of the ozone layer, noise, etc.) or indirectly (food, genetically modified organisms, etc.) to the quality of the environment.</skos:definition>
		<dct:description xml:lang="en">A descriptive approach to human health and safety will focus on the
  • descriptive geographical distribution of diseases, wellbeing of humans or other health and safety qualities showing geographical patterns, may also include probability descriptions.
  • causes and elements affecting health
  • wellbeing of humans, including quality of the human environment
  • safety issues, behaviour linked to safety
  • health care services

To illustrate kinds of geographical information which can be included in this INSPIRE theme, some examples on medical statistics and medical geography can be given:

General statistics on health - change over time
  • mortality – the number of death in relation to a total population over a given period of time
  • life expectancy – the average number of years newborn children may expect to live if death subsequently occurs in accordance with the mortality for each age group of the population within this period. Life expectancy may also be estimated as the expected remaining time of life at any particular age.
  • Morbidity: incidence of disease in relation to a total population over a given period of time. Morbidity can be described by many different indicators:
    - incidences: the number of new cases in relation to a total population over a given period of time
    - cumulative incidences: the total number of new cases for a longer period of time, e.g. several years, in relation to a total population
    - prevalence: the total number of cases registered in a population at a given time in relation to a total population
    - rate, age-specific rate, age-adjusted rate.
Relevant material on geographical patterns of health is comparison of the major sources of death or illness at different points in time. This can, for instance, illustrate epidemiological transitions, with a fall in infant mortality and infectious disease and a rise in degenerative diseases.

Incidence data on specific diseases or other health issues
Incidences overviews can be split by male/females, age, region or rural-urban sub-division, and data may give opportunities to depict trends over time. Examples which can be treated geographically:
• Kinds of diseases and illnesses: coronary heart disease, stroke, infant mortality, mortality related to cancer, morbidity overview, cardiovascular diseases, musculo-sceletal diseases, mental health problems, injuries, sexually transmitted diseases, infectious diseases.
• Cancer incidence in particular: Cancer comprises a variety of types with different geographical patterns. Incidence data from pubic registers material on age-specific trends, gender variations in a geographical context, incident rates and survival rates: Cancer of the tongue, mouth, throat, stomach, colon, rectum, lunge, prostate, kidney, urinary bladder, malignant melanoma, lymphatic cancer.

Causes of poor or good health – risk factors - exposures
The theme may also include focus on the causes of poor (or good) health. For the purpose of INSPIRE it is convenient to define health in an environmental context, viewing health as a result of an interplay between three factors, man as a biological organism, habitat and behaviour - the human organism's ability to withstand chemical, physical, biological, psychological or social stresses.
• Firstly, it can provide clues about the causes of disease. Although examples of geographical studies leading to basic new knowledge about disease causation are rare, geographical disease patterns may generate hypotheses about causes which can be followed up using other approaches, or suggestions from other research approaches can be tested geographically.
• Secondly, such information can be useful in the planning of strategies for health promotion.
• Thirdly, knowledge about geographical variations in different aspects of health can be useful in health care planning.

Geographical distribution over exposure elements may help understanding links between exposure and health or illness. A causation analysis should include the following two concepts: Risk factor: factor which is known to increase the risk of a disease or other problems: Exposure: to be exposed to a risk factor:
• Exposure to chemical agents in the environment, in air, water, food and soil, has been implicated in numerous adverse effects on humans from cancer to birth effects. E.g. geochemical geographical data may be used in analysis of exposure.
• Among exposures which have been shown to be carcinogenic the following can be mentioned; radioactive and ultraviolet radiation, some chemicals, stimulants such as alcohol and nicotine, food and some occupational factors.
• Two groups of hazardous chemicals – heavy metals and persistent organic pollutants (POPs) are currently receiving particular attention. Further attention should also be given to CMR (cancerogenic, mutagenic and reprotoxic chemicals), PBT (persistent, bioaccumulative, toxic chemicals) and vPvB (very persistent and very bioaccumulative substances), which are substances of special concern according to REACH. Exposure to heavy metals has been linked with developmental retardation various cancers and kidney damage. Exposure with gold and lead has also been associated with the development of auto-immunity. Growing evidence that POPs have serious human health effects.
• Exposure to GMOs in the environment, in air, water, food and soil is currently receiving particular attention since it may potentially cause adverse effects on human health and the environment.

Human well-being:
Human wellbeing may be linked to environmental stress, e.g. noise, heavy traffic, pollution, it may also be reflected in statistics on rates negative wellbeing, e.g. psychiatric problems, alcohol-related causes of illness, social problems or death, health problems or death by traffic accidents, injuries or death by other accidents, suicide in general or firearm suicide as a particular case.

Security
Security may contain issues like peoples' own experience or perception of their security situation, be linked to rates of a long range of indicators e.g. crime rates, or be probability maps for e.g. crime.

Health services
Health services may be interpreted as part of the theme health, as their occurrences and quality in closely linked to health and wellbeing. The issues may reflect public health services in a geographical context, - distribution of e.g. hospitals and similar institutions, medical laboratories or institutions for rehabilitation purposes. Details may be given on distribution, rates, and quality parameters about doctors, nurses, physiotherapists or other practitioners. It may also include services in the form of ambulance services, ambulance regions and other kinds of emergency management systems, where use of GIS have proved to improve performances. Peoples own health care of themselves and their families - by their next of kin – is another important service not commonly being registered.</dct:description>
		<skos:prefLabel xml:lang="bg">Здраве и безопасност на човека</skos:prefLabel>
		<skos:definition xml:lang="bg">Географско разпределение на преобладаващите патологии (алергии, рак, болести на дихателните пътища и др.), информация за въздействието върху човешкото здраве (биомаркери, намаляване на раждаемостта, епидемии) или за физическото състояние на човека (умора, стрес и други), пряко свързани (замърсяване на въздуха, химикали, изтъняване на озоновия слой, шум и др.) или непряко свързани (храна, генетично модифицирани организми и други) с качеството на околната среда.</skos:definition>
		<skos:prefLabel xml:lang="cs">Lidské zdraví a bezpečnost</skos:prefLabel>
		<skos:definition xml:lang="cs">Zeměpisné rozložení převládajícího výskytu patologických stavů (alergií, rakovin, nemocí dýchacího ústrojí atd.), informace o dopadu na zdraví (biomarkery, pokles plodnosti, epidemie) nebo životní podmínky (únava, stres atd.) související přímo (znečištění ovzduší, chemikálie, ztenčování ozonové vrstvy, hluk atd.) nebo nepřímo (potraviny, geneticky modifikované organismy atd.) s kvalitou životního prostředí.</skos:definition>
		<skos:prefLabel xml:lang="da">Sikkerhed</skos:prefLabel>
		<skos:definition xml:lang="da">og sundhed Geografisk fordeling af dominansen af patologier (allergier, kræft, luftvejssygdomme, osv.), oplysninger om indvirkningen på menneskers sundhed (biologiske markører, nedsat frugtbarhed, epidemier) eller trivsel (træthed, stress, osv.), der er direkte (luftforurening, kemikalier, udtynding af ozonlaget, støj, osv.) eller indirekte (fødevarer, genmodificerede organismer, osv.) knyttet til miljøkvaliteten.</skos:definition>
		<skos:prefLabel xml:lang="de">Gesundheit und Sicherheit</skos:prefLabel>
		<skos:definition xml:lang="de">Geografische Verteilung verstärkt auftretender pathologischer Befunde (Allergien, Krebserkrankungen, Erkrankungen der Atemwege usw.), Informationen über Auswirkungen auf die Gesundheit (Biomarker, Rückgang der Fruchtbarkeit, Epidemien) oder auf das Wohlbefinden (Ermüdung, Stress usw.) der Menschen in unmittelbarem Zusammenhang mit der Umweltqualität (Luftverschmutzung, Chemikalien, Abbau der Ozonschicht, Lärm usw.) oder in mittelbarem Zusammenhang mit der Umweltqualität (Nahrung, genetisch veränderte Organismen usw.).</skos:definition>
		<skos:prefLabel xml:lang="el">Ανθρώπινη υγεία και ασφάλεια</skos:prefLabel>
		<skos:definition xml:lang="el">Γεωγραφική κατανομή της κυριαρχίας παθολογιών (αλλεργίες, καρκίνοι, αναπνευστικές ασθένειες, κ.λπ.), πληροφορίες που καταδεικνύουν τις επιπτώσεις στην υγεία (βιοδείκτες, πτώση της γονιμότητας, επιδημίες) ή την ευεξία των ανθρώπων (κούραση, υπερένταση, κ.λπ.) που συνδέονται άμεσα (ατμοσφαιρική ρύπανση, χημικές ουσίες, καταστροφή της στιβάδας του όζοντος, θόρυβος, κ.λπ.) ή έμμεσα (τρόφιμα, γενετικώς τροποποιημένοι οργανισμοί, κ.λπ.) με την ποιότητα του περιβάλλοντος.</skos:definition>
		<skos:prefLabel xml:lang="es">Salud y seguridad humanas</skos:prefLabel>
		<skos:definition xml:lang="es">Distribución geográfica de la dominancia de patologías (alergias, cáncer, enfermedades respiratorias, etc.), la información que indique el efecto sobre la salud (marcadores biológicos, declive de la fertilidad, epidemias) o el bienestar humanos (cansancio, estrés, etc.) directamente vinculada con la calidad del medio ambiente (contaminación del aire, productos químicos, enrarecimiento de la capa de ozono, ruido, etc.) o indirectamente vinculada con dicha calidad (alimentos, organismos modificados genéticamente, etc.).</skos:definition>
		<skos:prefLabel xml:lang="et">Inimeste tervis ja ohutus</skos:prefLabel>
		<skos:definition xml:lang="et">Haiguste (allergiad, vähk, hingamisteede haigused jne) domineerimise geograafiline jaotumine, keskkonna kvaliteediga otseselt (õhusaaste, kemikaalid, osoonikihi kahanemine, müra jne) või kaudselt (toit, geneetiliselt muundatud organismid jne) seotud mõjusid inimeste tervisele (biomarkerid, viljatushaiguste sagenemine, epideemiad) või heaolule (väsimus, stress jne) puudutav teave.</skos:definition>
		<skos:prefLabel xml:lang="fi">Väestön terveys ja turvallisuus</skos:prefLabel>
		<skos:definition xml:lang="fi">Ympäristön laatuun välittömästi (esimerkiksi ilman pilaantuminen, kemikaalit, otsonikerroksen oheneminen, melu) tai välillisesti (esimerkiksi elintarvikkeet, muuntogeeniset organismit) yhteydessä olevien sairauksien (esimerkiksi allergiat, syövät, hengityselinsairaudet) maantieteellinen esiintyminen, tiedot, jotka osoittavat vaikutuksen terveyteen (esimerkiksi biologiset merkkiaineet, hedelmällisyyden väheneminen, epidemiat) tai ihmisten hyvinvointiin (esimerkiksi väsymys, stressi).</skos:definition>
		<skos:prefLabel xml:lang="fr">Santé et sécurité des personnes</skos:prefLabel>
		<skos:definition xml:lang="fr">Répartition géographique des pathologies dominantes (allergies, cancers, maladies respiratoires, etc.) liées directement (pollution de l'air, produits chimiques, appauvrissement de la couche d'ozone, bruit, etc.) ou indirectement (alimentation, organismes génétiquement modifiés, etc.) à la qualité de l'environnement, et ensemble des informations relatif à l'effet de celle-ci sur la santé des hommes (marqueurs biologiques, déclin de la fertilité, épidémies) ou leur bienêtre (fatigue, stress, etc.).</skos:definition>
		<skos:prefLabel xml:lang="hu">Emberi egészség és biztonság</skos:prefLabel>
		<skos:definition xml:lang="hu">A környezet minőségéhez közvetlenül (légszennyezés, vegyszerek, az ózonréteg elvékonyodása, zaj stb.) vagy közvetve (élelmiszer, genetikailag módosított szervezetek stb.) kapcsolódó patológiák (allergiás, daganatos és légúti megbetegedések stb.) dominanciájának földrajzi eloszlása, illetve ezen tényezőknek az emberi egészségre (biomarkerek, termékenységcsökkenés, járványok) vagy jólétre (fáradtság, stressz stb.) gyakorolt hatását jellemző információ.</skos:definition>
		<skos:prefLabel xml:lang="it">Salute umana e sicurezza</skos:prefLabel>
		<skos:definition xml:lang="it">Distribuzione geografica della prevalenza di patologie (allergie, tumori, malattie respiratorie, ecc.), le informazioni contenenti indicazioni sugli effetti relativi alla salute (indicatori biologici, riduzione della fertilità e epidemie) o al benessere degli esseri umani (affaticamento, stress, ecc.) in relazione alla qualità dell’ambiente, sia in via diretta (inquinamento atmosferico, sostanze chimiche, riduzione dello strato di ozono, rumore, ecc.) che indiretta (alimentazione, organismi geneticamente modificati, ecc.).</skos:definition>
		<skos:prefLabel xml:lang="lt">Žmonių sveikata ir sauga</skos:prefLabel>
		<skos:definition xml:lang="lt">Patologijų dominavimo geografinis pasiskirstymas (alergijos, vėžys, kvėpavimo takų ligos ir t. t.), informacija apie poveikį žmonių sveikatai (biomarkeriai, vaisingumo sumažėjimas, epidemijos) ar gerovei (nuovargis, stresas ir t. t.), tiesiogiai (oro tarša, cheminės medžiagos, ozono sluoksnio retėjimas, triukšmas ir t. t.) arba netiesiogiai (maistas, genetiškai modifikuoti organizmai ir t. t.) susijusi su aplinkos kokybe.</skos:definition>
		<skos:prefLabel xml:lang="lv">Cilvēku veselība un drošība</skos:prefLabel>
		<skos:definition xml:lang="lv">Dominējošo patoloģiju (alerģiju, vēža, elpošanas ceļu slimību, utt.) ģeogrāfiskā izplatība, informācija, kas norāda uz ietekmi uz veselību (biomarkeri, auglības mazināšana, epidēmijas) vai cilvēku labklājību (nogurumu, stresu, utt.), kas tieši (gaisa piesārņojums, ķīmiskās vielas, ozona slāņa noplicināšanās, trokšņi, utt.) vai netieši (pārtika, ģenētiski modificēti organismi, utt.) saistīta ar vides kvalitāti.</skos:definition>
		
		<skos:prefLabel xml:lang="mt">Is-saħħa u s-siġurtà tal-bniedem</skos:prefLabel>
		<skos:definition xml:lang="mt">Distribuzzjoni ġeografika tad-dominanza ta' patoloġiji (allerġiji, kankri, mard respiratorju, eċċ.), informazzjoni li tindika l-effett fuq is-saħħa (bijomarkaturi, tnaqqis fil-fertilità, epidemiji) jew il-benesseri tal-bnedmin (għejja, stress, eċċ.) b'konnessjoni diretta (tniġġis ta' l-arja, kimiki, tnaqqis tas-saff ta' l-ożonu, storbju, eċċ.) jew indiretta (ikel, organiżmi ġenetikament modifikati, eċċ.) mal-kwalità ta' l-ambjent.</skos:definition>		
		
		<skos:prefLabel xml:lang="nl">Menselijke gezondheid en veiligheid</skos:prefLabel>
		<skos:definition xml:lang="nl">De geografische spreiding van ziekten (allergieën, kankers, ademhalingsziekten, enz.), informatie over de gevolgen voor de gezondheid (biomarkers, vruchtbaarheidsdaling, epidemieën) of het welzijn van de mens (vermoeidheid, stress, enz.) die direct (luchtvervuiling, chemicaliën, aantasting van de ozonlaag, lawaai, enz.) of indirect (voedsel, genetisch gemodificeerde organismen, enz.) samenhangen met de kwaliteit van het milieu.</skos:definition>
		<skos:prefLabel xml:lang="pl">Zdrowie i bezpieczeństwo ludzi</skos:prefLabel>
		<skos:definition xml:lang="pl">Rozmieszczenie geograficzne występowania patologii chorobowych (alergii, nowotworów, chorób układu oddechowego itd.), informacje dotyczące wpływu na zdrowie (biomarkery, spadek płodności, epidemie) lub dobre samopoczucie ludzi (zmęczenie, stres itd.) związane bezpośrednio (zanieczyszczenie powietrza, chemikalia, zubożenie warstwy ozonowej, hałas itd.) lub pośrednio (pożywienie, organizmy zmodyfikowane genetycznie itd.) z jakością środowiska.</skos:definition>
		<skos:prefLabel xml:lang="pt">Saúde humana e segurança</skos:prefLabel>
		<skos:definition xml:lang="pt">Distribuição geográfica da dominância de patologias (alergias, cancros, doenças respiratórias, etc.), informações que indiquem o efeito da qualidade do ambiente sobre a saúde (biomarcadores, declínio da fertilidade, epidemias) ou sobre o bem-estar dos seres humanos (fadiga, tensão, stress, etc.) de forma directa (poluição do ar, produtos químicos, empobrecimento da camada de ozono, ruído, etc.) ou indirecta (alimentação, organismos geneticamente modificados, etc.).</skos:definition>
		<skos:prefLabel xml:lang="ro">Sănătate şi siguranţă umană</skos:prefLabel>
		<skos:definition xml:lang="ro">Distribuţia geografică a patologiilor dominante (alergii, tipuri de cancer, boli respiratorii etc.), precum şi informaţiile care indică efectul asupra sănătăţii (indicatorii biologici, scăderea fertilităţii, epidemiile) sau asupra bunăstării oamenilor (oboseala, stresul etc.), legat în mod direct (poluarea aerului, substanţele chimice, subţierea stratului de ozon, zgomotul etc.) sau indirect (mâncarea, organismele modificate genetic etc.) de calitatea mediului.</skos:definition>
		<skos:prefLabel xml:lang="sk">Ľudské zdravie a bezpečnosť</skos:prefLabel>
		<skos:definition xml:lang="sk">Geografická distribúcia najčastejších ochorení (alergie, nádorové ochorenia, ochorenia dýchacích ciest atď.), informácie o vplyve na zdravie (biologické ukazovatele, pokles plodnosti, epidémie) alebo telesný či duševný stav ľudí (únava, stres atď.), ktoré priamo (znečistenie ovzdušia, chemikálie, oslabenie ozónovej vrstvy, hluk atď.) alebo nepriamo (strava, geneticky upravené organizmy atď.) súvisia s kvalitou životného prostredia.</skos:definition>
		<skos:prefLabel xml:lang="sl">Zdravje in varnost prebivalstva</skos:prefLabel>
		<skos:definition xml:lang="sl">Geografska razporeditev pogostih patoloških pojavov (alergije, rakasta obolenja, obolenja dihalnih poti itd.), podatki o učinkih na zdravje (biološki označevalci, zmanjšana rodnost, epidemije) ali počutje ljudi (utrujenost, stres itd.), povezanih neposredno (onesnaženost zraka, kemikalije, tanjšanje ozonskega plašča, hrup itd.) ali posredno (hrana, genetsko spremenjeni organizmi itd.) s kakovostjo okolja.</skos:definition>
		<skos:prefLabel xml:lang="sv">Människors hälsa och säkerhet</skos:prefLabel>
		<skos:definition xml:lang="sv">Geografisk fördelning av dominansen av patologier (allergier, cancer, sjukdomar i andningsorganen osv.), all information om de effekter på människors hälsa (biomarkörer, minskad fertilitet, epidemier osv.) eller välbefinnande (trötthet, stress osv.) som har ett direkt (luftföroreningar, kemikalier, uttunning av ozonskiktet, buller osv.) eller ett indirekt (livsmedel, genetiskt modifierade organismer osv.) samband med miljöns kvalitet.</skos:definition>
		<!--
		<skos:prefLabel xml:lang="el">SAMPLE ALTERNATIVE EXPRESSION - αναφορά</skos:prefLabel>
		<skos:definition xml:lang="el">Συστήματα συντεταγμένων</skos:definition>
		<dct:description xml:lang="el">Συστήματα για μονοσήμαντη αναφορά χωρικών πληροφοριών στον χώρο, ως σύνολο συντεταγμένων (x,y,z) ή/και γεωγραφικό πλάτος και μήκος και ύψος, με βάση γεωδαιτικό οριζόντιο και κατακόρυφο σύστημα αναφοράς (datum).</dct:description>
		-->
		<skos:inScheme rdf:resource="http://inspire-registry.jrc.ec.europa.eu/registers/Themes/items"/>
	</inspire:Theme>
	<inspire:Theme rdf:about="http://inspire-registry.jrc.ec.europa.eu/registers/FCD/items/19">
		<!-- <owl:sameIndividualAs rdf:resource="http://www.eionet.europa.eu/gemet/theme_concepts?th=19&ns=5" /> -->
		<inspire:itemStatus>valid</inspire:itemStatus>
		<inspire:dateAccepted>2008-12-05T17:00:30.180+01:00</inspire:dateAccepted>
		<skos:prefLabel xml:lang="en">Utility and governmental services</skos:prefLabel>
		<skos:definition xml:lang="en">Includes utility facilities such as sewage, waste management, energy supply and water supply, administrative and social governmental services such as public administrations, civil protection sites, schools and hospitals.</skos:definition>
		<dct:description xml:lang="en">A very broad INSPIRE theme including different kinds of objects:
Utility services/networks: Physical construction for transport of defined products: These may include pipelines for transport of oil, gas, water, sewage or other pipelines. Transmission lines may include electrical, phone, cable-TV or other networks. Transmission lines for both land and at sea/water (bottom) is important. All kinds of transmission systems have nodes and are linked to facilities for production and treatment of different kinds of products. Despite being heavily interlinked, the themes in INSPIRE are treated separately – the production and treatment facilties are treated mainly in the theme production and industrial facilities. Transmission systems may be of different kinds;
• Oil and gas pipelines: Major lines from oil and gas fields/extraction areas and storage sites. Important production and treatment facilities of such resources is linked to a such a transport network, such as nuclear power stations, power stations, transformer stations and oil tanks. GISCO, Energy/ industry authorities, Companies
• Water pipelines: Location of water pipelines – large and local network. Large transmission lines are of interest here. Linked to production facilities for water for consumption/processes. Irrigation lines treated separately under agricultural facilities. Water supply institutions, Utilities/ health
• Sewage pipelines: Sewage network, linked to sewerage facilities. Major lines of interest here. Utilities
• Transmission lines- electrical: Data set showing larger transmission lines for electricity, both at land and sea. The location of lines is important knowledge for the energy sector itself, land use planners, construction, fisheries for sea cables. Parts of the information important in low flight hindrance databases. Large: national energy/industry institutions. Local authorities, Companies
• Transmission lines-phone/ data/cable-TV: Location of phone/ data: Rough data needed in land planning. Important transmission nodes, e.g. antennas, may be seen as part of the network. The cables placement can conflict other natural resource utilization activities, e.g. fisheries. Technical data accuracy for local level Companies
Rough pipeline and utility service databases exist at European level, e.g. GISCO database with scale 1: 1.000.000. Data within countries is non-homogenous. There are examples of national portals warning on construction, distributing maps/data on location of pipelines. At local and regional level the responsibility of government offices or different operators/ firms. In some countries there are national portals for information about cables etc in construction work.
Waste treatment facilities and waste storage:
It is important to identify the environmental protection facilities with unique identifiers. The data component category coincides with economic/statistical categories (NACE/SERIEE). Location by geographical point, by address or in some cases as area.
• Controlled waste treatment sites for non-hazardous waste at land: geographical location of official or regulated facilities for waste treatment and storage; Included in the spatial component category "environmental protection facilities"
o storage sites at land - landfills
o incinerators
o other treatment facilities
Information on kind of treatment, kind of substances treated, capacity, percentage biodegradable waste, energy recovery from incinerators and landfills
• Controlled waste treatment facilities for hazardous waste at land: geographical location of official or regulated facilities for treatment and storage of hazardous waste; Included in the spatial component category "environmental protection facilities". Reported according to SEVESO II Directive. Distinction between
o thermal treatment,
o landfills
o nuclear waste treatment and storage
o and other treatment for hazardous waste (e.g. chemical),
o other treatment facilities
Information about kind of treatment, kind of substances treated, capacity (and potential risks).
• Regulated areas for dumping of waste at sea: Areas at sea for dumping of waste, e.g. ships, oil drilling platforms, industrial waste, military waste. OSPAR Permits on marine dumping. Reporting per contracting party and site (?) waste category, number of permits issued, tonnes licensed and contracting party. Important in environmental management and management of biological resources at sea. . Submission of data for the Annual OSPAR Report on Dumping of wastes at Sea from OSPAR Convention for the protection of the marine environment of the north-east Atlantic. The anticipated delivery authorities could be sea management/ marine/ waste/ environmental authorities, OSPAR. Included in the spatial data component "area regulation".
Does also include nuclear waste. Example is Russian dumping sites: Official sources states a total of 0.45 PBq of liquid radioactive material has been dumped in the Barents Sea and 0.32 PBq in the Kara Sea. Most of the solid radioactive waste has been dumped along the east coast of Novaja Zemlya and the open Kara Sea. Some material on existing sites and amounts are available.
• Illegal or non-controlled dumping of waste - sea and land. Illegal landfills/"wildfills" on land areas are common, but policies are directed to reduce the number of such storage of waste. It is important in local waste management and pollution control to locate such illegal land fills, in order to carry out targeted actions. Non-controlled areas at sea where waste is recorded is also important, this can be shipwrecks, industrial waste, military waste, cars. OSPAR Permits on marine dumping.
• Mining waste: Mining waste is a special kind of waste. The residues from mining can contain a low content of metals or minerals not being economically extractable, but leaching can cause contamination of soil and water. The tailings of mining activities are usually located near the site of extraction. In management and assessment of mining waste there are needs for spatial data such as location of mines and tailings, water catchments, river network, water and sea, soil.
• Sewage sludge: generation, sewage pipelines network and sewage treatment facilities: Is treated as a group here:
o Sewerage/wastewater treatment facilities, Information on capacity, kind of treatment, category of recipient.
o Sewage networks treated under the data component: utilities.
o Sewage sludge spread to agricultural lands - regulated "permission zones"
o Sewage sludge spread - agricultural lands and soil deposits suitability mapping
Environmental. protection facilities
The theme does also include a specific kind of facilities: Environmental protection facilities include a series communal or private facilities of sewage/ wastewater treatment sites, waste treatment facilities (e.g. incineration , landfills), anti-noise constructions facilities, protection facilities against natural hazards (slide walls, flood walls etc). It is important to identify the environmental protection facilities with unique identifiers. The data component category coincides with economic/statistical categories (NACE/SERIEE). Location by geographical point, by address or in some cases as area.
Examples
• Waste treatment and disposal site - hazardous waste: Waste treatment plants location for hazardous waste. Major distinction between hazardous and non-hazardous waste. Distinction between thermal treatment, landfills and other treatment for hazardous waste (chemical/ radioactive),. incineration, landfills and other treatment for non-hazardous waste. Information about kind of treatment, kind of substances treated, capacity (and potential risks). Waste Directive (Directive 75/442/EEC), Mining Waste Directive (Directive 2006/21/EC), SEVESO II, WFD, MS to DG ENV
• Sewage/ wastewater treatment site: Wastewater treatment facilities, Information on capacity, kind of treatment, category of recipient. Sewage networks treated under the data component: utilities. WFD, MS to DG ENV, local authorities. Facilities defined in Directive 91/271/ECC (urban waste water) / industrial waste may be part of this general category of Sewage/wastewater treatment site.
Natural hazards protection facilities: Any kind of facilities or constructions protecting against natural hazards, e.g. land slide walls, flood walls etc). Hydrographic services, civil security, local authorities.
• Anti-noise constructions: Constructions/walls or other facilities for limiting the spread of noise from road, rail and air traffic, industrial or other noise. For industrial includes modification at the source. Workplace protection excluded. 6EAP
Administrative and social governmental services such as public administrations, civil protection, sites, schools, hospitals. The kinds of sites are commonly presented in governmental and municipal portals and map system as "point of interest"-data, and may be point-based location of a variety of categories of municipal and governmental services and social infrastructure.
• police stations,
• fire fighter stations
• hospitals
• health care centres
• care centres for the elderly
• schools and kindergartens
• renovation/ waste delivery sites
• government and municipal offices</dct:description>
		<skos:prefLabel xml:lang="bg">Комунално-битови и обществени услуги</skos:prefLabel>
		<skos:definition xml:lang="bg">Включват инфраструктура за комунално-битови услуги, например напоителни системи, управление на отпадъците, електроснабдяване и водоснабдяване, административни и социални обществени услуги, например публични администрации, обекти на гражданската защита, училища и болници.</skos:definition>
		<skos:prefLabel xml:lang="cs">Veřejné služby a služby veřejné správy</skos:prefLabel>
		<skos:definition xml:lang="cs">Zahrnují zařízení, jako například kanalizace, nakládání s odpady, zásobování energií a zásobování vodou, správní a sociální státní služby, jako například veřejnou správu, zařízení civilní ochrany, školy a nemocnice.</skos:definition>
		<skos:prefLabel xml:lang="da">Offentlig forsyningsvirksomhed og offentlige tjenesteydelser</skos:prefLabel>
		<skos:definition xml:lang="da">Omfatter forsyningsvirksomhed så som kloakering, affaldshåndtering, energiforsyning og vandforsyning, administrative og sociale offentlige tjenester som f.eks. offentlige administrationer, civilbeskyttelsesanlæg, skoler og hospitaler.</skos:definition>
		<skos:prefLabel xml:lang="de">Versorgungswirtschaft und staatliche Dienste</skos:prefLabel>
		<skos:definition xml:lang="de">Versorgungseinrichtungen wie Abwasser- und Abfallentsorgung, Energieversorgung und Wasserversorgung; staatliche Verwaltungs- und Sozialdienste wie öffentliche Verwaltung, Katastrophenschutz, Schulen und Krankenhäuser.</skos:definition>
		<skos:prefLabel xml:lang="el">Επιχειρήσεις κοινής ωφελείας και κρατικές υπηρεσίες</skos:prefLabel>
		<skos:definition xml:lang="el">Περιλαμβάνονται εγκαταστάσεις υπηρεσιών κοινής ωφελείας, όπως η αποχέτευση, η διαχείριση αποβλήτων, ο ενεργειακός εφοδιασμός και η υδροδότηση, οι διοικητικές και κοινωνικές κρατικές υπηρεσίες, όπως οι δημόσιες διοικήσεις, οι χώροι πολιτικής προστασίας, τα σχολεία και τα νοσοκομεία.</skos:definition>
		<skos:prefLabel xml:lang="es">Servicios de utilidad pública y estatales</skos:prefLabel>
		<skos:definition xml:lang="es">Incluye instalaciones de utilidad pública de alcantarillado, gestión de residuos, suministro de energía y suministro de agua, así como servicios estatales administrativos y sociales tales como administraciones públicas, sitios de protección civil, escuelas y hospitales.</skos:definition>
		<skos:prefLabel xml:lang="et">Kommunaal- ja riiklikud teenused</skos:prefLabel>
		<skos:definition xml:lang="et">Hõlmab tehnorajatisi nagu näiteks reovee ja jäätmete käitluse, energia- ja veevarustuse võrgud ja rajatised ning riiklikke haldus- ja sotsiaalteenuseid nagu riiklikud haldusorganid, kodanikukaitse alad, koolid ja haiglad.</skos:definition>
		<skos:prefLabel xml:lang="fi">Yleishyödylliset ja muut julkiset palvelut</skos:prefLabel>
		<skos:definition xml:lang="fi">Tämä käsittää yleishyödyllisten palvelujen laitokset, kuten viemäröinnin, jätehuollon, energiahuollon ja vesihuollon, sekä hallinnolliset ja sosiaaliset julkiset palvelut, kuten viranomaiset, väestönsuojat, koulut ja sairaalat.</skos:definition>
		<skos:prefLabel xml:lang="fr">Services d'utilité publique et services publics</skos:prefLabel>
		<skos:definition xml:lang="fr">Comprend les installations d'utilité publique, tels que les égouts ou les réseaux et installations liés à la gestion des déchets, à l'approvisionnement énergétique, à l'approvisionnement en eau, ainsi que les services administratifs et sociaux publics, tels que les administrations publiques, les sites de la protection civile, les écoles et les hôpitaux.</skos:definition>
		<skos:prefLabel xml:lang="hu">Közüzemi és közszolgáltatások</skos:prefLabel>
		<skos:definition xml:lang="hu">Magában foglalja az olyan közüzemi létesítményeket, mint például a szennyvíz- és hulladékgazdálkodás, az energiaellátás és a vízellátás, valamint az igazgatási és szociális közszolgáltatásokat, például a közigazgatási szerveket, a polgári védelmi létesítményeket, iskolákat és kórházakat.</skos:definition>
		<skos:prefLabel xml:lang="it">Servizi di pubblica utilità e servizi amministrativi</skos:prefLabel>
		<skos:definition xml:lang="it">Sono compresi sia impianti quali gli impianti fognari, di gestione dei rifiuti, di fornitura energetica, e di distribuzione idrica, sia servizi pubblici amministrativi e sociali quali le amministrazioni pubbliche, i siti della protezione civile, le scuole e gli ospedali.</skos:definition>
		<skos:prefLabel xml:lang="lt">Komunalinės įmonės ir valstybės tarnybos</skos:prefLabel>
		<skos:definition xml:lang="lt">Tai apima komunalinių įmonių infrastruktūrą, pavyzdžiui, kanalizaciją, atliekų tvarkymą, elektros energijos tiekimą ir vandens tiekimą, administracines ir socialines valstybės tarnybas, pavyzdžiui, viešojo administravimo įstaigas, civilinės saugos tarnybas, mokyklas ir ligonines.</skos:definition>
		<skos:prefLabel xml:lang="lv">Komunālie un valsts dienesti</skos:prefLabel>
		<skos:definition xml:lang="lv">Tas ietver tādu komunālo dienestu iekārtas kā kanalizācija, atkritumu apsaimniekošana, energoapgāde un ūdens apgāde, administratīvos un sociālos valsts dienestus, piemēram, valsts administrāciju, civilās aizsardzības novietnes, skolas un slimnīcas.</skos:definition>
		
		<skos:prefLabel xml:lang="mt">Servizzi ta' utilità u tal-gvern</skos:prefLabel>
		<skos:definition xml:lang="mt">Jinkludu faċilitajiet ta' utilità bħad-drenaġġ, l-immaniġġar ta' l-iskart, il-provvista ta' l-enerġija, il-provvista ta' l-ilma, isservizzi amministrattivi u soċjali tal-gvern bħal amministrazzjonijiet pubbliċi, siti għall-protezzjoni ċivili, skejjel u sptarijiet.</skos:definition>		
		
		<skos:prefLabel xml:lang="nl">Nutsdiensten en overheidsdiensten</skos:prefLabel>
		<skos:definition xml:lang="nl">Nutsvoorzieningen zoals riolering, afvalbeheer, energievoorziening, watervoorziening, bestuurlijke en maatschappelijke instanties van de overheid, zoals bestuurlijke overheden, civiele bescherming, scholen en ziekenhuizen.</skos:definition>
		<skos:prefLabel xml:lang="pl">Usługi użyteczności publicznej i służby państwowe</skos:prefLabel>
		<skos:definition xml:lang="pl">Obejmuje instalacje użyteczności publicznej takie jak: kanalizacja, zarządzanie odpadami, dostawa energii i dostawa wody, administracyjne i społeczne służby państwowe lub samorządowe, takie jak: administracja publiczna, obiekty ochrony cywilnej, szkoły i szpitale.</skos:definition>
		<skos:prefLabel xml:lang="pt">Serviços de utilidade pública e do Estado</skos:prefLabel>
		<skos:definition xml:lang="pt">Inclui instalações e serviços de utilidade pública, como redes de esgotos, gestão de resíduos, fornecimento de energia, abastecimento de água, serviços administrativos e sociais do Estado tais como administrações públicas, instalações da protecção civil, escolas e hospitais.</skos:definition>
		<skos:prefLabel xml:lang="ro">Servicii de utilitate publică şi servicii publice</skos:prefLabel>
		<skos:definition xml:lang="ro">Includ instalaţiile de utilitate publică, precum sistemele de canalizare, de gestionare a deşeurilor, de aprovizionare cu energie electrică şi apă, şi serviciile administrative şi sociale publice, precum adăposturile de protecţie civilă, şcolile şi spitalele.</skos:definition>
		<skos:prefLabel xml:lang="sk">Verejné a štátne služby</skos:prefLabel>
		<skos:definition xml:lang="sk">Patria sem verejné zariadenia, ako napríklad kanalizácia, nakladanie s odpadom, dodávka energie a dodávka vody, administratívne a sociálne štátne služby, ako napríklad verejná správa, miesta civilnej ochrany, školy a nemocnice.</skos:definition>
		<skos:prefLabel xml:lang="sl">Komunalne in javne storitve</skos:prefLabel>
		<skos:definition xml:lang="sl">Vključuje komunalne naprave kot so kanalizacija, ravnanje z odpadki, oskrba z energijo in preskrba z vodo, upravne in socialne vladne službe kot so javne uprave, sedeži civilne zaščite, šole in bolnišnice.</skos:definition>
		<skos:prefLabel xml:lang="sv">Allmännyttiga och offentliga tjänster</skos:prefLabel>
		<skos:definition xml:lang="sv">Inbegriper anläggningar för allmännyttiga tjänster, exempelvis för hantering av avloppsvatten, avfallshantering, energiförsörjning och vattenförsörjning, administrativa och sociala offentliga tjänster såsom offentliga förvaltningar, räddningstjänstens anläggningar, skolor och sjukhus.</skos:definition>
		<!--
		<skos:prefLabel xml:lang="el">SAMPLE ALTERNATIVE EXPRESSION - αναφορά</skos:prefLabel>
		<skos:definition xml:lang="el">Συστήματα συντεταγμένων</skos:definition>
		<dct:description xml:lang="el">Συστήματα για μονοσήμαντη αναφορά χωρικών πληροφοριών στον χώρο, ως σύνολο συντεταγμένων (x,y,z) ή/και γεωγραφικό πλάτος και μήκος και ύψος, με βάση γεωδαιτικό οριζόντιο και κατακόρυφο σύστημα αναφοράς (datum).</dct:description>
		-->
		<skos:inScheme rdf:resource="http://inspire-registry.jrc.ec.europa.eu/registers/Themes/items"/>
	</inspire:Theme>
	<inspire:Theme rdf:about="http://inspire-registry.jrc.ec.europa.eu/registers/FCD/items/20">
		<!-- <owl:sameIndividualAs rdf:resource="http://www.eionet.europa.eu/gemet/theme_concepts?th=20&ns=5" /> -->
		<inspire:itemStatus>valid</inspire:itemStatus>
		<inspire:dateAccepted>2008-12-05T17:00:30.239+01:00</inspire:dateAccepted>
		<skos:prefLabel xml:lang="en">Environmental monitoring facilities</skos:prefLabel>
		<skos:definition xml:lang="en">Location and operation of environmental monitoring facilities includes observation and measurement of emissions, of the state of environmental media and of other ecosystem parameters (biodiversity, ecological conditions of vegetation, etc.) by or on behalf of public authorities.</skos:definition>
		<dct:description xml:lang="en">Environmental monitoring facilities are facilities for observations and measurements of emissions, status and effects of environmental media (e.g. air, forest, marine water) and/or other environmental aspects (e.g. biodiversity, human health. The concept of monitoring may relate to systematic and hierarchical structures, including monitoring networks, monitoring stations, monitoring site and subsites. The monitoring sites may be permanently located at a site or can be temporal, only used for a certain time. Continuous moving monitoring facilities, e.g. on ships, may be a kind of monitoring facility. Monitoring sites in the form of locations and areas can be reported as georeferenced points, lines and polygons. In cases where data are classified or confidential, aggregation to grids may be a possibility. It is problematic that the definition of the theme refers to the kinds of delivery organisations to supply data, as the INSPIRE Directive in specific paragraphs defines for which organisations the directive is valid.</dct:description>
		<skos:prefLabel xml:lang="bg">Съоръжения за управление на околната среда</skos:prefLabel>
		<skos:definition xml:lang="bg">Местонахождението и действието на съоръжения за мониторинг на околната среда включват наблюдение и измерване на емисиите, на състоянието на факторите на околната среда и на други параметри на екосистемата (биологично разнообразие, екологични условия на флората и други), извършвани от публичните власти или от тяхно име.</skos:definition>
		<skos:prefLabel xml:lang="cs">Zařízení pro sledování životního prostředí</skos:prefLabel>
		<skos:definition xml:lang="cs">Rozmístění a provoz zařízení pro sledování životního prostředí zahrnuje pozorování a měření emisí, stavu složek životního prostředí a dalších ukazatelů ekosystému (druhové rozmanitosti, ekologických podmínek rostlinstva atd.) orgány veřejné správy nebo jejich jménem.</skos:definition>
		<skos:prefLabel xml:lang="da">Miljøovervågningsfaciliteter</skos:prefLabel>
		<skos:definition xml:lang="da">Lokalisering og drift af miljøovervågningsfaciliteter omfatter observation og måling af emissioner, af miljøelementernes tilstand og af andre økosystemparametre (biodiversitet, plantevækstens økologiske betingelser, osv.) foretaget af eller på vegne af offentlige myndigheder.</skos:definition>
		<skos:prefLabel xml:lang="de">Umweltüberwachung</skos:prefLabel>
		<skos:definition xml:lang="de">Standort und Betrieb von Umweltüberwachungseinrichtungen einschließlich Beobachtung und Messung von Schadstoffen, des Zustands von Umweltmedien und anderen Parametern des Ökosystems (Artenvielfalt, ökologischer Zustand der Vegetation usw.) durch oder im Auftrag von öffentlichen Behörden.</skos:definition>
		<skos:prefLabel xml:lang="el">Εγκαταστάσεις παρακολούθησης του περιβάλλοντος</skos:prefLabel>
		<skos:definition xml:lang="el">Η τοποθεσία και η λειτουργία των εγκαταστάσεων παρακολούθησης του περιβάλλοντος περιλαμβάνει την παρατήρηση και τη μέτρηση των εκπομπών, της κατάστασης των στοιχείων του περιβάλλοντος και άλλων παραμέτρων του οικοσυστήματος (βιοποικιλότητα, οικολογική κατάσταση της βλάστησης, κ.λπ.) από τις δημόσιες αρχές ή για λογαριασμό τους.</skos:definition>
		<skos:prefLabel xml:lang="es">Instalaciones de observación del medio ambiente</skos:prefLabel>
		<skos:definition xml:lang="es">La ubicación y funcionamiento de instalaciones de observación del medio ambiente, encargadas de observar y medir emisiones, el estado del medio ambiente y otros parámetros del ecosistema (biodiversidad, condiciones ecológicas de la vegetación, etc.), por parte de las autoridades públicas o en nombre de ellas.</skos:definition>
		<skos:prefLabel xml:lang="et">Keskkonnaseirerajatised</skos:prefLabel>
		<skos:definition xml:lang="et">Keskkonnaseirerajatiste asukoht ja kasutamine hõlmab heidete, keskkonnaelementide seisundi ja muude ökosüsteemi parameetrite (bioloogilise mitmekesisuse, taimkatte ökoloogiliste tingimuste jne) vaatlust ja mõõtmist avaliku võimu kandjate poolt või nende nimel.</skos:definition>
		<skos:prefLabel xml:lang="fi">Ympäristön tilan seurantalaitteet</skos:prefLabel>
		<skos:definition xml:lang="fi">Ympäristön tilan seurantalaitteiden sijaintiin ja käyttöön kuuluu päästöjen, ilman, maaperän ja veden tilan ja muiden ekosysteemin muuttujien (luonnon monimuotoisuus, kasviston ekologiset olot jne.) seuranta ja mittaukset, joista vastaavat viranomaiset tai muut toimijat viranomaisten puolesta.</skos:definition>
		<skos:prefLabel xml:lang="fr">Installations de suivi environnemental</skos:prefLabel>
		<skos:definition xml:lang="fr">La situation et le fonctionnement des installations de suivi environnemental comprennent l'observation et la mesure des émissions, de l'état du milieu environnemental et d'autres paramètres de l'écosystème (biodiversité, conditions écologiques de la végétation, etc.) par les autorités publiques ou pour leur compte.</skos:definition>
		<skos:prefLabel xml:lang="hu">Környezetvédelmi monitoringlétesítmények</skos:prefLabel>
		<skos:definition xml:lang="hu">A környezetvédelmi monitoringlétesítmények elhelyezkedése és működése magában foglalja a kibocsátásnak, a környezeti elemek állapotának, valamint az ökoszisztéma egyéb paramétereinek (biodiverzitás, a növényzet ökológiai állapota stb.) a hatóságok általi vagy a nevükben történő megfigyelését és mérését.</skos:definition>
		<skos:prefLabel xml:lang="it">Impianti di monitoraggio ambientale</skos:prefLabel>
		<skos:definition xml:lang="it">L'ubicazione e il funzionamento degli impianti di monitoraggio ambientale comprendono l'osservazione e la misurazione delle emissioni, dello stato dei comparti ambientali e di altri parametri dell'ecosistema (biodiversità, condizioni ecologiche della vegetazione, ecc.) da parte o per conto delle autorità pubbliche.</skos:definition>
		<skos:prefLabel xml:lang="lt">Aplinkos stebėsenos priemonės</skos:prefLabel>
		<skos:definition xml:lang="lt">Aplinkos stebėsenos priemonių vieta ir veikla, įskaitant valdžios institucijų arba jų vardu atliekamą išmetamų teršalų, aplinkos terpių būklės ir kitų ekosistemos parametrų (biologinės įvairovės, ekologinių augalijos sąlygų ir t. t.) stebėjimą ir matavimą.</skos:definition>
		<skos:prefLabel xml:lang="lv">Vides monitoringa iekārtas</skos:prefLabel>
		<skos:definition xml:lang="lv">Vides monitoringa iekārtu atrašanās vietas un pārvaldība, kas ietver emisiju, apkārtējās vides stāvokļa un citu ekosistēmas parametru (bioloģiskās daudzveidības, veģetācijas ekoloģisko apstākļu, utt.) novērošanu un mērīšanu, ko veic publiskās iestādes vai publisko iestāžu vārdā.</skos:definition>
		
		<skos:prefLabel xml:lang="mt">Faċilitajiet ta' monitoraġġ ambjentali</skos:prefLabel>
		<skos:definition xml:lang="mt">Posizzjoni u operazzjoni ta' faċilitajiet ta' monitoraġġ ambjentali jinkludi l-osservazzjoni u l-kejl ta' emissjonijiet, ta' listat tal-medji ambjentali u ta' parametri oħra ta' l-ekosistema (biodiversità, kondizzjonijiet ekoloġiċi ta' veġetazzjoni, eċċ.) permezz jew f'isem l-awtoritajiet pubbliċi.</skos:definition>		
		
		<skos:prefLabel xml:lang="nl">Milieubewakingsvoorzieningen</skos:prefLabel>
		<skos:definition xml:lang="nl">Locatie en werking van milieubewakingsvoorzieningen, met inbegrip van waarneming en meting van emissies, de staat van de milieucompartimenten en van andere ecosysteemparameters (biodiversiteit, ecologische omstandigheden van vegetatie, enz.) door of namens de overheidsinstanties.</skos:definition>
		<skos:prefLabel xml:lang="pl">Urządzenia do monitorowania środowiska</skos:prefLabel>
		<skos:definition xml:lang="pl">Lokalizacja i funkcjonowanie urządzeń do monitorowania środowiska obejmują obserwację i pomiary emisji, stanu zasobów środowiska i innych parametrów ekosystemu (różnorodności biologicznej, warunków ekologicznych wegetacji itd.) przez organy publiczne lub w ich imieniu.</skos:definition>
		<skos:prefLabel xml:lang="pt">Instalações de monitorização do ambiente</skos:prefLabel>
		<skos:definition xml:lang="pt">A localização e funcionamento de instalações de monitorização do ambiente inclui a observação e medição de emissões, do estado das diferentes componentes ambientais e de outros parâmetros dos ecossistemas (biodiversidade, condições ecológicas da vegetação, etc.) pelas autoridades públicas ou por conta destas.</skos:definition>
		<skos:prefLabel xml:lang="ro">Instalaţii de supraveghere a mediului</skos:prefLabel>
		<skos:definition xml:lang="ro">Amplasarea şi exploatarea instalaţiilor de supraveghere a mediului implică observarea şi măsurarea emisiilor, a stării mediului înconjurător şi a altor parametri ai ecosistemului (biodiversitate, condiţii ecologice ale vegetaţiei etc.) de către sau în numele autorităţilor publice.</skos:definition>
		<skos:prefLabel xml:lang="sk">Zariadenia na monitorovanie životného prostredia</skos:prefLabel>
		<skos:definition xml:lang="sk">Poloha a prevádzka zariadení na monitorovanie životného prostredia zahŕňa pozorovanie a meranie emisií, stavu zložiek životného prostredia a iných parametrov ekosystému (biodiverzity, ekologických podmienok vegetácie, atď.) vykonávané orgánmi verejnej moci alebo v ich mene.</skos:definition>
		<skos:prefLabel xml:lang="sl">Naprave in objekti za monitoring okolja</skos:prefLabel>
		<skos:definition xml:lang="sl">Nahajanje in delovanje naprav in objektov za spremljanje okolja vključuje opazovanje in merjenje emisij, stanja okolja in drugih parametrov ekosistema (biološka raznolikost, ekološki pogoji vegetacije itd.) s strani javnih organov ali v njihovem imenu.</skos:definition>
		<skos:prefLabel xml:lang="sv">Anläggningar för miljöövervakning</skos:prefLabel>
		<skos:definition xml:lang="sv">Placering och användning av anläggningar för miljöövervakning inbegriper iakttagelse och mätning av utsläpp, av situationen när det gäller miljömedier och av andra parametrar för ekosystemet (biologisk mångfald, ekologiska villkor för växtligheten etc.) som genomförs av offentliga myndigheter eller för deras räkning.</skos:definition>
		<!--
		<skos:prefLabel xml:lang="el">SAMPLE ALTERNATIVE EXPRESSION - αναφορά</skos:prefLabel>
		<skos:definition xml:lang="el">Συστήματα συντεταγμένων</skos:definition>
		<dct:description xml:lang="el">Συστήματα για μονοσήμαντη αναφορά χωρικών πληροφοριών στον χώρο, ως σύνολο συντεταγμένων (x,y,z) ή/και γεωγραφικό πλάτος και μήκος και ύψος, με βάση γεωδαιτικό οριζόντιο και κατακόρυφο σύστημα αναφοράς (datum).</dct:description>
		-->
		<skos:inScheme rdf:resource="http://inspire-registry.jrc.ec.europa.eu/registers/Themes/items"/>
	</inspire:Theme>
	<inspire:Theme rdf:about="http://inspire-registry.jrc.ec.europa.eu/registers/FCD/items/21">
		<!-- <owl:sameIndividualAs rdf:resource="http://www.eionet.europa.eu/gemet/theme_concepts?th=21&ns=5" /> -->
		<inspire:itemStatus>valid</inspire:itemStatus>
		<inspire:dateAccepted>2008-12-05T17:00:30.297+01:00</inspire:dateAccepted>
		<skos:prefLabel xml:lang="en">Production and industrial facilities</skos:prefLabel>
		<skos:definition xml:lang="en">Industrial production sites, including installations covered by Council Directive 96/61/EC of 24 September 1996 concerning integrated pollution prevention and control (1) and water abstraction facilities, mining, storage sites.</skos:definition>
		<dct:description xml:lang="en">Location of production industry, mines, waste/disposal sites and energy production facilities. Concerning industry these may be chemical, hydrocarbons (oil-gas), mines or any other industry. Usage of PRTR categories as common nomenclature for such facilities is relevant as it comprises a very broad set relevant industrial activities. The categorisation may be mapped to other international categorisation systems like NACE, SERIEE or ISIC.
The definition mentions also water abstraction, mining and storage sites. The latter may be storage sites for different kinds of "products" needed as input in industrial/production processes, or may be seen as storage sites for real products and also form "waste" from the production process.
The theme production and industrial facilities" must be seen as one of several thematic groups of "facilities" such as
- utility and government services
- environmental monitoring facilities
- agriculture and aquaculture facilities
The IMS paper (INSPIRE IMS, 2003) contained a different sub-grouping of utilities and facilities with the groups transmission lines and pipelines, environmental protection facilities, production facilities, industry, agricultural facilities, trade and service facilities. The first and last in the IMS is not mentioned as separate themes in the draft Directive text, neither is the environmental protection facility. Two new themes have been introduced: "Utility and governmental services" and "Environmental monitoring facilities".
The definition includes a reference to the IPPC directive. IPPC Directive (Directive 96/61/EC) describes the European Emission Register (EPER) in Art 15 (3). This Directive and the clauses have been affected, as the PRTR Regulation (Regulation (EG) Nr. 166/2006 of 18.01.2006) has become effective. This Regulation establishes an integrated pollutant release and transfer register at Community level (PRTR) - and it deletes (among others) Art. 15 (3) of the IPPC Directive.
Kinds of production/industry facilities:
Industrial sites: Agglomerations and individual localisation of major industry, including chemical, hydrocarbon refineries, forestry, fisheries etc. Id on firm/site. SEVESO II
Nuclear installation location: Will be used as a reference point for discharges from Nuclear Installations. Reporting on each production unit: Submission of data for the Annual Report on Liquid Discharges from Nuclear Installations from OSPAR Convention for the protection of the marine environment of the North-East Atlantic Ocean. This is a legal obligation for the following nations: Belgium, Denmark, France, Germany, Norway, Portugal, Spain, Sweden, Switzerland, the Netherlands, and United Kingdom. Not necessarily reporting on geographical location, but unit name/address or other id could link information to a geographical location. OSPAR/ HELCOM
Energy resource extraction and production site: Localisation of energy production sites for production of heat, electricity, oil and gas. The sites may include extraction sites, e.g. for oil and gas (platforms), hydropower stations, nuclear power plants, The sites also includes the distribution facilities for energy, storage sites, but not the network (See data component utilities).
Mines: Individual localisation of mines or generalised mining areas, including storage sites, landfills, sedimentation dams etc.</dct:description>
		<skos:prefLabel xml:lang="bg">Производствени и промишлени съоръжения</skos:prefLabel>
		<skos:definition xml:lang="bg">Промишлени обекти, включително инсталации, обхванати от Директива 96/61/ЕО на Съвета от 24 септември 1996 г. за комплексно предотвратяване и контрол на замърсяването (1), и съоръжения за водочерпене, минни съоръжения, складови обекти.</skos:definition>
		<skos:prefLabel xml:lang="cs">Výrobní a průmyslová zařízení</skos:prefLabel>
		<skos:definition xml:lang="cs">Místa s průmyslovou výrobou, včetně zařízení, na která se vztahuje směrnice Rady 96/61/ES ze dne 24. září 1996 o integrované prevenci a omezování znečištění (1), a zařízení na jímání vody, těžbu, skladiště a úložiště.</skos:definition>
		<skos:prefLabel xml:lang="da">Produktions- og industrifaciliteter</skos:prefLabel>
		<skos:definition xml:lang="da">Industrielle produktionsanlæg, herunder de anlæg, der er omfattet af Rådets direktiv 96/61/EF af 24. september 1996 om forebyggelse og bekæmpelse af forurening (1), og vandudvindingsanlæg, miner, oplagspladser.</skos:definition>
		<skos:prefLabel xml:lang="de">Produktions- und Industrieanlagen</skos:prefLabel>
		<skos:definition xml:lang="de">Standorte für industrielle Produktion, einschließlich durch die Richtlinie 96/61/EG des Rates vom 24. September 1996 über die integrierte Vermeidung und Verminderung der Umweltverschmutzung (1) erfasste Anlagen und Einrichtungen zur Wasserentnahme sowie Bergbau- und Lagerstandorte.</skos:definition>
		<skos:prefLabel xml:lang="el">Εγκαταστάσεις παραγωγής και βιομηχανικές εγκαταστάσεις</skos:prefLabel>
		<skos:definition xml:lang="el">Τοποθεσίες βιομηχανικής παραγωγής, συμπεριλαμβανομένων των εγκαταστάσεων που καλύπτονται από την οδηγία 96/61/ΕΚ του Συμβουλίου, της 24ης Σεπτεμβρίου 1996, σχετικά με την ολοκληρωμένη πρόληψη και έλεγχο της ρύπανσης (1), και εγκαταστάσεις υδροληψίας, εξόρυξης, χώροι αποθήκευσης.</skos:definition>
		<skos:prefLabel xml:lang="es">Instalaciones de producción e industriales</skos:prefLabel>
		<skos:definition xml:lang="es">Centros de producción industrial, incluidas las instalaciones contempladas en la Directiva 96/61/CE del Consejo, de 24 de septiembre de 1996, sobre la prevención y el control integrado de la contaminación (1), e instalaciones de extracción de agua, instalaciones mineras, centros de almacenamiento.</skos:definition>
		<skos:prefLabel xml:lang="et">Tootmis- ja tööstusrajatised</skos:prefLabel>
		<skos:definition xml:lang="et">Tööstusliku tootmise asukohad, sealhulgas nõukogu 24. septembri 1996. aasta direktiiviga 96/61/EÜ saastuse kompleksse vältimise ja kontrolli kohta (1) hõlmatud rajatised ning veevõtukohad, kaevandused ja ladustamiskohad.</skos:definition>
		<skos:prefLabel xml:lang="fi">Tuotanto- ja teollisuuslaitokset</skos:prefLabel>
		<skos:definition xml:lang="fi">Teollisuusalueet, mukaan luettuina ympäristön pilaantumisen ehkäisemisen ja vähentämisen yhtenäistämiseksi 24 päivänä syyskuuta 1996 annetun neuvoston direktiivin 96/61/EY (1) soveltamisalaan kuuluvat laitokset sekä vedenottamot, kaivokset ja varastoalueet.</skos:definition>
		<skos:prefLabel xml:lang="fr">Lieux de production et sites industriels</skos:prefLabel>
		<skos:definition xml:lang="fr">Sites de production industrielle, y compris les installations couvertes par la directive 96/61/CE du Conseil du 24 septembre 1996 relative à la prévention et à la réduction intégrées de la pollution (1) et les installations de captage d'eau, d'extraction minière et de stockage.</skos:definition>
		<skos:prefLabel xml:lang="hu">Termelő és ipari létesítmények</skos:prefLabel>
		<skos:definition xml:lang="hu">Ipari termelőhelyek, beleértve a környezetszennyezés integrált megelőzéséről és csökkentéséről szóló, 1996. szeptember 24-i 96/61/EK tanácsi irányelv (1) által szabályozott berendezéseket, valamint a vízkivételt, a bányászati és a tárolólétesítményeket.</skos:definition>
		<skos:prefLabel xml:lang="it">Produzione e impianti industriali</skos:prefLabel>
		<skos:definition xml:lang="it">Siti di produzione industriale; compresi gli impianti di cui alla direttiva 96/61/CE del Consiglio, del 24 settembre 1996, sulla prevenzione e la riduzione integrate dell'inquinamento (1) e gli impianti di estrazione dell’acqua, le attività estrattive e i siti di stoccaggio.</skos:definition>
		<skos:prefLabel xml:lang="lt">Gamybos ir pramonės įrenginiai</skos:prefLabel>
		<skos:definition xml:lang="lt">Pramoninės gamybos įmonės, įskaitant įrenginius, kuriems taikoma 1996 m. rugsėjo 24 d. Tarybos direktyva 96/61/EB dėl taršos integruotos prevencijos ir kontrolės (1), ir vandens ėmimo įmones, kasybos, sandėliavimo vietas.</skos:definition>
		<skos:prefLabel xml:lang="lv">Ražošanas un rūpniecības iekārtas</skos:prefLabel>
		<skos:definition xml:lang="lv">Rūpniecības ražošanas novietnes, tostarp iekārtas, kas iekļautas Padomes Direktīvā 96/61/EK (1996. gada 24. septembris) par piesārņojuma integrētu novēršanu un kontroli (1), un iekārtas, ko izmanto ūdens ņemšanai, kalnrūpniecībā vai uzglabāšanai.</skos:definition>
		
		<skos:prefLabel xml:lang="mt">Faċilitajiet ta' produzzjoni u industrijali</skos:prefLabel>
		<skos:definition xml:lang="mt">Siti ta' produzzjoni industrijali, inklużi installazzjonijiet koperti mid-Direttiva tal-Kunsill 96/61/KE ta' l- 24 ta' Settembru 1996 dwar il-prevenzjoni u l-kontroll integrat tat-tniġġis (1) u faċilitajiet ta' astrazzjoni ta' l-ilma, tħaffir ta' minjieri, siti ta' ħażna.</skos:definition>		
		
		<skos:prefLabel xml:lang="nl">Faciliteiten voor productie en industrie</skos:prefLabel>
		<skos:definition xml:lang="nl">Industriële productievestigingen, met inbegrip van installaties die onder Richtlijn 96/61/EG van de Raad van 24 september 1996 inzake geïntegreerde preventie en bestrijding van verontreiniging (1) vallen en waterontrekkingsfaciliteiten, mijnbouw, opslagplaatsen.</skos:definition>
		<skos:prefLabel xml:lang="pl">Obiekty produkcyjne i przemysłowe</skos:prefLabel>
		<skos:definition xml:lang="pl">Zakłady przemysłowe, w tym obiekty objęte dyrektywą 96/61/WE z dnia 24 września 1996 r. dotycząca zintegrowanego zapobiegania zanieczyszczeniom i ich kontroli (1) oraz urządzenia poboru wody, miejsca wydobycia i składowiska.</skos:definition>
		<skos:prefLabel xml:lang="pt">Instalações industriais e de produção</skos:prefLabel>
		<skos:definition xml:lang="pt">Locais de produção industrial, incluindo instalações abrangidas pela Directiva 96/61/CE do Conselho, de 24 de Setembro de 1996, relativa à prevenção e controlo integrados da poluição (1), e instalações de captação de água, minas, locais de armazenagem.</skos:definition>
		<skos:prefLabel xml:lang="ro">Instalaţii de producţie şi industriale</skos:prefLabel>
		<skos:definition xml:lang="ro">Parcuri de producţie industrială, inclusiv instalaţiile reglementate de Directiva 96/61/CE a Consiliului din 24 septembrie 1996 privind prevenirea şi controlul integrat al poluării (1), precum şi instalaţiile de captare a apei, de extracţie minieră şi locurile de depozitare.</skos:definition>
		<skos:prefLabel xml:lang="sk">Výrobné a priemyselné zariadenia</skos:prefLabel>
		<skos:definition xml:lang="sk">Priemyselné výrobné podniky vrátane zariadení, na ktoré sa vzťahuje smernica Rady 96/61/ES z 24. septembra 1996 o integrovanej prevencii a kontrole znečisťovania životného prostredia (1), a zariadenia na čerpanie vody, bane, sklady.</skos:definition>
		<skos:prefLabel xml:lang="sl">Proizvodni in industrijski objekti in naprave</skos:prefLabel>
		<skos:definition xml:lang="sl">Območja za industrijsko proizvodnjo, vključno z obrati, ki jih zajema Direktiva Sveta 96/61/ES z dne 24. septembra 1996 o celovitem preprečevanju in nadzorovanju onesnaževanja (1) ter objekti in napravami za odvzem vode, rudniki, skladišči.</skos:definition>
		<skos:prefLabel xml:lang="sv">Produktions- och industrianläggningar</skos:prefLabel>
		<skos:definition xml:lang="sv">Industriella produktionsställen, inbegripet anläggningar som omfattas av rådets direktiv 96/61/EG av den 24 september 1996 om samordnande åtgärder för att förebygga och begränsa föroreningar (1) samt vattenverk, gruvor och upplagsplatser.</skos:definition>
		<!--
		<skos:prefLabel xml:lang="el">SAMPLE ALTERNATIVE EXPRESSION - αναφορά</skos:prefLabel>
		<skos:definition xml:lang="el">Συστήματα συντεταγμένων</skos:definition>
		<dct:description xml:lang="el">Συστήματα για μονοσήμαντη αναφορά χωρικών πληροφοριών στον χώρο, ως σύνολο συντεταγμένων (x,y,z) ή/και γεωγραφικό πλάτος και μήκος και ύψος, με βάση γεωδαιτικό οριζόντιο και κατακόρυφο σύστημα αναφοράς (datum).</dct:description>
		-->
		<skos:inScheme rdf:resource="http://inspire-registry.jrc.ec.europa.eu/registers/Themes/items"/>
	</inspire:Theme>
	<inspire:Theme rdf:about="http://inspire-registry.jrc.ec.europa.eu/registers/FCD/items/22">
		<!-- <owl:sameIndividualAs rdf:resource="http://www.eionet.europa.eu/gemet/theme_concepts?th=22&ns=5" /> -->
		<inspire:itemStatus>valid</inspire:itemStatus>
		<inspire:dateAccepted>2008-12-05T17:00:30.361+01:00</inspire:dateAccepted>
		<skos:prefLabel xml:lang="en">Agricultural and aquaculture facilities</skos:prefLabel>
		<skos:definition xml:lang="en">Farming equipment and production facilities (including irrigation systems, greenhouses and stables).</skos:definition>
		<dct:description xml:lang="en">Agricultural facilities: The farming facilities are constructions used in agricultural production. Agriculture is defined to include cropping of annual crops or perennials and rearing/ breeding of animals. Forestry in general is probably not included, but intensive forestry plantations on former fields may be included? Facilities can be classified according to the NACE1.1 used in official statistics when relevant. The ISIC system for classification of industrial sites may also be relevant. Examples of farming productions facilities are irrigation systems, greenhouses, stables, tanks and pipelines. The definition of a facility should be clarified, e.g. if facilities such as wall systems for prevention of erosion, channel systems used in irrigation, terrace systems used for fruit production are constructions outside the scope of a "facility".
Aquaculture facilities: Productions and treatment facilities for fish, mussels, seaweed and other kinds of aquaculture. Aquaculture does only include permanent or semi-permanent systems for breeding of the organisms, and does not include locations for catching animals or plants in their natural environment. Aquaculture facilities may exist both in marine waters, inland water environments and as terrestrial production systems.</dct:description>
		<skos:prefLabel xml:lang="bg">Селскостопански и водностопански съоръжения</skos:prefLabel>
		<skos:definition xml:lang="bg">Оборудване за селски стопанства и производствени мощности (включително поливни системи, парници и обори).</skos:definition>
		<skos:prefLabel xml:lang="cs">Zemědělská a akvakulturní zařízení</skos:prefLabel>
		<skos:definition xml:lang="cs">Vybavení a zařízení zemědělské výroby (včetně zavlažovacích systémů, skleníků a stájí).</skos:definition>
		<skos:prefLabel xml:lang="da">Landbrugs- og akvakulturanlæg</skos:prefLabel>
		<skos:definition xml:lang="da">Landbrugsudstyr og -produktionsanlæg (herunder vandingssystemer, drivhuse og stalde).</skos:definition>
		<skos:prefLabel xml:lang="de">Landwirtschaftliche Anlagen und Aquakulturanlagen</skos:prefLabel>
		<skos:definition xml:lang="de">Landwirtschaftliche Anlagen und Produktionsstätten (einschließlich Bewässerungssystemen, Gewächshäusern und Ställen).</skos:definition>
		<skos:prefLabel xml:lang="el">Γεωργικές εγκαταστάσεις και εγκαταστάσεις υδατοκαλλιέργειας</skos:prefLabel>
		<skos:definition xml:lang="el">Γεωργικός εξοπλισμός και εγκαταστάσεις παραγωγής (συμπεριλαμβανομένων των συστημάτων άρδευσης, των θερμοκηπίων και των στάβλων).</skos:definition>
		<skos:prefLabel xml:lang="es">Instalaciones agrícolas y de acuicultura</skos:prefLabel>
		<skos:definition xml:lang="es">Equipamiento e instalaciones de producción agraria (incluidos sistemas de regadío, invernaderos y establos).</skos:definition>
		<skos:prefLabel xml:lang="et">Põllumajandus- ja vesiviljelusrajatised</skos:prefLabel>
		<skos:definition xml:lang="et">Põllumajandusseadmed ja tootmisrajatised (sealhulgas niisutussüsteemid, kasvuhooned ja laudad).</skos:definition>
		<skos:prefLabel xml:lang="fi">Maatalous- ja vesiviljelylaitokset</skos:prefLabel>
		<skos:definition xml:lang="fi">Maatalouden tuotantolaitteet ja -laitteistot (mukaan luettuina kastelujärjestelmät, kasvihuoneet ja eläinsuojat).</skos:definition>
		<skos:prefLabel xml:lang="fr">Installations agricoles et aquacoles</skos:prefLabel>
		<skos:definition xml:lang="fr">Équipement et installations de production agricoles (y compris les systèmes d'irrigation, les serres et les étables).</skos:definition>
		<skos:prefLabel xml:lang="hu">Mezőgazdasági és akvakultúra-ágazati létesítmények</skos:prefLabel>
		<skos:definition xml:lang="hu">Mezőgazdasági eszközök és termelőlétesítmények (beleértve az öntözőrendszereket, üvegházakat és istállókat).</skos:definition>
		<skos:prefLabel xml:lang="it">Impianti agricoli e di acquacoltura</skos:prefLabel>
		<skos:definition xml:lang="it">Apparecchiature e impianti di produzione agricola (compresi i sistemi di irrigazione, le serre e le stalle).</skos:definition>
		<skos:prefLabel xml:lang="lt"> Žemės ūkio ir akvakultūros infrastruktūra</skos:prefLabel>
		<skos:definition xml:lang="lt">Žemės ūkio įrenginiai ir gamybos infrastruktūra (įskaitant drėkinimo sistemas, šiltnamius ir tvartus).</skos:definition>
		<skos:prefLabel xml:lang="lv">Lauksaimniecības un akvakultūras iekārtas</skos:prefLabel>
		<skos:definition xml:lang="lv">Lauksaimniecības ierīces un ražošanas iekārtas (tostarp apūdeņošanas sistēmas, siltumnīcas un staļļi).</skos:definition>
		
		<skos:prefLabel xml:lang="mt">Faċilitajiet agrikoli u ta' l-akwakultura</skos:prefLabel>
		<skos:definition xml:lang="mt">Tagħmir tal-biedja u faċilitajiet ta' produzzjoni (inklużi sistemi ta' irrigazzjoni, serer u stalel).</skos:definition>		
		
		<skos:prefLabel xml:lang="nl">Faciliteiten voor landbouw en aquacultuur</skos:prefLabel>
		<skos:definition xml:lang="nl">Landbouwuitrusting en productiefaciliteiten (met inbegrip van irrigatiesystemen, broeikassen en stallen).</skos:definition>
		<skos:prefLabel xml:lang="pl">Obiekty rolnicze oraz akwakultury</skos:prefLabel>
		<skos:definition xml:lang="pl">Urządzenia rolnicze oraz urządzenia produkcyjne (łącznie z systemami nawadniania, szklarniami i stajniami).</skos:definition>
		<skos:prefLabel xml:lang="pt">Instalações agrícolas e aquícolas</skos:prefLabel>
		<skos:definition xml:lang="pt">Equipamento e instalações de explorações agrícolas e aquícolas (incluindo sistemas de irrigação, estufas e viveiros, e estábulos).</skos:definition>
		<skos:prefLabel xml:lang="ro">Instalaţii agricole şi pentru acvacultură</skos:prefLabel>
		<skos:definition xml:lang="ro">Echipament şi instalaţii de producţie agricolă (inclusiv sisteme de irigaţie, sere şi grajduri).</skos:definition>
		<skos:prefLabel xml:lang="sk">Poľnohospodárske zariadenia a zariadenia akvakultúry</skos:prefLabel>
		<skos:definition xml:lang="sk">Poľnohospodárske vybavenie a výrobné zariadenia (vrátane zavlažovacích systémov, skleníkov a stajní).</skos:definition>
		<skos:prefLabel xml:lang="sl">Objekti in naprave za kmetijstvo in ribogojstvo</skos:prefLabel>
		<skos:definition xml:lang="sl">Kmetijska oprema ter proizvodni objekti in naprave (vključno z namakalnimi sistemi, rastlinjaki in hlevi).</skos:definition>
		<skos:prefLabel xml:lang="sv">Jordbruks- och vattenbruksanläggningar</skos:prefLabel>
		<skos:definition xml:lang="sv">Jordbruksutrustning och produktionsanläggningar (inbegripet bevattningssystem, växthus och djurstallar).</skos:definition>
		<!--
		<skos:prefLabel xml:lang="el">SAMPLE ALTERNATIVE EXPRESSION - αναφορά</skos:prefLabel>
		<skos:definition xml:lang="el">Συστήματα συντεταγμένων</skos:definition>
		<dct:description xml:lang="el">Συστήματα για μονοσήμαντη αναφορά χωρικών πληροφοριών στον χώρο, ως σύνολο συντεταγμένων (x,y,z) ή/και γεωγραφικό πλάτος και μήκος και ύψος, με βάση γεωδαιτικό οριζόντιο και κατακόρυφο σύστημα αναφοράς (datum).</dct:description>
		-->
		<skos:inScheme rdf:resource="http://inspire-registry.jrc.ec.europa.eu/registers/Themes/items"/>
	</inspire:Theme>
	<inspire:Theme rdf:about="http://inspire-registry.jrc.ec.europa.eu/registers/FCD/items/23">
		<!-- <owl:sameIndividualAs rdf:resource="http://www.eionet.europa.eu/gemet/theme_concepts?th=23&ns=5" /> -->
		<inspire:itemStatus>valid</inspire:itemStatus>
		<inspire:dateAccepted>2008-12-05T17:00:30.420+01:00</inspire:dateAccepted>
		<skos:prefLabel xml:lang="en">Population distribution — demography</skos:prefLabel>
		<skos:definition xml:lang="en">Geographical distribution of people, including population characteristics and activity levels, aggregated by grid, region, administrative unit or other analytical unit.</skos:definition>
		<dct:description xml:lang="en">There is a long tradition in collecting demographic and economic/activity statistics. All geographical levels interested, includes municipal and intra-municipal levels. Common to have statistics with geographical breakdown on country level, regional/ county level and municipal level. In some countries also information on census districts. These last decades, the statistical offices have started producing demographic and socio-economic statistics in large urban areas with a reference to blocks of houses and to process these data with a GIS. In some countries, the methodology chosen refers to aggregation of location-based information (address/households) on a grid (e.g. 1x1 km or 0.1x0.1 km).
Includes a broad spectrum of information sources, such as regional statistics at EuroStat; other European and National data, Regional data and Local breakdowns. The theme may thematically be divided into several components. The Directive text points at broad groups of sub-themes
- population characteristics
- population/ human activity levels
Concerning population information, this will or can include total population, age: population figures for each year class or aggregated year classes (0-5, 6-15, 16-20, 21-30, 31-40, 41-50, 51-67, 68-80, over 81). It could also include gender, mortality, life expectancy, migration. Figures could be offered as yearly versions, one could also like to give information of changes over time, such as growth/reduction in population, e.g. last 2 years, last 5 years, last 10 years. It could also include details on average night and day figures for some of the components. The sub-theme of population could include socio-economic information about the population, such as number of households, rate of employment, education, income, households with children etc.
Themes relevant to local, regional and national statistics also includes topics such as resource exploitation, agricultural production and a variety of environmental themes. Concerning "activity levels" used in the definition of the theme, this is probably an inclusion of a theme being treated separately in the INSPIRE position paper – namely "economic activities/local statistics". Economic activities including production, consumption, stocks, income, employment: statistics referred to administrative units, grids, facilities, networks, addresses, monetary and physical units. Economic data on transport and traffic are classified here. In general, economic activities are described according to the NACE rev.1.1. The NACE is the official classification of economic activities in the European Union and covers all industries. Examples relating directly to the protection of the environment is given underneath:
• 23.30 (part) Processing of nuclear fuel
• 37.10 Recycling of metal waste and scrap
• 37.20 Recycling of non-metal waste and scrap
• 41.00 Collection, purification and distribution of water
• 51.57 Wholesale of waste and scrap
• 90.01 Collection and treatment of sewage
• 90.02 Collection and treatment of other waste
• 90.03 Sanitation, remediation and similar activities
• In other industries, Environmental protection activities and expenditure need additional data, as it is presented in the SERIEE handbook (CEPA), EuroStat 1994 (Version 2002).
Population distribution could also mean geographical aggregations of buildings into settlements, villages, townships, towns, cities. Data may be materialised as hierarchical settlement databases with details on population figures for geographical objects either centre point location or area/settlement extent. Population distribution may also be or functional or physical characterisation of built-up areas within a settlement area. One example of an overall functional zoning can be the distribution of CBD areas within a city (CBD=Central business district). Detailed area categorisation can be done, e.g. kind of apartment, flat, cooperative society, self-owned, house/villa, semi-detached house, terrace house, apartment block.
Disaggregating of statistics is a methodology for transforming data at a higher aggregation to lower aggregates based on models. The EEA European population base introduces a transformation of statistics from administrative regions to small grid cells by a model based on knowledge of population distribution – land cover. Figures are aggregated to grid cells, and may therefore be seen as within the definition of this theme.
Population censuses take place with a periodicity of e.g. 10 years. In between, administrative registers of civil state supply a regular flow of data used generally for presenting annual statistics. New trends in statistics will probably lead to abandon the national censuses of large countries for a rotating system based on regional censuses supplemented by a broader collection of data from administrative registers.</dct:description>
		<skos:prefLabel xml:lang="bg">Разпределение на населението — демография</skos:prefLabel>
		<skos:definition xml:lang="bg">Географско разпределение на населението, включително характеристики на населението и нива на дейност, представено обобщено по координати, регион, административна единица или друга аналитична единица.</skos:definition>
		<skos:prefLabel xml:lang="cs">Rozložení obyvatelstva – demografie</skos:prefLabel>
		<skos:definition xml:lang="cs">Zeměpisné rozložení osob, včetně charakteristik obyvatelstva a druhů činnosti, seskupených podle souřadnicové sítě, regionu, správní jednotky nebo jiné analytické jednotky.</skos:definition>
		<skos:prefLabel xml:lang="da">Befolkningsfordeling — demografi</skos:prefLabel>
		<skos:definition xml:lang="da">Den geografiske fordeling af befolkningen, herunder befolkningskarakteristika og aktivitetsniveauer, i kvadratnetceller, forvaltningsenheder eller andre analytiske enheder.</skos:definition>
		<skos:prefLabel xml:lang="de">Verteilung der Bevölkerung — Demografie</skos:prefLabel>
		<skos:definition xml:lang="de">Geografische Verteilung der Bevölkerung, einschließlich Bevölkerungsmerkmalen und Tätigkeitsebenen, zusammengefasst nach Gitter, Region, Verwaltungseinheit oder sonstigen analytischen Einheiten.</skos:definition>
		<skos:prefLabel xml:lang="el">Κατανομή πληθυσμού — δημογραφία</skos:prefLabel>
		<skos:definition xml:lang="el">Γεωγραφική κατανομή του πληθυσμού, συμπεριλαμβανομένων των χαρακτηριστικών του πληθυσμού και των επιπέδων δραστηριοτήτων, ανά κάνναβο, περιοχή, διοικητική ενότητα ή άλλη ενότητα ανάλυσης.</skos:definition>
		<skos:prefLabel xml:lang="es">Distribución de la población — demografía</skos:prefLabel>
		<skos:definition xml:lang="es">Distribución geográfica de la población referidas a una cuadrícula, región, unidad administrativa u otro tipo de unidad analítica, incluyendo las características de la población y sus niveles de actividad.</skos:definition>
		<skos:prefLabel xml:lang="et">Elanikkonna jaotumine – demograafia</skos:prefLabel>
		<skos:definition xml:lang="et">Elanike, sealhulgas rahvastiku näitajate ja tegevuste geograafiline jaotumine ruutvõrgu, piirkondade, haldusüksuste või muude analüütiliste üksuste alusel.</skos:definition>
		<skos:prefLabel xml:lang="fi">Väestöjakauma – demografia</skos:prefLabel>
		<skos:definition xml:lang="fi">Väestön maantieteellinen jakautuminen, mukaan lukien väestöä koskevat tunnusluvut ja taloudellisen toimeliaisuuden tasot, yhdisteltynä ruudukoittain, alueittain, hallintoyksiköittäin tai muiden analyyttisten yksiköitten mukaisesti jaoteltuna.</skos:definition>
		<skos:prefLabel xml:lang="fr">Répartition de la population — démographie</skos:prefLabel>
		<skos:definition xml:lang="fr">Répartition géographique des personnes, avec les caractéristiques de population et les niveaux d'activité, regroupées par grille, région, unité administrative ou autre unité analytique.</skos:definition>
		<skos:prefLabel xml:lang="hu">A népesség eloszlása – demográfia</skos:prefLabel>
		<skos:definition xml:lang="hu">A népesség földrajzi eloszlása – beleértve a népességi jellemzőket és a tevékenységi szinteket is – térképrács, régió, közigazgatási egység vagy más elemzési egység alapján összesítve.</skos:definition>
		<skos:prefLabel xml:lang="it">Distribuzione della popolazione — demografia</skos:prefLabel>
		<skos:definition xml:lang="it">Distribuzione geografica della popolazione, comprese le relative caratteristiche ed i livelli di attività, aggregata per griglia, regione, unità amministrativa o altra unità analitica.</skos:definition>
		<skos:prefLabel xml:lang="lt">Gyventojų pasiskirstymas – demografija</skos:prefLabel>
		<skos:definition xml:lang="lt">Geografinis žmonių pasiskirstymas, įskaitant gyventojų savybes ir aktyvumo lygius, pagal tinklelį, regioną, administracinį ar kitą analitinį vienetą.</skos:definition>
		<skos:prefLabel xml:lang="lv">Iedzīvotāju sadalījums – demogrāfija</skos:prefLabel>
		<skos:definition xml:lang="lv">Iedzīvotāju ģeogrāfiskais sadalījums, tostarp iedzīvotāju raksturojumi un darbības līmeņi, grupējot pēc koordinātu tīkla, reģiona, administratīvām vai citām analītiskām vienībām.</skos:definition>
		
		<skos:prefLabel xml:lang="mt">Distribuzzjoni tal-popolazzjoni – demografija</skos:prefLabel>
		<skos:definition xml:lang="mt">Distribuzzjoni ġeografika ta' nies, inkluż karatteristiċi ta' popolazzjoni u livelli ta' attivitajiet, miġbura flimkien skond il-grilja, ir-reġjun, l-unità amministrattiva jew unità analitika oħra.</skos:definition>		
		
		<skos:prefLabel xml:lang="nl">Spreiding van de bevolking — demografie</skos:prefLabel>
		<skos:definition xml:lang="nl">Geografische spreiding van de bevolking, met inbegrip van bevolkingskenmerken en activiteitsniveaus, verzameld per raster, regio, administratieve eenheid of andere analytische eenheid.</skos:definition>
		<skos:prefLabel xml:lang="pl">Rozmieszczenie ludności – demografia</skos:prefLabel>
		<skos:definition xml:lang="pl">Geograficzne rozmieszczenie ludności, łącznie z poziomami aktywności i charakterystyką ludności, pogrupowanej według siatki geograficznej, regionu, jednostki administracyjnej lub innej jednostki analitycznej.</skos:definition>
		<skos:prefLabel xml:lang="pt">Distribuição da população — demografia</skos:prefLabel>
		<skos:definition xml:lang="pt">Distribuição geográfica da população, incluindo características demográficas e níveis de actividade, agregada por quadrícula, região, unidade administrativa ou outra unidade analítica.</skos:definition>
		<skos:prefLabel xml:lang="ro">Repartizarea populaţiei – demografie</skos:prefLabel>
		<skos:definition xml:lang="ro">Repartizare geografică a populaţiei, inclusiv caracteristicile populaţiei şi nivelurile de activitate, regrupate pe grilă, regiune, unitate administrativă sau altă unitate analitică.</skos:definition>
		<skos:prefLabel xml:lang="sk">Rozmiestnenie obyvateľstva – demografia</skos:prefLabel>
		<skos:definition xml:lang="sk">Geografické rozmiestnenie obyvateľstva vrátane charakteristík obyvateľstva a úrovní činností zoskupené podľa siete, regiónu, administratívnej jednotky alebo inej analytickej jednotky.</skos:definition>
		<skos:prefLabel xml:lang="sl">Porazdelitev prebivalstva – demografski podatki</skos:prefLabel>
		<skos:definition xml:lang="sl">Geografska porazdelitev ljudi, vključno z značilnostmi populacije in ravnmi aktivnosti, razvrščenih po koordinatah, regiji, upravni enoti ali drugi analitični enoti.</skos:definition>
		<skos:prefLabel xml:lang="sv">Befolkningsfördelning – demografi</skos:prefLabel>
		<skos:definition xml:lang="sv">Geografisk fördelning av människor, inbegripet befolkningskarakteristiska och sysselsättningsgrader, i rutnät, regioner, administrativa enheter eller andra analysenheter.</skos:definition>
		<!--
		<skos:prefLabel xml:lang="el">SAMPLE ALTERNATIVE EXPRESSION - αναφορά</skos:prefLabel>
		<skos:definition xml:lang="el">Συστήματα συντεταγμένων</skos:definition>
		<dct:description xml:lang="el">Συστήματα για μονοσήμαντη αναφορά χωρικών πληροφοριών στον χώρο, ως σύνολο συντεταγμένων (x,y,z) ή/και γεωγραφικό πλάτος και μήκος και ύψος, με βάση γεωδαιτικό οριζόντιο και κατακόρυφο σύστημα αναφοράς (datum).</dct:description>
		-->
		<skos:inScheme rdf:resource="http://inspire-registry.jrc.ec.europa.eu/registers/Themes/items"/>
	</inspire:Theme>
	<inspire:Theme rdf:about="http://inspire-registry.jrc.ec.europa.eu/registers/FCD/items/24">
		<!-- <owl:sameIndividualAs rdf:resource="http://www.eionet.europa.eu/gemet/theme_concepts?th=24&ns=5" /> -->
		<inspire:itemStatus>valid</inspire:itemStatus>
		<inspire:dateAccepted>2008-12-05T17:00:30.487+01:00</inspire:dateAccepted>
		<skos:prefLabel xml:lang="en">Area management/restriction/regulation zones and reporting units</skos:prefLabel>
		<skos:definition xml:lang="en">Areas managed, regulated or used for reporting at international, European, national, regional and local levels. Includes dumping sites, restricted areas around drinking water sources, nitrate-vulnerable zones, regulated fairways at sea or large inland waters, areas for the dumping of waste, noise restriction zones, prospecting and mining permit areas, river basin districts, relevant reporting units and coastal zone management areas.</skos:definition>
		<dct:description xml:lang="en">A wide range of management areas both at European, national, regional and local levels. The themes and its feature types allow information content from any sector – e.g. environmental, transport, health, education, energy, fisheries, agriculture.
Sector-specific management areas contain information about management zones in sectors, not already being covered by the INSPIRE theme "Administrative units". Here only a few examples are given. These may include health care management regions, defence enrolement regions, school regions, fire fighter management regions, police responsibility regions, rescue operation regions, National and IMO adopted Traffic Separation Schemes (TSS) and Deep Water Routes, Military Practice Areas, Explosive Dumping Grounds etc.
Different regimens and regulations may be relevant, some examples are given;
- Safety at Sea - SOLAS - dissemination of data and information for safe navigation - NAVAREA commitments may be relevant to the specification process
River Basin Districts, management area for WFD, is not specifically being defined a subset of water catchments, and is therefore relevant to be defined as a separate management area. Sub-units for reporting under the Water Framework Directive is being discussed, but not yet decided. In the specification process care should be given to differences in definition, nature-based delineation relevant to water catchments, delineation based on administrative decisions conflicting nature-based catchment boundaries relevant for river management zones. WFD: art 2, annex I, ii): River basin district means the area of land and sea, made up of one or more neighbouring river basins together with their associated groundwater and coastal waters, which is identified under Article 3(1) as the main unit for management of river basins. WFD: Annex I, ii): Geographical coverage of the river basin district- the names of the main rivers within the river basin district together with a precise description of the boundaries of the river basin district. Anticipated sources: Environmental / hydrological institutions, Mandatory reporting from MC. The implementation of delineation in the countries may not reflect the nature-based definition in the WFD.</dct:description>
		<skos:prefLabel xml:lang="bg">Управление на територията/ограничени/регулирани зони и отчетни единици</skos:prefLabel>
		<skos:definition xml:lang="bg">Зони, управлявани, регулирани или използвани за докладване на международно, европейско, национално, регионално и местно равнище. Включва складови обекти, ограничени райони около източници на питейна вода, уязвими от замърсяване с нитрати зони, контролирани морски проходи или големи вътрешни водни пътища, райони за складиране на отпадъци, зони с наложени ограничения върху шума, проучвателни и минни райони, райони на речни басейни, съответни отчетни единици и зони за управление на брегови райони. 25.4.2007 г. BG Официален вестник на Европейския съюз L 108/13</skos:definition>
		<skos:prefLabel xml:lang="cs">Správní oblasti/chráněná pásma/regulovaná území a jednotky podávající hlášení</skos:prefLabel>
		<skos:definition xml:lang="cs">Oblasti spravované, regulované nebo používané pro hlášení na mezinárodní, evropské, celostátní, regionální nebo místní úrovni. Zahrnuje skládky, pásma hygienické ochrany vodních zdrojů, oblasti zranitelné dusičnany, regulované plavební dráhy na moři nebo rozsáhlých vnitrozemských vodních plochách, oblasti pro ukládání odpadů, pásma s omezením hladiny hluku, povolená průzkumná a těžební území, oblasti povodí, příslušné jednotky pro podávání hlášení a pásma pobřežní správy.</skos:definition>
		<skos:prefLabel xml:lang="da">Forvaltede og regulerede områder samt områder med brugsbegrænsning og indberetningsenheder</skos:prefLabel>
		<skos:definition xml:lang="da">Områder, der forvaltes, reguleres eller benyttes som indberetningsenheder på internationalt, europæisk, nationalt, regionalt og lokalt plan. Omfatter affaldsdepoter, områder med brugsbegrænsninger af hensyn til drikkevandsindvinding, nitratfølsomme områder, regulerede sejlruter til søs og på større indlandsvandområder, områder for dumpning af affald, områder med støjbegrænsning, områder, hvor der er tilladelse til efterforskning og minedrift, vandområdedistrikter, relevante indberetningsenheder samt områder for kystzoneforvaltning.</skos:definition>
		<skos:prefLabel xml:lang="de">Bewirtschaftungsgebiete/Schutzgebiete/geregelte Gebiete und Berichterstattungseinheiten</skos:prefLabel>
		<skos:definition xml:lang="de">Auf internationaler, europäischer, nationaler, regionaler und lokaler Ebene bewirtschaftete, geregelte oder zu Zwecken der Berichterstattung herangezogene Gebiete. Dazu zählen Deponien, Trinkwasserschutzgebiete, nitratempfindliche Gebiete, geregelte Fahrwasser auf See oder auf großen Binnengewässern, Gebiete für die Abfallverklappung, Lärmschutzgebiete, für Exploration und Bergbau ausgewiesene Gebiete, Flussgebietseinheiten, entsprechende Berichterstattungseinheiten und Gebiete des Küstenzonenmanagements.</skos:definition>
		<skos:prefLabel xml:lang="el"> Ζώνες διαχείρισης/περιορισμού/ρύθμισης εκτάσεων και μονάδες αναφοράς</skos:prefLabel>
		<skos:definition xml:lang="el">Εκτάσεις υπό διαχείριση, υπό ρύθμιση ή χρησιμοποιούμενες για αναφορά σε διεθνές, ευρωπαϊκό, εθνικό, περιφερειακό και τοπικό επίπεδο. Περιλαμβάνονται χώροι απόρριψης, προστατευόμενες περιοχές γύρω από πηγές πόσιμου νερού, ζώνες ευάλωτες στη νιτρορρύπανση, κανονιστικά ρυθμιζόμενοι δίαυλοι θαλάσσιας ή εσωτερικής ναυσιπλοΐας, περιοχές για τη βύθιση αποβλήτων, ζώνες προστασίας από τον θόρυβο, περιοχές όπου επιτρέπεται η μεταλλευτική έρευνα και εξόρυξη, διοικητικές περιοχές ποτάμιων λεκανών, σχετικές μονάδες αναφοράς και περιοχές διαχείρισης παράκτιας ζώνης.</skos:definition>
		<skos:prefLabel xml:lang="es">Zonas sujetas a ordenación, a restricciones o reglamentaciones y unidades de notificación</skos:prefLabel>
		<skos:definition xml:lang="es">Zonas gestionadas, reglamentadas o utilizadas para la elaboración de informes para organismos internacionales, europeos, nacionales, regionales y locales. Se incluirán vertederos, zonas restringidas alrededor de lugares de extracción de agua potable, zonas sensibles a los nitratos, rutas marítimas o por grandes vías navegables reglamentadas, zonas de vertido, zonas de restricción de ruidos, zonas de prospección o extracción minera, demarcaciones hidrográficas, las correspondientes unidades de notificación y planes de ordenación de zonas costeras.</skos:definition>
		<skos:prefLabel xml:lang="et">Üldplaneering/piirangu-/reguleeritud tsoonid ja aruandlusüksused</skos:prefLabel>
		<skos:definition xml:lang="et">Alad, mille haldamisest, reguleerimisest või kasutamisest antakse aru rahvusvahelisel, Euroopa, riiklikul, piirkondlikul ja kohalikul tasandil. Hõlmab kaadamiskohti, joogiveeallikate ümber asuvaid piirangutsoone, nitraaditundlikke tsoone, reguleeritavaid laevateid merel või suurtel siseveekogudel, jäätmete kaadamise alasid, mürapiirangutsoone, geoloogiliste uuringute ja kaevanduste alasid, valgalasid, asjakohaseid aruandlusüksusi ning rannikukaitsealasid.</skos:definition>
		<skos:prefLabel xml:lang="fi">Aluesuunnittelun, rajoitusten ja sääntelyn piiriin kuuluvat alueet ja raportointiyksiköt</skos:prefLabel>
		<skos:definition xml:lang="fi">Alueet, joita hoidetaan, säännellään tai käytetään kansainvälisen, Euroopan, kansallisen, alueellisen tai paikallisen tason raportointiin. Sisältää kaatopaikat, juomavedenottopaikkoja ympäröivät suoja-alueet, nitraatin aiheuttamalle pilaantumiselle alttiit alueet, säännellyt laivaväylät merellä tai suurilla sisävesillä, jätteiden upottamiskiellon soveltamisalaan kuuluvat alueet, melurajoitusalueet, luonnonvarojen tai malmin etsintäalueet, ja kaivostoiminnan lupa-alueet, vesipiirit, asiaankuuluvat raportointiyksiköt ja rannikkoalueiden hallinta-alueet.</skos:definition>
		<skos:prefLabel xml:lang="fr">Zones de gestion, de restriction ou de réglementation et unités de déclaration</skos:prefLabel>
		<skos:definition xml:lang="fr">Zones gérées, réglementées ou utilisées pour les rapports aux niveaux international, européen, national, régional et local. Sont inclus les décharges, les zones restreintes aux alentours des sources d'eau potable, les zones vulnérables aux nitrates, les chenaux réglementés en mer ou les eaux intérieures importantes, les zones destinées à la décharge de déchets, les zones soumises à limitation du bruit, les zones faisant l'objet de permis d'exploration et d'extraction minière, les districts hydrographiques, les unités correspondantes utilisées pour les rapports et les zones de gestion du littoral.</skos:definition>
		<skos:prefLabel xml:lang="hu">Területgazdálkodási/-korlátozási/-szabályozási övezetek és adatszolgáltató egységek</skos:prefLabel>
		<skos:definition xml:lang="hu">A nemzetközi, európai, nemzeti, regionális és helyi szintű adatszolgáltatás céljából irányított, szabályozott vagy használt területek. Ide tartoznak a lerakóhelyek, az ivóvízforrásokat övező korlátozás alá tartozó területek, a nitrátérzékeny területek, a tengeri hajóutak vagy nagy kiterjedésű belvizek szabályozott hajózóútjai, a hulladéklerakásra kijelölt területek, a zajvédelmi zónák, az előkészítő és bányászatiengedély-köteles területek, a folyómedri kerületek, a megfelelő adatszolgáltató egységek és a tengerparti igazgatási térségek.</skos:definition>
		<skos:prefLabel xml:lang="it">Zone sottoposte a gestione/limitazioni/regolamentazione e unità con obbligo di comunicare dati</skos:prefLabel>
		<skos:definition xml:lang="it">Aree gestite, regolamentate o utilizzate per la comunicazione di dati a livello internazionale, europeo, nazionale, regionale e locale. Sono comprese le discariche, le zone vietate attorno alle sorgenti di acqua potabile, le zone sensibili ai nitrati, le vie navigabili regolamentate in mare o in acque interne di grandi dimensioni, le zone per lo smaltimento dei rifiuti, le zone di limitazione del rumore, le zone in cui sono autorizzate attività di prospezione ed estrazione, i distretti idrografici, le pertinenti unità con obbligo di comunicare dati e le aree in cui vigono piani di gestione delle zone costiere.</skos:definition>
		<skos:prefLabel xml:lang="lt">Tvarkomos teritorijos, ribojamos ir reglamentuojamos zonos bei vienetai, už kuriuos atsiskaitoma</skos:prefLabel>
		<skos:definition xml:lang="lt">Tvarkomos/ribojamos/reglamentuojamos zonos ir vienetai, už kuriuos atsiskaitoma tarptautiniu, Europos, nacionaliniu, regioniniu arba vietos lygmeniu tvarkomos ir reglamentuojamos zonos arba zonos, apie kurias rengiamos ataskaitos. Tai apima sąvartynus, ribotos veiklos zonas aplink geriamo vandens šaltinius, nitratų pažeidžiamas zonas, reglamentuojamus jūros arba didelių vidaus vandenų farvaterius, atliekų aikšteles, zonas, kuriose ribojamas triukšmas, vietas, kuriose reikalingas leidimas žvalgybai ar kasinėjimui, upių baseinų sritis, atitinkamas vietoves, apie kurias rengiamos ataskaitos, ir pakrančių zonos tvarkymo vietoves.</skos:definition>
		<skos:prefLabel xml:lang="lv">Apgabala pārvaldības/ierobežojumu/reglamentētas zonas un ziņošanas vienības</skos:prefLabel>
		<skos:definition xml:lang="lv">Apgabali, ko pārvalda, reglamentē vai lieto, lai sniegtu ziņojumus starptautiskā, Eiropas, valsts, reģiona un pašvaldības līmenī. Ietver izgāztuves, liegumus ap dzeramā ūdens avotiem, pret nitrātiem jutīgas zonas, reglamentētus kuģu ceļus jūrā vai lielos iekšzemes ūdeņos, atkritumu izgāšanas apgabalus, zonas ar trokšņu ierobežojumiem, zonas, kurās atļauta ģeoloģisko atradņu izpēte un izrakteņu ieguve, upju baseinu apgabalus, attiecīgas ziņošanas vienības un krasta zonas apsaimniekošanas apgabalus.</skos:definition>
		
		<skos:prefLabel xml:lang="mt">Amministrazzjoni ta' żoni/restrizzjoni/żoni regolati u unitajiet ta' rapportar</skos:prefLabel>
		<skos:definition xml:lang="mt">Żoni amministrati, regolati jew użati għar-rappurtar fuq il-livell internazzjonali, Ewropew, nazzjonali, reġjonali u lokali. Huma inklużi siti użati għar-radam, żoni ristretti madwar għejjun ta' l-ilma għax-xorb, żoni vulnerabbli għannitrati, kanali regolati fil-baħar jew f'ilmijiet interni kbar, żoni għar-radam ta' l-iskart, żoni għar-restrizzjoni ta' listorbju, żoni b'permess għat-tħaffir u għat-tiftix ta' minerali, distretti ta' baċiri tax-xmajjar, unitajiet ta' rapportar rilevanti u żoni ta' amministrazzjoni ta' l-inħawi tal-kosta.</skos:definition>		
		
		<skos:prefLabel xml:lang="nl">Gebiedsbeheer, gebieden waar beperkingen gelden, gereguleerde gebieden en rapportage-eenheden</skos:prefLabel>
		<skos:definition xml:lang="nl">Gebieden die worden beheerd, gereguleerd of gebruikt voor rapportage op internationaal, Europees, nationaal, regionaal en lokaal niveau, met inbegrip van stortplaatsen, gebieden rond drinkwaterbronnen waar beperkingen gelden, nitraatgevoelige gebieden, gereguleerde vaarwegen op zee of op grote binnenwateren, gebieden voor het storten van afval, gebieden waar geluidsbeperkingen gelden, gebieden met toestemming voor exploratie en mijnbouw, stoomgebieden, relevante rapportage-eenheden en gebieden voor kustbeheer.</skos:definition>
		<skos:prefLabel xml:lang="pl">Gospodarowanie obszarem/strefy ograniczone/regulacyjne oraz jednostki sprawozdawcze</skos:prefLabel>
		<skos:definition xml:lang="pl">Obszary zarządzane, regulowane lub wykorzystywane do celów sprawozdawczych na poziomie międzynarodowym, europejskim, krajowym, regionalnym i lokalnym. Obejmują również wysypiska śmieci, obszary o ograniczonym dostępie wokół ujęć wody pitnej, strefy zagrożone przez azotany, uregulowane drogi wodne na morzach lub wodach śródlądowych o dużej powierzchni, obszary przeznaczone pod wysypiska śmieci, strefy ograniczeń hałasu, obszary wymagające zezwolenia na poszukiwania i wydobycie, obszary dorzeczy, odpowiednie jednostki sprawozdawcze i obszary zarządzania strefą brzegową.</skos:definition>
		<skos:prefLabel xml:lang="pt">Zonas de gestão/restrição/regulamentação e unidades de referência</skos:prefLabel>
		<skos:definition xml:lang="pt">Zonas geridas, regulamentadas ou utilizadas para a comunicação de dados a nível internacional, europeu, nacional, regional e local. Compreende aterros, zonas de acesso restrito em torno de nascentes de água potável, zonas sensíveis aos nitratos, vias navegáveis regulamentadas no mar ou em águas interiores de grandes dimensões, zonas de descarga de resíduos, zonas de ruído condicionado, zonas autorizadas para efeitos de prospecção e extracção mineira, bacias hidrográficas, unidades de referência pertinentes e zonas abrangidas pela gestão das zonas costeiras.</skos:definition>
		<skos:prefLabel xml:lang="ro">Zone de administrare/restricţie/reglementare şi unităţi de raportare</skos:prefLabel>
		<skos:definition xml:lang="ro">Zone administrate, reglementate sau folosite pentru raportarea la nivel internaţional, european, naţional, regional şi local. Sunt incluse gropile de gunoi, zonele restricţionate din apropierea surselor de apă potabilă, zonele vulnerabile la nitraţi, şenalele navigabile reglementate de pe mare sau din apele interne importante, zonele destinate descărcării deşeurilor, zonele în care au fost introduse limite de zgomot, zonele care fac obiectul unui permis de prospectare şi de exploatare minieră, districtele hidrografice, unităţile de raportare corespunzătoare şi zonele de administrare a litoralului.</skos:definition>
		<skos:prefLabel xml:lang="sk">Spravované/obmedzené/regulované zóny a jednotky podávajúce správy</skos:prefLabel>
		<skos:definition xml:lang="sk">Oblasti, ktoré sú spravované, regulované alebo využívané na podávanie správ na medzinárodnej, európskej, celoštátnej, regionálnej a miestnej úrovni. Patria sem skládky, ochranné pásma v okolí zdrojov pitnej vody, oblasti citlivé na dusík, regulované plavebné cesty na mori alebo na rozsiahlych vnútrozemských vodných plochách a tokoch, oblasti určené na skladovanie odpadu, oblasti s obmedzením hluku, oblasti, v ktorých je povolený prieskum a ťažba, oblasti povodí, príslušné jednotky na podávanie správ a oblasti správy pobrežných zón.</skos:definition>
		<skos:prefLabel xml:lang="sl">Območja upravljanja/zaprta območja/regulirana območja in poročevalske enote</skos:prefLabel>
		<skos:definition xml:lang="sl">Območja, ki se upravljajo, urejajo ali uporabljajo za poročanje na mednarodni, evropski, nacionalni, regionalni in lokalni ravni. Vključujejo odlagališča odpadkov, zaprta območja okrog virov pitne vode, cone, občutljive na nitrate, urejene plovne poti po morju ali velikih celinskih vodah, območja za odlaganje odpadkov, cone z omejitvijo hrupa, območja, kjer je potrebno dovoljenje za iskanje rud in rudarjenje, predele povodij, ustrezne poročevalske enote in območja upravljanja obalnih con.</skos:definition>
		<skos:prefLabel xml:lang="sv">Områden med särskild förvaltning/begränsningar/reglering samt enheter för rapportering</skos:prefLabel>
		<skos:definition xml:lang="sv">Områden som förvaltas, regleras eller används för rapportering på internationell, europeisk, nationell, regional och lokal nivå. Innefattar avfallsdeponier, skyddsområden runt dricksvattentäkter, områden som är känsliga för nitratbelastning, reglerade farleder till havs och i större inlandsvatten, områden för dumpning av avfall, områden med bullerrestriktioner, områden med tillstånd för prospektering och gruvbrytning, avrinningsdistrikt, relevanta enheter för rapportering och områden med kustförvaltning.</skos:definition>
		<!--
		<skos:prefLabel xml:lang="el">SAMPLE ALTERNATIVE EXPRESSION - αναφορά</skos:prefLabel>
		<skos:definition xml:lang="el">Συστήματα συντεταγμένων</skos:definition>
		<dct:description xml:lang="el">Συστήματα για μονοσήμαντη αναφορά χωρικών πληροφοριών στον χώρο, ως σύνολο συντεταγμένων (x,y,z) ή/και γεωγραφικό πλάτος και μήκος και ύψος, με βάση γεωδαιτικό οριζόντιο και κατακόρυφο σύστημα αναφοράς (datum).</dct:description>
		-->
		<skos:inScheme rdf:resource="http://inspire-registry.jrc.ec.europa.eu/registers/Themes/items"/>
	</inspire:Theme>
	<inspire:Theme rdf:about="http://inspire-registry.jrc.ec.europa.eu/registers/FCD/items/25">
		<!-- <owl:sameIndividualAs rdf:resource="http://www.eionet.europa.eu/gemet/theme_concepts?th=25&ns=5" /> -->
		<inspire:itemStatus>valid</inspire:itemStatus>
		<inspire:dateAccepted>2008-12-05T17:00:30.546+01:00</inspire:dateAccepted>
		<skos:prefLabel xml:lang="en">Natural risk zones</skos:prefLabel>
		<skos:definition xml:lang="en">Vulnerable areas characterised according to natural hazards (all atmospheric, hydrologic, seismic, volcanic and wildfire phenomena that, because of their location, severity, and frequency, have the potential to seriously affect society), e.g. floods, landslides and subsidence, avalanches, forest fires, earthquakes, volcanic eruptions.</skos:definition>
		<dct:description xml:lang="en">"Natural risk zones" are zones where natural hazards areas intersect with highly populated areas and/or areas of particular environmental/ cultural/ economic value. Risk in this context is defined as: risk = hazard x probability of its occurrence x vulnerability of the exposed populations and of the environmental, cultural and economic assets in the zone considered.
Natural hazards are natural processes or phenomena occurring in the biosphere that may constitute a damaging event. Natural hazards can be classified by origin namely: geological, hydrometeorological or biological. Hazardous events can vary in magnitude or intensity, frequency, duration, area of extent, speed of onset, spatial dispersion and temporal spacing. An international definition on hazard is relevant in defining the theme. The internationally agreed terminology on disasters should be adopted in this document (UNISDR): Hazards is defined as a potentially damaging physical event, phenomenon or human activity that may cause the loss of life or injury, property damage, social and economic disruption or environmental degradation. Hazards can include latent conditions that may represent future threats and can have different origins: natural (geological, hydrometeorological and biological) or induced by human processes (environmental degradation and technological hazards). Hazards can be single, sequential or combined in their origin and effects. Each hazard is characterised by its location, intensity, frequency and probability.
Geological hazards are natural earth processes or phenomena that may cause the loss of life or injury, property damage, social and economic disruption or environmental degradation. Geological hazard includes internal earth processes or tectonic origin, such as earthquakes, geological fault activity, tsunamis, volcanic activity and emissions as well as external processes such as mass movements: landslides, rockslides, rock falls or avalanches, surfaces collapses, expansive soils and debris or mud flows. Geological hazards can be single, sequential or combined in their origin and effects.
Hydrometeorological hazards are natural processes or phenomena of atmospheric, hydrological or oceanographic nature, which may cause the loss of life or injury, property damage, social and economic disruption or environmental degradation. Hydrometeorological hazards include: floods, debris and mud floods; tropical cyclones, storm surges, thunder/hailstorms, rain and wind storms, blizzards and other severe storms; drought, desertification, wildland fires, temperature extremes, sand or dust storms; permafrost and snow or ice avalanches. Hydrometeorological hazards can be single, sequential or combined in their origin and effects.
Many of the hazards are sudden in their nature. However, several categories of natural hazards with major impacts on civil security and on environmental/ cultural and economic assets are not sudden in nature. They may be permanent phenomena going unnoticed (e.g..: radon gas emanations, deficit or excess of elements in soils and water), or slow phenomena (slow ground motion). Technological hazards are commonly sudden failure of a construction or a process causing significant damage. Natural hazards have the potential to precipitate technological hazards. Usually continuous processes like pollution/emission is not classified as hazards. However, repeated emissions might be called hazards, e.g. large scale chemical, radiation or oil spills. Continuous pollution and other environmental problems may have an adverse effect also on the size and frequency of some kinds of natural hazards.
Knowledge about "Natural hazards areas" is important in the identification and delineation of risk zones. The natural hazards areas may reflect all atmospheric, meteorological, hydrologic, geological and wildfire phenomena that, because of their location, severity, and frequency, have the potential to seriously affect society, e.g. floods, landslides and subsidence, avalanches, forest fires, earthquakes, volcanic eruptions, shrinking and swelling soils, radon gas emanations, deficit or excess of trace elements in soils or water. Data and services are probably needed for both risk assessment and emergency situations Special warning services may be relevant.
Underneath is given examples of some important natural hazards, with information on occurrence: location and frequency and with some information on the datasets, coverage etc.
Areas prone to flooding by inland waters and lakes:
Areas flooded due to exceptional raise of water table in groundwater, rivers and lakes, affecting adjacent land or areas further away being at the same altitude or lower than the flooding water. Affecting housing and industrial sites, agricultural land, transport network, sewage systems, dams etc: Occurrence: Flat river plains, delta areas, valley bottoms and shorelines.
• Physical mapping of areas susceptible to flooding, line for highest recorded level, also division into zones with different susceptibility classes. Data needs: detailed elevation model and measurements in the field
• Areas with certain regulations/ restrictions for different land use/ resource use linked to flooding risk.
• Constructions for flood control
• Data set on restriction zones on land use/ building/ activities downstream reservoirs in case of reservoir brake-down
• Drainage capacity of ground and soil sealing areas with low drainage capacity
Areas prone to flooding by spring tide/ exceptional sea level rise
Areas prone to flooding due to exceptional raise of water table the sea and backwaters, affecting adjacent land or areas further away being at the same altitude or lower than the flooding water. Affecting housing and industrial sites, agricultural land, transport network, sewage systems, dams etc Occurrence: Flat coastal areas, areas lower than original sea level. Commonly harbours, trade areas etc. Frequency: Floods, as storms, are among the most common natural disasters in Europe – with the effect of being of the most costly in terms of economy and insurance.
• Physical mapping of areas susceptible to flooding, line for highest recorded level, also division into zones with different susceptibility classes. Data needs: detailed elevation model and/or measurements in the field.
- measures by radar satellites or air born equipment to measure water level
- field measurement
• Constructions for flood control
• Areas with certain regulations/ restrictions for different land use/ resource use linked to flooding risk.
Earthquakes
Earthquakes are widespread in the EU and other European Countries. The most destructive events have occurred in the Mediterranean countries, particularly Greece and Italy, which are in the collision zone between the Eurasian and African crustal plates. Through the last three decades several thousand persons have died and injured, several hundred thousand became homeless in events in Greece and Italy. Data needed for getting overview and handling the hazard:
• date and time of occurence; - epicenter location, depth, with a liability index - Magnitude and type of magnitude used - Observations (local intensity (MSK 1964 standard) with a liability index) - Triggered effects - Fault
• Data needed for emergency/ rescue operations
Volcano eruptions:
A few active volcanoes exist in the EU and other European Countries. The activity is low and generally the threats are minimal compared to other natural hazards. Some destructive events have occurred in the Mediterranean countries, such as Italy over the past decades. Actions are usually coped with at the local level.
• It is difficult to outline important spatial data sets linked to volcano activities. There might exist maps on expected lava flow channels and restriction areas for certain activities.
Mud slides, land slides and quick (saline leached) clay soils slides:
• clay rich shrinking and swelling soils
• areas of unstable terrain, slide area divided into zones of different susceptibility classes
• borehole locations with further information on the salt content etc
• affected area if area is subject to slumping and landslip
• Areas with activity restrictions – which kinds of operations are allowed in order to prevent slides and which areas are not to be built on. Different countries have different threshold levels e.g. concerning slope degree on land used for buildings, the values depending on the ground condition (soil, clay, bedrock)
Areas prone to mountain blocks slides and stone slides:
Occurrence: Mountain block slides mostly in alpine environment with "young landscapes" where frost and water erosion is active, stone slides areas with steep slopes and loose material. Problems occur where land use includes settlements, infrastructure etc.
• Physical mapping of areas susceptible to land block slides divided into zones with different susceptibility classes. Based on mapping of bedrock structures.
• Physical mapping of areas susceptible to stone slides divided into zones with different susceptibility classes. Further info on kind of material. A rough assessment can be based on analysis of slope angle, slope length and rock stability.
• Anticipated affected areas followed by a land block slide; the stone masses themselves and following flooded areas.
• Areas with certain regulations/ restrictions for different land use/ resource use linked to land block slide risk and stone slide risk.
• Constructions for directing stone slides
Areas prone to snow slides - avalanches:
Occurrence: In areas with significant snow cover combined with steep slopes. Wind will affect the creation of snowdrifts.
• Physical mapping of areas susceptible to snow slides divided into zones with different susceptibility classes
• Areas with certain regulations/ restrictions for different land use/ resource use linked to snow slide risk.
• Constructions for directing slides
Areas susceptible to forest, bush and grassland fires
Areas susceptible to forest, bush and grassland fires can be analysed by using
• Satellite images
• Vegetation cover, composition and strata
• Elevation data
• Meteorological data, Precipitation, temperature, winds,
Areas of installations prone to storms/ wind damage
Occurrence: Unclear picture; seas, coastal areas and narrow valleys, but also other areas within the continent. In addition storms, as floods, are among the most common natural disasters in Europe – thus also being the most costly in terms of economy and insurance.
• Data sets. Areas with recorded extreme wind
Coastal erosion
Coastal erosion is an important and costly category of natural hazard of growing significance in a climate change context
Radon areas
Natural radiation from bedrocks and unconsolidated rocks are considered as natural risk zones due to a possible high radon concentration in indoor air.</dct:description>
		<skos:prefLabel xml:lang="bg">Природни рискови зони</skos:prefLabel>
		<skos:definition xml:lang="bg">Уязвими райони, определени в зависимост от вида природен риск (всички атмосферни, хидрологични, сеизмични, вулканични и огнени явления, които поради местонахождението, силата и честотата на проявление могат да засегнат сериозно обществото), например наводнения, свличане и пропадане на земни маси, лавини, горски пожари, земетресения, изригвания на вулкани.</skos:definition>
		<skos:prefLabel xml:lang="cs">Oblasti ohrožené přírodními riziky</skos:prefLabel>
		<skos:definition xml:lang="cs">Zranitelné oblasti označené podle přírodního nebezpečí (všechny povětrnostní, hydrologické, seismické a sopečné úkazy, jakož i ničivé požáry, které mohou mít vzhledem ke svému výskytu, závažnosti a četnosti vážný dopad na společnost), např. povodně, sesuvy a sesedání půdy, laviny, lesní požáry, zemětřesení, sopečné výbuchy.</skos:definition>
		<skos:prefLabel xml:lang="da">Områder med naturlige risici</skos:prefLabel>
		<skos:definition xml:lang="da">Sårbare områder, karakteriseret efter naturlige risici (alle atmosfæriske, hydrologiske, seismiske og vulkanske fænomener samt brande, som på grund af stedet, hvor de forekommer, deres omfang og hyppighed kan få alvorlige følger for samfundet), f.eks. oversvømmelser, jordskred og sammensynkning, laviner, skovbrande, jordskælv og vulkanudbrud.</skos:definition>
		<skos:prefLabel xml:lang="de">Gebiete mit naturbedingten Risiken</skos:prefLabel>
		<skos:definition xml:lang="de">Gefährdete Gebiete, eingestuft nach naturbedingten Risiken (sämtliche atmosphärischen, hydrologischen, seismischen, vulkanischen Phänomene sowie Naturfeuer, die aufgrund ihres örtlichen Auftretens sowie ihrer Schwere und Häufigkeit signifikante Auswirkungen auf die Gesellschaft haben können), z. B. Überschwemmungen, Erdrutsche und Bodensenkungen, Lawinen, Waldbrände, Erdbeben oder Vulkanausbrüche.</skos:definition>
		<skos:prefLabel xml:lang="el">Ζώνες φυσικών κινδύνων</skos:prefLabel>
		<skos:definition xml:lang="el">Χαρακτηρισμός ευάλωτων περιοχών ανάλογα με τους φυσικούς κινδύνους (όλα τα ατμοσφαιρικά, υδρολογικά, σεισμικά, ηφαιστειακά φαινόμενα και τα φαινόμενα καταστροφικών πυρκαγιών που, λόγω της θέσης, της σφοδρότητας και της συχνότητάς τους, είναι δυνατό να έχουν σοβαρές επιπτώσεις στην κοινωνία), π.χ. πλημμύρες, κατολισθήσεις και καθιζήσεις, χιονοστιβάδες, δασικές πυρκαγιές, σεισμοί, εκρήξεις ηφαιστείων.</skos:definition>
		<skos:prefLabel xml:lang="es">Zonas de riesgos naturales</skos:prefLabel>
		<skos:definition xml:lang="es">Zonas vulnerables caracterizadas por la existencia de riesgos de carácter natural (cualquier fenómeno atmosférico, hidrológico, sísmico, volcánico o incendio natural que, debido a su localización, gravedad o frecuencia, pueda afectar negativamente a la población), p. ej., inundaciones, corrimientos de tierra y hundimientos, aludes, incendios forestales, terremotos, erupciones volcánicas.</skos:definition>
		<skos:prefLabel xml:lang="et">Looduslikud ohutsoonid</skos:prefLabel>
		<skos:definition xml:lang="et">Tundlikud alad, mida iseloomustavad looduslikud riskitegurid (kõik atmosfäärilised, hüdroloogilised, seismilised, vulkaanilised ja looduspõlengute nähtused, mis oma asukoha, intensiivsuse ja sageduse tõttu võivad ühiskonnale tõsist kahju tuua), nt üleujutused, maalihked ja pinnase vajumine, laviinid, metsatulekahjud, maavärinad, vulkaanipursked.</skos:definition>
		<skos:prefLabel xml:lang="fi">Luonnonriskialueet</skos:prefLabel>
		<skos:definition xml:lang="fi">Luonnonkatastrofien (kaikki ilmakehästä johtuvat, hydrologiset, seismiset, tuliperäiset ja maastopaloilmiöt, joilla sijaintinsa, vakavuutensa ja yleisyytensä vuoksi voi mahdollisesti olla vakavia vaikutuksia yhteiskuntaan), kuten tulvien, maanvyöryjen ja vajoamisen, lumivyöryjen, metsäpalojen, maanjäristysten ja tulivuortenpurkausten, mukaan luokitellut riskialueet.</skos:definition>
		<skos:prefLabel xml:lang="fr">Zones à risque naturel</skos:prefLabel>
		<skos:definition xml:lang="fr">Zones sensibles caractérisées en fonction des risques naturels (tous les phénomènes atmosphériques, hydrologiques, sismiques, volcaniques, ainsi que les feux de friche qui peuvent, en raison de leur situation, de leur gravité et de leur fréquence, nuire gravement à la société), tels qu'inondations, glissements et affaissements de terrain, avalanches, incendies de forêts, tremblements de terre et éruptions volcaniques.</skos:definition>
		<skos:prefLabel xml:lang="hu">Természeti kockázati zónák</skos:prefLabel>
		<skos:definition xml:lang="hu">Természeti veszélyek, így pl. árvizek, földcsuszamlások, felszínsüllyedések, lavinák, erdőtüzek, földrengések, vulkánkitörések (minden légköri, hidrológiai, szeizmikus, vulkanikus és futótűzjelenség, amely – helye, súlyossága és előfordulási gyakorisága alapján – magában hordozza a komoly társadalmi károk okozásának lehetőségét) alapján jellemzett veszélyeztetett területek.</skos:definition>
		<skos:prefLabel xml:lang="it">Zone a rischio naturale</skos:prefLabel>
		<skos:definition xml:lang="it">Zone sensibili caratterizzate in base ai rischi naturali (cioè tutti i fenomeni atmosferici, idrologici, sismici, vulcanici e gli incendi che, per l’ubicazione, la gravità e la frequenza, possono avere un grave impatto sulla società), ad esempio inondazioni, slavine e subsidenze, valanghe, incendi di boschi/foreste, terremoti, eruzioni vulcaniche.</skos:definition>
		<skos:prefLabel xml:lang="lt">Gamtinių pavojų zonos</skos:prefLabel>
		<skos:definition xml:lang="lt">Pažeidžiamos vietovės, suskirstytos pagal gamtinio pavojaus pobūdį (visi atmosferiniai, hidrologiniai, seisminiai, vulkaniniai ir savaiminių gaisrų reiškiniai, kurie dėl savo vietos, stiprumo ir dažnumo kelia didelę grėsmę visuomenei), pvz., potvyniai, nuošliaužos ir žemės nusėdimas, griūtys, miškų gaisrai, žemės drebėjimai, ugnikalnių išsiveržimai.</skos:definition>
		<skos:prefLabel xml:lang="lv">Dabas apdraudējuma zonas</skos:prefLabel>
		<skos:definition xml:lang="lv">Apgabali, kam raksturīgi dabas apdraudējumi (visas atmosfēriskās, hidroloģiskās, seismiskās, vulkāniskās parādības un dabiskie ugunsgrēki, kas sakarā ar atrašanās vietu, apjomu vai biežumu var nopietni skart sabiedrību), piemēram, plūdi, zemes nogruvumi un iegrimšana, lavīnas, mežu ugunsgrēki, zemestrīces un vulkānu izvirdumi.</skos:definition>
		
		<skos:prefLabel xml:lang="mt">Żoni ta' riskju naturali</skos:prefLabel>
		<skos:definition xml:lang="mt">Żoni vulnerabbli kkaratterizzati skond perikli naturali (kull fenomenu atmosferiku, idroloġiku, sismiku, vulkaniku u tan-nirien mifruxa li, minħabba fejn jinsabu, il-qawwa, u l-frekwenza tagħhom, għandhom il-potenzjal li jaffettwaw b'mod gravi s-soċjetà), eż. għargħar, żerżiq ta' l-art u ċediment ta' l-art, valangi, nirien fil-foresti, terremoti, eruzzjonijiet vulkaniċi.</skos:definition>		
		
		<skos:prefLabel xml:lang="nl">Gebieden met natuurrisico'es</skos:prefLabel>
		<skos:definition xml:lang="nl">Kwetsbare gebieden die worden gekenmerkt door natuurrisico's (alle atmosferische, hydrologische, seismische, vulkanische verschijnselen en ongecontroleerde branden die door hun locatie, hevigheid en frequentie, mogelijk ernstige maatschappelijke gevolgen kunnen hebben), zoals overstromingen, aardverschuivingen en -verzakkingen, lawines, bosbranden, aardbevingen en vulkaanuitbarstingen.</skos:definition>
		<skos:prefLabel xml:lang="pl">Strefy zagrożenia naturalnego</skos:prefLabel>
		<skos:definition xml:lang="pl">Obszary zagrożone charakteryzowane na podstawie zagrożeń naturalnych (wszystkie zjawiska atmosferyczne, hydrologiczne, sejsmiczne, wulkaniczne oraz pożary, które, ze względu na swoją lokalizację, dotkliwość i częstotliwość mogą wywierać poważny wpływ na społeczeństwo), np. powodzie, osunięcia ziemi i osiadanie gruntu, lawiny, pożary lasów, trzęsienia ziemi, wybuchy wulkanów.</skos:definition>
		<skos:prefLabel xml:lang="pt">Zonas de risco natural</skos:prefLabel>
		<skos:definition xml:lang="pt">Zonas sensíveis, caracterizadas de acordo com os riscos naturais (todos os fenómenos atmosféricos, hidrológicos, sísmicos, vulcânicos e os incêndios que, pela sua localização, gravidade e frequência, possam afectar gravemente a sociedade), como sejam inundações, deslizamentos de terras e subsidências, avalanches, incêndios florestais, sismos, erupções vulcânicas.</skos:definition>
		<skos:prefLabel xml:lang="ro">Zone de risc natural</skos:prefLabel>
		<skos:definition xml:lang="ro">Zone vulnerabile caracterizate în funcţie de riscurile naturale (orice fenomen atmosferic, hidrologic, seismic, vulcanic, precum şi incendiile, care, din cauza locaţiei, a gravităţii şi a frecvenţei, pot afecta grav societatea), precum inundaţiile, alunecările şi surpările de teren, avalanşele, incendiile forestiere, cutremurele de pământ şi erupţiile vulcanice.</skos:definition>
		<skos:prefLabel xml:lang="sk">Zóny prírodného rizika</skos:prefLabel>
		<skos:definition xml:lang="sk">Citlivé oblasti charakterizované podľa prírodných rizík (všetky atmosférické, hydrologické, seizmické, vulkanické javy a ničivé požiare, ktoré môžu mať s ohľadom na ich polohu, závažnosť a početnosť vážny vplyv na spoločnosť), napr. záplavy, zosuvy pôdy a pokles terénu, lavíny, lesné požiare, zemetrasenia, sopečné výbuchy.</skos:definition>
		<skos:prefLabel xml:lang="sl">Območja nevarnosti naravnih nesreč</skos:prefLabel>
		<skos:definition xml:lang="sl">Ranljiva območja, opredeljena glede na naravna tveganja (vsi atmosferski, hidrološki, seizmični, vulkanski pojavi in požari, ki zaradi svoje lokacije, resnosti in pogostosti lahko resno ogrozijo družbo), npr. poplave, zemeljski plazovi in pogrezanje tal, snežni plazovi, gozdni požari, potresi, vulkanski izbruhi.</skos:definition>
		<skos:prefLabel xml:lang="sv">Naturliga riskområden</skos:prefLabel>
		<skos:definition xml:lang="sv">Sårbara områden klassificerade efter naturliga risker (alla atmosfäriska, hydrologiska, seismiska och vulkaniska fenomen samt bränder som på grund av läge, omfattning och frekvens har potential att allvarligt påverka samhället), exempelvis översvämningar, jordskred och sättningar, laviner, skogsbränder, jordbävningar, vulkanutbrott.</skos:definition>
		<!--
		<skos:prefLabel xml:lang="el">SAMPLE ALTERNATIVE EXPRESSION - αναφορά</skos:prefLabel>
		<skos:definition xml:lang="el">Συστήματα συντεταγμένων</skos:definition>
		<dct:description xml:lang="el">Συστήματα για μονοσήμαντη αναφορά χωρικών πληροφοριών στον χώρο, ως σύνολο συντεταγμένων (x,y,z) ή/και γεωγραφικό πλάτος και μήκος και ύψος, με βάση γεωδαιτικό οριζόντιο και κατακόρυφο σύστημα αναφοράς (datum).</dct:description>
		-->
		<skos:inScheme rdf:resource="http://inspire-registry.jrc.ec.europa.eu/registers/Themes/items"/>
	</inspire:Theme>
	<inspire:Theme rdf:about="http://inspire-registry.jrc.ec.europa.eu/registers/FCD/items/26">
		<!-- <owl:sameIndividualAs rdf:resource="http://www.eionet.europa.eu/gemet/theme_concepts?th=26&ns=5" /> -->
		<inspire:itemStatus>valid</inspire:itemStatus>
		<inspire:dateAccepted>2008-12-05T17:00:30.610+01:00</inspire:dateAccepted>
		<skos:prefLabel xml:lang="en">Atmospheric conditions</skos:prefLabel>
		<skos:definition xml:lang="en">Physical conditions in the atmosphere. Includes spatial data based on measurements, on models or on a combination thereof and includes measurement locations.</skos:definition>
		<dct:description xml:lang="en">Historical versions of the theme definition are found in the INSPIRE IMS and Scoping papers:
• Spatial data reflecting the physical conditions of the air and atmosphere, either as isolines, grids or other spatial forms. These can be based on measurements or models. This could also include the measurement locations. (INSPIRE IMS, 2003)
• Physical conditions in the atmosphere, represented as lines, grids or points. Includes spatial data sets based on measurements, on models or on a combination thereof and includes measurement locations. (INSPIRE Scoping, 2004)
In order to place into context the range of spatial data types relevant to this theme, we consider the typical ‘forecast cycle’ of a national meteorological service (NMS). This will: (a) collect meteorological observations over (say) a six-hour interval, (b) ‘assimilate’ these into a numerical model to produce an estimate of the current atmospheric state, (c) use this analysis as the initial condition for a model forecast run forward in time (typically out to several days). Four broad types of data are involved at different phases of the cycle:
1. Observations: around 11000 surface stations globally make up the Global Observing System, reporting such atmospheric parameters as weather, cloud, temperature, humidity, wind, visibility, pressure. A subset of these stations make ‘climate observations’ which include daily temperature minimum and maximum, sunshine hours, rainfall amount etc. In addition, around 1000 ‘upper-air’ stations make radiosonde (free-rising balloon) observations of pressure, wind, temperature and humidity. Voluntary observing ship and drifting buoys make marine observations including sea surface temperature, and wave height and period. Several hundred thousand reports per day of pressure, winds and temperature are made from aircraft observations.
2. Synoptic analysis: Gridded wind, temperature, humidity, geopotential height, precipitation, etc. Also, ‘sensible weather’ elements (fronts, cloud, thunderstorm activity etc) will be analysed.
3. Forecasts: Numerous forecast products are produced operationally. A conventional weather forecast contains similar elements to the synoptic analysis.
4. Climatological data: Long-term time-series’ of data (either observations or analyses) may be analysed statistically to create climatologies (e.g. 20th century decadal averages, seasonal/monthly minimum or maximum, etc.).
There is considerable overlap and ambiguity between the themes ‘Atmospheric conditions’ and ‘Meteorological geographical features’ – e.g. weather conditions (‘Meteorological geographical features’) including precipitation, temperature, wind etc. are precisely components of the atmospheric state (‘Atmospheric conditions’). Numerous suggestions have been made by stakeholders to resolve this ambiguity. They include:
• merging the themes (it is impossible to amend the Directive, but it would be sensible to consider the themes jointly during data specification development)
• distinguishing ‘field-based data’ (Atmospheric conditions) from ‘point-based data’ (Meteorological geographical features)
• distinguishing ‘time-series &amp; near-real-time data’ (Atmospheric conditions) from ‘gridded climate data’ (Meteorological geographical features)
• distinguishing ‘climate data’ (Atmospheric conditions) from ‘observations and forecasts’ (Meteorological geographical features)
To resolve the ambiguity between themes, we consider the multi-level approach to data needs assessment applied in the INSPIRE ‘Environmental Thematic User Needs Position Paper’ (2002). Data at local or regional level are often needed for management and policy implementation, while lower resolution (‘smaller scale’) data are often required for reporting and policy development/evaluation. The latter includes summaries and integrated data products.
The scope of ‘Atmospheric conditions’ thematic data should be limited to (six-hourly) synoptic analyses and forecasts (typically gridded model fields), climatological data, and other integrated and/or summary data.
Ambiguity remains in some areas. For instance, it is unclear whether the Directive definition should include air quality information (e.g. airborne particulates, atmospheric chemistry). Similarly, while marine observations are collected in support of meteorological forecasting, they include parameters associated with the oceanographic/sea themes. Certain physical parameters of the atmospheric boundary-layer could be associated either to the atmospheric or oceanographic themes. These ambiguities are referred to the TWG and will be informed also by Use Cases and User Requirements.
The WMO operates a dedicated network (the Global Telecommunications System) to distribute observations and data products. Data exchange is governed by WMO Resolution 40, which provides for free and unrestricted exchange of observational data ‘essential’ for forecast activities. ‘Additional’ nominated data and products may be provided with charge, while all data must be supplied free of charge (excluding costs of reproduction and delivery) for research and education. . The ECOMET Catalogue (http://www.meteo.oma.be/ECOMET/Categories of data and products.htm) provides a ‘one-stop shop’ index of both ‘essential’ and chargeable data and product offerings from European NMSs. A similar catalogue is available for the European Centre for Medium-range Weather Forecasting (ECMWF) (http://www.ecmwf.int/products/catalogue/).</dct:description>
		<skos:prefLabel xml:lang="bg">Атмосферни условия</skos:prefLabel>
		<skos:definition xml:lang="bg">Физически атмосферни условия. Включва пространствени данни, основаващи се на измервания, на модели или на комбинация от двете, както и местата, където са направени измерванията.</skos:definition>
		<skos:prefLabel xml:lang="cs">Stav ovzduší</skos:prefLabel>
		<skos:definition xml:lang="cs">Fyzikální stav ovzduší. Zahrnuje prostorová data založená na měřeních, modelech nebo jejich kombinaci, jakož i místa měření.</skos:definition>
		<skos:prefLabel xml:lang="da">Atmosfæriske forhold</skos:prefLabel>
		<skos:definition xml:lang="da">Fysiske forhold i atmosfæren. Omfatter geodata, der bygger på målinger, modeller eller begge dele; omfatter også målepunkternes placering.</skos:definition>
		<skos:prefLabel xml:lang="de">Atmosphärische Bedingungen</skos:prefLabel>
		<skos:definition xml:lang="de">Physikalische Bedingungen in der Atmosphäre. Dazu zählen Geodaten auf der Grundlage von Messungen, Modellen oder einer Kombination aus beiden sowie Angabe der Messstandorte.</skos:definition>
		<skos:prefLabel xml:lang="el">Ατμοσφαιρικές συνθήκες</skos:prefLabel>
		<skos:definition xml:lang="el">Φυσικές ιδιότητες της ατμόσφαιρας. Περιλαμβάνονται χωρικά δεδομένα βασιζόμενα σε μετρήσεις, σε μοντέλα ή σε συνδυασμό τους, καθώς και οι τοποθεσίες μετρήσεων.</skos:definition>
		<skos:prefLabel xml:lang="es">Condiciones atmosféricas</skos:prefLabel>
		<skos:definition xml:lang="es">Condiciones físicas de la atmósfera. Se incluirán datos espaciales basados en mediciones, modelos o en una combinación de ambos, así como los lugares de medición.</skos:definition>
		<skos:prefLabel xml:lang="et">Atmosfääritingimused</skos:prefLabel>
		<skos:definition xml:lang="et">Füüsikalised tingimused atmosfääris. Hõlmab mõõtmiste ja modelleerimise tulemusel või nende kahe meetodi kombineerimisel saadud ruumiandmeid ning mõõtmiskohti.</skos:definition>
		<skos:prefLabel xml:lang="fi">Ilmakehän tila</skos:prefLabel>
		<skos:definition xml:lang="fi">Ilmakehän fysikaaliset olosuhteet. Sisältää mittauksiin, malleihin tai näiden yhdistelmiin perustuvia paikkatietoja sekä tiedot mittauspaikoista.</skos:definition>
		<skos:prefLabel xml:lang="fr">Conditions atmosphériques</skos:prefLabel>
		<skos:definition xml:lang="fr">Conditions physiques dans l'atmosphère. Comprend les données géographiques fondées sur des mesures, sur des modèles ou sur une combinaison des deux, ainsi que les lieux de mesure.</skos:definition>
		<skos:prefLabel xml:lang="hu">Légköri viszonyok</skos:prefLabel>
		<skos:definition xml:lang="hu">A légkör fizikai jellemzői. Ide tartoznak a méréseken, modelleken vagy ezek kombinációján alapuló téradatok, továbbá a mérési helyek.</skos:definition>
		<skos:prefLabel xml:lang="it">Condizioni atmosferiche</skos:prefLabel>
		<skos:definition xml:lang="it">Condizioni fisiche dell’atmosfera. Questa voce comprende i dati territoriali basati su misurazioni, su modelli o su una combinazione dei due e comprende i punti di misurazione.</skos:definition>
		<skos:prefLabel xml:lang="lt">Atmosferos sąlygos</skos:prefLabel>
		<skos:definition xml:lang="lt">Fizinės atmosferos sąlygos. Tai apima matavimais, modeliais arba abiem būdais pagrįstus erdvinius duomenis, nurodant matavimo vietas.</skos:definition>
		<skos:prefLabel xml:lang="lv">Atmosfēras apstākļi</skos:prefLabel>
		<skos:definition xml:lang="lv">Fizikālie atmosfēras apstākļi. Tie ietver telpiskos datus, kuru pamatā ir mērījumi vai modeļi, vai to kombinācija, kā arī norādes par to veikšanas vietu.</skos:definition>
		
		<skos:prefLabel xml:lang="mt">Kondizzjonijiet atmosferiċi</skos:prefLabel>
		<skos:definition xml:lang="mt">Kondizzjonijiet fiżiċi fl-atmosfera. Hija inkluża data ġeografika bbażata fuq kejl, fuq mudelli jew fuq il-kombinazzjoni tagħhom kif ukoll is-siti tal-kejl.</skos:definition>		
		
		<skos:prefLabel xml:lang="nl">Atmosferische omstandigheden</skos:prefLabel>
		<skos:definition xml:lang="nl">Fysische omstandigheden in de atmosfeer, met inbegrip van ruimtelijke gegevens die gebaseerd zijn op metingen, modellen of een combinatie daarvan, en met inbegrip van meetlocaties.</skos:definition>
		<skos:prefLabel xml:lang="pl">Warunki atmosferyczne</skos:prefLabel>
		<skos:definition xml:lang="pl">Warunki fizyczne w atmosferze. Obejmują dane przestrzenne oparte na pomiarach, modelach lub na kombinacji tych dwóch elementów, a także lokalizacje pomiarów.</skos:definition>
		<skos:prefLabel xml:lang="pt">Condições atmosféricas</skos:prefLabel>
		<skos:definition xml:lang="pt">Condições físicas da atmosfera. Inclui dados geográficos baseados em medições, em modelos ou numa combinação de ambos, bem como os sítios de medição.</skos:definition>
		<skos:prefLabel xml:lang="ro">Condiţii atmosferice</skos:prefLabel>
		<skos:definition xml:lang="ro">Condiţiile fizice din atmosferă. Sunt incluse datele spaţiale bazate pe măsurători, pe modele sau pe o combinaţie între acestea, precum şi locaţiile de efectuare a măsurătorilor.</skos:definition>
		<skos:prefLabel xml:lang="sk">Atmosférické podmienky</skos:prefLabel>
		<skos:definition xml:lang="sk">Fyzikálne podmienky v atmosfére. Patria sem priestorové údaje založené na meraniach, modeloch alebo na kombinácii meraní a modelov vrátane miest meraní.</skos:definition>
		<skos:prefLabel xml:lang="sl">Ozračje</skos:prefLabel>
		<skos:definition xml:lang="sl">Fizikalne razmere v atmosferi. Vključujejo prostorske podatke, ki temeljijo na merjenjih, vzorcih ali na kombinaciji leteh, in merilne lokacije.</skos:definition>
		<skos:prefLabel xml:lang="sv">Atmosfäriska förhållanden</skos:prefLabel>
		<skos:definition xml:lang="sv">Fysikaliska förhållanden i atmosfären. Inbegriper rumsliga data baserade på mätningar, modeller eller en kombination av dessa, samt mätpunkternas läge.</skos:definition>
		<!--
		<skos:prefLabel xml:lang="el">SAMPLE ALTERNATIVE EXPRESSION - αναφορά</skos:prefLabel>
		<skos:definition xml:lang="el">Συστήματα συντεταγμένων</skos:definition>
		<dct:description xml:lang="el">Συστήματα για μονοσήμαντη αναφορά χωρικών πληροφοριών στον χώρο, ως σύνολο συντεταγμένων (x,y,z) ή/και γεωγραφικό πλάτος και μήκος και ύψος, με βάση γεωδαιτικό οριζόντιο και κατακόρυφο σύστημα αναφοράς (datum).</dct:description>
		-->
		<skos:inScheme rdf:resource="http://inspire-registry.jrc.ec.europa.eu/registers/Themes/items"/>
	</inspire:Theme>
	<inspire:Theme rdf:about="http://inspire-registry.jrc.ec.europa.eu/registers/FCD/items/27">
		<!-- <owl:sameIndividualAs rdf:resource="http://www.eionet.europa.eu/gemet/theme_concepts?th=27&ns=5" /> -->
		<inspire:itemStatus>valid</inspire:itemStatus>
		<inspire:dateAccepted>2008-12-05T17:00:30.669+01:00</inspire:dateAccepted>
		<skos:prefLabel xml:lang="en">Meteorological geographical features</skos:prefLabel>
		<skos:definition xml:lang="en">Weather conditions and their measurements; precipitation, temperature, evapotranspiration, wind speed and direction.</skos:definition>
		<dct:description xml:lang="en">Historical versions of the theme definition are found in the INSPIRE IMS and Scoping papers:
• Weather conditions and their measurements; precipitation, temperature, evapotranspiration, wind. (INSPIRE IMS, 2003)
• Weather conditions and their measurements; precipitation, temperature, evapotranspiration, wind speed and direction (INSPIRE Scoping, 2004)
In order to place into context the range of spatial data types relevant to this theme, we consider the typical ‘forecast cycle’ of a national meteorological service (NMS). This will: (a) collect meteorological observations over (say) a six-hour interval, (b) ‘assimilate’ these into a numerical model to produce an estimate of the current atmospheric state, (c) use this analysis as the initial condition for a model forecast run forward in time (typically out to several days). Four broad types of data are involved at different phases of the cycle:
1. Observations: around 11000 surface stations globally make up the Global Observing System, reporting such atmospheric parameters as weather, cloud, temperature, humidity, wind, visibility, pressure. A subset of these stations make ‘climate observations’ which include daily temperature minimum and maximum, sunshine hours, rainfall amount etc. In addition, around 1000 ‘upper-air’ stations make radiosonde (free-rising balloon) observations of pressure, wind, temperature and humidity. Voluntary observing ship and drifting buoys make marine observations including sea surface temperature, and wave height and period. Several hundred thousand reports per day of pressure, winds and temperature are made from aircraft observations.
2. Synoptic analysis: Gridded wind, temperature, humidity, geopotential height, precipitation, etc. Also, ‘sensible weather’ elements (fronts, cloud, thunderstorm activity etc) will be analysed.
3. Forecasts: Numerous forecast products are produced operationally. A conventional weather forecast contains similar elements to the synoptic analysis.
4. Climatological data: Long-term time-series’ of data (either observations or analyses) may be analysed statistically to create climatologies (e.g. 20th century decadal averages, seasonal/monthly minimum or maximum, etc.).
There is considerable overlap and ambiguity between the themes ‘Atmospheric conditions’ and ‘Meteorological geographical features’ – e.g. weather conditions (‘Meteorological geographical features’) including precipitation, temperature, wind etc. are precisely components of the atmospheric state (‘Atmospheric conditions’). Numerous suggestions have been made by stakeholders to resolve this ambiguity. They include:
• merging the themes (it is impossible to amend the Directive, but it would be sensible to consider the themes jointly during data specification development)
• distinguishing ‘field-based data’ (Atmospheric conditions) from ‘point-based data’ (Meteorological geographical features)
• distinguishing ‘time-series &amp; near-real-time data’ (Atmospheric conditions) from ‘gridded climate data’ (Meteorological geographical features)
• distinguishing ‘climate data’ (Atmospheric conditions) from ‘observations and forecasts’ (Meteorological geographical features)
To resolve the ambiguity between themes, we consider the multi-level approach to data needs assessment applied in the INSPIRE ‘Environmental Thematic User Needs Position Paper’ (2002). Data at local or regional level are often needed for management and policy implementation, while lower resolution (‘smaller scale’) data are often required for reporting and policy development/evaluation. The latter includes summaries and integrated data products.
The scope of ‘Meteorological geographical features’ thematic data should be limited to local-level high-resolution (weather-related) data, typically observations.
• This includes synoptic observations from stations making up the WMO RA VI (European) Regional Basic Synoptic Network.
The WMO operates a dedicated network (the Global Telecommunications System) to distribute observations and data products. Data exchange is governed by WMO Resolution 40, which provides for free and unrestricted exchange of observational data ‘essential’ for forecast activities. ‘Additional’ nominated data and products may be provided with charge, while all data must be supplied free of charge (excluding costs of reproduction and delivery) for research and education. The ECOMET Catalogue (http://www.meteo.oma.be/ECOMET/Categories of data and products.htm) provides a ‘one-stop shop’ index of both ‘essential’ and chargeable data and product offerings from European NMSs. A similar catalogue is available for the European Centre for Medium-range Weather Forecasting (ECMWF) (http://www.ecmwf.int/products/catalogue/).</dct:description>
		<skos:prefLabel xml:lang="bg">Метеорологични географски характеристики</skos:prefLabel>
		<skos:definition xml:lang="bg">Атмосферни условия и измерването им; валежи, температура, евапотранспирация, скорост и посока на вятъра.</skos:definition>
		<skos:prefLabel xml:lang="cs">Zeměpisné meteorologické prvky</skos:prefLabel>
		<skos:definition xml:lang="cs">Povětrnostní podmínky a jejich měření; srážky, teplota, výpar z půdy a rostlinného pokryvu, rychlost a směr větru.</skos:definition>
		<skos:prefLabel xml:lang="da">Meteorologisk-geografiske forhold</skos:prefLabel>
		<skos:definition xml:lang="da">Vejrforhold og målinger heraf; nedbør, temperatur, evapotranspiration, vindhastighed og -retning.</skos:definition>
		<skos:prefLabel xml:lang="de">Meteorologisch-geografische Kennwerte</skos:prefLabel>
		<skos:definition xml:lang="de">Witterungsbedingungen und deren Messung; Niederschlag, Temperatur, Gesamtverdunstung (Evapotranspiration), Windgeschwindigkeit und Windrichtung.</skos:definition>
		<skos:prefLabel xml:lang="el">Μετεωρολογικά γεωγραφικά χαρακτηριστικά</skos:prefLabel>
		<skos:definition xml:lang="el">Καιρικές συνθήκες και οι μετρήσεις τους· ατμοσφαιρικές κατακρημνίσεις, θερμοκρασία, εξατμισοδιαπνοή, ταχύτητα και διεύθυνση ανέμου.</skos:definition>
		<skos:prefLabel xml:lang="es">Aspectos geográficos de carácter meteorológico</skos:prefLabel>
		<skos:definition xml:lang="es">Condiciones meteorológicas y sus mediciones; precipitaciones, temperaturas, evapotranspiración, velocidad y dirección del viento.</skos:definition>
		<skos:prefLabel xml:lang="et">Meteoroloogilis-geograafilised tunnusjooned</skos:prefLabel>
		<skos:definition xml:lang="et">Ilmastikutingimused ja nende mõõtmine; sademed, temperatuur, aurumine, tuule kiirus ja suund.</skos:definition>
		<skos:prefLabel xml:lang="fi">Ilmaston maantieteelliset ominaispiirteet</skos:prefLabel>
		<skos:definition xml:lang="fi">Sääolot ja niihin liittyvät mittaukset; sademäärä, lämpötila, kokonaishaihdunta, tuulen nopeus ja suunta.</skos:definition>
		<skos:prefLabel xml:lang="fr">Caractéristiques géographiques météorologiques</skos:prefLabel>
		<skos:definition xml:lang="fr">Conditions météorologiques et leur mesure: précipitations, température, évapotranspiration, vitesse et direction du vent.</skos:definition>
		<skos:prefLabel xml:lang="hu">Meteorológiai földrajzi jellemzők</skos:prefLabel>
		<skos:definition xml:lang="hu">Időjárási viszonyok és mérésük; csapadék, hőmérséklet, a felszín és a növényzet párolgása, a szél sebessége és iránya.</skos:definition>
		<skos:prefLabel xml:lang="it">Elementi geografici meteorologici</skos:prefLabel>
		<skos:definition xml:lang="it">Condizioni meteorologiche e relative misurazioni; precipitazioni, temperatura, evapotraspirazione, velocità e direzione dei venti.</skos:definition>
		<skos:prefLabel xml:lang="lt">Meteorologinės geografinės sąlygos</skos:prefLabel>
		<skos:definition xml:lang="lt">Oro sąlygos ir jų matavimai; krituliai, temperatūra, evapotranspiracija, vėjo greitis ir kryptis.</skos:definition>
		<skos:prefLabel xml:lang="lv">Meteoroloģiski ģeogrāfiskie raksturlielumi</skos:prefLabel>
		<skos:definition xml:lang="lv">Laika apstākļi un to mērījumi; nokrišņi, temperatūra, iztvaikošana, vēja ātrums un virziens.</skos:definition>
		
		<skos:prefLabel xml:lang="mt">Karatteristiċi ġeografiċi meteoroloġiċi</skos:prefLabel>
		<skos:definition xml:lang="mt">Il-kondizzjonijiet tat-temp u l-kejl tagħhom; il-preċipitazzjoni, it-temperatura, l-evapotraspirazzjoni, il-veloċità u ddirezzjoni tar-riħ.</skos:definition>		
		
		<skos:prefLabel xml:lang="nl">Meteorologische geografische kenmerken</skos:prefLabel>
		<skos:definition xml:lang="nl">Weersomstandigheden en de meting daarvan; neerslag, temperatuur, verdamping, windsnelheid en windrichting.</skos:definition>
		<skos:prefLabel xml:lang="pl">Warunki meteorologiczno-geograficzne</skos:prefLabel>
		<skos:definition xml:lang="pl">Warunki atmosferyczne i ich pomiary; opad atmosferyczny, temperatura, ewapotranspiracja, prędkość i kierunek wiatru.</skos:definition>
		<skos:prefLabel xml:lang="pt">Características geometeorológicas</skos:prefLabel>
		<skos:definition xml:lang="pt">Condições atmosféricas e sua medição; precipitação, temperatura, evapotranspiração, velocidade e direcção do vento.</skos:definition>
		<skos:prefLabel xml:lang="ro">Caracteristici geografice meteorologice</skos:prefLabel>
		<skos:definition xml:lang="ro">Condiţiile meteorologice şi măsurătorile acestora: precipitaţii, temperatură, evapotranspiraţie, viteza şi direcţia vântului.</skos:definition>
		<skos:prefLabel xml:lang="sk">Meteorologické geografické prvky</skos:prefLabel>
		<skos:definition xml:lang="sk">Poveternostné podmienky a ich merania; zrážky, teplota, evapotranspirácia, rýchlosť a smer vetra.</skos:definition>
		<skos:prefLabel xml:lang="sl">Meteorološke značilnosti</skos:prefLabel>
		<skos:definition xml:lang="sl">Vremenske razmere in njihova merjenja; padavine, temperatura, izhlapevanje, hitrost in smer vetra.</skos:definition>
		<skos:prefLabel xml:lang="sv">Geografiska meteorologiska förhållanden</skos:prefLabel>
		<skos:definition xml:lang="sv">Väderförhållanden och mätningar av dessa; nederbörd, temperatur, evapotranspiration, vindhastighet och vindriktning.</skos:definition>
		<!--
		<skos:prefLabel xml:lang="el">SAMPLE ALTERNATIVE EXPRESSION - αναφορά</skos:prefLabel>
		<skos:definition xml:lang="el">Συστήματα συντεταγμένων</skos:definition>
		<dct:description xml:lang="el">Συστήματα για μονοσήμαντη αναφορά χωρικών πληροφοριών στον χώρο, ως σύνολο συντεταγμένων (x,y,z) ή/και γεωγραφικό πλάτος και μήκος και ύψος, με βάση γεωδαιτικό οριζόντιο και κατακόρυφο σύστημα αναφοράς (datum).</dct:description>
		-->
		<skos:inScheme rdf:resource="http://inspire-registry.jrc.ec.europa.eu/registers/Themes/items"/>
	</inspire:Theme>
	<inspire:Theme rdf:about="http://inspire-registry.jrc.ec.europa.eu/registers/FCD/items/28">
		<!-- <owl:sameIndividualAs rdf:resource="http://www.eionet.europa.eu/gemet/theme_concepts?th=28&ns=5" /> -->
		<inspire:itemStatus>valid</inspire:itemStatus>
		<inspire:dateAccepted>2008-12-05T17:00:30.726+01:00</inspire:dateAccepted>
		<skos:prefLabel xml:lang="en">Oceanographic geographical features</skos:prefLabel>
		<skos:definition xml:lang="en">Physical conditions of oceans (currents, salinity, wave heights, etc.).</skos:definition>
		<dct:description xml:lang="en">Historical versions of the theme definition are found in the INSPIRE IMS and Scoping papers:
• The measurable physical conditions of oceans e.g. salinity, oxygen, other chemical components, currents. Representation e.g. as isolines, grids or other spatial organisation. Based on measurements directly or combined with models. (INSPIRE IMS, 2003)
• Physical conditions of oceans (e.g. currents, salinity, etc) represented as lines, grids or points. Includes spatial data sets based on measurements, on models or on a combination thereof and includes measurement locations (INSPIRE Scoping, 2004)
Both ‘Oceanographic geographical features’ and ‘Sea-regions’ are concerned with physical conditions of marine water-masses. (This is a similar overlap to that which exists for themes 7.13 “Atmospheric Conditions” and 7.14 “Meteorological geographical features”.) To resolve the ambiguity, we consider the multi-level approach to data needs assessment applied in ETC. Data at local or regional level are often needed for management and policy implementation, while lower resolution (‘smaller scale’) data are often required for reporting and policy development/evaluation. The latter includes summaries and integrated data products.
We regard the theme “Oceanographic geographical features” as being concerned with the high seas and larger oceanic physical/dynamic structures.
Operational forecasting of ocean dynamic physical conditions – together with the prerequisite observations – are key elements of this theme (e.g. through the GMES Marine Core Service), with France and UK both running a operational facilities.
Relevant observational data include:
• remote-sensing of sea surface temperature, dynamic topography (by satellite altimeter), synthetic aperture radar winds, ocean colour (for primary productivity and sedimentation)
• drifting buoys – surface velocity, temperature, atmospheric pressure
• ships-of-opportunity and regular voluntary observing ships provide temperature (bathythermograph) profiles
• Argo floats provide temperature and salinity profiles</dct:description>
		<skos:prefLabel xml:lang="bg">Океанографски географски характеристики</skos:prefLabel>
		<skos:definition xml:lang="bg">Физическо състояние на океаните (течения, соленост, височина на вълните и други).</skos:definition>
		<skos:prefLabel xml:lang="cs">Zeměpisné oceánografické prvky</skos:prefLabel>
		<skos:definition xml:lang="cs">Fyzikální stav oceánů (proudy, slanost, výška vln atd.).</skos:definition>
		<skos:prefLabel xml:lang="da">Oceanografiske/geografiske forhold</skos:prefLabel>
		<skos:definition xml:lang="da">Fysiske forhold til havs (strømme, saltholdighed, bølgehøjde osv.)</skos:definition>
		<skos:prefLabel xml:lang="de">Ozeanografisch-geografische Kennwerte</skos:prefLabel>
		<skos:definition xml:lang="de">Physikalische Bedingungen der Ozeane (Strömungsverhältnisse, Salinität, Wellenhöhe usw.).</skos:definition>
		<skos:prefLabel xml:lang="el">Ωκεανογραφικά γεωγραφικά χαρακτηριστικά</skos:prefLabel>
		<skos:definition xml:lang="el">Φυσικές ιδιότητες των ωκεανών (ρεύματα, αλατότητα, ύψος κυμάτων, κ.λπ.).</skos:definition>
		<skos:prefLabel xml:lang="es">Rasgos geográficos oceanográficos</skos:prefLabel>
		<skos:definition xml:lang="es">Condiciones físicas de los océanos (corrientes, salinidad, altura del oleaje, etc.).</skos:definition>
		<skos:prefLabel xml:lang="et">Okeanograafilis-geograafilised tunnusjooned</skos:prefLabel>
		<skos:definition xml:lang="et">Füüsikalised tingimused ookeanides (hoovused, soolasisaldus, lainekõrgus jne).</skos:definition>
		<skos:prefLabel xml:lang="fi">Merentutkimuksen maantieteelliset ominaispiirteet</skos:prefLabel>
		<skos:definition xml:lang="fi">Merialueitten fysikaaliset olosuhteet (esimerkiksi virtaukset, suolapitoisuus ja aaltojen korkeus).</skos:definition>
		<skos:prefLabel xml:lang="fr">Caractéristiques géographiques océanographiques</skos:prefLabel>
		<skos:definition xml:lang="fr">Conditions physiques des océans (courants, salinité, hauteur des vagues, etc.).</skos:definition>
		<skos:prefLabel xml:lang="hu">Oceanográfiai földrajzi jellemzők</skos:prefLabel>
		<skos:definition xml:lang="hu">Az óceánok fizikai jellemzői (áramlatok, sótartalom, hullámmagasság stb.).</skos:definition>
		<skos:prefLabel xml:lang="it">Elementi geografici oceanografici</skos:prefLabel>
		<skos:definition xml:lang="it">Elementi geografici oceanografici</skos:definition>
		<skos:prefLabel xml:lang="lt">Okeanografinės geografinės sąlygos</skos:prefLabel>
		<skos:definition xml:lang="lt">Fizinės vandenynų charakteristikos (srovės, druskingumas, bangų aukštis ir t. t.).</skos:definition>
		<skos:prefLabel xml:lang="lv">Okeanogrāfiski ģeogrāfiskie raksturlielumi</skos:prefLabel>
		<skos:definition xml:lang="lv">Okeānu fizikālie apstākļi (straumes, sāļums, viļņu augstums, utt.).</skos:definition>
		
		<skos:prefLabel xml:lang="mt">Karatteristiċi ġeografiċi oċeanografiċi</skos:prefLabel>
		<skos:definition xml:lang="mt">Kondizzjonijiet fiżiċi ta' l-oċeani (kurrenti, imluħa, għoli tal-mewġ, eċċ.).</skos:definition>		
		
		<skos:prefLabel xml:lang="nl">Oceanografische geografische kenmerken</skos:prefLabel>
		<skos:definition xml:lang="nl">Fysische kenmerken van oceanen (stroming, zoutgehalte, golfhoogte, enz.).</skos:definition>
		<skos:prefLabel xml:lang="pl">Warunki oceanograficzno-geograficzne</skos:prefLabel>
		<skos:definition xml:lang="pl">Warunki fizyczne oceanów (prądy, zasolenie, wysokość fal itd.).</skos:definition>
		<skos:prefLabel xml:lang="pt">Características oceanográficas</skos:prefLabel>
		<skos:definition xml:lang="pt">Condições físicas dos oceanos (correntes, salinidade, altura das ondas, etc.).</skos:definition>
		<skos:prefLabel xml:lang="ro">Caracteristici geografice oceanografice</skos:prefLabel>
		<skos:definition xml:lang="ro">Condiţii fizice ale oceanelor (curenţi, salinitate, înălţimea valurilor etc.).</skos:definition>
		<skos:prefLabel xml:lang="sk">Oceánografické geografické prvky</skos:prefLabel>
		<skos:definition xml:lang="sk">Fyzikálne vlastnosti oceánov (prúdy, slanosť, výška vĺn atď.).</skos:definition>
		<skos:prefLabel xml:lang="sl">Oceanogeografske značilnosti</skos:prefLabel>
		<skos:definition xml:lang="sl">Fizikalne razmere oceanov (tokovi, slanost, višina valov itd.).</skos:definition>
		<skos:prefLabel xml:lang="sv">Geografiska oceanografiska förhållanden</skos:prefLabel>
		<skos:definition xml:lang="sv">Fysikaliska förhållanden i oceanerna (strömmar, salthalt, våghöjd osv.).</skos:definition>
		<!--
		<skos:prefLabel xml:lang="el">SAMPLE ALTERNATIVE EXPRESSION - αναφορά</skos:prefLabel>
		<skos:definition xml:lang="el">Συστήματα συντεταγμένων</skos:definition>
		<dct:description xml:lang="el">Συστήματα για μονοσήμαντη αναφορά χωρικών πληροφοριών στον χώρο, ως σύνολο συντεταγμένων (x,y,z) ή/και γεωγραφικό πλάτος και μήκος και ύψος, με βάση γεωδαιτικό οριζόντιο και κατακόρυφο σύστημα αναφοράς (datum).</dct:description>
		-->
		<skos:inScheme rdf:resource="http://inspire-registry.jrc.ec.europa.eu/registers/Themes/items"/>
	</inspire:Theme>
	<inspire:Theme rdf:about="http://inspire-registry.jrc.ec.europa.eu/registers/FCD/items/29">
		<!-- <owl:sameIndividualAs rdf:resource="http://www.eionet.europa.eu/gemet/theme_concepts?th=29&ns=5" /> -->
		<inspire:itemStatus>valid</inspire:itemStatus>
		<inspire:dateAccepted>2008-12-05T17:00:30.846+01:00</inspire:dateAccepted>
		<skos:prefLabel xml:lang="en">Sea regions</skos:prefLabel>
		<skos:definition xml:lang="en">Physical conditions of seas and saline water bodies divided into regions and sub-regions with common characteristics.</skos:definition>
		<dct:description xml:lang="en">A historical version of the theme definition is found in the INSPIRE IMS paper:
• Seas and saline water bodies divided into regions and sub-regions. Each region with common characteristics, concerning water flow/ circulation, adjacent river catchments, bio-chemical or temperature of water, based on scientific criteria. Detailed information at regional level exist. (INSPIRE IMS, 2003)
Both ‘Oceanographic geographical features’ and ‘Sea-regions’ are concerned with physical conditions of marine water-masses. (This is a similar overlap to that which exists for themes 7.13 “Atmospheric Conditions” and 7.14 “Meteorological geographical features”.) To resolve the ambiguity, we consider the multi-level approach to data needs assessment applied in ETC. Data at local or regional level are often needed for management and policy implementation, while lower resolution (‘smaller scale’) data are often required for reporting and policy development/evaluation. The latter includes summaries and integrated data products.
We regard the “Sea regions” theme as focussing on the local/regional level coastal zone.
Whereas 7.15 ‘Oceanographic geographical features’ focuses on physical conditions and general circulation of offshore oceanic waters, the ‘Sea regions’ theme is concerned with marine features of the coastal zone – regions defined as ‘transitional waters’ and ‘coastal waters’ in the Water Framework Directive:
• transitional waters: bodies of surface water in the vicinity of river mouths which are partly saline in character as a result of their proximity to coastal waters but which are substantially influenced by freshwater flows
• coastal waters: surface water on the landward side of a line, every point of which is at a distance of one nautical mile on the seaward side from the nearest point of the baseline from which the breadth of territorial waters is measured, extending where appropriate up to the outer limit of transitional waters
The World Meteorological Organisation also has a geometry-based sea region classification, dividing the ocean into Marsden Squares.
Both biotic and physical parameters and indicators are important in the classification and delineation of sea regions. Physical data requirements for important indicators defined in the WFD and the Integrated Coastal Zone Management policy are outlined in the ETC paper. These include:
• nutrients (nitrate, phosphate and nitrogen: phosphorus ratio) by regional sea and water body type
• concentrations of hazardous substances and pollutants (incl. heavy metals, persistent organic pollutants)
• productivity indicators (incl. surface cholorophyll-a)
• biological classification of waters
• water masses/layers characterised by bulk temperature and salinity properties
• polar area features (incl. pack ice)
• wind (climatological and meteorolog• benthic parameters (sediment, benthic communities/habitats)
• sea level
• chemical species and concentrations
• physical characteristics (incl. temperature, salinity)
• currents (including surface currents)
• tidal zones
• waves</dct:description>
		<skos:prefLabel xml:lang="bg">Морски региони</skos:prefLabel>
		<skos:definition xml:lang="bg">Физическо състояние на моретата и солени водни маси, разделени на региони и подрегиони с общи характеристики.</skos:definition>
		<skos:prefLabel xml:lang="cs">Mořské oblasti</skos:prefLabel>
		<skos:definition xml:lang="cs">Fyzikální stav moří a slaných vod rozdělených do regionů a subregionů se společnými vlastnostmi.</skos:definition>
		<skos:prefLabel xml:lang="da">Havområder</skos:prefLabel>
		<skos:definition xml:lang="da">Fysiske forhold i have og saltholdige søer, opdelt på områder og delområder med fælles egenskaber.</skos:definition>
		<skos:prefLabel xml:lang="de">Meeresregionen</skos:prefLabel>
		<skos:definition xml:lang="de">Physikalische Bedingungen von Meeren und salzhaltigen Gewässern, aufgeteilt nach Regionen und Teilregionen mit gemeinsamen Merkmalen.</skos:definition>
		<skos:prefLabel xml:lang="el">Θαλάσσιες περιοχές</skos:prefLabel>
		<skos:definition xml:lang="el">Φυσικές ιδιότητες των θαλασσών και των αλατούχων υδατικών συστημάτων, με υποδιαίρεση ανά περιοχές και υποπεριοχές με κοινά χαρακτηριστικά.</skos:definition>
		<skos:prefLabel xml:lang="es">Regiones marinas</skos:prefLabel>
		<skos:definition xml:lang="es">Condiciones físicas de los mares y masas de aguas salinas, por regiones y subregiones con características comunes.</skos:definition>
		<skos:prefLabel xml:lang="et">Merepiirkonnad</skos:prefLabel>
		<skos:definition xml:lang="et">Füüsikalised tingimused meredes ja soolase veega veekogudes, mis on ühiste tunnuste alusel jaotatud piirkondadeks ja alampiirkondadeks.</skos:definition>
		<skos:prefLabel xml:lang="fi">Merialueet</skos:prefLabel>
		<skos:definition xml:lang="fi">Yhteisten ominaispiirteitten mukaisesti alueisiin ja osa-alueisiin jaoteltujen merien ja suolaisten vesistöjen fyysiset olosuhteet.</skos:definition>
		<skos:prefLabel xml:lang="fr">Régions maritimes</skos:prefLabel>
		<skos:definition xml:lang="fr">Conditions physiques des mers et des masses d'eau salée divisées en régions et en sous-régions à caractéristiques communes.</skos:definition>
		<skos:prefLabel xml:lang="hu">Tengeri régiók</skos:prefLabel>
		<skos:definition xml:lang="hu">A tengerek és sósvizű víztestek fizikai jellemzői, közös tulajdonságaik alapján régiókra és alrégiókra osztva.</skos:definition>
		<skos:prefLabel xml:lang="it">Regioni marine</skos:prefLabel>
		<skos:definition xml:lang="it">Condizioni fisiche dei mari e dei corpi idrici salmastri suddivisi in regioni e sottoregioni con caratteristiche comuni.</skos:definition>
		<skos:prefLabel xml:lang="lt">Jūrų regionai</skos:prefLabel>
		<skos:definition xml:lang="lt">Jūrų ir sūrių vandens telkinių, pagal bendras charakteristikas suskirstytų į regionus ir paregionius, fizinės charakteristikos.</skos:definition>
		<skos:prefLabel xml:lang="lv">Jūru reģioni</skos:prefLabel>
		<skos:definition xml:lang="lv">Pēc noteiktām kopīgām iezīmēm izveidotos apgabalos un apakšapgabalos sadalītu jūru un sālsūdens ūdenstilpņu fiziskie stāvokļi.</skos:definition>
		
		<skos:prefLabel xml:lang="mt">Reġjuni tal-baħar</skos:prefLabel>
		<skos:definition xml:lang="mt">Kondizzjonijiet fiżiċi ta' l-ibħra u korpi ta' ilma mielaħ imqassma f'reġjuni u sub-reġjuni b'karatteristiċi komuni.</skos:definition>		
		
		<skos:prefLabel xml:lang="nl">Zeegebieden</skos:prefLabel>
		<skos:definition xml:lang="nl">Fysische kenmerken van zeeën en zoutwateroppervlakken, ingedeeld in regio's en subregio's met gemeenschappelijke kenmerken.</skos:definition>
		<skos:prefLabel xml:lang="pl">Regiony morskie</skos:prefLabel>
		<skos:definition xml:lang="pl">Warunki fizyczne mórz i akwenów słonowodnych w podziale na regiony i subregiony o wspólnych cechach.</skos:definition>
		<skos:prefLabel xml:lang="pt">Regiões marinhas</skos:prefLabel>
		<skos:definition xml:lang="pt">Condições físicas dos mares e massas de água salinas divididas em regiões e sub-regiões com características comuns.</skos:definition>
		<skos:prefLabel xml:lang="ro">Regiuni maritime</skos:prefLabel>
		<skos:definition xml:lang="ro">Condiţii fizice ale mărilor şi corpurilor de apă sărată divizate în regiuni şi subregiuni cu caracteristici comune.</skos:definition>
		<skos:prefLabel xml:lang="sk">Morské regióny</skos:prefLabel>
		<skos:definition xml:lang="sk">Fyzikálne vlastnosti morí a útvarov slanej vody rozdelených na regióny a podregióny so spoločnými vlastnosťami.</skos:definition>
		<skos:prefLabel xml:lang="sl">Morske regije</skos:prefLabel>
		<skos:definition xml:lang="sl">Fizikalne razmere morij in slanih vodnih teles, razdeljenih v regije in podregije s skupnimi značilnostmi.</skos:definition>
		<skos:prefLabel xml:lang="sv">Havsområden</skos:prefLabel>
		<skos:definition xml:lang="sv">Fysikaliska förhållanden i hav och saltsjöar indelade i områden och delområden med likartade egenskaper.</skos:definition>
		<!--
		<skos:prefLabel xml:lang="el">SAMPLE ALTERNATIVE EXPRESSION - αναφορά</skos:prefLabel>
		<skos:definition xml:lang="el">Συστήματα συντεταγμένων</skos:definition>
		<dct:description xml:lang="el">Συστήματα για μονοσήμαντη αναφορά χωρικών πληροφοριών στον χώρο, ως σύνολο συντεταγμένων (x,y,z) ή/και γεωγραφικό πλάτος και μήκος και ύψος, με βάση γεωδαιτικό οριζόντιο και κατακόρυφο σύστημα αναφοράς (datum).</dct:description>
		-->
		<skos:inScheme rdf:resource="http://inspire-registry.jrc.ec.europa.eu/registers/Themes/items"/>
	</inspire:Theme>
	<inspire:Theme rdf:about="http://inspire-registry.jrc.ec.europa.eu/registers/FCD/items/30">
		<!-- <owl:sameIndividualAs rdf:resource="http://www.eionet.europa.eu/gemet/theme_concepts?th=30&ns=5" /> -->
		<inspire:itemStatus>valid</inspire:itemStatus>
		<inspire:dateAccepted>2008-12-05T17:00:30.910+01:00</inspire:dateAccepted>
		<skos:prefLabel xml:lang="en">Bio-geographical regions</skos:prefLabel>
		<skos:definition xml:lang="en">Areas of relatively homogeneous ecological conditions with common characteristics.</skos:definition>
		<dct:description xml:lang="en">Data component description:
Bio-geographical regions show the extent of areas with common characteristics, usually based on climatic, topographic and geobotanical information. Thus the bio-geographical regions show areas with relatively homogeneous ecological conditions. Included in this theme is vegetation map data. The determination of structure and composition of the vegetation is based essentially on stands of ecosystems and their correlation with particular site conditions, commonly based on plant-sociological classification. Vegetation can be mapped either as actual/existing or potential vegetation cover. The classification of potential vegetation depicts the potential distribution of the main natural plant communities. The mapping is based essentially on remaining stands of natural or near-natural ecosystems corresponding to the actual climatic and edaphic conditions. Several high-level data exists for Pan-European level, large-scale data with fragmented systems, resolution and coverage.
Once produced, the bio-geographical data and potential vegetation map data potential vegetation maps are relatively stable and regarded as reference data/maps. Mapping of existing vegetation at local level needs to be updated to depict changes in vegetation.
• Nomenclature: The high-level and pan-European data follow agreed nomenclatures. Concerning local and regional data, there exist a broad variety of nomenclatures, e.g. in vegetation mapping.
• Span in accuracy: Bio-geographical regional data commonly small-scale data, e.g. in 1: 1 mill or smaller. Vegetation data are commonly more detailed, at local level medium precision data, 1: 50.000 or better. Common scales used are 1:25.000 and 1: 10.000.
• Clarification about definition, boundary to other INSPIRE themes: Boundary between land cover and bio-geographical regions.</dct:description>
		<skos:prefLabel xml:lang="bg">Биогеографски региони</skos:prefLabel>
		<skos:definition xml:lang="bg">Райони с относително еднородни екологични условия с общи характеристики.</skos:definition>
		<skos:prefLabel xml:lang="cs">Bioregiony</skos:prefLabel>
		<skos:definition xml:lang="cs">Oblasti s poměrně stejnorodými ekologickými podmínkami a společnými vlastnostmi.</skos:definition>
		<skos:prefLabel xml:lang="da">Biogeografiske regioner</skos:prefLabel>
		<skos:definition xml:lang="da">Områder, der har relativt ensartede økologiske forhold med fælles egenskaber.</skos:definition>
		<skos:prefLabel xml:lang="de">Biogeografische Regionen</skos:prefLabel>
		<skos:definition xml:lang="de">Gebiete mit relativ homogenen ökologischen Bedingungen und gemeinsamen Merkmalen.</skos:definition>
		<skos:prefLabel xml:lang="el">Βιογεωγραφικές περιοχές</skos:prefLabel>
		<skos:definition xml:lang="el">Περιοχές σχετικώς ομοιογενών οικολογικών συνθηκών με κοινά χαρακτηριστικά.</skos:definition>
		<skos:prefLabel xml:lang="es">Regiones biogeográficas</skos:prefLabel>
		<skos:definition xml:lang="es">Zonas dotadas de condiciones ecológicas relativamente homogéneas con unas características comunes.</skos:definition>
		<skos:prefLabel xml:lang="et">Bio-geograafilised piirkonnad</skos:prefLabel>
		<skos:definition xml:lang="et">Suhteliselt ühetaoliste ökoloogiliste tingimustega ja ühiste tunnustega piirkonnad.</skos:definition>
		<skos:prefLabel xml:lang="fi">Biomaantieteelliset alueet</skos:prefLabel>
		<skos:definition xml:lang="fi">Alueet, joilla on suhteellisen yhtenäiset ekologiset olosuhteet ja yhteisiä ominaispiirteitä.</skos:definition>
		<skos:prefLabel xml:lang="fr">Régions biogéographiques</skos:prefLabel>
		<skos:definition xml:lang="fr">Zones présentant des conditions écologiques relativement homogènes avec des caractéristiques communes.</skos:definition>
		<skos:prefLabel xml:lang="hu">Biogeográfiai régiók</skos:prefLabel>
		<skos:definition xml:lang="hu">Közös tulajdonságokkal bíró, viszonylag homogén ökológiai jellemzőkkel rendelkező térségek.</skos:definition>
		<skos:prefLabel xml:lang="it">Regioni biogeografiche</skos:prefLabel>
		<skos:definition xml:lang="it">Aree che presentano condizioni ecologiche relativamente omogenee con caratteristiche comuni.</skos:definition>
		<skos:prefLabel xml:lang="lt">Biogeografiniai regionai</skos:prefLabel>
		<skos:definition xml:lang="lt">Teritorijos, kurioms būdingos palyginti homogeniškos ekologinės sąlygos ir panašios charakteristikos.</skos:definition>
		<skos:prefLabel xml:lang="lv">Bioģeogrāfiskie reģioni</skos:prefLabel>
		<skos:definition xml:lang="lv">Apgabali ar relatīvi viendabīgiem ekoloģiskiem apstākļiem un noteiktām kopīgam iezīmēm.</skos:definition>
		
		<skos:prefLabel xml:lang="mt">Reġjuni bijo-ġeografiċi</skos:prefLabel>
		<skos:definition xml:lang="mt">Żoni ta' kondizzjonijiet ekoloġiċi relattivament omoġenji b'karatteristiċi komuni.</skos:definition>		
		
		<skos:prefLabel xml:lang="nl">Biogeografische gebieden</skos:prefLabel>
		<skos:definition xml:lang="nl">Gebieden met betrekkelijk homogene ecologische omstandigheden die gemeenschappelijke kenmerken vertonen.</skos:definition>
		<skos:prefLabel xml:lang="pl">Regiony biogeograficzne</skos:prefLabel>
		<skos:definition xml:lang="pl">Obszary o stosunkowo jednorodnych warunkach ekologicznych i o wspólnych cechach.</skos:definition>
		<skos:prefLabel xml:lang="pt">Regiões biogeográficas</skos:prefLabel>
		<skos:definition xml:lang="pt">Zonas de condições ecológicas relativamente homogéneas com características comuns.</skos:definition>
		<skos:prefLabel xml:lang="ro">Regiuni biogeografice</skos:prefLabel>
		<skos:definition xml:lang="ro">Zone care prezintă condiţii ecologice relativ omogene, având caracteristici comune.</skos:definition>
		<skos:prefLabel xml:lang="sk">Biogeografické regióny</skos:prefLabel>
		<skos:definition xml:lang="sk">Oblasti s pomerne rovnorodými ekologickými vlastnosťami so spoločnými vlastnosťami.</skos:definition>
		<skos:prefLabel xml:lang="sl">Biogeografske regije</skos:prefLabel>
		<skos:definition xml:lang="sl">Območja z relativno homogenimi ekološkimi razmerami s skupnimi značilnostmi.</skos:definition>
		<skos:prefLabel xml:lang="sv">Biogeografiska regioner</skos:prefLabel>
		<skos:definition xml:lang="sv">Områden som har relativt homogena ekologiska förhållanden med likartade egenskaper.</skos:definition>
		<!--
		<skos:prefLabel xml:lang="el">SAMPLE ALTERNATIVE EXPRESSION - αναφορά</skos:prefLabel>
		<skos:definition xml:lang="el">Συστήματα συντεταγμένων</skos:definition>
		<dct:description xml:lang="el">Συστήματα για μονοσήμαντη αναφορά χωρικών πληροφοριών στον χώρο, ως σύνολο συντεταγμένων (x,y,z) ή/και γεωγραφικό πλάτος και μήκος και ύψος, με βάση γεωδαιτικό οριζόντιο και κατακόρυφο σύστημα αναφοράς (datum).</dct:description>
		-->
		<skos:inScheme rdf:resource="http://inspire-registry.jrc.ec.europa.eu/registers/Themes/items"/>
	</inspire:Theme>
	<inspire:Theme rdf:about="http://inspire-registry.jrc.ec.europa.eu/registers/FCD/items/31">
		<!-- <owl:sameIndividualAs rdf:resource="http://www.eionet.europa.eu/gemet/theme_concepts?th=31&ns=5" /> -->
		<inspire:itemStatus>valid</inspire:itemStatus>
		<inspire:dateAccepted>2008-12-05T17:00:30.966+01:00</inspire:dateAccepted>
		<skos:prefLabel xml:lang="en">Habitats and biotopes</skos:prefLabel>
		<skos:definition xml:lang="en">Geographical areas characterised by specific ecological conditions, processes, structure, and (life support) functions that physically support the organisms that live there. Includes terrestrial and aquatic areas distinguished by geographical, abiotic and biotic features, whether entirely natural or semi-natural.</skos:definition>
		<dct:description xml:lang="en">The "Habitats and biotopes" category of spatial data defined in the INSPIRE Directive is one of several themes in a wider grouping of biological organisms and biological communities - biodiversity. Includes habitats and biotopes as areas and their boundaries. Common to all spatial data that falls under this category is characterisation of the distribution of geographical areas being functional areas for living organisms, biotopes being the spatial and biotic environment of a biotic community/biocoenosis, while habitats being the spatial environment of specific species.
Both climatic, geological, chemical and biological conditions affect distribution of species and communities, thus distribution and conditions of habitats and biotopes. Some species have strict specific requirements to the environment, while others are accepting broad ranges in environmental conditions. Thus biotopes and habitats may vary broadly between different organisms. Some species changes biotopes throughout the year, by changes in seasons or due to migration. Some biotopes/habitats are depending on management, e.g. all kinds of cultural landscapes. Time series in mapping may be used to identify changes in biotopes/habitats.
Description of living areas for any kind of biota, usually used as a term for describing areas used by zoo-biota. Habitats commonly follow geobotanical/ bio-geographical regions/ vegetation types. In rough terms land cover classes and vegetation classes represent terrestrial habitats. Habitats can also be described at more detailed levels e.g. hedgerows, creeks etc. At sea differences in temperature, salinity, current, depth, topography, seabed geology or sediment conditions may form different habitats. Habitats and biotopes data can be made both by mapping in the field, remote sensing and aerial photography interpretation or modelling.
Different documents and communities follow different definitions for habitats and biotopes. An example is the Council Directive 92/43/EEC on the Conservation of natural habitats and of wild fauna and flora. EUNIS has been developed as an international nomenclature for habitats. Different countries or communities have different classification systems. There may be difficulties in mapping accurately certain habitat classes between national nomenclatures and also between national and European nomenclatures. To find common European definitions and nomenclatures need to take into account both national systems and the different definitions used by international communities.
Habitats and biotopes does only include areas represented by natural boundaries and classified according to their ecological or physical condition. Habitats and biotopes being designated as protected sites is not included, they fall under another category of INSPIRE themes, namely "Protected sites", as these represent administrative area regulation and not ecologically founded boundaries.
The terms natural or semi-natural needs clarification, artificial landscapes being habitats (cultural landscapes like town areas, cultivated land, orchards, pastures etc) may be defined to be out of the scope of the theme.</dct:description>
		<skos:prefLabel xml:lang="bg">Местообитания и биотопи</skos:prefLabel>
		<skos:definition xml:lang="bg">Географски райони, характеризиращи се със специфични екологични условия, процеси, структура и (животоподпо- магащи) функции, подпомагащи физически организмите, които ги обитават. Включват земни или водни райони, отличаващи се с напълно естествени или полуестествени географски, абиотични и биотични характеристики.</skos:definition>
		<skos:prefLabel xml:lang="cs">Stanoviště a biotopy</skos:prefLabel>
		<skos:definition xml:lang="cs">Zeměpisné oblasti vyznačující se zvláštními ekologickými podmínkami, procesy, strukturami a (životně důležitými) funkcemi, které skýtají fyzickou podporu organismům, které v nich žijí. Zahrnují pozemské a vodní oblasti rozlišené podle zeměpisných, abiotických a biotických prvků, přirozené i částečně přirozené povahy.</skos:definition>
		<skos:prefLabel xml:lang="da">Levesteder og biotoper</skos:prefLabel>
		<skos:definition xml:lang="da">Geografiske områder, der er kendetegnet ved særlige økologiske forhold, processer, strukturer og (livsunderstøttende) funktioner, og som er det fysiske grundlag for de organismer, der lever der. Omfatter land- og vandområder, som er kendetegnet ved særlige geografiske, abiotiske eller biotiske forhold, uanset om de er helt eller delvis naturlige.</skos:definition>
		<skos:prefLabel xml:lang="de">Lebensräume und Biotope</skos:prefLabel>
		<skos:definition xml:lang="de">Geografische Gebiete mit spezifischen ökologischen Bedingungen, Prozessen, Strukturen und (lebensunterstützenden) Funktionen als physische Grundlage für dort lebende Organismen. Dies umfasst auch durch geografische, abiotische und biotische Merkmale gekennzeichnete natürliche oder naturnahe terrestrische und aquatische Gebiete.</skos:definition>
		<skos:prefLabel xml:lang="el">Ενδιαιτήματα και βιότοποι</skos:prefLabel>
		<skos:definition xml:lang="el">Γεωγραφικές περιοχές που χαρακτηρίζονται από ειδικές οικολογικές συνθήκες, διαδικασίες, δομή και λειτουργίες (υποστήριξης της ζωής) οι οποίες στηρίζουν φυσικά τους οργανισμούς που ενδιαιτούν. Περιλαμβάνονται χερσαίες και υδάτινες εκτάσεις, διακρινόμενες ανάλογα με τα γεωγραφικά, αβιοτικά και βιοτικά χαρακτηριστικά τους, ανεξαρτήτως εάν είναι πλήρως φυσικές ή ημιφυσικές.</skos:definition>
		<skos:prefLabel xml:lang="es">Hábitats y biotopos</skos:prefLabel>
		<skos:definition xml:lang="es">Zonas geográficas caracterizadas por unas condiciones ecológicas específicas, procesos, estructuras y funciones de apoyo vital que sean soporte físico de los organismos que viven en ellas. Se incluirán zonas terrestres y acuáticas diferenciadas por sus características geográficas, abióticas y bióticas, tanto si son enteramente naturales como seminaturales.</skos:definition>
		<skos:prefLabel xml:lang="et">Elupaigad ja biotoobid</skos:prefLabel>
		<skos:definition xml:lang="et">Geograafilised alad, mida iseloomustavad spetsiifilised ökoloogilised tingimused, protsessid, struktuurid ja (elu alalhoiu-) funktsioonid, mis füüsiliselt toetavad seal elavaid organisme. Hõlmab maa- ja veealasid, mida eristatakse geograafiliste, abiootiliste ja biootiliste tunnuste järgi ja mis on täielikult looduslikud või poollooduslikud.</skos:definition>
		<skos:prefLabel xml:lang="fi">Elinympäristöt ja biotoopit</skos:prefLabel>
		<skos:definition xml:lang="fi">Maantieteelliset alueet, joille ovat ominaisia erityiset ekologiset olosuhteet, prosessit, rakenne ja (elämää ylläpitävät) toiminnot, jotka tukevat fysikaalisesti alueella eläviä organismeja. Sisältää maa- ja vesialueet, joilla on omat maantieteelliset, abioottiset ja bioottiset ominaisuutensa ja jotka ovat joko luonnontilassa tai osittain luonnontilassa.</skos:definition>
		<skos:prefLabel xml:lang="fr">Habitats et biotopes</skos:prefLabel>
		<skos:definition xml:lang="fr">Zones géographiques ayant des caractéristiques écologiques particulières — conditions, processus, structures et fonctions (de maintien de la vie) — favorables aux organismes qui y vivent. Sont incluses les zones terrestres et aquatiques qui se distinguent par leurs caractéristiques géographiques, abiotiques ou biotiques, qu'elles soient naturelles ou semi-naturelles.</skos:definition>
		<skos:prefLabel xml:lang="hu">Élőhelyek és biotópok</skos:prefLabel>
		<skos:definition xml:lang="hu">Olyan földrajzi területek, amelyeket különleges ökológiai feltételek, folyamatok, struktúra és (az élet fenntartásához kapcsolódó) funkciók jellemeznek, amelyek az ott élő organizmusok számára kedvező fizikai feltételeket teremtenek. Ide tartoznak azok a szárazföldi és vízi térségek, amelyeket – akár teljesen természetesek, akár félig természetesek – földrajzi, abiotikus és biotikus jellemzőik alapján különböztetnek meg.</skos:definition>
		<skos:prefLabel xml:lang="it">Habitat e biotopi</skos:prefLabel>
		<skos:definition xml:lang="it">Aree geografiche caratterizzate da condizioni ecologiche specifiche, processi, strutture e funzioni (di supporto alla vita) che supportano materialmente gli organismi che le abitano. Sono comprese le zone terrestri e acquatiche, interamente naturali o seminaturali, distinte in base agli elementi geografici, abiotici e biotici.</skos:definition>
		<skos:prefLabel xml:lang="lt">Buveinės ir biotopai</skos:prefLabel>
		<skos:definition xml:lang="lt">Geografinės teritorijos, kurioms būdingos specifinės ekologinės sąlygos, procesai, struktūra ir (gyvybės palaikymo) funkcijos, sudarančios gyvenimui tinkamas fizines sąlygas ten gyvenantiems organizmams. Tai apima visiškai natūralias ir pusiau natūralias sausumos ir vandens teritorijas, kurios turi skirtingas geografines, abiotines ir biotines sąlygas.</skos:definition>
		<skos:prefLabel xml:lang="lv">Dzīvotnes un biotopi</skos:prefLabel>
		<skos:definition xml:lang="lv">Ģeogrāfiskie apgabali, kuros ir īpaši ekoloģiskie apstākļi, procesi, struktūra, un (dzīvības atbalsta) funkcijas, kas fiziski atbalsta organismus, kuri tajos dzīvo. Tie ietver pilnīgi un daļēji dabīgas sauszemes vai ūdens platības, ko raksturo ģeogrāfiski, abiotiski un biotiski faktori.</skos:definition>
		
		<skos:prefLabel xml:lang="mt">L-abitati naturali u l-bijotopi</skos:prefLabel>
		<skos:definition xml:lang="mt">Żoni ġeografiċi kkaratterizzati minn kondizzjonijiet ekoloġiċi, proċessi, struttura, u funzjonijiet (sostenn tal-ħajja) speċifiċi li jsostnu fiżikament l-organiżmi li jgħixu fihom. Huma inklużi żoni ta' l-art jew ta' l-ilma li jingħarfu permezz ta' karatteristiċi ġeografiċi, abijotiċi u bijotiċi, sew jekk għal kollox naturali kif ukoll jekk semi-naturali.</skos:definition>		
		
		<skos:prefLabel xml:lang="nl">Habitats en biotopen</skos:prefLabel>
		<skos:definition xml:lang="nl">Geografische gebieden die worden gekenmerkt door specifieke ecologische omstandigheden, processen, structuur en (leven ondersteunende) functies die fysiek de daar levende organismen ondersteunen, met inbegrip van volledig natuurlijke of semi-natuurlijke land- en wateroppervlakken, onderscheiden naar geografische, abiotische en biotische kenmerken.</skos:definition>
		<skos:prefLabel xml:lang="pl">Siedliska i obszary przyrodniczo jednorodne</skos:prefLabel>
		<skos:definition xml:lang="pl">Obszary geograficzne odznaczające się szczególnymi warunkami przyrodniczymi, procesami, strukturą i (podtrzymującymi życie) funkcjami, które fizycznie umożliwiają egzystencję żyjącym na nich organizmom. Obejmują obszary lądowe i wodne wyróżniające się cechami geograficznymi, abiotycznymi i biotycznymi, czy to w całości naturalne czy też półnaturalne.</skos:definition>
		<skos:prefLabel xml:lang="pt">Habitats e biótopos</skos:prefLabel>
		<skos:definition xml:lang="pt">Zonas geográficas caracterizadas por condições ecológicas, processos, estrutura e funções (de apoio às necessidades básicas) específicos que constituem o suporte físico dos organismos que nelas vivem. Inclui zonas terrestres e aquáticas, naturais ou semi-naturais, diferenciadas pelas suas características geográficas, abióticas e bióticas.</skos:definition>
		<skos:prefLabel xml:lang="ro">Habitate şi biotopuri</skos:prefLabel>
		<skos:definition xml:lang="ro">Zone geografice caracterizate prin condiţii ecologice specifice, procese, structură şi funcţii (de menţinere a vieţii pe pământ) care sprijină fizic organismele care trăiesc acolo. Sunt incluse zonele terestre şi acvatice care se disting prin caracteristicile lor geografice, abiotice şi biotice, indiferent că acestea sunt naturale sau seminaturale.</skos:definition>
		<skos:prefLabel xml:lang="sk">Habitaty a biotopy</skos:prefLabel>
		<skos:definition xml:lang="sk">Geografické oblasti, pre ktoré sú charakteristické špecifické ekologické vlastnosti, procesy, štruktúra a (pre život dôležité) funkcie, ktoré fyzikálne podporujú organizmy žijúce na ich území. Patria sem suchozemské a vodné oblasti rozlíšené podľa geografických, abiotických a biotických prvkov, buď výhradne prírodné, alebo poloprírodné.</skos:definition>
		<skos:prefLabel xml:lang="sl">Habitati in biotopi</skos:prefLabel>
		<skos:definition xml:lang="sl">Geografska območja, za katera so značilne posebne ekološke razmere, procesi, struktura in funkcije, ki fizično omogočajo organizmom, da tam živijo. Vključujejo kopenska in vodna območja, ki se razlikujejo po geografskih, abiotskih in biotskih značilnostih, ne glede na to, ali so popolnoma naravna ali polnaravna.</skos:definition>
		<skos:prefLabel xml:lang="sv">Naturtyper och biotoper</skos:prefLabel>
		<skos:definition xml:lang="sv">Geografiska områden som kännetecknas av särskilda ekologiska förhållanden, processer, strukturer och (livsstödjande) funktioner och som är fysiska livsmiljöer för organismer som lever där. Inbegriper land- och vattenområden med särskilda geografiska, abiotiska och biotiska egenskaper, oavsett om de är naturliga eller delvis naturliga.</skos:definition>
		<!--
		<skos:prefLabel xml:lang="el">SAMPLE ALTERNATIVE EXPRESSION - αναφορά</skos:prefLabel>
		<skos:definition xml:lang="el">Συστήματα συντεταγμένων</skos:definition>
		<dct:description xml:lang="el">Συστήματα για μονοσήμαντη αναφορά χωρικών πληροφοριών στον χώρο, ως σύνολο συντεταγμένων (x,y,z) ή/και γεωγραφικό πλάτος και μήκος και ύψος, με βάση γεωδαιτικό οριζόντιο και κατακόρυφο σύστημα αναφοράς (datum).</dct:description>
		-->
		<skos:inScheme rdf:resource="http://inspire-registry.jrc.ec.europa.eu/registers/Themes/items"/>
	</inspire:Theme>
	<inspire:Theme rdf:about="http://inspire-registry.jrc.ec.europa.eu/registers/FCD/items/32">
		<!-- <owl:sameIndividualAs rdf:resource="http://www.eionet.europa.eu/gemet/theme_concepts?th=32&ns=5" /> -->
		<inspire:itemStatus>valid</inspire:itemStatus>
		<inspire:dateAccepted>2008-12-05T17:00:31.028+01:00</inspire:dateAccepted>
		<skos:prefLabel xml:lang="en">Species distribution</skos:prefLabel>
		<skos:definition xml:lang="en">Geographical distribution of occurrence of animal and plant species aggregated by grid, region, administrative unit or other analytical unit.</skos:definition>
		<dct:description xml:lang="en">Pan-European, national or local mapping initiatives, resulting in spatial data for species in terrestrial and marine environments, e.g. for birds, insects, mammals, amphibians, reptiles, fish or vascular plants.
Clarification:
• The definition in INSPIRE Directive proposal does not include individual observations or other point based data, but focuses on aggregated versions of data about geographical distribution of species. Aggregation can be at any level of resolution, e.g. in geographical grid systems divided into 100x100 meter grid or 50x50km grid cells. Possibly also point-based observations and isolines generation between observations should be accepted and included in INSPIRE. Possibly these can be defined as options in the "other analytical unit". Aggregation may also be interpreted not only as space-based aggregation, but time-based aggregation as well.
• Only species are mentioned in the INSPIRE definition. But earlier INSPIRE documents (INPIRE IMS, 2003) mentions both species or species grouped e.g. to families.</dct:description>
		<skos:prefLabel xml:lang="bg">Разпределение на видовете</skos:prefLabel>
		<skos:definition xml:lang="bg">Географско разпределение на животинските и растителните видове, представено обобщено по координати, регион, административна единица или друга аналитична единица.</skos:definition>
		<skos:prefLabel xml:lang="cs">Rozložení druhů</skos:prefLabel>
		<skos:definition xml:lang="cs">Zeměpisné rozložení výskytu živočišných a rostlinných druhů seskupených podle souřadnicové sítě, regionu, správní jednotky nebo jiné analytické jednotky.</skos:definition>
		<skos:prefLabel xml:lang="da">Artsfordeling</skos:prefLabel>
		<skos:definition xml:lang="da">Den geografiske fordeling af forekomsten af dyre- og plantearter i kvadratnetceller, forvaltningsenheder eller andre analytiske enheder.</skos:definition>
		<skos:prefLabel xml:lang="de">Verteilung der Arten</skos:prefLabel>
		<skos:definition xml:lang="de">Geografische Verteilung des Auftretens von Tier- und Pflanzenarten, zusammengefasst in Gittern, Region, Verwaltungseinheit oder sonstigen analytischen Einheiten.</skos:definition>
		<skos:prefLabel xml:lang="el">Κατανομή ειδών</skos:prefLabel>
		<skos:definition xml:lang="el">Γεωγραφική κατανομή ειδών πανίδας και χλωρίδας, ανά κάνναβο, περιοχή, διοικητική ενότητα ή άλλη ενότητα ανάλυσης.</skos:definition>
		<skos:prefLabel xml:lang="es">Distribución de las especies</skos:prefLabel>
		<skos:definition xml:lang="es">Distribución geográfica de las especies animales y vegetales referidas a una cuadrícula, región, unidad administrativa u otro tipo de unidad analítica.</skos:definition>
		<skos:prefLabel xml:lang="et">Liikide jaotumine</skos:prefLabel>
		<skos:definition xml:lang="et">Taime- ja loomaliikide geograafiline levik ruutvõrgu, piirkondade, haldusüksuste või muude jaotusüksuste kaupa.</skos:definition>
		<skos:prefLabel xml:lang="fi">Lajien levinneisyys</skos:prefLabel>
		<skos:definition xml:lang="fi">Eläin- ja kasvilajien esiintymien maantieteellinen levinneisyys ruudukoittain, alueittain, hallintoyksiköittäin tai muiden analyyttisten yksiköitten mukaisesti jaoteltuna.</skos:definition>
		<skos:prefLabel xml:lang="fr">Répartition des espèces</skos:prefLabel>
		<skos:definition xml:lang="fr">Répartition géographique de l'occurrence des espèces animales et végétales regroupées par grille, région, unité administrative ou autre unité analytique.</skos:definition>
		<skos:prefLabel xml:lang="hu">A fajok megoszlása</skos:prefLabel>
		<skos:definition xml:lang="hu">Az állat- és növényfajok előfordulásának földrajzi eloszlása, térképrács, régió, közigazgatási egység vagy más elemzési egység alapján összesítve.</skos:definition>
		<skos:prefLabel xml:lang="it">Distribuzione delle specie</skos:prefLabel>
		<skos:definition xml:lang="it">Distribuzione geografica delle specie animali e vegetali aggregate per griglia, regione, unità amministrativa o altra unità analitica.</skos:definition>
		<skos:prefLabel xml:lang="lt">Rūšių pasiskirstymas</skos:prefLabel>
		<skos:definition xml:lang="lt">Geografinis gyvūnų ir augalų rūšių pasiskirstymas pagal tinklelį, regioną, administracinį ar kitą analitinį vienetą.</skos:definition>
		<skos:prefLabel xml:lang="lv">Sugu izplatība</skos:prefLabel>
		<skos:definition xml:lang="lv">Dzīvnieku un augu sugu ģeogrāfiskais sadalījums, grupējot pēc koordinātu tīkla, reģiona, administratīvām vai citām analītiskām vienībām.</skos:definition>
		
		<skos:prefLabel xml:lang="mt">Distribuzzjoni ta' l-ispeċi</skos:prefLabel>
		<skos:definition xml:lang="mt">Distribuzzjoni ġeografika ta' l-okkorrenza ta' speċi ta' annimali u ta' pjanti miġbura flimkien skond il-grilja, ir-reġjun, l-unità amministrattiva jew unità analitika oħra.</skos:definition>		
		
		<skos:prefLabel xml:lang="nl">Spreiding van soorten</skos:prefLabel>
		<skos:definition xml:lang="nl">Geografische spreiding van dier- en plantensoorten per raster, regio, administratieve eenheid of andere analytische eenheid.</skos:definition>
		<skos:prefLabel xml:lang="pl">Rozmieszczenie gatunków</skos:prefLabel>
		<skos:definition xml:lang="pl">Geograficzne rozmieszczenie występowania gatunków zwierząt i roślin pogrupowanych według siatki geograficznej, regionu, jednostki administracyjnej lub innej jednostki analitycznej.</skos:definition>
		<skos:prefLabel xml:lang="pt">Distribuição das espécies</skos:prefLabel>
		<skos:definition xml:lang="pt">Distribuição geográfica da ocorrência de espécies animais e vegetais agregadas por quadrícula, região, unidade administrativa ou outra unidade analítica.</skos:definition>
		<skos:prefLabel xml:lang="ro">Repartizarea speciilor</skos:prefLabel>
		<skos:definition xml:lang="ro">Repartizarea geografică a speciilor de animale şi plante, regrupate pe grilă, regiune, unitate administrativă sau altă unitate analitică.</skos:definition>
		<skos:prefLabel xml:lang="sk">Výskyt druhov</skos:prefLabel>
		<skos:definition xml:lang="sk">Geografické rozdelenie výskytu živočíšnych a rastlinných druhov zoskupený podľa siete, regiónu, administratívnej jednotky alebo inej analytickej jednotky.</skos:definition>
		<skos:prefLabel xml:lang="sl">Porazdelitev vrst</skos:prefLabel>
		<skos:definition xml:lang="sl">Geografska porazdelitev pojavljanja živalskih in rastlinskih vrst, razvrščenih po koordinatah, regiji, upravni enoti ali drugi analitični enoti.</skos:definition>
		<skos:prefLabel xml:lang="sv">Arters utbredning</skos:prefLabel>
		<skos:definition xml:lang="sv">Geografisk fördelning av djur- och växtarters förekomst i rutnät, regioner, administrativa enheter eller andra analytiska enheter.</skos:definition>
		<!--
		<skos:prefLabel xml:lang="el">SAMPLE ALTERNATIVE EXPRESSION - αναφορά</skos:prefLabel>
		<skos:definition xml:lang="el">Συστήματα συντεταγμένων</skos:definition>
		<dct:description xml:lang="el">Συστήματα για μονοσήμαντη αναφορά χωρικών πληροφοριών στον χώρο, ως σύνολο συντεταγμένων (x,y,z) ή/και γεωγραφικό πλάτος και μήκος και ύψος, με βάση γεωδαιτικό οριζόντιο και κατακόρυφο σύστημα αναφοράς (datum).</dct:description>
		-->
		<skos:inScheme rdf:resource="http://inspire-registry.jrc.ec.europa.eu/registers/Themes/items"/>
	</inspire:Theme>
	<inspire:Theme rdf:about="http://inspire-registry.jrc.ec.europa.eu/registers/FCD/items/33">
		<!-- <owl:sameIndividualAs rdf:resource="http://www.eionet.europa.eu/gemet/theme_concepts?th=33&ns=5" /> -->
		<inspire:itemStatus>valid</inspire:itemStatus>
		<inspire:dateAccepted>2008-12-05T17:00:31.088+01:00</inspire:dateAccepted>
		<skos:prefLabel xml:lang="en">Energy resources</skos:prefLabel>
		<skos:definition xml:lang="en">Energy resources including hydrocarbons, hydropower, bio-energy, solar, wind, etc., where relevant including depth/height information on the extent of the resource.</skos:definition>
		<dct:description xml:lang="en">Pan-European, national or local initiatives on mapping occur, resulting from governmental initiatives or private interests. There is a main distinction between fossil fuels and renewable energy resources. The concept of energy resources provides focus to the resource aspect and the extent/distribution of the resources. Thus, the technical constructions for abstraction, transport and treatment are not covered by this theme. However they are to a large extent covered in other themes, such as production and industrial facilities. Energy use, e.g. petrol consumption, is not covered by this theme. Licence areas, permission areas or planning areas linked to energy resource exploitation is covered by the theme "Area management/restriction/regulation zones and reporting areas".
The term resource can be problematic to define, the quantification and thus location of a resource is depending on the technical and economic situation. Resource aspects should not only be restricted to the resources under utilisation, but should also include un-utilised resources.
Fossil fuel resources include
• Oil accumulation: hydrocarbot fields, petroleum volumes
• Natural gas accumulations, including solid methane clathrates
• Coal, lignite or peat deposits
• Uranium ore deposits
For these resources the nature, location and 3D geometry of the deposit (= geological resource) of the deposit, the nature of the economic energy carrier and the size of the reserves at a point in time are key attributes.
The different kinds of renewable energy resources may include:
• Hydropower: Water resources especially mapped according to energy potential. Commonly undertaken in the MS, carried out by governmental bodies or private firms.
• Bio-energy resources: Forest resources, “scrap” forest, cereals or agricultural residues can be used for energy purposes, e.g. in the form of firewood or biodiesel. The resources or supply is sometimes being estimated and mapped.
• Wind energy: Country inventories of wind energy is being done in areas where wind is being utilised or planned utilised. Estimated by wind measurement together with topographical information. Example: http://www.nve.no/vindatlas/
• Geothermal energy: The Earth's natural heat flow is of high interest as a renewable and clean energy source. Mapping of the resource can be available or relevant at local, regional or national levels. A Pan-European Atlas was published in 2002 by the EC (see reference materials). Geothermal energy systems use the natural heat of the subsoil by utilising warm groundwater from surficial deposits for direct heating or electricity generation (open system). Alternatively, shallow geothermal flows are exploited by ground source heat pumps (closed system). Common heat sources in bedrock or subsoil may be utilized - a circulation of an antifreeze solution in collector hoses which are lowered into relatively shallow boreholes bedrock or circulation of ground water from deep boreholes in bedrock. Heat pumps are suitable, too, for example for extraction of heat from air, rivers, seas and artificial components.
• Solar power and resources: In order to reduce the need for extra heating solar conditions at local sites are important to bring into account in local planning. National, regional and local inventories on solar energy conditions is needed, relating to heating needs. Systems for storing solar heat is found at some locations. Solar resources may also be used in electricity production, through the use of solar cell technology (silicium cells). Air-based heat pumps can use solar energy stored in the air.
• Other energy resources such as waves, currents etc.: The different kinds of renewable energy resources is long. The list above is only giving some examples.
The quantification of the resources may be aggregated or detailed. The detailed information is to a large extent private business information. This includes for instance data about the internal structure of geological structures within oil fields. Within the INSPIRE context the data in question will mainly be aggregation and overview data. However, for public planning purposes at the local level detailed information about some of the renewable energy resources may be relevant.
The geographical representation of the resources (objects) may be different in different scales. In the mapping and exploitation of the resources 2-d (ordinary maps) and 3-d geographical data are being used. Resources may be mapped by natural boundaries. Aggregated or overview information can be referring to grid cells in a geographical grid system, administrative units/areas, statistical units/areas or points.</dct:description>
		<skos:prefLabel xml:lang="bg">Енергийни източници</skos:prefLabel>
		<skos:definition xml:lang="bg">Енергийни източници, включително въглеводород, водна енергия, биоенергия, слънчева енергия, енергия от вятър и други; по целесъобразност се включва информация за дълбочина/височина на района на източника.</skos:definition>
		<skos:prefLabel xml:lang="cs">Energetické zdroje</skos:prefLabel>
		<skos:definition xml:lang="cs">Energetické zdroje, včetně uhlovodíků, vodní energie, bioenergie, sluneční a větrné energie atd., případně včetně informací o hloubce nebo výšce týkajících se rozsahu zdroje.</skos:definition>
		<skos:prefLabel xml:lang="da">Energiressourcer</skos:prefLabel>
		<skos:definition xml:lang="da">Energiressourcer, herunder kulbrinter, vandkraft, bioenergi, sol, vind osv. samt, hvis det er relevant, dybde-/ højdeoplysninger om ressourcens omfang.</skos:definition>
		<skos:prefLabel xml:lang="de">Energiequellen</skos:prefLabel>
		<skos:definition xml:lang="de">Energiequellen wie Kohlenwasserstoffe, Wasserkraft, Bioenergie, Sonnen- und Windenergie usw., gegebenenfalls mit Tiefen- bzw. Höhenangaben zur Ausdehnung der Energiequelle.</skos:definition>
		<skos:prefLabel xml:lang="el">Ενεργειακοί πόροι</skos:prefLabel>
		<skos:definition xml:lang="el">Ενεργειακοί πόροι, μεταξύ άλλων υδρογονάνθρακες, υδροηλεκτρική ενέργεια, βιοενέργεια, ηλιακή ενέργεια, αιολική ενέργεια, κ.λπ., συμπεριλαμβανομένων, κατά περίπτωση, πληροφοριών περί του βάθους και του ύψους όσον αφορά την έκταση του εκάστοτε πόρου.</skos:definition>
		<skos:prefLabel xml:lang="es">Recursos energéticos</skos:prefLabel>
		<skos:definition xml:lang="es">Recursos energéticos: hidrocarburos, energía hidroeléctrica, bioenergía, energía solar y eólica, etc., incluyendo, cuando proceda, la información de profundidad y altura del volumen de los recursos.</skos:definition>
		<skos:prefLabel xml:lang="et">Energiaressursid</skos:prefLabel>
		<skos:definition xml:lang="et">Energiaressursid, sealhulgas süsivesinikud, hüdroenergia, bioenergia, päikese-, tuule- jne energia, sealhulgas koos asjakohase sügavust/kõrgust puudutava teabega ressursi mahu kohta.</skos:definition>
		<skos:prefLabel xml:lang="fi">Energiavarat</skos:prefLabel>
		<skos:definition xml:lang="fi">Energiavarat, mukaan lukien hiilivedyt, vesivoima, bioenergia, aurinko, tuuli jne., mukaan luettuina tarvittaessa syvyys-/korkeustiedot kyseisen luonnonvaran laajuudesta.</skos:definition>
		<skos:prefLabel xml:lang="fr">Sources d'énergie</skos:prefLabel>
		<skos:definition xml:lang="fr">Sources d'énergie comprenant les hydrocarbures, l'énergie hydraulique, la bioénergie, l'énergie solaire, l'énergie éolienne, etc., le cas échéant accompagnées d'informations relatives à la profondeur/la hauteur de la source.</skos:definition>
		<skos:prefLabel xml:lang="hu">Energiaforrások</skos:prefLabel>
		<skos:definition xml:lang="hu">Energiaforrások, beleértve a szénhidrogéneket, vízenergiát, bioenergiát, nap- és szélenergiát stb., adott esetben beleértve az erőforrás mértékére vonatkozó mélységi/magassági információt.</skos:definition>
		<skos:prefLabel xml:lang="it">Risorse energetiche</skos:prefLabel>
		<skos:definition xml:lang="it">Risorse energetiche, compresi gli idrocarburi, l'energia idroelettrica, la bioenergia, l'energia solare, eolica, ecc., ove opportuno anche informazioni, in termini di altezza/profondità, sull'entità della risorsa.</skos:definition>
		<skos:prefLabel xml:lang="lt">Energijos ištekliai</skos:prefLabel>
		<skos:definition xml:lang="lt">Energijos ištekliai, įskaitant angliavandenilius, hidroenergiją, bioenergiją, saulės ir vėjo energiją ir t. t., tam tikrais atvejais įskaitant informaciją apie išteklių apimties gylį/aukštį.</skos:definition>
		<skos:prefLabel xml:lang="lv">Enerģijas resursi</skos:prefLabel>
		<skos:definition xml:lang="lv">Enerģijas resursi, tostarp ogļūdeņraži, ūdens enerģija, bioenerģija, saules enerģija, vēja enerģija, utt., attiecīgā gadījumā ietverot informāciju par dziļumu/augstumu attiecībā uz resursu apmēru.</skos:definition>
		
		<skos:prefLabel xml:lang="mt">Riżorsi ta' enerġija</skos:prefLabel>
		<skos:definition xml:lang="mt">Riżorsi ta' enerġija inklużi idrokarboni, enerġija idro-elettrika, bijo-enerġija, bix-xemx, bir-riħ, eċċ., fejn ikun rilevanti, inkluża informazzjoni dwar il-fond/l-għoli rigward id-daqs tar-riżors.</skos:definition>		
		
		<skos:prefLabel xml:lang="nl">Energiebronnen</skos:prefLabel>
		<skos:definition xml:lang="nl">Energiebronnen met inbegrip van koolwaterstof, waterkracht, bio-energie, zon, wind enz., waar passend met inbegrip van diepte/hoogte-informatie over de omvang van de bron.</skos:definition>
		<skos:prefLabel xml:lang="pl">Zasoby energetyczne</skos:prefLabel>
		<skos:definition xml:lang="pl">Zasoby energii, w tym węglowodory, energia wodna, bioenergia, energia słoneczna, wiatrowa itd., w odpowiednich przypadkach łącznie z informacjami dotyczącymi głębokości/wysokości i rozmiarów danych zasobów.</skos:definition>
		<skos:prefLabel xml:lang="pt">Recursos energéticos</skos:prefLabel>
		<skos:definition xml:lang="pt">Recursos energéticos, incluindo os de hidrocarbonetos, hidroeléctricos, de bio-energias, de energia solar, eólica, etc., incluindo, quando pertinente, informação sobre as cotas de profundidade/altura do recurso.</skos:definition>
		<skos:prefLabel xml:lang="ro">Resurse energetice</skos:prefLabel>
		<skos:definition xml:lang="ro">Resurse energetice precum hidrocarburi, energia hidraulică, bioenergia, energia solară, energia eoliană etc., însoţite de informaţii privind adâncimea/înălţimea la care se află resursa, după caz.</skos:definition>
		<skos:prefLabel xml:lang="sk">Zdroje energie</skos:prefLabel>
		<skos:definition xml:lang="sk">Zdroje energie vrátane uhľovodíkov, vodnej energie, energie z biomasy, solárnej energie, veternej energie atď., ak je to možné vrátane informácie o šírke a dĺžke rozlohy zdroja.</skos:definition>
		<skos:prefLabel xml:lang="sl">Energetski viri</skos:prefLabel>
		<skos:definition xml:lang="sl">Energetski viri, vključno z ogljikovodiki, vodno energijo, bioenergijo, soncem, vetrom itd., kjer je to ustrezno vključno s podatki o globini/višini glede velikosti vira.</skos:definition>
		<skos:prefLabel xml:lang="sv">Energiresurser</skos:prefLabel>
		<skos:definition xml:lang="sv">Energiresurser, inbegripet kolväten, vattenkraft, bioenergi, sol, vind osv., i tillämpliga fall med djup-/höjdinformation om resursens omfattning.</skos:definition>
		<!--
		<skos:prefLabel xml:lang="el">SAMPLE ALTERNATIVE EXPRESSION - αναφορά</skos:prefLabel>
		<skos:definition xml:lang="el">Συστήματα συντεταγμένων</skos:definition>
		<dct:description xml:lang="el">Συστήματα για μονοσήμαντη αναφορά χωρικών πληροφοριών στον χώρο, ως σύνολο συντεταγμένων (x,y,z) ή/και γεωγραφικό πλάτος και μήκος και ύψος, με βάση γεωδαιτικό οριζόντιο και κατακόρυφο σύστημα αναφοράς (datum).</dct:description>
		-->
		<skos:inScheme rdf:resource="http://inspire-registry.jrc.ec.europa.eu/registers/Themes/items"/>
	</inspire:Theme>
	<inspire:Theme rdf:about="http://inspire-registry.jrc.ec.europa.eu/registers/FCD/items/34">
		<!-- <owl:sameIndividualAs rdf:resource="http://www.eionet.europa.eu/gemet/theme_concepts?th=34&ns=5" /> -->
		<inspire:itemStatus>valid</inspire:itemStatus>
		<inspire:dateAccepted>2008-12-05T17:00:31.146+01:00</inspire:dateAccepted>
		<skos:prefLabel xml:lang="en">Mineral resources</skos:prefLabel>
		<skos:definition xml:lang="en">Mineral resources including metal ores, industrial minerals, etc., where relevant including depth/height information on the extent of the resource.</skos:definition>
		<dct:description xml:lang="en">The mineral resources data theme refers to the description of natural concentrations of very diverse minerals of potential or proven economic interest. Important attributes are the nature, genesis, location, extent/distribution of these resources. The economic and technical data related to the location of areas licensed for exploration or mining, to the exploitation of deposits, transport, treatment and waste disposal are not covered by this theme. However, storing of material near mines and quarries is necessary. Knowledge how the constituents affect the surroundings is of importance, e.g. leakage from sulphides etc. They are to a large extent covered in other themes, such as production and industrial facilities. Energy minerals such as coal, uranium, oil and gas are excluded in this theme, as they are found in theme "energy resources". Exploration licence areas and areas permitted for mining are covered by the theme "Area management/restriction/regulation zones and reporting areas".
Mineral resources data refers to:
• Anomalies: locations where background concentrations of potentially valuable elements in soils, stream sediments or rocks onshore or offshore exceed the normal background values expected given the local geological context. Such maps are widely used in mineral exploration. Attributes are location, chemical elements, nature of the sampled element (s), analytical value(s);
• Occurrences: points or areas where concentrations of a given mineral (s) are observed but without a proven economic potential. Attributes are location, nature of the mineral(s), analytical data, nature of the host rock, geometry/ morphology of the observed occurrence(s)
• Deposits: areas bearing mineral concentrations with economic potential. Attributes are detailed below
A mineral resource encompasses all quantities of mineral resources, discovered and undiscovered, that are contained in, or have been produced from, naturally occurring accumulations on or within the earth’s crust.
Resource information is generally available for deposits held by companies listed on the Western stock markets, as they face reporting obligations. National legislation also influences the detail of data publicly available. Detailed data or data related to some rare metals deposits with high-technology applications, may be difficult to obtain considered to be of economic/ private interest and therefore, problematic to distribute.
The mineral resources sector is divided in a number of segments, differentiated by the technologies involved in exploration and mining, the markets and the nature of the exploited material(s):
• Metal mining (non-energy metallic ores, uranium pertaining to the energy sector);
• Industrial minerals;
• Construction minerals and rocks; e.g. natural stone (dimension stone), sand and gravel and crushed bedrock aggregates
• Ornamental stones;
• Precious and semi-precious stones.
The description of the three first categories is included in the European Commission (DG Enterprise) document listed among the reference documents (Box 1 provides a comprehensive definition). The definitions included in that document should to be adhered to, in order to promote consistency of the semantics used in EC documents. Ornamental stones are all those rocks that are used for ornamental purposes inside and outside of constructions (marble, granite, labradorite, syenite …). Precious and semi-precious minerals are used for jewelry (an overlap exists with the ornamental stones segment some colourful semi-precious minerals being used for both jewelry and decoration).</dct:description>
		<skos:prefLabel xml:lang="bg">Минерални ресурси</skos:prefLabel>
		<skos:definition xml:lang="bg">Минерални ресурси, включително метални руди, промишлени минерали и други; по целесъобразност се включва информация за дълбочина/височина на находището на ресурса.</skos:definition>
		<skos:prefLabel xml:lang="cs">Nerostné suroviny</skos:prefLabel>
		<skos:definition xml:lang="cs">Nerostné suroviny, včetně kovových rud, průmyslových surovin atd., případně včetně informací o hloubce nebo výšce týkajících se rozsahu zdroje.</skos:definition>
		<skos:prefLabel xml:lang="da">Mineralressourcer</skos:prefLabel>
		<skos:definition xml:lang="da">Mineralressourcer, herunder metalmalme, industrmineraler osv. samt, hvis det er relevant, dybde-/højdeoplysninger om ressourcens omfang.</skos:definition>
		<skos:prefLabel xml:lang="de">Mineralische Bodenschätze</skos:prefLabel>
		<skos:definition xml:lang="de">Mineralische Bodenschätze wie Metallerze, Industrieminerale usw., gegebenenfalls mit Tiefen- bzw. Höhenangaben zur Ausdehnung der Bodenschätze.</skos:definition>
		<skos:prefLabel xml:lang="el">Ορυκτοί πόροι</skos:prefLabel>
		<skos:definition xml:lang="el">Ορυκτοί πόροι, μεταξύ άλλων και μεταλλεύματα, βιομηχανικά μεταλλεύματα, κ.λπ., συμπεριλαμβανομένων, κατά περίπτωση, πληροφοριών περί του βάθους και του ύψους όσον αφορά την έκταση του εκάστοτε πόρου.</skos:definition>
		<skos:prefLabel xml:lang="es">Recursos minerales</skos:prefLabel>
		<skos:definition xml:lang="es">Recursos minerales: minerales metalíferos, minerales industriales, etc., incluyendo, cuando proceda, la información de profundidad y altura del volumen de los recursos.</skos:definition>
		<skos:prefLabel xml:lang="et">Maavarad</skos:prefLabel>
		<skos:definition xml:lang="et">Maavarad, sealhulgas metallimaagid, tööstuslikud mineraalid jne, sealhulgas koos asjakohase sügavust/kõrgust puudutava teabega ressursi mahu kohta.</skos:definition>
		<skos:prefLabel xml:lang="fi">Mineraalivarat</skos:prefLabel>
		<skos:definition xml:lang="fi">Mineraalivarat, mukaan lukien metallimalmit, teollisuusmineraalit jne., mukaan luettuina tarvittaessa syvyys-/ korkeustiedot kyseisen luonnonvaran laajuudesta.</skos:definition>
		<skos:prefLabel xml:lang="fr">Ressources minérales</skos:prefLabel>
		<skos:definition xml:lang="fr">Ressources minérales comprenant les minerais métalliques, les minéraux industriels, etc., le cas échéant accompagnées d'informations relatives à la profondeur/la hauteur de la ressource.</skos:definition>
		<skos:prefLabel xml:lang="hu">Ásványi nyersanyagok</skos:prefLabel>
		<skos:definition xml:lang="hu">Ásványi nyersanyagok, beleértve a fémek érceit, ipari ásványokat stb., adott esetben beleértve a nyersanyag kiterjedésére vonatkozó mélységi/magassági információkat.</skos:definition>
		<skos:prefLabel xml:lang="it">Risorse minerarie</skos:prefLabel>
		<skos:definition xml:lang="it">Risorse minerarie, compresi i minerali metallici, i minerali industriali, ecc., ove opportuno anche informazioni, in termini di altezza/profondità, sull'entità della risorsa.</skos:definition>
		<skos:prefLabel xml:lang="lt"> Naudingosios iškasenos</skos:prefLabel>
		<skos:definition xml:lang="lt">Naudingosios iškasenos, įskaitant metalų rūdas, pramonei naudojamas naudingąsias iškasenas ir t. t., tam tikrais atvejais įskaitant informaciją apie išteklių apimties gylį/aukštį.</skos:definition>
		<skos:prefLabel xml:lang="lv">Derīgo izrakteņu resursi</skos:prefLabel>
		<skos:definition xml:lang="lv">Derīgo izrakteņu resursi, tostarp metālu rūdas, rūpnieciski iegūstamie izrakteņi, utt., attiecīgā gadījumā ietverot informāciju par dziļumu/augstumu attiecībā uz resursu apmēru.</skos:definition>
		
		<skos:prefLabel xml:lang="mt">Riżorsi minerali</skos:prefLabel>
		<skos:definition xml:lang="mt">Riżorsi minerali inklużi minerali tal-metall, minerali industrijali, eċċ, fejn rilevanti inkluża informazzjoni dwar il-- fond/l-għoli rigward id-daqs tar-riżors.</skos:definition>		
		
		<skos:prefLabel xml:lang="nl">Minerale bronnen</skos:prefLabel>
		<skos:definition xml:lang="nl">Minerale bronnen met inbegrip van metaalertsen, industriële mineralen enz., waar passend met inbegrip van diepte/ hoogte-informatie over de omvang van de bron.</skos:definition>
		<skos:prefLabel xml:lang="pl">Zasoby mineralne</skos:prefLabel>
		<skos:definition xml:lang="pl">Zasoby mineralne, w tym rudy metali, minerały przemysłowe itd., w odpowiednich przypadkach łącznie z informacjami dotyczącymi głębokości/wysokości i rozmiarów danych zasobów.</skos:definition>
		<skos:prefLabel xml:lang="pt">Recursos minerais</skos:prefLabel>
		<skos:definition xml:lang="pt">Recursos minerais, incluindo minérios metálicos, minerais industriais, etc., incluindo, quando pertinente, informação sobre as cotas de profundidade/altura do recurso.</skos:definition>
		<skos:prefLabel xml:lang="ro">Resurse minerale</skos:prefLabel>
		<skos:definition xml:lang="ro">Resurse minerale precum minereurile metalifere, minereurile industriale etc., însoţite de informaţii privind adâncimea/ înălţimea la care se află resursa, după caz.</skos:definition>
		<skos:prefLabel xml:lang="sk">Zdroje nerastných surovín</skos:prefLabel>
		<skos:definition xml:lang="sk">Zdroje nerastných surovín vrátane kovových rúd, priemyselných nerastov atď., ak je to možné vrátane informácie o šírke a dĺžke rozlohy zdroja.</skos:definition>
		<skos:prefLabel xml:lang="sl">Mineralni viri</skos:prefLabel>
		<skos:definition xml:lang="sl">Mineralni viri, vključno s kovinskimi rudami, industrijskimi mineralnimi surovinami itd. kjer je ustrezno, vključno s podatki o globini/višini glede velikosti vira.</skos:definition>
		<skos:prefLabel xml:lang="sv">Mineralfyndigheter</skos:prefLabel>
		<skos:definition xml:lang="sv">Mineralfyndigheter, bland annat malm, industrimineraler osv., i tillämpliga fall med djup-/höjdinformation om resursens omfattning.</skos:definition>
		<!--
		<skos:prefLabel xml:lang="el">SAMPLE ALTERNATIVE EXPRESSION - αναφορά</skos:prefLabel>
		<skos:definition xml:lang="el">Συστήματα συντεταγμένων</skos:definition>
		<dct:description xml:lang="el">Συστήματα για μονοσήμαντη αναφορά χωρικών πληροφοριών στον χώρο, ως σύνολο συντεταγμένων (x,y,z) ή/και γεωγραφικό πλάτος και μήκος και ύψος, με βάση γεωδαιτικό οριζόντιο και κατακόρυφο σύστημα αναφοράς (datum).</dct:description>
		-->
		<skos:inScheme rdf:resource="http://inspire-registry.jrc.ec.europa.eu/registers/Themes/items"/>
	</inspire:Theme>
	<inspire:SpatialObjectType rdf:about="http://inspire-registry.jrc.ec.europa.eu/registers/FCD/items/105">
		<inspire:itemStatus>valid</inspire:itemStatus>
		<inspire:dateAccepted>2008-12-05T17:02:10.597+01:00</inspire:dateAccepted>
		<skos:prefLabel xml:lang="en">Watercourse</skos:prefLabel>
		<skos:definition xml:lang="en">A natural or man-made flowing watercourse or stream.</skos:definition>
		<skos:prefLabel xml:lang="el">SAMPLE ALTERNATIVE EXPRESSION - αναφορά</skos:prefLabel>
		<skos:definition xml:lang="el">Συστήματα συντεταγμένων</skos:definition>
		<dct:description xml:lang="el">Συστήματα για μονοσήμαντη αναφορά χωρικών πληροφοριών στον χώρο, ως σύνολο συντεταγμένων (x,y,z) ή/και γεωγραφικό πλάτος και μήκος και ύψος, με βάση γεωδαιτικό οριζόντιο και κατακόρυφο σύστημα αναφοράς (datum).</dct:description>
		<skos:inScheme rdf:resource="http://inspire-registry.jrc.ec.europa.eu/registers/FCD/items"/>
	</inspire:SpatialObjectType>
	<inspire:SpatialObjectType rdf:about="http://inspire-registry.jrc.ec.europa.eu/registers/FCD/items/129">
		<inspire:itemStatus>valid</inspire:itemStatus>
		<inspire:dateAccepted>2008-12-05T17:02:12.709+01:00</inspire:dateAccepted>
		<skos:prefLabel xml:lang="en">lock</skos:prefLabel>
		<skos:definition xml:lang="en">An enclosure with a pair or series of gates used for raising or lowering vessels as they pass from one water level to another</skos:definition>
		<skos:prefLabel xml:lang="el">SAMPLE ALTERNATIVE EXPRESSION - αναφορά</skos:prefLabel>
		<skos:definition xml:lang="el">Συστήματα συντεταγμένων</skos:definition>
		<dct:description xml:lang="el">Συστήματα για μονοσήμαντη αναφορά χωρικών πληροφοριών στον χώρο, ως σύνολο συντεταγμένων (x,y,z) ή/και γεωγραφικό πλάτος και μήκος και ύψος, με βάση γεωδαιτικό οριζόντιο και κατακόρυφο σύστημα αναφοράς (datum).</dct:description>
		<skos:inScheme rdf:resource="http://inspire-registry.jrc.ec.europa.eu/registers/FCD/items"/>
	</inspire:SpatialObjectType>
	<inspire:SpatialObjectType rdf:about="http://inspire-registry.jrc.ec.europa.eu/registers/FCD/items/132">
		<inspire:itemStatus>valid</inspire:itemStatus>
		<inspire:dateAccepted>2008-12-05T17:02:12.958+01:00</inspire:dateAccepted>
		<skos:prefLabel xml:lang="en">Sluice</skos:prefLabel>
		<skos:definition xml:lang="en">An open, inclined conduit fitted with a gate for regulating water flow</skos:definition>
		<skos:prefLabel xml:lang="el">SAMPLE ALTERNATIVE EXPRESSION - αναφορά</skos:prefLabel>
		<skos:definition xml:lang="el">Συστήματα συντεταγμένων</skos:definition>
		<dct:description xml:lang="el">Συστήματα για μονοσήμαντη αναφορά χωρικών πληροφοριών στον χώρο, ως σύνολο συντεταγμένων (x,y,z) ή/και γεωγραφικό πλάτος και μήκος και ύψος, με βάση γεωδαιτικό οριζόντιο και κατακόρυφο σύστημα αναφοράς (datum).</dct:description>
		<skos:inScheme rdf:resource="http://inspire-registry.jrc.ec.europa.eu/registers/FCD/items"/>
	</inspire:SpatialObjectType>
	<inspire:SpatialObjectType rdf:about="http://inspire-registry.jrc.ec.europa.eu/registers/FCD/items/142">
		<inspire:itemStatus>valid</inspire:itemStatus>
		<inspire:dateAccepted>2010-01-19T16:18:34.604+01:00</inspire:dateAccepted>
		<skos:prefLabel xml:lang="en">Pipe</skos:prefLabel>
		<skos:definition xml:lang="en">A tube for the conveyance of solids, liquids or gases.</skos:definition>
		<dct:description xml:lang="en">NOTE Regarded as a candidate spatial object in Annex III theme 'Utility and governmental services' due to its role in water supply, which is mentioned in the definition 2007/2/EC Ann III. 6.
This type is a candidate type to be considered by the spatial data theme Utility and governmental services in Annex III to Directive 2007/2/EC.</dct:description>
		<skos:prefLabel xml:lang="el">SAMPLE ALTERNATIVE EXPRESSION - αναφορά</skos:prefLabel>
		<skos:definition xml:lang="el">Συστήματα συντεταγμένων</skos:definition>
		<dct:description xml:lang="el">Συστήματα για μονοσήμαντη αναφορά χωρικών πληροφοριών στον χώρο, ως σύνολο συντεταγμένων (x,y,z) ή/και γεωγραφικό πλάτος και μήκος και ύψος, με βάση γεωδαιτικό οριζόντιο και κατακόρυφο σύστημα αναφοράς (datum).</dct:description>
		<skos:inScheme rdf:resource="http://inspire-registry.jrc.ec.europa.eu/registers/FCD/items"/>
	</inspire:SpatialObjectType>
	<inspire:Theme rdf:about="http://inspire-registry.jrc.ec.europa.eu/registers/FCD/items/156">
		<!-- <owl:sameIndividualAs rdf:resource="http://www.eionet.europa.eu/gemet/theme_concepts?th=4&ns=5" /> -->
		<inspire:itemStatus>valid</inspire:itemStatus>
		<inspire:dateAccepted>2008-12-05T17:05:20.842+01:00</inspire:dateAccepted>
		<skos:prefLabel xml:lang="en">Administrative units</skos:prefLabel>
		<skos:definition xml:lang="en">Units of administration, dividing areas where Member States have and/or exercise jurisdictional rights, for local, regional and national governance, separated by administrative boundaries.</skos:definition>
		<dct:description xml:lang="en">Each national territory is divided into administrative units. The administrative units are separated by administrative boundaries. Administrative units and administrative boundaries form a partition of space. According to user requirements it will be distinguished between land and (coastal) water parts of administrative units. The INSPIRE theme ‘Administrative units’ refers to the division of areas where Member States have and/or exercise jurisdictional rights, for local, regional and national governance, i.e. units at the cadastral parcel level are excluded as well as territorial waters, which are in fact assigned to the INSPIRE themes ‘Cadastral parcels’, ‘Hydrography’ (Annex I) and/or ‘Sea regions’.(Annex III). It does not include related systems such as census districts, post office regions and other sector-specific regions, but it will contain a reference to national statistical units at local level (LAU) and to the Nomenclature of Territorial Units for Statistics (NUTS) established by Eurostat.</dct:description>
		<skos:prefLabel xml:lang="bg">Административни единици</skos:prefLabel>
		<skos:definition xml:lang="bg">Административни единици, отделени с административни граници и отграничаващи райони, върху които държавите-членки имат и/или упражняват юридически правомощия, за целите на местното, регионалното и националнотоуправление.</skos:definition>
		<skos:prefLabel xml:lang="cs">Správní jednotky</skos:prefLabel>
		<skos:definition xml:lang="cs">Správní jednotky rozdělující území, ve kterém členské státy mají nebo vykonávají svrchovaná práva, pro účely místní, regionální a státní správy, oddělené správními hranicemi.</skos:definition>
		<skos:prefLabel xml:lang="da">Administrative enheder</skos:prefLabel>
		<skos:definition xml:lang="da">Forvaltningsenheder, der inddeler områder, hvor medlemsstaterne har og/eller udøver jurisdiktionelle rettigheder på lokalt, regionalt og nationalt plan, adskilt af administrative grænser.</skos:definition>
		<skos:prefLabel xml:lang="de">Verwaltungseinheiten</skos:prefLabel>
		<skos:definition xml:lang="de">Lokale, regionale und nationale Verwaltungseinheiten, die die Gebiete abgrenzen, in denen die Mitgliedstaaten Hoheitsbefugnisse haben und/oder ausüben und die durch Verwaltungsgrenzen voneinander getrennt sind.</skos:definition>
		<skos:prefLabel xml:lang="el">Διοικητικές ενότητες</skos:prefLabel>
		<skos:definition xml:lang="el">Διοικητικές ενότητες που χωρίζουν περιοχές επί των οποίων κράτη μέλη έχουν ή/και ασκούν δικαιοδοτικά δικαιώματα σε τοπικό, περιφερειακό και εθνικό επίπεδο, χωρίζονται από διοικητικά όρια.</skos:definition>
		<skos:prefLabel xml:lang="es">Unidades administrativas</skos:prefLabel>
		<skos:definition xml:lang="es">Unidades administrativas en que se dividan las áreas en las que los Estados miembros tienen y/o ejercen derechos jurisdiccionales, a efectos de administración local, regional y nacional, separadas por límites administrativos.</skos:definition>
		<skos:prefLabel xml:lang="et">Haldusüksused</skos:prefLabel>
		<skos:definition xml:lang="et">Halduspiiridega eraldatud haldusüksused, mis jagavad liikmesriikide jurisdiktsiooni all olevad alad kohaliku, piirkondliku ja riikliku juhtimise eesmärgil.</skos:definition>
		<skos:prefLabel xml:lang="fi">Hallinnolliset yksiköt</skos:prefLabel>
		<skos:definition xml:lang="fi">Hallinnolliset yksiköt, jotka jakavat alueen, jolla jäsenvaltioilla on tai jolla ne käyttävät lainkäyttöoikeuksia, paikalliseen, alueelliseen ja valtakunnalliseen hallintoon ja jotka erotetaan toisistaan hallinnollisin rajoin.</skos:definition>
		<skos:prefLabel xml:lang="fr">Unités administratives</skos:prefLabel>
		<skos:definition xml:lang="fr">Unités d'administration séparées par des limites administratives et délimitant les zones dans lesquelles les États membres détiennent et/ou exercent leurs compétences, aux fins de l'administration locale, régionale et nationale.</skos:definition>
		<skos:prefLabel xml:lang="hu">Közigazgatási egységek</skos:prefLabel>
		<skos:definition xml:lang="hu">Az olyan nemzeti területeket, amelyeken a tagállamok joghatósággal rendelkeznek és/vagy joghatóságot gyakorolnak, helyi, regionális és országos egységekre osztó, közigazgatási határvonalakkal elválasztott igazgatási egységek.</skos:definition>
		<skos:prefLabel xml:lang="it">Unità amministrative</skos:prefLabel>
		<skos:definition xml:lang="it">Unità amministrative di suddivisione delle zone su cui gli Stati membri hanno e/o esercitano la loro giurisdizione a livello locale, regionale e nazionale, delimitate da confini amministrativi.</skos:definition>
		<skos:prefLabel xml:lang="lt">Administraciniai vienetai</skos:prefLabel>
		<skos:definition xml:lang="lt">Administracinėmis ribomis atskirti vietos, regionų ir nacionalinės valdžios administraciniai vienetai, į kuriuos padalijamos teritorijos, kurios priklauso valstybės narės jurisdikcijai ir (arba) kuriose ji vykdo jurisdikciją.</skos:definition>
		<skos:prefLabel xml:lang="lv">Administratīvas vienības</skos:prefLabel>
		<skos:definition xml:lang="lv">Administratīvas vienības, kas sadala apgabalus, kuros dalībvalstīm ir jurisdikcija un/vai kurā tās to īsteno, pašvaldību, reģionu un valsts pārvaldes nolūkā, kas sadalītas ar administratīvo robežu palīdzību.</skos:definition>
		
		<skos:prefLabel xml:lang="mt">Unitajiet amministrattivi</skos:prefLabel>
		<skos:definition xml:lang="mt">Unitajiet ta' amministrazzjoni, li jaqsmu żoni fejn Stati Membri għandhom u/jew jeżerċitaw drittijiet ġurisdizzjonali, għal governanza reġjonali, lokali u nazzjonali, separati minn konfini amministrattivi.</skos:definition>		
		
		<skos:prefLabel xml:lang="nl">Administratieve eenheden</skos:prefLabel>
		<skos:definition xml:lang="nl">Door administratieve grenzen gescheiden lokale, regionale en nationale bestuurlijke eenheden die deel uitmaken van gebieden waarover de lidstaten rechtsbevoegdheid hebben en/of uitoefenen.</skos:definition>
		<skos:prefLabel xml:lang="pl"> Jednostki administracyjne</skos:prefLabel>
		<skos:definition xml:lang="pl">Jednostki administracyjne, dzielące obszary, na których państwa członkowskie mają lub wykonują uprawnienia jurysdykcyjne, dla celów sprawowania władzy na poziomie lokalnym, regionalnym i krajowym, oddzielone granicami administracyjnymi.</skos:definition>
		<skos:prefLabel xml:lang="pt">Unidades administrativas</skos:prefLabel>
		<skos:definition xml:lang="pt">Unidades administrativas, zonas de divisão sobre as quais os Estados-Membros possuam e/ou exerçam direitos jurisdicionais, para efeitos de governação local, regional e nacional, separadas por fronteiras administrativas.</skos:definition>
		<skos:prefLabel xml:lang="ro">Unităţi administrative</skos:prefLabel>
		<skos:definition xml:lang="ro">Unităţi de administrare, de delimitare a zonelor în care statele membre deţin şi/sau îşi exercită competenţa, la nivel local, regional şi naţional, separate prin limite administrative.</skos:definition>
		<skos:prefLabel xml:lang="sk">Správne jednotky</skos:prefLabel>
		<skos:definition xml:lang="sk">Správne jednotky rozdeľujúce oblasti, v ktorých členské štáty majú právomoc rozhodovať a/alebo vykonávajú túto právomoc na účely miestneho, regionálneho a celoštátneho riadenia, oddelené správnymi hranicami.</skos:definition>
		<skos:prefLabel xml:lang="sl">Upravne enote</skos:prefLabel>
		<skos:definition xml:lang="sl">Upravne enote za lokalno, regionalno in nacionalno upravo, ki razdeljujejo območja, na katerih države članice imajo in/ali izvajajo jurisdikcijo, ločene z upravnimi mejami.</skos:definition>
		<skos:prefLabel xml:lang="sv">Administrativa enheter</skos:prefLabel>
		<skos:definition xml:lang="sv">Administrativa enheters, som delar upp områden där medlemsstater har och/eller utövar jurisdiktion, på lokal, regional och nationell nivå, åtskilda av administrativa gränser.</skos:definition>
		<!--
		<skos:prefLabel xml:lang="el">SAMPLE ALTERNATIVE EXPRESSION - αναφορά</skos:prefLabel>
		<skos:definition xml:lang="el">Συστήματα συντεταγμένων</skos:definition>
		<dct:description xml:lang="el">Συστήματα για μονοσήμαντη αναφορά χωρικών πληροφοριών στον χώρο, ως σύνολο συντεταγμένων (x,y,z) ή/και γεωγραφικό πλάτος και μήκος και ύψος, με βάση γεωδαιτικό οριζόντιο και κατακόρυφο σύστημα αναφοράς (datum).</dct:description>
		-->
		<skos:inScheme rdf:resource="http://inspire-registry.jrc.ec.europa.eu/registers/Themes/items"/>
	</inspire:Theme>
	<inspire:Theme rdf:about="http://inspire-registry.jrc.ec.europa.eu/registers/FCD/items/158">
		<!-- <owl:sameIndividualAs rdf:resource="http://www.eionet.europa.eu/gemet/theme_concepts?th=9&ns=5" /> -->
		<inspire:itemStatus>valid</inspire:itemStatus>
		<inspire:dateAccepted>2008-12-05T17:05:47.575+01:00</inspire:dateAccepted>
		<skos:prefLabel xml:lang="en">Protected sites</skos:prefLabel>
		<skos:definition xml:lang="en">Area designated or managed within a framework of international, Community and Member States' legislation to achieve specific conservation objectives.</skos:definition>
		<dct:description xml:lang="en">Area designated or managed within a framework of international, Community and Member States' legislation to achieve specific conservation objectives 
According to IUCN and adopted for the INSPIRE context a protected site is: An area of land and/or sea especially dedicated to the protection and maintenance of biological diversity, and of natural and associated cultural resources, and managed through legal or other effective means.

Protected sites may be located in terrestrial, aquatic and/or marine environments, and may be under either public or private ownership. They may include localities with protection targets defined by different sectors and based on different objectives, especially dedicated to the conservation of nature, the protection and maintenance of biological diversity and of natural and where appropriate associated cultural resources. The sites may receive protection due to more than one type of objectives, and may have a double or multifarious designation status.  Protected sites differ from environmentally founded classifications of natural or cultural objects and also from “area covering” designations as included in CDDA, as localisation, boundary and area of protected sites are based on formal, legal or administrative agreements or decisions.
Although all protected sites meet the general purposes contained in this definition, in practise the precise purposes for which protected sites are managed differ greatly. The main purposes of designation are  specified in categories of CDDA (4.5.2 National designation type category) and according to the typology developed in the Standard Data Form for Natura2000 under the Habitat Directive, furthermore, categories of IUCN for Protected Sites and other international designation types have to be applied. 

A new classification system of protected sites with an overall set of categories under the INSPIRE directive, therefore, has to include Sites of Community Importance (SCI) under the Habitat directive and Special Protection Areas (SPA) under the Birds directive, as well as further designation types on a global level.
This definition of protected sites does not exclude man-made objects or other kinds of cultural heritage sites – protected sites may therefore include where formal protection is given to buildings, archaeological sites of all pre-historic and historic times, including medieval sites/constructions or other cultural objects. This may also be applied to protected sites comprising specific geological, hydrogeological or geomorphological values.

Protected sites in many cases have a formal delineation documentation in cadastral databases. However, delineation injunctions for protected sites are manifold and may just as often not follow cadastral boundaries (e.g. for reasons of generalisation in small scale maps for Natura2000). Being spatial objects under the INSPIRE directive, however, protected sites need to have distinct boundaries of their own, rather than being a mere specific category of some other spatial object type.

Examples of legislation and policies regulating protected sites are Habitat directive (1992) (Directive 92/43/EEC), Birds directive (Directive 79/409/EEC), World Heritage, Ramsar Convention, Barcelona Convention, Helsinki Convention, OSPAR Convention, national law and other international sector policies.</dct:description>
		<skos:prefLabel xml:lang="bg">Защитени обекти</skos:prefLabel>
		<skos:definition xml:lang="bg">Район, определен или управляван съгласно международно законодателство, законодателство на Общността или на държавите-членки за постигане на определени цели за опазване на такива обекти.</skos:definition>
		<skos:prefLabel xml:lang="cs">Chráněná území</skos:prefLabel>
		<skos:definition xml:lang="cs">Území určená nebo spravovaná v rámci mezinárodních právních předpisů a právních předpisů Společenství a členských států pro dosažení konkrétních cílů jejich ochrany.</skos:definition>
		<skos:prefLabel xml:lang="da">Beskyttede lokaliteter</skos:prefLabel>
		<skos:definition xml:lang="da">Områder, der er udpeget eller forvaltes inden for en ramme af international, fællesskabs- og medlemsstatslovgivning for at nå bestemte bevaringsmål.</skos:definition>
		<skos:prefLabel xml:lang="de">Schutzgebiete</skos:prefLabel>
		<skos:definition xml:lang="de">Gebiete, die im Rahmen des internationalen und des gemeinschaftlichen Rechts sowie des Rechts der Mitgliedstaaten ausgewiesen sind oder verwaltet werden, um spezifische Erhaltungsziele zu erreichen.</skos:definition>
		<skos:prefLabel xml:lang="el">Προστατευόμενες τοποθεσίες</skos:prefLabel>
		<skos:definition xml:lang="el">Εκτάσεις χαρακτηρισμένες ή υποκείμενες σε διαχείριση σε ένα πλαίσιο διεθνούς, κοινοτικού και εθνικού δικαίου για την επίτευξη συγκεκριμένων στόχων διατήρησης.</skos:definition>
		<skos:prefLabel xml:lang="es">Lugares protegidos</skos:prefLabel>
		<skos:definition xml:lang="es">Zonas designadas o gestionadas dentro de un marco legislativo internacional, comunitario o propio de los Estados miembros, para la consecución de unos objetivos de conservación específicos.</skos:definition>
		<skos:prefLabel xml:lang="et">Kaitsealused kohad</skos:prefLabel>
		<skos:definition xml:lang="et">Ala, mis on kindlaksmääratud või mida hallatakse rahvusvaheliste, ühenduse või liikmesriikide õigusaktide raames konkreetsete kaitse-eesmärkide saavutamiseks.</skos:definition>
		<skos:prefLabel xml:lang="fi">Suojellut alueet</skos:prefLabel>
		<skos:definition xml:lang="fi">Erityisten suojelutavoitteiden saavuttamiseksi kansainvälisen, yhteisön ja jäsenvaltioiden lainsäädännön puitteissa nimetty tai hoidettu alue.</skos:definition>
		<skos:prefLabel xml:lang="fr">Sites protégés</skos:prefLabel>
		<skos:definition xml:lang="fr">Zone désignée ou gérée dans un cadre législatif international, communautaire ou national en vue d'atteindre des objectifs spécifiques de conservation.</skos:definition>
		<skos:prefLabel xml:lang="hu">Védett helyek</skos:prefLabel>
		<skos:definition xml:lang="hu">Különleges természetvédelmi célok elérése érdekében – nemzetközi, közösségi és tagállami jogszabályok keretében – kijelölt vagy kezelt terület.</skos:definition>
		<skos:prefLabel xml:lang="it">Siti protetti</skos:prefLabel>
		<skos:definition xml:lang="it">Aree designate o gestite in un quadro legislativo internazionale, comunitario o degli Stati membri per conseguire obiettivi di conservazione specifici.</skos:definition>
		<skos:prefLabel xml:lang="lt">Saugomos teritorijos</skos:prefLabel>
		<skos:definition xml:lang="lt">Teritorija, nustatyta ar tvarkoma pagal tarptautinius, Bendrijos ir valstybių narių teisės aktus, siekiant konkrečių apsaugos tikslų.</skos:definition>
		<skos:prefLabel xml:lang="lv">Aizsargājamas teritorijas</skos:prefLabel>
		<skos:definition xml:lang="lv">Teritorijas, kas noteiktas vai pārvaldītas saistībā ar starptautiskiem, Kopienas un dalībvalstu tiesību aktiem, lai nodrošinātu īpašu dabas aizsardzības mērķu īstenošanu.</skos:definition>
		
		<skos:prefLabel xml:lang="mt">Siti protetti</skos:prefLabel>
		<skos:definition xml:lang="mt">Żona indikata jew amministrata f'qafas ta' leġiżlazzjoni internazzjonali, Komunitarja u ta' l-Istati Membri sabiex jintlaħqu objettivi speċifiċi ta' konservazzjoni.</skos:definition>		
		
		<skos:prefLabel xml:lang="nl">Beschermde gebieden</skos:prefLabel>
		<skos:definition xml:lang="nl">Gebieden die worden aangeduid of beheerd in het kader van internationale en communautaire wetgeving of wetgeving van de lidstaten om specifieke doelstellingen op het vlak van milieubescherming te verwezenlijken.</skos:definition>
		<skos:prefLabel xml:lang="pl">Obszary chronione</skos:prefLabel>
		<skos:definition xml:lang="pl">Obszar wyznaczony lub zarządzany w ramach prawa międzynarodowego, wspólnotowego lub państw członkowskich, w celu osiągnięcia szczególnych celów ochrony.</skos:definition>
		<skos:prefLabel xml:lang="pt">Sítios protegidos</skos:prefLabel>
		<skos:definition xml:lang="pt">Zonas designadas ou geridas no âmbito de legislação internacional, comunitária ou dos Estados-Membros para a prossecução de objectivos específicos de conservação.</skos:definition>
		<skos:prefLabel xml:lang="ro">Zone protejate</skos:prefLabel>
		<skos:definition xml:lang="ro">Zone desemnate sau administrate într-un cadru legislativ internaţional, comunitar sau intern, în vederea îndeplinirii unor obiective specifice de conservare.</skos:definition>
		<skos:prefLabel xml:lang="sk">Chránené územia</skos:prefLabel>
		<skos:definition xml:lang="sk">Oblasti vymedzené alebo spravované v rámci medzinárodných právnych predpisov, právnych predpisov Spoločenstva a právnych predpisov členských štátov na účely dosiahnutia osobitných ochranárskych cieľov.</skos:definition>
		<skos:prefLabel xml:lang="sl">Zavarovana območja</skos:prefLabel>
		<skos:definition xml:lang="sl">Področje, ki se določi ali upravlja v okviru mednarodnega prava in prava držav članic in Skupnosti z namenom, da se dosežejo posebni cilji ohranjanja.</skos:definition>
		<skos:prefLabel xml:lang="sv">Skyddade områden</skos:prefLabel>
		<skos:definition xml:lang="sv">Områden som är utsedda eller förvaltas inom ramen för internationell lagstiftning, gemenskapslagstiftning och medlemsstaternas lagstiftning för att uppnå specifika miljövårdsmål.</skos:definition>
		<!--
		<skos:prefLabel xml:lang="el">SAMPLE ALTERNATIVE EXPRESSION - αναφορά</skos:prefLabel>
		<skos:definition xml:lang="el">Συστήματα συντεταγμένων</skos:definition>
		<dct:description xml:lang="el">Συστήματα για μονοσήμαντη αναφορά χωρικών πληροφοριών στον χώρο, ως σύνολο συντεταγμένων (x,y,z) ή/και γεωγραφικό πλάτος και μήκος και ύψος, με βάση γεωδαιτικό οριζόντιο και κατακόρυφο σύστημα αναφοράς (datum).</dct:description>
		-->
		<skos:inScheme rdf:resource="http://inspire-registry.jrc.ec.europa.eu/registers/Themes/items"/>
	</inspire:Theme>
	<inspire:Theme rdf:about="http://inspire-registry.jrc.ec.europa.eu/registers/FCD/items/159">
		<!-- <owl:sameIndividualAs rdf:resource="http://www.eionet.europa.eu/gemet/theme_concepts?th=3&ns=5" /> -->
		<inspire:itemStatus>valid</inspire:itemStatus>
		<inspire:dateAccepted>2008-12-05T17:06:10.666+01:00</inspire:dateAccepted>
		<skos:prefLabel xml:lang="en">Geographical Names</skos:prefLabel>
		<skos:definition xml:lang="en">Names of areas, regions, localities, cities, suburbs, towns or settlements, or any geographical or topographical feature of public or historical interest</skos:definition>
		<dct:description xml:lang="en">A geographical name is a proper noun applied to a natural, man-made or cultural feature on Earth.

 A feature can have different names in one or several languages and the names may be provided, together with appropriate information on the feature, in different products like maps and gazetteers as well as respective services.

An endonym is a name for a geographical feature in an official or well-established language occurring in that area where the feature is situated. An exonym is a name used in a specific language for a geographical feature situated outside the area where that language is widely spoken, and differing in form from the respective endonym(s) in the area where the geographical feature is situated. (UNGEGN, 2007).

In some cases names can be applied as attributes of appropriately modeled spatial objects. However, often the definition, classification, geometry and other attributes of these objects do not correspond with the respective named features. Besides, commonly named features such as elevations, islands, natural shoreline features and stretches of water bodies are seldom modeled as objects in spatial data sets.

A geographical name serves as a means to identify a location. Gazetteers and gazetteer services associate the names with corresponding features – or locations – by means of co-ordinates, feature types and/or other necessary information. A multi-lingual gazetteer (service) shall most probably be established as a part of INSPIRE.</dct:description>
		<skos:prefLabel xml:lang="bg">Географски наименования</skos:prefLabel>
		<skos:definition xml:lang="bg">Наименования на области, региони, местности, големи градове, предградия, малки градове или населени места, или географска или топографска характеристика от обществен или исторически интерес.</skos:definition>
		<skos:prefLabel xml:lang="cs">Zeměpisné názvy</skos:prefLabel>
		<skos:definition xml:lang="cs">Jména oblastí, regionů, míst, velkoměst, předměstí, měst nebo sídel nebo jakýchkoli zeměpisných nebo topografických útvarů veřejného zájmu nebo historického významu.</skos:definition>
		<skos:prefLabel xml:lang="da">Stednavne</skos:prefLabel>
		<skos:definition xml:lang="da">Navne på områder, regioner, lokaliteter, byer, forstæder, bebyggelser og alle former for geografiske og topografiske objekter af offentlig eller historisk interesse.</skos:definition>
		<skos:prefLabel xml:lang="de">Geografische Bezeichnungen</skos:prefLabel>
		<skos:definition xml:lang="de">Namen von Gebieten, Regionen, Orten, Großstädten, Vororten, Städten oder Siedlungen sowie jedes geografische oder topografische Merkmal von öffentlichem oder historischem Interesse.</skos:definition>
		<skos:prefLabel xml:lang="el">Τοπωνύμια</skos:prefLabel>
		<skos:definition xml:lang="el">Τοπωνύμια εκτάσεων, περιοχών, τοποθεσιών, πόλεων, προαστίων, κωμοπόλεων ή οικισμών, ή οποιοδήποτε γεωγραφικό ή τοπογραφικό χαρακτηριστικό δημόσιου ή ιστορικού ενδιαφέροντος.</skos:definition>
		<skos:prefLabel xml:lang="es">Nombres geográficos</skos:prefLabel>
		<skos:definition xml:lang="es">Nombres de zonas, regiones, localidades, ciudades, periferias, poblaciones o asentamientos, o cualquier rasgo geográfico o topográfico de interés público o histórico.</skos:definition>
		<skos:prefLabel xml:lang="et">Geograafilised nimed</skos:prefLabel>
		<skos:definition xml:lang="et">Alade, piirkondade, kohtade, linnade, äärelinnade, alevite või asulate nimed või muud üldist või ajaloolist huvi pakkuvad mis tahes geograafilised või topograafilised tunnused.</skos:definition>
		<skos:prefLabel xml:lang="fi">Paikannimet</skos:prefLabel>
		<skos:definition xml:lang="fi">Maa-alueiden, alueiden, paikkakuntien, suurkaupunkien, esikaupunkien, kaupunkien tai taajamien nimet tai muut sellaisten maantieteellisten tai topografisten kohteiden nimet, joilla on yleistä tai historiallista merkitystä.</skos:definition>
		<skos:prefLabel xml:lang="fr">Dénominations géographiques</skos:prefLabel>
		<skos:definition xml:lang="fr">Noms de zones, de régions, de localités, de grandes villes, de banlieues, de villes moyennes ou d'implantations, ou tout autre élément géographique ou topographique d'intérêt public ou historique.</skos:definition>
		<skos:prefLabel xml:lang="hu">Földrajzi nevek</skos:prefLabel>
		<skos:definition xml:lang="hu">Területek, régiók, helységek, nagyvárosok, elővárosok, városok vagy települések, illetve bármely, a nyilvánosság érdeklődésére számot tartó vagy történeti jelentősségre szert tett földrajzi vagy topográfiai jellegzetesség.</skos:definition>
		<skos:prefLabel xml:lang="it">Nomi geografici</skos:prefLabel>
		<skos:definition xml:lang="it">Denominazione di aree, regioni, località, città, periferie, paesi o centri abitati, o qualsiasi elemento geografico o topografico di interesse pubblico o storico.</skos:definition>
		<skos:prefLabel xml:lang="lt">Geografiniai pavadinimai</skos:prefLabel>
		<skos:definition xml:lang="lt">Sričių, regionų, vietovių, miestų, priemiesčių, miestelių, gyvenviečių ar kitų viešąją ar istorinę reikšmę turinčių geografinių ar topografinių elementų pavadinimai.</skos:definition>
		<skos:prefLabel xml:lang="lv">Toponīmi</skos:prefLabel>
		<skos:definition xml:lang="lv">Rajonu, reģionu, apvidu, lielpilsētu, priekšpilsētu, pilsētu, apdzīvotu vietu vai jebkādu valsts mēroga vai vēsturiskas nozīmes ģeogrāfisku vai topogrāfisku objektu nosaukumi.</skos:definition>
		
		<skos:prefLabel xml:lang="mt">Ismijiet ġeografiċi</skos:prefLabel>
		<skos:definition xml:lang="mt">Ismijiet ta' żoni, reġjuni, lokalitajiet, bliet, subborgi, jew inħawi abitati oħra, jew kull karatteristika ġeografika jew topografika ta' interess pubbliku jew storiku.</skos:definition>		
		
		<skos:prefLabel xml:lang="nl">Geografische namen</skos:prefLabel>
		<skos:definition xml:lang="nl">Namen van gebieden, regio's, plaatsen, steden, voorsteden, gemeenten, nederzettingen, of andere geografische of topografische kenmerken van openbaar of historisch belang.</skos:definition>
		<skos:prefLabel xml:lang="pl">Nazwy geograficzne</skos:prefLabel>
		<skos:definition xml:lang="pl">Nazwy obszarów, regionów, miejscowości, miast, przedmieść lub osiedli, albo każdy inny obiekt geograficzny lub topograficzny o znaczeniu publicznym lub historycznym.</skos:definition>
		<skos:prefLabel xml:lang="pt">Toponímia</skos:prefLabel>
		<skos:definition xml:lang="pt">Denominações das zonas, regiões, localidades, cidades, subúrbios, pequenas cidades ou povoações, ou de qualquer entidade geográfica ou topográfica de interesse público ou histórico.</skos:definition>
		<skos:prefLabel xml:lang="ro">Denumiri geografice</skos:prefLabel>
		<skos:definition xml:lang="ro">Nume de zone, regiuni, localităţi, oraşe mari, suburbii, oraşe mici sau aşezări, sau orice alt element geografic ori topografic de interes public sau istoric.</skos:definition>
		<skos:prefLabel xml:lang="sk">Zemepisné názvy</skos:prefLabel>
		<skos:definition xml:lang="sk">Názvy oblastí, regiónov, lokalít, veľkomiest, predmestí, miest alebo osád alebo akéhokoľvek zemepisného či topografického prvku verejného alebo historického významu.</skos:definition>
		<skos:prefLabel xml:lang="sl">Zemljepisna imena</skos:prefLabel>
		<skos:definition xml:lang="sl">Imena območij, regij, krajev, velemest, predmestij, mest ali zaselkov ali kateri koli geografski ali topografski pojav javnega ali zgodovinskega pomena.</skos:definition>
		<skos:prefLabel xml:lang="sv">Geografiska namn</skos:prefLabel>
		<skos:definition xml:lang="sv">Namn på områden, regioner, platser, städer, förorter, tätorter och annan bebyggelse, samt andra geografiska och topografiska företeelser av allmänt eller historiskt intresse.</skos:definition>
		<!--
		<skos:prefLabel xml:lang="el">SAMPLE ALTERNATIVE EXPRESSION - αναφορά</skos:prefLabel>
		<skos:definition xml:lang="el">Συστήματα συντεταγμένων</skos:definition>
		<dct:description xml:lang="el">Συστήματα για μονοσήμαντη αναφορά χωρικών πληροφοριών στον χώρο, ως σύνολο συντεταγμένων (x,y,z) ή/και γεωγραφικό πλάτος και μήκος και ύψος, με βάση γεωδαιτικό οριζόντιο και κατακόρυφο σύστημα αναφοράς (datum).</dct:description>
		-->
		<skos:inScheme rdf:resource="http://inspire-registry.jrc.ec.europa.eu/registers/Themes/items"/>
	</inspire:Theme>
	<inspire:Theme rdf:about="http://inspire-registry.jrc.ec.europa.eu/registers/FCD/items/160">
		<!-- <owl:sameIndividualAs rdf:resource="http://www.eionet.europa.eu/gemet/theme_concepts?th=5&ns=5" /> -->
		<inspire:itemStatus>valid</inspire:itemStatus>
		<inspire:dateAccepted>2008-12-05T17:06:25.515+01:00</inspire:dateAccepted>
		<skos:prefLabel xml:lang="en">Addresses</skos:prefLabel>
		<skos:definition xml:lang="en">Location of properties based on address identifiers, usually by road name, house number, postal code.</skos:definition>
		<dct:description xml:lang="en">An address is an identification of the fixed location of a property. The full address is a hierarchy consisting of components such as geographic names, with an increasing level of detail, e.g.: town, then street name, then house number or name. It may also include a post code or other postal descriptors. The address may include a path of access but this depends on the function of the address.

Addresses serve several purposes, these include the four uses described in the Dutch Address Registration catalogue: (i) location (e.g. for visits or the delivery of mail), (ii) identification (e.g. in context of a building registration), (iii) jurisdiction (e.g. authority responsible for the property identified by the address), and (iv) sorting and ordering (VROM 2006). There may be other uses identified in the INSPIRE user requirements survey, for example, to aid emergency response.

A number of different object types can be related to property. The most commonly recognised types that have addresses are land parcels and buildings (including flats or apartments). However, other object types, such as water pumping stations, and agricultural buildings, are also types of property. Although they do not receive post they may need to have an address for other functions. This is true in both rural and urban areas. Some other property types that might have addresses include a sports ground, a foothold or a mooring place. Collectively, objects which can have addresses are referred to as addressable objects. 

The location of an address is most often defined so that it characterises the location of the related addressable object.
Although all national or local address systems share similar concepts and general properties, differences exist in formal and informal standards, rules, schemas and data models within Europe. Differences also exist in the extent of the address system, for example, it may be simplified in rural areas. (From revised D2.3)</dct:description>
		<skos:prefLabel xml:lang="bg">Адреси</skos:prefLabel>
		<skos:definition xml:lang="bg">Местонахождение на имоти, обозначено чрез адресни данни, обичайно чрез наименование на улица, номер на сграда и пощенски код.</skos:definition>
		<skos:prefLabel xml:lang="cs">Adresy</skos:prefLabel>
		<skos:definition xml:lang="cs">Poloha nemovitostí podle adresních identifikátorů, obvykle pomocí názvu ulice, čísla domu, poštovního směrovacího čísla.</skos:definition>
		<skos:prefLabel xml:lang="da">Adresser</skos:prefLabel>
		<skos:definition xml:lang="da">Lokalisering af ejendomme på grundlag af adresseidenter, normalt ved hjælp af vejnavn, husnummer og postnummer.</skos:definition>
		<skos:prefLabel xml:lang="de">Adressen</skos:prefLabel>
		<skos:definition xml:lang="de">Lokalisierung von Grundstücken anhand von Adressdaten, in der Regel Straßenname, Hausnummer und Postleitzahl.</skos:definition>
		<skos:prefLabel xml:lang="el"> Διευθύνσεις</skos:prefLabel>
		<skos:definition xml:lang="el">Θέση ακινήτων με βάση τη διεύθυνση, συνήθως με όνομα οδού, αριθμό οικίας και ταχυδρομικό κώδικα.</skos:definition>
		<skos:prefLabel xml:lang="es">Direcciones</skos:prefLabel>
		<skos:definition xml:lang="es">Localización de las propiedades, basada en identificadores de direcciones, por ejemplo, el nombre de la vía pública, el número de la finca, el código postal.</skos:definition>
		<skos:prefLabel xml:lang="et">Aadressid</skos:prefLabel>
		<skos:definition xml:lang="et">Maavalduste asukoht aadressi elementide, tavaliselt tee või tänava nime, majanumbri ja postiindeksi järgi.</skos:definition>
		<skos:prefLabel xml:lang="fi">Osoitteet</skos:prefLabel>
		<skos:definition xml:lang="fi">Kiinteistöjen sijainti, joka perustuu osoitetietoon, jossa tavallisesti kadunnimi, talon numero ja postinumero.</skos:definition>
		<skos:prefLabel xml:lang="fr">Adresses</skos:prefLabel>
		<skos:definition xml:lang="fr">Localisation des propriétés fondée sur les identifiants des adresses, habituellement le nom de la rue, le numéro de la maison et le code postal.</skos:definition>
		<skos:prefLabel xml:lang="hu">Címek</skos:prefLabel>
		<skos:definition xml:lang="hu">Az ingatlanok helye címazonosítók – rendszerint utcanév, házszám, irányítószám – alapján.</skos:definition>
		<skos:prefLabel xml:lang="it">Indirizzi</skos:prefLabel>
		<skos:definition xml:lang="it">Localizzazione delle proprietà basata su identificatori di indirizzo, in genere nome della via, numero civico, codice postale.</skos:definition>
		<skos:prefLabel xml:lang="lt">Adresai</skos:prefLabel>
		<skos:definition xml:lang="lt">Nuosavybės vieta pagal adreso duomenis, paprastai gatvės pavadinimą, namo numerį, pašto kodą.</skos:definition>
		<skos:prefLabel xml:lang="lv">Adreses</skos:prefLabel>
		<skos:definition xml:lang="lv">Īpašumu ģeogrāfiskā atrašanās vieta, pamatojoties uz adreses identifikatoriem; parasti tie ir ceļu nosaukumi, māju numuri, pasta indeksi.</skos:definition>
		
		<skos:prefLabel xml:lang="mt">Indirizzi</skos:prefLabel>
		<skos:definition xml:lang="mt">Pożizzjoni ta' proprjetajiet ibbażata fuq identifikaturi ta' l-indirizzi, normalment bl-isem tat-triq, in-numru tad-dar, ilkodiċi postali.</skos:definition>		
		
		<skos:prefLabel xml:lang="nl">Adressen</skos:prefLabel>
		<skos:definition xml:lang="nl">Locatie van onroerende zaken, gebaseerd op adresaanduidingen, gewoonlijk aan de hand van de straatnaam, het huisnummer en de postcode.</skos:definition>
		<skos:prefLabel xml:lang="pl">Adresy</skos:prefLabel>
		<skos:definition xml:lang="pl">Lokalizacja nieruchomości na podstawie danych adresowych, zazwyczaj nazwy ulicy, numeru budynku, kodu pocztowego.</skos:definition>
		<skos:prefLabel xml:lang="pt">Endereços</skos:prefLabel>
		<skos:definition xml:lang="pt">Localização de propriedades com base em identificadores de endereço, em regra, o nome da rua, o número da porta e o código postal.</skos:definition>
		<skos:prefLabel xml:lang="ro">Adrese</skos:prefLabel>
		<skos:definition xml:lang="ro">Localizare a proprietăţilor, bazată pe identificatori de adresă, de obicei numele străzii, numărul casei şi codul poştal.</skos:definition>
		<skos:prefLabel xml:lang="sk">Adresy</skos:prefLabel>
		<skos:definition xml:lang="sk">Poloha nehnuteľností založená na identifikátoroch obsiahnutých v adrese, obyčajne podľa názvu ulice, čísla domu, poštového smerovacieho čísla.</skos:definition>
		<skos:prefLabel xml:lang="sl">Naslovi</skos:prefLabel>
		<skos:definition xml:lang="sl">Lokacija nepremičnin, ki temelji na identifikatorjih naslova, običajno z imenom ulice, hišno številko, poštno številko.</skos:definition>
		<skos:prefLabel xml:lang="sv">Adresser</skos:prefLabel>
		<skos:definition xml:lang="sv">Läge för fastigheter på grundval av adressuppgifter, vanligen i form av gatunamn, gatunummer och postnummer.</skos:definition>
		<!--
		<skos:prefLabel xml:lang="el">SAMPLE ALTERNATIVE EXPRESSION - αναφορά</skos:prefLabel>
		<skos:definition xml:lang="el">Συστήματα συντεταγμένων</skos:definition>
		<dct:description xml:lang="el">Συστήματα για μονοσήμαντη αναφορά χωρικών πληροφοριών στον χώρο, ως σύνολο συντεταγμένων (x,y,z) ή/και γεωγραφικό πλάτος και μήκος και ύψος, με βάση γεωδαιτικό οριζόντιο και κατακόρυφο σύστημα αναφοράς (datum).</dct:description>
		-->
		<skos:inScheme rdf:resource="http://inspire-registry.jrc.ec.europa.eu/registers/Themes/items"/>
	</inspire:Theme>
	<inspire:Theme rdf:about="http://inspire-registry.jrc.ec.europa.eu/registers/FCD/items/161">
		<!-- <owl:sameIndividualAs rdf:resource="http://www.eionet.europa.eu/gemet/theme_concepts?th=6&ns=5" /> -->
		<inspire:itemStatus>valid</inspire:itemStatus>
		<inspire:dateAccepted>2008-12-05T17:06:40.007+01:00</inspire:dateAccepted>
		<skos:prefLabel xml:lang="en">Cadastral Parcels</skos:prefLabel>
		<skos:definition xml:lang="en">Areas defined by cadastral registers or equivalent</skos:definition>
		<dct:description xml:lang="en">The INSPIRE Directive focuses on the geographical part of cadastral data. 
In the INSPIRE context, cadastral parcels will be mainly used as locators for geo-information in general, including environmental data. 
As much as possible, in the INSPIRE context, cadastral parcels should be forming a partition of national territory. Cadastral parcel should be considered as a single area of Earth surface, under homogeneous real property rights and unique ownership (adapted from UN ECE 2004 and WG-CPI, 2006). 
Remark: By unique ownership is meant that the ownership is held by one or several owners for the whole parcel. By homogeneous property rights is meant that rights of ownership, leases and mortgages affect the whole parcel. This does not apply to specific rights as servitudes which may only affect part of the parcel.
In the definition given by the INSPIRE directive, "or equivalent" refers to all public agencies and institutions other than the main traditional/nominal cadastre or land registry, that register parts of the Earth's surface such as special domains, urban cadastres, public lands, which spatially complement the registrations by the main cadastre or land registry.
Cadastral parcels are considered in the INSPIRE scope if they are available as vector data.
Rights and owners are out of the INSPIRE scope.
Buildings, land use, addresses are considered in other INSPIRE themes.</dct:description>
		<skos:prefLabel xml:lang="bg">Кадастрални парцели</skos:prefLabel>
		<skos:definition xml:lang="bg">Райони, посочени в кадастрални регистри или други равностойни документи.</skos:definition>
		<skos:prefLabel xml:lang="cs">Katastrální parcely</skos:prefLabel>
		<skos:definition xml:lang="cs">Území vymezená v katastru nemovitostí nebo v obdobném rejstříku.</skos:definition>
		<skos:prefLabel xml:lang="da">Matrikulære parceller</skos:prefLabel>
		<skos:definition xml:lang="da">Arealer, der er defineret i matrikelregistre eller lignende.</skos:definition>
		<skos:prefLabel xml:lang="de">Flurstücke/Grundstücke (Katasterparzellen)</skos:prefLabel>
		<skos:definition xml:lang="de">Gebiete, die anhand des Grundbuchs oder gleichwertiger Verzeichnisse bestimmt werden.</skos:definition>
		<skos:prefLabel xml:lang="el">Γεωτεμάχια κτηματολογίου</skos:prefLabel>
		<skos:definition xml:lang="el">Εκτάσεις που ορίζονται από κτηματολογικά μητρώα ή αντίστοιχες.</skos:definition>
		<skos:prefLabel xml:lang="es">Parcelas catastrales</skos:prefLabel>
		<skos:definition xml:lang="es">Áreas determinadas por registros catastrales o equivalentes.</skos:definition>
		<skos:prefLabel xml:lang="et">Katastriüksused</skos:prefLabel>
		<skos:definition xml:lang="et">Katastritunnuste või võrdväärsete tunnustega kindlaksmääratud alad.</skos:definition>
		<skos:prefLabel xml:lang="fi">Kiinteistöt</skos:prefLabel>
		<skos:definition xml:lang="fi">Alueet, jotka on määritelty kiinteistörekisterissä tai vastaavassa.</skos:definition>
		<skos:prefLabel xml:lang="fr">Parcelles cadastrales</skos:prefLabel>
		<skos:definition xml:lang="fr">Zones définies par les registres cadastraux ou équivalents.</skos:definition>
		<skos:prefLabel xml:lang="hu">Kataszteri parcellák</skos:prefLabel>
		<skos:definition xml:lang="hu">Kataszteri nyilvántartásokkal – vagy ezzel egyenértékű módon – meghatározott területek.</skos:definition>
		<skos:prefLabel xml:lang="it">Parcelle catastali</skos:prefLabel>
		<skos:definition xml:lang="it">Aree definite dai registri catastali o equivalenti.</skos:definition>
		<skos:prefLabel xml:lang="lt">Kadastro sklypai</skos:prefLabel>
		<skos:definition xml:lang="lt">Kadastrų registruose ar panašiai apibrėžti plotai.</skos:definition>
		<skos:prefLabel xml:lang="lv">Kadastrāli zemes gabali</skos:prefLabel>
		<skos:definition xml:lang="lv">Teritorijas, kas noteiktas kadastra reģistros vai līdzīgās sistēmās.</skos:definition>
		
		<skos:prefLabel xml:lang="mt">Pakketti katastali</skos:prefLabel>
		<skos:definition xml:lang="mt">Żoni ddefiniti b'reġistri katastali jew l-ekwivalenti.</skos:definition>		
		
		<skos:prefLabel xml:lang="nl">Kadastrale percelen</skos:prefLabel>
		<skos:definition xml:lang="nl">Gebieden die worden bepaald door kadastrale registers of een equivalent daarvan.</skos:definition>
		<skos:prefLabel xml:lang="pl">Działki katastralne</skos:prefLabel>
		<skos:definition xml:lang="pl">Obszary określone na podstawie rejestrów katastralnych lub ich odpowiedników.</skos:definition>
		<skos:prefLabel xml:lang="pt">Parcelas cadastrais</skos:prefLabel>
		<skos:definition xml:lang="pt">Áreas definidas por registos cadastrais ou equivalentes.</skos:definition>
		<skos:prefLabel xml:lang="ro">Parcele cadastrale</skos:prefLabel>
		<skos:definition xml:lang="ro">Zone stabilite de registrele cadastrale sau echivalente.</skos:definition>
		<skos:prefLabel xml:lang="sk">Katastrálne parcely</skos:prefLabel>
		<skos:definition xml:lang="sk">Územia vymedzené katastrálnymi registrami alebo rovnocennými registrami.</skos:definition>
		<skos:prefLabel xml:lang="sl">Katastrske parcele</skos:prefLabel>
		<skos:definition xml:lang="sl">Področja, ki jih opredeljujejo zemljiški kataster ali enakovredni registri.</skos:definition>
		<skos:prefLabel xml:lang="sv">Fastighetsområden</skos:prefLabel>
		<skos:definition xml:lang="sv">Områden definierade av fastighetsregister eller motsvarande.</skos:definition>
		<!--
		<skos:prefLabel xml:lang="el">SAMPLE ALTERNATIVE EXPRESSION - αναφορά</skos:prefLabel>
		<skos:definition xml:lang="el">Συστήματα συντεταγμένων</skos:definition>
		<dct:description xml:lang="el">Συστήματα για μονοσήμαντη αναφορά χωρικών πληροφοριών στον χώρο, ως σύνολο συντεταγμένων (x,y,z) ή/και γεωγραφικό πλάτος και μήκος και ύψος, με βάση γεωδαιτικό οριζόντιο και κατακόρυφο σύστημα αναφοράς (datum).</dct:description>
		-->
		<skos:inScheme rdf:resource="http://inspire-registry.jrc.ec.europa.eu/registers/Themes/items"/>
	</inspire:Theme>
	<inspire:Theme rdf:about="http://inspire-registry.jrc.ec.europa.eu/registers/FCD/items/162">
		<!-- <owl:sameIndividualAs rdf:resource="http://www.eionet.europa.eu/gemet/theme_concepts?th=7&ns=5" /> -->
		<inspire:itemStatus>valid</inspire:itemStatus>
		<inspire:dateAccepted>2008-12-05T17:06:52.954+01:00</inspire:dateAccepted>
		<skos:prefLabel xml:lang="en">Transport networks</skos:prefLabel>
		<skos:definition xml:lang="en">Road, rail, air and water transport networks and related infrastructure. Includes links between different networks. Also includes the trans-European transport network as defined in Decision No 1692/96/EC of the European Parliament and of the Council of 23 July 1996 on Community Guidelines for the development of the trans-European transport network (1) and future revisions of that Decision.

(1) OJ L 228, 9.9.1996, p. 1. Decision as last amended by Council Regulation (EC) No 1791/2006 (OJ L 363, 20.12.2006, p. 1).</skos:definition>
		<dct:description xml:lang="en">The transport component should comprise an integrated transport network, and related features, that are seamless within each national border. In accordance with article 10.2 of the Directive, national transport networks may also be seamless at European level, i.e. connected at national borders. Transportation data includes topographic features related to transport by road, rail, water, and air. It is important that the features form networks where appropriate, and that links between different networks are established, i.e multi-modal nodes, especially at the local level, in order to satisfy the requirements for intelligent transport systems such as location based services (LBS) and telematics. The transport network should also support the referencing of transport flow to enable our navigation services.</dct:description>
		<skos:prefLabel xml:lang="bg">Транспортни мрежи</skos:prefLabel>
		<skos:definition xml:lang="bg">Автомобилни, железопътни, въздушни и водни транспортни мрежи и прилежаща инфраструктура. Включват връзки между различните мрежи. Включват също така и Трансевропейската транспортна мрежа, определена в Решение № 1692/96/ЕО на Европейския парламент и на Съвета от 23 юли 1996 г. относно общностните насоки за развитие на Трансевропейската транспортна мрежа (1) и бъдещо преразглеждане на това решение.</skos:definition>
		<skos:prefLabel xml:lang="cs">Dopravní sítě</skos:prefLabel>
		<skos:definition xml:lang="cs">Silniční, železniční, letecké a vodní dopravní sítě a související infrastruktura. Zahrnují spojnice mezi jednotlivými sítěmi. Zahrnují rovněž transevropskou dopravní síť, jak je vymezena v rozhodnutí Evropského parlamentu a Rady č. 1692/96/ES ze dne 23. července 1996 o hlavních směrech Společenství pro rozvoj transevropské dopravní sítě (1) a v budoucích změnách uvedeného rozhodnutí.</skos:definition>
		<skos:prefLabel xml:lang="da">Transportnet</skos:prefLabel>
		<skos:definition xml:lang="da">Transportnet for biler, tog, fly og skibe med tilhørende infrastruktur. Omfatter forbindelser mellem de forskellige net. Omfatter også det transeuropæiske transportnet som defineret i Europa-Parlamentets og Rådets beslutning nr. 1692/96/EF af 23. juli 1996 om Fællesskabets retningslinjer for udvikling af det transeuropæiske transportnet (1) og fremtidige ændringer af denne beslutning.</skos:definition>
		<skos:prefLabel xml:lang="de">Verkehrsnetze</skos:prefLabel>
		<skos:definition xml:lang="de">Verkehrsnetze und zugehörige Infrastruktureinrichtungen für Straßen-, Schienen- und Luftverkehr sowie Schifffahrt. Umfasst auch die Verbindungen zwischen den verschiedenen Netzen. Umfasst auch das transeuropäische Verkehrsnetz im Sinne der Entscheidung Nr. 1692/96/EG des Europäischen Parlaments und des Rates vom 23. Juli 1996 über gemeinschaftliche Leitlinien für den Aufbau eines transeuropäischen Verkehrsnetzes (1) und künftiger Überarbeitungen dieser Entscheidung.</skos:definition>
		<skos:prefLabel xml:lang="el">Δίκτυα μεταφορών</skos:prefLabel>
		<skos:definition xml:lang="el">Δίκτυα οδικών, σιδηροδρομικών, αεροπορικών και υδάτινων μεταφορών και οι αντίστοιχες υποδομές. Περιλαμβάνονται οι συνδέσεις μεταξύ των διαφόρων δικτύων. Περιλαμβάνεται επίσης το διευρωπαϊκό δίκτυο μεταφορών, όπως ορίζεται στην απόφαση αριθ. 1692/96/EΚ του Ευρωπαϊκού Κοινοβουλίου και του Συμβουλίου, της 23ης Ιουλίου 1996, περί των κοινοτικών προσανατολισμών για την ανάπτυξη του διευρωπαϊκού δικτύου μεταφορών (1) και στις μελλοντικές αναθεωρήσεις της εν λόγω απόφασης.</skos:definition>
		<skos:prefLabel xml:lang="es">Redes de transporte</skos:prefLabel>
		<skos:definition xml:lang="es">Redes de carreteras, ferrocarril, transporte aéreo y vías navegables, con sus correspondientes infraestructuras. Se incluirán las conexiones entre redes diferentes. Se incluirá también la red transeuropea de transporte, según la definición de la Decisión no 1692/96/CE del Parlamento Europeo y del Consejo, de 23 de julio de 1996, sobre las orientaciones comunitarias para el desarrollo de la red transeuropea de transporte (1), y de las futuras revisiones de dicha Decisión.</skos:definition>
		<skos:prefLabel xml:lang="et">Transpordivõrgud</skos:prefLabel>
		<skos:definition xml:lang="et">Maantee-, raudtee-, õhu- ja veetranspordivõrgud ja nendega seotud infrastruktuurid. Sisaldab eri võrkude vahelisi ühendusi. Hõlmab ka Euroopa Parlamendi ja nõukogu 23. juuli 1996. aasta otsuses 1692/96/EÜ üleeuroopalise transpordivõrgu arendamist käsitlevate ühenduse suuniste kohta, (1) määratletud üleeuroopalist transpordivõrku ja selle otsuse edaspidiseid muudatusi.</skos:definition>
		<skos:prefLabel xml:lang="fi">Liikenneverkot</skos:prefLabel>
		<skos:definition xml:lang="fi">Tie-, raide-, ilma- ja vesiliikenneverkot ja niihin liittyvä infrastruktuuri. Sisältää eri verkkojen väliset yhteydet. Sisältää myös Euroopan laajuisen liikenneverkon sellaisena kuin se on määritelty yhteisön suuntaviivoista Euroopan laajuisen liikenneverkon kehittämiseksi 23 päivänä heinäkuuta 1996 tehdyssä Euroopan parlamentin ja neuvoston päätöksessä N:o 1692/96/EY (1) ja tämän päätöksen tulevissa tarkistuksissa.</skos:definition>
		<skos:prefLabel xml:lang="fr">Réseaux de transport</skos:prefLabel>
		<skos:definition xml:lang="fr">Réseaux routier, ferroviaire, aérien et navigable ainsi que les infrastructures associées. Sont également incluses les correspondances entre les différents réseaux, ainsi que le réseau transeuropéen de transport tel que défini dans la décision no 1692/96/CE du Parlement européen et du Conseil du 23 juillet 1996 sur les orientations communautaires pour le développement du réseau transeuropéen de transport (1) et les révisions futures de cette décision.</skos:definition>
		<skos:prefLabel xml:lang="hu">Közlekedési hálózatok</skos:prefLabel>
		<skos:definition xml:lang="hu">Közúti, vasúti, légi és vízi közlekedési hálózatok és a kapcsolódó infrastruktúra. Ide tartoznak a különféle hálózatok közötti összeköttetések is. Magában foglalja továbbá a transzeurópai közlekedési hálózat fejlesztésére vonatkozó közösségi iránymutatásokról szóló, 1996. július 23-i 1692/96/EK európai parlamenti és tanácsi határozatban (1) meghatározott transzeurópai közlekedési hálózatot és e határozat jövőbeli felülvizsgálatait is.</skos:definition>
		<skos:prefLabel xml:lang="it">Reti di trasporto</skos:prefLabel>
		<skos:definition xml:lang="it">Reti di trasporto su strada, su rotaia, per via aerea e per vie navigabili e relative infrastrutture. Questa voce comprende i collegamenti tra le varie reti e anche la rete transeuropea di trasporto di cui alla decisione n. 1692/96/CE del Parlamento europeo e del Consiglio, del 23 luglio 1996, sugli orientamenti comunitari per lo sviluppo della rete transeuropee dei trasporti (1) e successive revisioni.</skos:definition>
		<skos:prefLabel xml:lang="lt">Transporto tinklai</skos:prefLabel>
		<skos:definition xml:lang="lt">Keliai, geležinkeliai, oro ir vandens transporto tinklai bei su jais susijusi infrastruktūra. Įtraukiamos sąsajos tarp skirtingų tinklų. Taip pat apima 1996 m. liepos 23 d. Europos Parlamente ir Tarybos sprendime Nr. 1692/96/EB, pateikiančiame Bendrijos gaires dėl transeuropinio transporto tinklo plėtros (1), ir jo vėlesniuose pakeitimuose apibrėžtą transeuropinį transporto tinklą.</skos:definition>
		<skos:prefLabel xml:lang="lv">Transporta tīkli</skos:prefLabel>
		<skos:definition xml:lang="lv">Autoceļi, dzelzceļa, gaisa un ūdens transporta tīkli un ar tiem saistītā infrastruktūra. Tie ietver arī dažādu tīklu savienojumus. Tie ietver arī Eiropas transporta tīklu, kā tas definēts Eiropas Parlamenta un Padomes Lēmumā Nr. 1692/96/EK (1996. gada 23. jūlijs) par Kopienas pamatnostādnēm Eiropas transporta tīkla attīstībai (1) un minētā lēmuma turpmākajos grozījumos.</skos:definition>
		
		<skos:prefLabel xml:lang="mt">Networks tat-trasport</skos:prefLabel>
		<skos:definition xml:lang="mt">Networks tat-trasport tat-triq, tal-ferrovija, ta' l-ajru u ta' l-ilma u infrastruttura relatata. Huma inklużi l-kollegamenti bejn networks differenti. Huma inklużi wkoll in-network trans-Ewropew tat-trasport kif definit fid-Deċiżjoni Nru 1692/96/KE tal-Parlament Ewropew u tal-Kunsill tat-23 ta' Lulju 1996 dwar il-Linji Gwida tal-Komunità għalliżvilupp ta' network trans-Ewropew tat-trasport (1) u r-reviżjonijiet futuri ta' dik id-Deċiżjoni.</skos:definition>		
		
		<skos:prefLabel xml:lang="nl">Vervoersnetwerken</skos:prefLabel>
		<skos:definition xml:lang="nl">Netwerken voor vervoer over de weg, per spoor, in de lucht en over het water en de aanverwante infrastructuur met inbegrip van koppelingen tussen verschillende netwerken en het trans-Europees vervoersnetwerk, zoals gedefinieerd in Beschikking nr. 1692/96/EG van het Europees Parlement en de Raad van 23 juli 1996 betreffende communautaire richtsnoeren voor de ontwikkeling van een trans-Europees vervoersnet (1) en de latere herzieningen van deze beschikking.</skos:definition>
		<skos:prefLabel xml:lang="pl">Sieci transportowe</skos:prefLabel>
		<skos:definition xml:lang="pl">Sieci transportu drogowego, kolejowego, lotniczego i wodnego oraz związana z nimi infrastruktura. Obejmują połączenia pomiędzy różnymi sieciami. Zalicza się do nich także transeuropejską sieć transportową w rozumieniu decyzji nr 1692/96/WE Parlamentu Europejskiego i Rady z dnia 23 czerwca 1996 r. w sprawie wspólnotowych wytycznych dotyczących rozwoju transeuropejskiej sieci transportowej (1) wraz z jej przyszłymi zmianami.</skos:definition>
		<skos:prefLabel xml:lang="pt">Redes de transporte</skos:prefLabel>
		<skos:definition xml:lang="pt">Redes de transporte rodoviário, ferroviário, aéreo e por via navegável, e respectivas infra-estruturas. Inclui as ligações entre as diferentes redes. Inclui também a rede transeuropeia de transportes definida na Decisão n.o 1692/96/CE do Parlamento Europeu e do Conselho, de 23 de Julho de 1996, sobre as orientações comunitárias para o desenvolvimento da rede transeuropeia de transportes (1), e as futuras revisões dessa decisão.</skos:definition>
		<skos:prefLabel xml:lang="ro">Reţele de transport</skos:prefLabel>
		<skos:definition xml:lang="ro">Reţele de transport rutier, feroviar, aerian şi pe apă şi infrastructura asociată. Cuprinde, de asemenea, legături între diferite reţele. Mai cuprinde şi reţeaua transeuropeană de transport, astfel cum este definită în Decizia nr. 1692/96/CE a Parlamentului European şi a Consiliului din 23 iulie 1996 privind orientările comunitare pentru dezvoltarea reţelei transeuropene de transport (1) şi modificările ulterioare.</skos:definition>
		<skos:prefLabel xml:lang="sk">Dopravné siete</skos:prefLabel>
		<skos:definition xml:lang="sk">Cestné, železničné, letecké a vodné dopravné siete a s nimi súvisiaca infraštruktúra. Patria sem prepojenia medzi jednotlivými sieťami. Zahŕňajú tiež transeurópsku dopravnú sieť vymedzenú v rozhodnutí Európskeho parlamentu a Rady č. 1692/96/ES z 23. júla 1996 o základných usmerneniach Spoločenstva pre rozvoj transeurópskej dopravnej siete (1) a budúcich revíziách uvedeného rozhodnutia.</skos:definition>
		<skos:prefLabel xml:lang="sl">Prometna omrežja</skos:prefLabel>
		<skos:definition xml:lang="sl">Cestna, železniška, zračna in vodna prometna omrežja ter z njimi povezana infrastruktura. Vključuje povezave med različnimi omrežji. Vključuje tudi vseevropsko prometno omrežje, kakor je določeno v Odločbi št. 1692/96/ES Evropskega parlamenta in Sveta z dne 23. julija 1996 o smernicah Skupnosti za razvoj vseevropskega prometnega omrežja (1), in prihodnje preglede te odločbe.</skos:definition>
		<skos:prefLabel xml:lang="sv">Transportnät</skos:prefLabel>
		<skos:definition xml:lang="sv">Väg-, järnvägs-, luft- och sjötransportnät och tillhörande infrastruktur. Innefattar länkar mellan olika nät. Innefattar också det transeuropeiska transportnät som definieras i Europaparlamentets och rådets beslut nr 1692/96/EG av den 23 juli 1996 om gemenskapens riktlinjer för utbyggnad av det transeuropeiska transportnätet (1) samt framtida ändringar av det beslutet.</skos:definition>
		<!--
		<skos:prefLabel xml:lang="el">SAMPLE ALTERNATIVE EXPRESSION - αναφορά</skos:prefLabel>
		<skos:definition xml:lang="el">Συστήματα συντεταγμένων</skos:definition>
		<dct:description xml:lang="el">Συστήματα για μονοσήμαντη αναφορά χωρικών πληροφοριών στον χώρο, ως σύνολο συντεταγμένων (x,y,z) ή/και γεωγραφικό πλάτος και μήκος και ύψος, με βάση γεωδαιτικό οριζόντιο και κατακόρυφο σύστημα αναφοράς (datum).</dct:description>
		-->
		<skos:inScheme rdf:resource="http://inspire-registry.jrc.ec.europa.eu/registers/Themes/items"/>
	</inspire:Theme>
	<inspire:Theme rdf:about="http://inspire-registry.jrc.ec.europa.eu/registers/FCD/items/163">
		<!-- <owl:sameIndividualAs rdf:resource="http://www.eionet.europa.eu/gemet/theme_concepts?th=8&ns=5" /> -->
		<inspire:itemStatus>valid</inspire:itemStatus>
		<inspire:dateAccepted>2008-12-05T17:07:06.479+01:00</inspire:dateAccepted>
		<skos:prefLabel xml:lang="en">Hydrography</skos:prefLabel>
		<skos:definition xml:lang="en">Hydrographic elements, including marine areas and all other water bodies and items related to them, including river basins and sub-basins. Where appropriate, according to the definitions set out in Directive 2000/60/EC of the European Parliament and of the Council of 23 October 2000 establishing a framework for Community action in the field of water policy, and in the form of networks.</skos:definition>
		<dct:description xml:lang="en">The theme “Hydrography” is a basic reference component and, therefore, of interest for many users and uses.

For mapping purposes (to provide a map background for orientation and to understand place relationships), it includes the representation of all main hydrographic elements – both natural and artificial. To fulfill reporting requirements of EC water-related directives it includes the river and channel network; surface water bodies within river basin districts are categorised as rivers, lakes, transitional waters or coastal waters, or as artificial surface water bodies or heavily modified surface water bodies. Furthermore, a topologically-sound river network is necessary for GIS-based spatial analysis and modeling.

Geographically, the theme “Hydrography” covers all inland water and marine areas covered by river basin districts as defined by WFD.</dct:description>
		<skos:prefLabel xml:lang="bg">Хидрография</skos:prefLabel>
		<skos:definition xml:lang="bg">Хидрографски елементи, включително морски райони и други водни маси и свързани с тях елементи, включително речни басейни и подбасейни. По целесъобразност съгласно определенията, посочени в Директива 2000/60/ЕО на Европейския парламент и на Съвета от 23 октомври 2000 г. за установяване на рамка за действията на Общността в областта на политиката за водите (2) и под формата на мрежи.</skos:definition>
		<skos:prefLabel xml:lang="cs">Vodopis</skos:prefLabel>
		<skos:definition xml:lang="cs">Přírodní prvky, včetně mořských oblastí a všech ostatních s nimi souvisejících vodních těles a prvků, včetně povodí a dílčích povodí. Případně v souladu s definicemi uvedenými ve směrnici Evropského parlamentu a Rady 2000/60/ES ze dne 23. října 2000, kterou se stanoví rámec pro činnost Společenství v oblasti vodní politiky (2), a v podobě sítí.</skos:definition>
		<skos:prefLabel xml:lang="da">Hydrograf</skos:prefLabel>
		<skos:definition xml:lang="da">Hydrografiske elementer, herunder havområder og alle andre vandområder og dertil knyttede forekomster, herunder også vandløbsoplande og vandløbsdeloplande. I givet fald i henhold til definitionerne i Europa-Parlamentets og Rådets direktiv 2000/60/EF af 23. oktober 2000 om fastlæggelse af en ramme for Fællesskabets vandpolitiske foranstaltninger (2) og i form af net.</skos:definition>
		<skos:prefLabel xml:lang="de">Gewässernetz</skos:prefLabel>
		<skos:definition xml:lang="de">Elemente des Gewässernetzes, einschließlich Meeresgebieten und allen sonstigen Wasserkörpern und hiermit verbundenen Teilsystemen, darunter Einzugsgebiete und Teileinzugsgebiete. Gegebenenfalls gemäß den Definitionen der Richtlinie 2000/60/EG des Europäischen Parlaments und des Rates vom 23. Oktober 2000 zur Schaffung eines Ordnungsrahmens für Maßnahmen der Gemeinschaft im Bereich der Wasserpolitik (2) und in Form von Netzen.</skos:definition>
		<skos:prefLabel xml:lang="el">Υδρογραφία</skos:prefLabel>
		<skos:definition xml:lang="el">Υδρογραφικά στοιχεία, όπου περιλαμβάνονται οι θαλάσσιες περιοχές και όλα τα άλλα υδατικά συστήματα και σχετιζόμενα στοιχεία, μεταξύ των οποίων και οι λεκάνες και υπολεκάνες απορροής ποταμών. Κατά περίπτωση, σύμφωνα με τους ορισμούς της οδηγίας 2000/60/ΕΚ του Ευρωπαϊκού Κοινοβουλίου και του Συμβουλίου, της 23ης Οκτωβρίου 2000, για τη θέσπιση πλαισίου κοινοτικής δράσης στον τομέα της πολιτικής των υδάτων (2) και υπό μορφή δικτύων.</skos:definition>
		<skos:prefLabel xml:lang="es">Hidrografía</skos:prefLabel>
		<skos:definition xml:lang="es">Elementos hidrográficos, incluidas las zonas marinas y todas las otras masas de agua y elementos relacionados con ellas, así como las cuencas y subcuencas hidrográficas. Cuando proceda, según lo definido en la Directiva 2000/60/CE del Parlamento Europeo y del Consejo, de 23 de octubre de 2000, por la que se establece un marco comunitario de actuación en el ámbito de la política de aguas (2), y en forma de redes.</skos:definition>
		<skos:prefLabel xml:lang="et">Hüdrograafia</skos:prefLabel>
		<skos:definition xml:lang="et">Hüdrograafilised objektid, sealhulgas merealad ning kõik muud veekogud ja nendega seotud objektid, sealhulgas vesikonnad ja alamvesikonnad. Kui see on asjakohane, vastavalt Euroopa Parlamendi ja nõukogu 23. oktoobri 2000. aasta direktiivis 2000/60/EÜ, millega kehtestatakse ühenduse veepoliitika alane tegevusraamistik (2) määratletule ning võrkude kujul.</skos:definition>
		<skos:prefLabel xml:lang="fi">Hydrografia</skos:prefLabel>
		<skos:definition xml:lang="fi">Hydrografiset elementit, mukaan luettuina merialueet ja kaikki muut vesimuodostumat ja niihin liittyvät kohteet, mukaan lukien vesistöalueet ja vesistöalueen osat. Tarvittaessa yhteisön vesipolitiikan puitteista 23 päivänä lokakuuta 2000 annetussa Euroopan parlamentin ja neuvoston direktiivissä 2000/60/EY (2) olevien määritelmien mukaan ja verkostomuodossa.</skos:definition>
		<skos:prefLabel xml:lang="fr">Hydrographie</skos:prefLabel>
		<skos:definition xml:lang="fr">Éléments hydrographiques, y compris les zones maritimes ainsi que toutes les autres masses d'eau et les éléments qui y sont liés, y compris les bassins et sous-bassins hydrographiques. Conformes, le cas échéant, aux définitions établies par la directive 2000/60/CE du Parlement européen et du Conseil du 23 octobre 2000 établissant un cadre pour une politique communautaire dans le domaine de l'eau (2) et sous forme de réseaux.</skos:definition>
		<skos:prefLabel xml:lang="hu">Vízrajz</skos:prefLabel>
		<skos:definition xml:lang="hu">Vízrajzi elemek, beleértve a tengeri területeket, minden egyéb víztestet és azzal kapcsolatos elemet, többek között a vízgyűjtőket és részvízgyűjtőket. Adott esetben a vízpolitika terén a közösségi fellépés kereteinek meghatározásáról szóló, 2000. október 23-i 2000/60/EK európai parlamenti és tanácsi irányelv (2) fogalommeghatározásaival összhangban és hálózati formában.</skos:definition>
		<skos:prefLabel xml:lang="it">Idrografia</skos:prefLabel>
		<skos:definition xml:lang="it">Elementi idrografici, comprese le zone marine e tutti gli altri corpi ed elementi idrici ad esse correlati, tra cui i bacini e sub bacini idrografici. Eventualmente in conformità delle definizioni contenute nella direttiva 2000/60/CE del Parlamento europeo e del Consiglio, del 23 ottobre 2000, che istituisce un quadro per l'azione comunitaria in materia di acque (2), e sotto forma di reti.</skos:definition>
		<skos:prefLabel xml:lang="lt">Hidrografija</skos:prefLabel>
		<skos:definition xml:lang="lt">Hidrografiniai elementai, įskaitant jūros zonas ir visus kitus vandens telkinius bei su jais susijusius elementus, įskaitant upių baseinus ir pabaseinius. Kur tikslinga, pagal 2000 m. spalio 23 d. Europos Parlamento ir Tarybos direktyvą 2000/60/EB, nustatančią Bendrijos veiksmų vandens politikos srityje pagrindus (2), ir tinklų pavidalu.</skos:definition>
		<skos:prefLabel xml:lang="lv">Hidrogrāfija</skos:prefLabel>
		<skos:definition xml:lang="lv">Hidrogrāfijas elementi, tostarp jūras teritorijas un visas citas ūdenstilpnes un ar tiem saistītie elementi, tostarp upju baseini un apakšbaseini. Attiecīgā gadījumā atbilstīgi definīcijām, kas izklāstītas Eiropas Parlamenta un Padomes Direktīvā 2000/60/EK (2000. gada 23. oktobris), ar ko izveido sistēmu Kopienas rīcībai ūdens resursu politikas jomā (2), un tīklu veidā.</skos:definition>
		
		<skos:prefLabel xml:lang="mt">Idrografija</skos:prefLabel>
		<skos:definition xml:lang="mt">Elementi idrografiċi, inklużi żoni marittimi, u kull korp ieħor ta' l-ilma u oġġetti relatati magħhom, inklużi baċiri taxxmajjar u sub-baċiri. Fejn xieraq, skond id-definizzjonijiet fid-Direttiva 2000/60/KE tal-Parlament Ewropew u tal- Kunsill tat-23 ta' Ottubru 2000 li tistabbilixxi qafas għall-azzjoni Komunitarja fil-qasam tal-politika ta' l-ilma (2) u filforma ta' networks.</skos:definition>		
		
		<skos:prefLabel xml:lang="nl">Hydrografie</skos:prefLabel>
		<skos:definition xml:lang="nl">Hydrografische elementen, waaronder mariene gebieden en alle andere waterlichamen en daarmee verband houdende elementen, met inbegrip van stroomgebieden en deelstroomgebieden, in voorkomend geval volgens de omschrijvingen vermeld in Richtlijn 2000/60/EG van het Europees Parlement en de Raad van 23 oktober 2000 tot vaststelling van een kader voor communautaire maatregelen betreffende het waterbeleid (2) en in de vorm van netwerken.</skos:definition>
		<skos:prefLabel xml:lang="pl">Hydrografia</skos:prefLabel>
		<skos:definition xml:lang="pl">Elementy hydrograficzne, w tym obszary morskie lub inne części wód oraz związane z nimi obiekty, łącznie z dorzeczami i zlewniami. W odpowiednich przypadkach zgodnie z definicjami zawartymi w dyrektywie 2000/60/WE Parlamentu Europejskiego i Rady z dnia 23 października 2000 r. ustanawiającej ramy wspólnotowego działania w dziedzinie polityki wodnej (2) oraz w formie sieci.</skos:definition>
		<skos:prefLabel xml:lang="pt">Hidrografia</skos:prefLabel>
		<skos:definition xml:lang="pt">Elementos hidrográficos, incluindo zonas marinhas e todas as outras massas de água e elementos com eles relacionados, incluindo bacias e sub-bacias hidrográficas. Quando adequado, de acordo com as definições da Directiva 2000/60/CE do Parlamento Europeu e do Conselho, de 23 de Outubro de 2000, que estabelece um quadro de acção comunitária no domínio da política da água (2), e sob a forma de redes.</skos:definition>
		<skos:prefLabel xml:lang="ro">Hidrografie</skos:prefLabel>
		<skos:definition xml:lang="ro">Elementele hidrografice, inclusiv zonele marine, precum şi toate celelalte corpuri de apă şi elementele legate de acestea, inclusiv bazinele şi sub-bazinele hidrografice. După caz, în conformitate cu definiţiile din Directiva 2000/60/CE a Parlamentului European şi a Consiliului din 23 octombrie 2000 de stabilire a unui cadru de politică comunitară în domeniul apei (2) şi sub formă de reţele.</skos:definition>
		<skos:prefLabel xml:lang="sk">Hydrografia</skos:prefLabel>
		<skos:definition xml:lang="sk">Hydrografické prvky vrátane morských oblastí a všetkých ostatných vodných útvarov a objektov vzťahujúcich sa k nim vrátane povodí riek a čiastkových povodí. Ak je to možné, v súlade s vymedzeniami pojmov ustanovenými v smernici Európskeho parlamentu a Rady 2000/60/ES z 23. októbra 2000, ktorou sa stanovuje rámec pôsobnosti pre opatrenia Spoločenstva v oblasti vodného hospodárstva (2), a v podobe sietí.</skos:definition>
		<skos:prefLabel xml:lang="sl">Hidrografija</skos:prefLabel>
		<skos:definition xml:lang="sl">Hidrografski elementi, ki vključujejo morska območja ter vsa druga vodna telesa in z njimi povezane dele, vključno s povodji in porečji. Po potrebi v skladu z opredelitvami v Direktivi 2000/60/ES Evropskega parlamenta in Sveta z dne 23. oktobra 2000 o določitvi okvira za ukrepe Skupnosti na področju vodne politike (2) in v obliki omrežij.</skos:definition>
		<skos:prefLabel xml:lang="sv">Hydrografi</skos:prefLabel>
		<skos:definition xml:lang="sv">Hydrografiska element, inbegripet havsområden och alla andra vattenförekomster och därtill hörande inslag, inbegripet avrinningsområden och delavrinningsområden. I förekommande fall i enlighet med definitionerna i Europaparlamentets och rådets direktiv 2000/60/EG av den 23 oktober 2000 om upprättande av en ram för gemenskapens åtgärder på vattenpolitikens område (2) och i form av nät.</skos:definition>
		<!--
		<skos:prefLabel xml:lang="el">SAMPLE ALTERNATIVE EXPRESSION - αναφορά</skos:prefLabel>
		<skos:definition xml:lang="el">Συστήματα συντεταγμένων</skos:definition>
		<dct:description xml:lang="el">Συστήματα για μονοσήμαντη αναφορά χωρικών πληροφοριών στον χώρο, ως σύνολο συντεταγμένων (x,y,z) ή/και γεωγραφικό πλάτος και μήκος και ύψος, με βάση γεωδαιτικό οριζόντιο και κατακόρυφο σύστημα αναφοράς (datum).</dct:description>
		-->
		<skos:inScheme rdf:resource="http://inspire-registry.jrc.ec.europa.eu/registers/Themes/items"/>
	</inspire:Theme>
	<inspire:SpatialObjectType rdf:about="http://inspire-registry.jrc.ec.europa.eu/registers/FCD/items/164">
		<inspire:itemStatus>valid</inspire:itemStatus>
		<inspire:dateAccepted>2009-01-22T15:06:36.745+01:00</inspire:dateAccepted>
		<skos:prefLabel xml:lang="en">Gazetteer</skos:prefLabel>
		<skos:definition xml:lang="en">directory of instances of location types in a spatial reference system</skos:definition>
		<dct:description xml:lang="en">n/a</dct:description>
		<skos:prefLabel xml:lang="el">SAMPLE ALTERNATIVE EXPRESSION - αναφορά</skos:prefLabel>
		<skos:definition xml:lang="el">Συστήματα συντεταγμένων</skos:definition>
		<dct:description xml:lang="el">Συστήματα για μονοσήμαντη αναφορά χωρικών πληροφοριών στον χώρο, ως σύνολο συντεταγμένων (x,y,z) ή/και γεωγραφικό πλάτος και μήκος και ύψος, με βάση γεωδαιτικό οριζόντιο και κατακόρυφο σύστημα αναφοράς (datum).</dct:description>
		<skos:inScheme rdf:resource="http://inspire-registry.jrc.ec.europa.eu/registers/FCD/items"/>
	</inspire:SpatialObjectType>
	<inspire:SpatialObjectType rdf:about="http://inspire-registry.jrc.ec.europa.eu/registers/FCD/items/165">
		<inspire:itemStatus>valid</inspire:itemStatus>
		<inspire:dateAccepted>2009-01-22T15:06:38.211+01:00</inspire:dateAccepted>
		<skos:prefLabel xml:lang="en">Location Instance</skos:prefLabel>
		<skos:definition xml:lang="en">identifiable place in the real world</skos:definition>
		<dct:description xml:lang="en">n/a</dct:description>
		<skos:prefLabel xml:lang="el">SAMPLE ALTERNATIVE EXPRESSION - αναφορά</skos:prefLabel>
		<skos:definition xml:lang="el">Συστήματα συντεταγμένων</skos:definition>
		<dct:description xml:lang="el">Συστήματα για μονοσήμαντη αναφορά χωρικών πληροφοριών στον χώρο, ως σύνολο συντεταγμένων (x,y,z) ή/και γεωγραφικό πλάτος και μήκος και ύψος, με βάση γεωδαιτικό οριζόντιο και κατακόρυφο σύστημα αναφοράς (datum).</dct:description>
		<skos:inScheme rdf:resource="http://inspire-registry.jrc.ec.europa.eu/registers/FCD/items"/>
	</inspire:SpatialObjectType>
	<inspire:SpatialObjectType rdf:about="http://inspire-registry.jrc.ec.europa.eu/registers/FCD/items/170">
		<inspire:itemStatus>valid</inspire:itemStatus>
		<inspire:dateAccepted>2009-01-22T15:06:56.946+01:00</inspire:dateAccepted>
		<skos:prefLabel xml:lang="en">Network</skos:prefLabel>
		<skos:definition xml:lang="en">collection of network elements</skos:definition>
		<dct:description xml:lang="en">The reason for collecting certain elements in a certain network may vary (e.g. connected elements for the same mode of transport).</dct:description>
		<skos:prefLabel xml:lang="el">SAMPLE ALTERNATIVE EXPRESSION - αναφορά</skos:prefLabel>
		<skos:definition xml:lang="el">Συστήματα συντεταγμένων</skos:definition>
		<dct:description xml:lang="el">Συστήματα για μονοσήμαντη αναφορά χωρικών πληροφοριών στον χώρο, ως σύνολο συντεταγμένων (x,y,z) ή/και γεωγραφικό πλάτος και μήκος και ύψος, με βάση γεωδαιτικό οριζόντιο και κατακόρυφο σύστημα αναφοράς (datum).</dct:description>
		<skos:inScheme rdf:resource="http://inspire-registry.jrc.ec.europa.eu/registers/FCD/items"/>
	</inspire:SpatialObjectType>
	<inspire:SpatialObjectType rdf:about="http://inspire-registry.jrc.ec.europa.eu/registers/FCD/items/179">
		<inspire:itemStatus>valid</inspire:itemStatus>
		<inspire:dateAccepted>2009-01-22T15:22:01.823+01:00</inspire:dateAccepted>
		<skos:prefLabel xml:lang="en">Access Restriction</skos:prefLabel>
		<skos:definition xml:lang="en">A restriction on the acces to a transport element.</skos:definition>
		<skos:prefLabel xml:lang="el">SAMPLE ALTERNATIVE EXPRESSION - αναφορά</skos:prefLabel>
		<skos:definition xml:lang="el">Συστήματα συντεταγμένων</skos:definition>
		<dct:description xml:lang="el">Συστήματα για μονοσήμαντη αναφορά χωρικών πληροφοριών στον χώρο, ως σύνολο συντεταγμένων (x,y,z) ή/και γεωγραφικό πλάτος και μήκος και ύψος, με βάση γεωδαιτικό οριζόντιο και κατακόρυφο σύστημα αναφοράς (datum).</dct:description>
		<skos:inScheme rdf:resource="http://inspire-registry.jrc.ec.europa.eu/registers/FCD/items"/>
	</inspire:SpatialObjectType>
	<inspire:SpatialObjectType rdf:about="http://inspire-registry.jrc.ec.europa.eu/registers/FCD/items/181">
		<inspire:itemStatus>valid</inspire:itemStatus>
		<inspire:dateAccepted>2009-01-22T15:22:04.801+01:00</inspire:dateAccepted>
		<skos:prefLabel xml:lang="en">Condition Of Facility</skos:prefLabel>
		<skos:definition xml:lang="en">State of a transport network element with regards to its completion and use.</skos:definition>
		<skos:prefLabel xml:lang="el">SAMPLE ALTERNATIVE EXPRESSION - αναφορά</skos:prefLabel>
		<skos:definition xml:lang="el">Συστήματα συντεταγμένων</skos:definition>
		<dct:description xml:lang="el">Συστήματα για μονοσήμαντη αναφορά χωρικών πληροφοριών στον χώρο, ως σύνολο συντεταγμένων (x,y,z) ή/και γεωγραφικό πλάτος και μήκος και ύψος, με βάση γεωδαιτικό οριζόντιο και κατακόρυφο σύστημα αναφοράς (datum).</dct:description>
		<skos:inScheme rdf:resource="http://inspire-registry.jrc.ec.europa.eu/registers/FCD/items"/>
	</inspire:SpatialObjectType>
	<inspire:SpatialObjectType rdf:about="http://inspire-registry.jrc.ec.europa.eu/registers/FCD/items/183">
		<inspire:itemStatus>valid</inspire:itemStatus>
		<inspire:dateAccepted>2009-01-22T15:22:05.236+01:00</inspire:dateAccepted>
		<skos:prefLabel xml:lang="en">Maintenance Authority</skos:prefLabel>
		<skos:definition xml:lang="en">The authority responsible for maintenance of the transport element.</skos:definition>
		<skos:prefLabel xml:lang="el">SAMPLE ALTERNATIVE EXPRESSION - αναφορά</skos:prefLabel>
		<skos:definition xml:lang="el">Συστήματα συντεταγμένων</skos:definition>
		<dct:description xml:lang="el">Συστήματα για μονοσήμαντη αναφορά χωρικών πληροφοριών στον χώρο, ως σύνολο συντεταγμένων (x,y,z) ή/και γεωγραφικό πλάτος και μήκος και ύψος, με βάση γεωδαιτικό οριζόντιο και κατακόρυφο σύστημα αναφοράς (datum).</dct:description>
		<skos:inScheme rdf:resource="http://inspire-registry.jrc.ec.europa.eu/registers/FCD/items"/>
	</inspire:SpatialObjectType>
	<inspire:SpatialObjectType rdf:about="http://inspire-registry.jrc.ec.europa.eu/registers/FCD/items/184">
		<inspire:itemStatus>valid</inspire:itemStatus>
		<inspire:dateAccepted>2009-01-22T15:22:05.459+01:00</inspire:dateAccepted>
		<skos:prefLabel xml:lang="en">Owner Authority</skos:prefLabel>
		<skos:definition xml:lang="en">The authority owning the transport element.</skos:definition>
		<skos:prefLabel xml:lang="el">SAMPLE ALTERNATIVE EXPRESSION - αναφορά</skos:prefLabel>
		<skos:definition xml:lang="el">Συστήματα συντεταγμένων</skos:definition>
		<dct:description xml:lang="el">Συστήματα για μονοσήμαντη αναφορά χωρικών πληροφοριών στον χώρο, ως σύνολο συντεταγμένων (x,y,z) ή/και γεωγραφικό πλάτος και μήκος και ύψος, με βάση γεωδαιτικό οριζόντιο και κατακόρυφο σύστημα αναφοράς (datum).</dct:description>
		<skos:inScheme rdf:resource="http://inspire-registry.jrc.ec.europa.eu/registers/FCD/items"/>
	</inspire:SpatialObjectType>
	<inspire:SpatialObjectType rdf:about="http://inspire-registry.jrc.ec.europa.eu/registers/FCD/items/185">
		<inspire:itemStatus>valid</inspire:itemStatus>
		<inspire:dateAccepted>2009-01-22T15:22:05.716+01:00</inspire:dateAccepted>
		<skos:prefLabel xml:lang="en">Restriction For Vehicles</skos:prefLabel>
		<skos:definition xml:lang="en">Restriction on vehicles on a transport element.</skos:definition>
		<skos:prefLabel xml:lang="el">SAMPLE ALTERNATIVE EXPRESSION - αναφορά</skos:prefLabel>
		<skos:definition xml:lang="el">Συστήματα συντεταγμένων</skos:definition>
		<dct:description xml:lang="el">Συστήματα για μονοσήμαντη αναφορά χωρικών πληροφοριών στον χώρο, ως σύνολο συντεταγμένων (x,y,z) ή/και γεωγραφικό πλάτος και μήκος και ύψος, με βάση γεωδαιτικό οριζόντιο και κατακόρυφο σύστημα αναφοράς (datum).</dct:description>
		<skos:inScheme rdf:resource="http://inspire-registry.jrc.ec.europa.eu/registers/FCD/items"/>
	</inspire:SpatialObjectType>
	<inspire:SpatialObjectType rdf:about="http://inspire-registry.jrc.ec.europa.eu/registers/FCD/items/189">
		<inspire:itemStatus>valid</inspire:itemStatus>
		<inspire:dateAccepted>2009-01-22T15:22:08.771+01:00</inspire:dateAccepted>
		<skos:prefLabel xml:lang="en">Transport Property</skos:prefLabel>
		<skos:definition xml:lang="en">A reference to a property that falls upon the network. This property can apply to the whole of the network element it is associated with or - for linear spatial objects - be described using linear referencing.</skos:definition>
		<skos:prefLabel xml:lang="el">SAMPLE ALTERNATIVE EXPRESSION - αναφορά</skos:prefLabel>
		<skos:definition xml:lang="el">Συστήματα συντεταγμένων</skos:definition>
		<dct:description xml:lang="el">Συστήματα για μονοσήμαντη αναφορά χωρικών πληροφοριών στον χώρο, ως σύνολο συντεταγμένων (x,y,z) ή/και γεωγραφικό πλάτος και μήκος και ύψος, με βάση γεωδαιτικό οριζόντιο και κατακόρυφο σύστημα αναφοράς (datum).</dct:description>
		<skos:inScheme rdf:resource="http://inspire-registry.jrc.ec.europa.eu/registers/FCD/items"/>
	</inspire:SpatialObjectType>
	<inspire:SpatialObjectType rdf:about="http://inspire-registry.jrc.ec.europa.eu/registers/FCD/items/190">
		<inspire:itemStatus>valid</inspire:itemStatus>
		<inspire:dateAccepted>2009-01-22T15:22:09.005+01:00</inspire:dateAccepted>
		<skos:prefLabel xml:lang="en">Form Of Way</skos:prefLabel>
		<skos:definition xml:lang="en">A classification based on the physical properties of the Road Link. [TWG TN, based on EuroRoadS]</skos:definition>
		<skos:prefLabel xml:lang="el">SAMPLE ALTERNATIVE EXPRESSION - αναφορά</skos:prefLabel>
		<skos:definition xml:lang="el">Συστήματα συντεταγμένων</skos:definition>
		<dct:description xml:lang="el">Συστήματα για μονοσήμαντη αναφορά χωρικών πληροφοριών στον χώρο, ως σύνολο συντεταγμένων (x,y,z) ή/και γεωγραφικό πλάτος και μήκος και ύψος, με βάση γεωδαιτικό οριζόντιο και κατακόρυφο σύστημα αναφοράς (datum).</dct:description>
		<skos:inScheme rdf:resource="http://inspire-registry.jrc.ec.europa.eu/registers/FCD/items"/>
	</inspire:SpatialObjectType>
	<inspire:SpatialObjectType rdf:about="http://inspire-registry.jrc.ec.europa.eu/registers/FCD/items/192">
		<inspire:itemStatus>valid</inspire:itemStatus>
		<inspire:dateAccepted>2009-01-22T15:22:10.875+01:00</inspire:dateAccepted>
		<skos:prefLabel xml:lang="en">Number Of Lanes</skos:prefLabel>
		<skos:definition xml:lang="en">The number of lanes of a road element.</skos:definition>
		<dct:description xml:lang="en">SOURCE Adapated from [Euroroads].</dct:description>
		<skos:prefLabel xml:lang="el">SAMPLE ALTERNATIVE EXPRESSION - αναφορά</skos:prefLabel>
		<skos:definition xml:lang="el">Συστήματα συντεταγμένων</skos:definition>
		<dct:description xml:lang="el">Συστήματα για μονοσήμαντη αναφορά χωρικών πληροφοριών στον χώρο, ως σύνολο συντεταγμένων (x,y,z) ή/και γεωγραφικό πλάτος και μήκος και ύψος, με βάση γεωδαιτικό οριζόντιο και κατακόρυφο σύστημα αναφοράς (datum).</dct:description>
		<skos:inScheme rdf:resource="http://inspire-registry.jrc.ec.europa.eu/registers/FCD/items"/>
	</inspire:SpatialObjectType>
	<inspire:SpatialObjectType rdf:about="http://inspire-registry.jrc.ec.europa.eu/registers/FCD/items/200">
		<inspire:itemStatus>valid</inspire:itemStatus>
		<inspire:dateAccepted>2009-01-22T15:22:15.360+01:00</inspire:dateAccepted>
		<skos:prefLabel xml:lang="en">Speed Limit</skos:prefLabel>
		<skos:definition xml:lang="en">Limit for the speed of a vehicle on a road.</skos:definition>
		<dct:description xml:lang="en">SOURCE [Euroroads].</dct:description>
		<skos:prefLabel xml:lang="el">SAMPLE ALTERNATIVE EXPRESSION - αναφορά</skos:prefLabel>
		<skos:definition xml:lang="el">Συστήματα συντεταγμένων</skos:definition>
		<dct:description xml:lang="el">Συστήματα για μονοσήμαντη αναφορά χωρικών πληροφοριών στον χώρο, ως σύνολο συντεταγμένων (x,y,z) ή/και γεωγραφικό πλάτος και μήκος και ύψος, με βάση γεωδαιτικό οριζόντιο και κατακόρυφο σύστημα αναφοράς (datum).</dct:description>
		<skos:inScheme rdf:resource="http://inspire-registry.jrc.ec.europa.eu/registers/FCD/items"/>
	</inspire:SpatialObjectType>
	<inspire:SpatialObjectType rdf:about="http://inspire-registry.jrc.ec.europa.eu/registers/FCD/items/211">
		<inspire:itemStatus>valid</inspire:itemStatus>
		<inspire:dateAccepted>2009-01-22T15:22:20.338+01:00</inspire:dateAccepted>
		<skos:prefLabel xml:lang="en">Railway Station Node</skos:prefLabel>
		<skos:definition xml:lang="en">A railway node which represents the location of a railway station along the railway network.</skos:definition>
		<skos:prefLabel xml:lang="el">SAMPLE ALTERNATIVE EXPRESSION - αναφορά</skos:prefLabel>
		<skos:definition xml:lang="el">Συστήματα συντεταγμένων</skos:definition>
		<dct:description xml:lang="el">Συστήματα για μονοσήμαντη αναφορά χωρικών πληροφοριών στον χώρο, ως σύνολο συντεταγμένων (x,y,z) ή/και γεωγραφικό πλάτος και μήκος και ύψος, με βάση γεωδαιτικό οριζόντιο και κατακόρυφο σύστημα αναφοράς (datum).</dct:description>
		<skos:inScheme rdf:resource="http://inspire-registry.jrc.ec.europa.eu/registers/FCD/items"/>
	</inspire:SpatialObjectType>
	<inspire:SpatialObjectType rdf:about="http://inspire-registry.jrc.ec.europa.eu/registers/FCD/items/251">
		<inspire:itemStatus>valid</inspire:itemStatus>
		<inspire:dateAccepted>2009-01-22T16:00:14.796+01:00</inspire:dateAccepted>
		<skos:prefLabel xml:lang="en">Named Place</skos:prefLabel>
		<skos:definition xml:lang="en">Any real world entity referred to by one or several proper nouns.</skos:definition>
		<skos:prefLabel xml:lang="el">SAMPLE ALTERNATIVE EXPRESSION - αναφορά</skos:prefLabel>
		<skos:definition xml:lang="el">Συστήματα συντεταγμένων</skos:definition>
		<dct:description xml:lang="el">Συστήματα για μονοσήμαντη αναφορά χωρικών πληροφοριών στον χώρο, ως σύνολο συντεταγμένων (x,y,z) ή/και γεωγραφικό πλάτος και μήκος και ύψος, με βάση γεωδαιτικό οριζόντιο και κατακόρυφο σύστημα αναφοράς (datum).</dct:description>
		<skos:inScheme rdf:resource="http://inspire-registry.jrc.ec.europa.eu/registers/FCD/items"/>
	</inspire:SpatialObjectType>
	<inspire:SpatialObjectType rdf:about="http://inspire-registry.jrc.ec.europa.eu/registers/FCD/items/252">
		<inspire:itemStatus>valid</inspire:itemStatus>
		<inspire:dateAccepted>2009-01-22T16:00:52.211+01:00</inspire:dateAccepted>
		<skos:prefLabel xml:lang="en">Administrative unit</skos:prefLabel>
		<skos:definition xml:lang="en">Unit of administration where a Member State has and/or exercises jurisdictional rights, for local, regional and national governance.</skos:definition>
		<skos:prefLabel xml:lang="el">SAMPLE ALTERNATIVE EXPRESSION - αναφορά</skos:prefLabel>
		<skos:definition xml:lang="el">Συστήματα συντεταγμένων</skos:definition>
		<dct:description xml:lang="el">Συστήματα για μονοσήμαντη αναφορά χωρικών πληροφοριών στον χώρο, ως σύνολο συντεταγμένων (x,y,z) ή/και γεωγραφικό πλάτος και μήκος και ύψος, με βάση γεωδαιτικό οριζόντιο και κατακόρυφο σύστημα αναφοράς (datum).</dct:description>
		<skos:inScheme rdf:resource="http://inspire-registry.jrc.ec.europa.eu/registers/FCD/items"/>
	</inspire:SpatialObjectType>
	<inspire:SpatialObjectType rdf:about="http://inspire-registry.jrc.ec.europa.eu/registers/FCD/items/255">
		<inspire:itemStatus>valid</inspire:itemStatus>
		<inspire:dateAccepted>2009-01-22T16:00:53.563+01:00</inspire:dateAccepted>
		<skos:prefLabel xml:lang="en">Administrative boundary</skos:prefLabel>
		<skos:definition xml:lang="en">A line of demarcation between administratively controlled areas (administrative units).</skos:definition>
		<skos:prefLabel xml:lang="el">SAMPLE ALTERNATIVE EXPRESSION - αναφορά</skos:prefLabel>
		<skos:definition xml:lang="el">Συστήματα συντεταγμένων</skos:definition>
		<dct:description xml:lang="el">Συστήματα για μονοσήμαντη αναφορά χωρικών πληροφοριών στον χώρο, ως σύνολο συντεταγμένων (x,y,z) ή/και γεωγραφικό πλάτος και μήκος και ύψος, με βάση γεωδαιτικό οριζόντιο και κατακόρυφο σύστημα αναφοράς (datum).</dct:description>
		<skos:inScheme rdf:resource="http://inspire-registry.jrc.ec.europa.eu/registers/FCD/items"/>
	</inspire:SpatialObjectType>
	<inspire:SpatialObjectType rdf:about="http://inspire-registry.jrc.ec.europa.eu/registers/FCD/items/262">
		<inspire:itemStatus>valid</inspire:itemStatus>
		<inspire:dateAccepted>2010-01-13T16:54:34.425+01:00</inspire:dateAccepted>
		<skos:prefLabel xml:lang="en">Habitat (Habitats and Biotopes)</skos:prefLabel>
		<skos:definition xml:lang="en">Geographical areas characterised by specific ecological conditions, processes, structure and (life support) functions that physically support the organisms that live there.</skos:definition>
		<dct:description xml:lang="en">Includes terrestrial and aquatic areas distinguished by geographical, abiotic and biotic features, whether entirely natural or semi-natural.
NOTE Many other attributes may be added to this class when the theme is properly developed as part of Annex III. Currently, only those attributes needed to support the Protected Sites theme in Annex I are included.
Package: Habitats and Biotopes [Candidate type that might be extended in Annex II/III INSPIRE data specification].</dct:description>
		<skos:prefLabel xml:lang="el">SAMPLE ALTERNATIVE EXPRESSION - αναφορά</skos:prefLabel>
		<skos:definition xml:lang="el">Συστήματα συντεταγμένων</skos:definition>
		<dct:description xml:lang="el">Συστήματα για μονοσήμαντη αναφορά χωρικών πληροφοριών στον χώρο, ως σύνολο συντεταγμένων (x,y,z) ή/και γεωγραφικό πλάτος και μήκος και ύψος, με βάση γεωδαιτικό οριζόντιο και κατακόρυφο σύστημα αναφοράς (datum).</dct:description>
		<skos:inScheme rdf:resource="http://inspire-registry.jrc.ec.europa.eu/registers/FCD/items"/>
	</inspire:SpatialObjectType>
	<inspire:SpatialObjectType rdf:about="http://inspire-registry.jrc.ec.europa.eu/registers/FCD/items/263">
		<inspire:itemStatus>valid</inspire:itemStatus>
		<inspire:dateAccepted>2010-01-13T16:54:34.673+01:00</inspire:dateAccepted>
		<skos:prefLabel xml:lang="en">Species Aggregation Unit (Species Distribution)</skos:prefLabel>
		<skos:definition xml:lang="en">The aggregation unit over which the species is distributed.</skos:definition>
		<dct:description xml:lang="en">This model only includes ProtectedSite as an aggregation unit, but others may be added in the future (for example, administrative units and grid units).
Candidate type that might be extended in Annex II/III INSPIRE data specification.</dct:description>
		<skos:prefLabel xml:lang="el">SAMPLE ALTERNATIVE EXPRESSION - αναφορά</skos:prefLabel>
		<skos:definition xml:lang="el">Συστήματα συντεταγμένων</skos:definition>
		<dct:description xml:lang="el">Συστήματα για μονοσήμαντη αναφορά χωρικών πληροφοριών στον χώρο, ως σύνολο συντεταγμένων (x,y,z) ή/και γεωγραφικό πλάτος και μήκος και ύψος, με βάση γεωδαιτικό οριζόντιο και κατακόρυφο σύστημα αναφοράς (datum).</dct:description>
		<skos:inScheme rdf:resource="http://inspire-registry.jrc.ec.europa.eu/registers/FCD/items"/>
	</inspire:SpatialObjectType>
	<inspire:SpatialObjectType rdf:about="http://inspire-registry.jrc.ec.europa.eu/registers/FCD/items/264">
		<inspire:itemStatus>valid</inspire:itemStatus>
		<inspire:dateAccepted>2010-01-13T16:54:34.946+01:00</inspire:dateAccepted>
		<skos:prefLabel xml:lang="en">Species Distribution (Species Distribution)</skos:prefLabel>
		<skos:definition xml:lang="en">The geographical distribution of occurrence of animal or plant species aggregated by grid, region, administrative unit or other analytical unit.</skos:definition>
		<dct:description xml:lang="en">NOTE Many other attributes may be added to this class when the theme is properly developed as part of Annex III. Currently, only those attributes needed to support the Protected Sites theme in Annex I are included.
Package: Species Distribution [Candidate type that might be extended in Annex II/III INSPIRE data specification]</dct:description>
		<skos:prefLabel xml:lang="el">SAMPLE ALTERNATIVE EXPRESSION - αναφορά</skos:prefLabel>
		<skos:definition xml:lang="el">Συστήματα συντεταγμένων</skos:definition>
		<dct:description xml:lang="el">Συστήματα για μονοσήμαντη αναφορά χωρικών πληροφοριών στον χώρο, ως σύνολο συντεταγμένων (x,y,z) ή/και γεωγραφικό πλάτος και μήκος και ύψος, με βάση γεωδαιτικό οριζόντιο και κατακόρυφο σύστημα αναφοράς (datum).</dct:description>
		<skos:inScheme rdf:resource="http://inspire-registry.jrc.ec.europa.eu/registers/FCD/items"/>
	</inspire:SpatialObjectType>
	<inspire:SpatialObjectType rdf:about="http://inspire-registry.jrc.ec.europa.eu/registers/FCD/items/265">
		<inspire:itemStatus>valid</inspire:itemStatus>
		<inspire:dateAccepted>2010-01-12T18:32:26.537+01:00</inspire:dateAccepted>
		<skos:prefLabel xml:lang="en">Address</skos:prefLabel>
		<skos:definition xml:lang="en">An identification of the fixed location of property by means of a structured composition of geographic names and identifiers.</skos:definition>
		<dct:description xml:lang="en">NOTE 1 The spatial object, referenced by the address, is defined as the "addressable object". The addressable object is not within the application schema, but it is possible to represent the address' reference to a cadastral parcel or a building through associations. It should, however, be noted that in different countries and regions, different traditions and/or regulations determine which object types should be regarded as addressable objects. 

NOTE 2 In most situations the addressable objects are current, real world objects. However, addresses may also reference objects which are planned, under construction or even historical.

NOTE 3 Apart from the identification of the addressable objects (like e.g. buildings), addresses are very often used by a large number of other applications to identify object types e.g. statistics of the citizens living in the building, for taxation of the business entities that occupy the building, and the utility installations. 

NOTE 4 For different purposes, the identification of an address can be represented  in different ways (see example s 2 and 3). 

EXAMPLE 1 A property can e.g., be a plot of land, building, part of building, way of access or other construction,

EXAMPLE 2 In the Netherlands the primary addressable objects are buildings and dwellings which may include parts of buildings, mooring places or places for the permanent placement of trailers (mobile homes), in the UK it is the lowest level of unit for the delivery of services, in the Czech Republic it is buildings and entrance doors. 

EXAMPLE 3 Addresses can be represented differently. In a human readable form an address in Spain and an address in Denmark could be represented like this: "Calle Mayor, 13, Cortijo del Marqués, 41037 Écija, Sevilla, España" or "Wildersgade 60A, st. th, 1408 Copenhagen K., Denmark".</dct:description>
		<skos:prefLabel xml:lang="el">SAMPLE ALTERNATIVE EXPRESSION - αναφορά</skos:prefLabel>
		<skos:definition xml:lang="el">Συστήματα συντεταγμένων</skos:definition>
		<dct:description xml:lang="el">Συστήματα για μονοσήμαντη αναφορά χωρικών πληροφοριών στον χώρο, ως σύνολο συντεταγμένων (x,y,z) ή/και γεωγραφικό πλάτος και μήκος και ύψος, με βάση γεωδαιτικό οριζόντιο και κατακόρυφο σύστημα αναφοράς (datum).</dct:description>
		<skos:inScheme rdf:resource="http://inspire-registry.jrc.ec.europa.eu/registers/FCD/items"/>
	</inspire:SpatialObjectType>
	<inspire:SpatialObjectType rdf:about="http://inspire-registry.jrc.ec.europa.eu/registers/FCD/items/266">
		<inspire:itemStatus>valid</inspire:itemStatus>
		<inspire:dateAccepted>2010-01-12T18:32:26.974+01:00</inspire:dateAccepted>
		<skos:prefLabel xml:lang="en">Address Area Name</skos:prefLabel>
		<skos:definition xml:lang="en">An address component which represents the name of a geographic area or locality that groups a number of addressable objects for addressing purposes, without being an administrative unit.</skos:definition>
		<dct:description xml:lang="en">NOTE 1 In some countries and regions an address area is a true subdivision of an administrative unit (most often a municipality), so that every address area is fully inside the municipality and so that every part of the municipality is within an address area. In other countries, the concept of address area names is less strict and based on local tradition or specific needs. 

NOTE 2 In some situations an address area name is not required to obtain unambiguousness; instead the purpose is to make the complete address more informative and descriptive, adding a well known place name (e.g. of a village or community) to the address. This is particularly useful if the municipality or post code covers a large area. 

EXAMPLE 1 In Sweden a "Kommundel" (en: Municipal sub division) is a type of address area names that ensures that street names are unique within the sub division. 

EXAMPLE 2 In Spain an "Entidad de población" (en: population entity) has the same function. It is the general address area which depending on its characteristics can be classified as "Entidad Singular" (en: singular entity) or "Entidad Colectiva" (en: collective entity). Moreover, according to the population distribution, these areas can contain one or several "Núcleo de población" (en: population core) and/or "Población diseminada" (en:scattered population).

EXAMPLE 3 In Denmark "Supplerende bynavn" (en: Supplementary town name) is sometimes compulsory to ensure uniqueness of street names within the post code, sometimes it is just useful extra information, that makes the address more informative.</dct:description>
		<skos:prefLabel xml:lang="el">SAMPLE ALTERNATIVE EXPRESSION - αναφορά</skos:prefLabel>
		<skos:definition xml:lang="el">Συστήματα συντεταγμένων</skos:definition>
		<dct:description xml:lang="el">Συστήματα για μονοσήμαντη αναφορά χωρικών πληροφοριών στον χώρο, ως σύνολο συντεταγμένων (x,y,z) ή/και γεωγραφικό πλάτος και μήκος και ύψος, με βάση γεωδαιτικό οριζόντιο και κατακόρυφο σύστημα αναφοράς (datum).</dct:description>
		<skos:inScheme rdf:resource="http://inspire-registry.jrc.ec.europa.eu/registers/FCD/items"/>
	</inspire:SpatialObjectType>
	<inspire:SpatialObjectType rdf:about="http://inspire-registry.jrc.ec.europa.eu/registers/FCD/items/267">
		<inspire:itemStatus>valid</inspire:itemStatus>
		<inspire:dateAccepted>2010-01-12T18:32:27.434+01:00</inspire:dateAccepted>
		<skos:prefLabel xml:lang="en">Address Component</skos:prefLabel>
		<skos:definition xml:lang="en">Identifier or geographic name of a specific geographic area, location, or other spatial object which defines the scope of an address.</skos:definition>
		<dct:description xml:lang="en">NOTE 1 Four different subclasses of address components are defined: 
o    Administrative unit name, which may include name of country, name of municipality, name of district
o    Address area name like e.g. name of village or settlement 
o    Thoroughfare name, most often road name  
o    Postal descriptor 
In order to construct an address, these subclasses are often structured hierarchically.

NOTE 2 It is the combination of the address locator and the address components, which makes a specific address spatial object readable and unambiguous for the human user. 

EXAMPLE The combination of the locator "13" and the address components "Calle Mayor" (thoroughfare name), "Cortijo del Marqués" (address area name), "41037" (postal descriptor), "Écija", "Sevilla" and "España" (administrative unit names) makes this specific address spatial object readable and unambiguous.</dct:description>
		<skos:prefLabel xml:lang="el">SAMPLE ALTERNATIVE EXPRESSION - αναφορά</skos:prefLabel>
		<skos:definition xml:lang="el">Συστήματα συντεταγμένων</skos:definition>
		<dct:description xml:lang="el">Συστήματα για μονοσήμαντη αναφορά χωρικών πληροφοριών στον χώρο, ως σύνολο συντεταγμένων (x,y,z) ή/και γεωγραφικό πλάτος και μήκος και ύψος, με βάση γεωδαιτικό οριζόντιο και κατακόρυφο σύστημα αναφοράς (datum).</dct:description>
		<skos:inScheme rdf:resource="http://inspire-registry.jrc.ec.europa.eu/registers/FCD/items"/>
	</inspire:SpatialObjectType>
	<inspire:SpatialObjectType rdf:about="http://inspire-registry.jrc.ec.europa.eu/registers/FCD/items/268">
		<inspire:itemStatus>valid</inspire:itemStatus>
		<inspire:dateAccepted>2010-01-12T18:32:27.542+01:00</inspire:dateAccepted>
		<skos:prefLabel xml:lang="en">Administrative Unit Name</skos:prefLabel>
		<skos:definition xml:lang="en">An address component which represents the name of a unit of administration where a Member State has and/or exercises jurisdictional rights, for local, regional and national governance.</skos:definition>
		<skos:prefLabel xml:lang="el">SAMPLE ALTERNATIVE EXPRESSION - αναφορά</skos:prefLabel>
		<skos:definition xml:lang="el">Συστήματα συντεταγμένων</skos:definition>
		<dct:description xml:lang="el">Συστήματα για μονοσήμαντη αναφορά χωρικών πληροφοριών στον χώρο, ως σύνολο συντεταγμένων (x,y,z) ή/και γεωγραφικό πλάτος και μήκος και ύψος, με βάση γεωδαιτικό οριζόντιο και κατακόρυφο σύστημα αναφοράς (datum).</dct:description>
		<skos:inScheme rdf:resource="http://inspire-registry.jrc.ec.europa.eu/registers/FCD/items"/>
	</inspire:SpatialObjectType>
	<inspire:SpatialObjectType rdf:about="http://inspire-registry.jrc.ec.europa.eu/registers/FCD/items/269">
		<inspire:itemStatus>valid</inspire:itemStatus>
		<inspire:dateAccepted>2010-01-12T18:32:28.021+01:00</inspire:dateAccepted>
		<skos:prefLabel xml:lang="en">Postal Descriptor</skos:prefLabel>
		<skos:definition xml:lang="en">An address component which represents the identification of a subdivision of addresses and postal delivery points in a country, region or city for postal purposes.</skos:definition>
		<dct:description xml:lang="en">NOTE 1 The postal descriptor is specified by means of a post code and/or names of the associated post office, town or area.

NOTE 2 In some countries post codes are seen as a proper geographic subdivision of the country, in other countries the post code is regarded only as an attribute that characterizes a (usually small) number of adjacent postal delivery points and addresses. 

NOTE 3 The postal descriptors are created and developed on the basis of postal requirements (e.g. efficient sorting, logistics, transport and distribution). Consequently, there is not often  a tight relationship between the postal areas and administrative units in the same area.

NOTE 4 The structure schema and formats of national postal descriptor systems are different. Sometimes (for example  in the UK) the post code itself is the only information required for a valid address; in other situations both the post code and the associated name of post office or town is required. Sometimes there is a simple 11 relationship between the code and the name; in other situations a set of postcodes are associated with a single post office or town.

NOTE 5 In some countries like e.g. The Republic of Ireland, no post code system currently exists, therefore the postal descriptor is only represented by the name of the post town. 

EXAMPLE 1 In the UK the post code "EC4M 7DR" is sufficient, as a postal descriptor, while the related town name "London" is informative, but not necessary in the postal address. 

EXAMPLE 2 In Sweden all postcodes starting with "80" is related to the postal name "Gävle". Therefore in the postal descriptor "802 74 Gävle", the postcode "802 74" bears all postal necessary information, while the town name "Gävle" is extra information. 

EXAMPLE 3 In Denmark, outside the centre of Copenhagen, each postcode has a 1:1 relationship to one post name only: Postcode "6372" relates to the village "Bylderup-Bov". 

EXAMPLE 4 In Germany the lowest level of the Postal descriptor (the 5 digit Postleitzahl) often does not fall within an administrative unit (e.g. municipality). The Postleitzahl is handled completely independent from the hierarchal systematic of the addresses. In addition, some "Postleitzahlen" represent not a delivery area, but institutions with a big amount of post.</dct:description>
		<skos:prefLabel xml:lang="el">SAMPLE ALTERNATIVE EXPRESSION - αναφορά</skos:prefLabel>
		<skos:definition xml:lang="el">Συστήματα συντεταγμένων</skos:definition>
		<dct:description xml:lang="el">Συστήματα για μονοσήμαντη αναφορά χωρικών πληροφοριών στον χώρο, ως σύνολο συντεταγμένων (x,y,z) ή/και γεωγραφικό πλάτος και μήκος και ύψος, με βάση γεωδαιτικό οριζόντιο και κατακόρυφο σύστημα αναφοράς (datum).</dct:description>
		<skos:inScheme rdf:resource="http://inspire-registry.jrc.ec.europa.eu/registers/FCD/items"/>
	</inspire:SpatialObjectType>
	<inspire:SpatialObjectType rdf:about="http://inspire-registry.jrc.ec.europa.eu/registers/FCD/items/270">
		<inspire:itemStatus>valid</inspire:itemStatus>
		<inspire:dateAccepted>2010-01-12T18:32:28.425+01:00</inspire:dateAccepted>
		<skos:prefLabel xml:lang="en">Thoroughfare Name</skos:prefLabel>
		<skos:definition xml:lang="en">An address component which represents the name of a passage or way through from one location to another.</skos:definition>
		<dct:description xml:lang="en">NOTE 1 A thoroughfare can, e.g., be a road or a waterway

NOTE 2 Thoroughfare names includes names of squares and of cul de sacs, and they can also represent the network of smaller roads or paths e.g. in a small village or settlement.</dct:description>
		<skos:prefLabel xml:lang="el">SAMPLE ALTERNATIVE EXPRESSION - αναφορά</skos:prefLabel>
		<skos:definition xml:lang="el">Συστήματα συντεταγμένων</skos:definition>
		<dct:description xml:lang="el">Συστήματα για μονοσήμαντη αναφορά χωρικών πληροφοριών στον χώρο, ως σύνολο συντεταγμένων (x,y,z) ή/και γεωγραφικό πλάτος και μήκος και ύψος, με βάση γεωδαιτικό οριζόντιο και κατακόρυφο σύστημα αναφοράς (datum).</dct:description>
		<skos:inScheme rdf:resource="http://inspire-registry.jrc.ec.europa.eu/registers/FCD/items"/>
	</inspire:SpatialObjectType>
	<inspire:SpatialObjectType rdf:about="http://inspire-registry.jrc.ec.europa.eu/registers/FCD/items/271">
		<inspire:itemStatus>valid</inspire:itemStatus>
		<inspire:dateAccepted>2010-01-12T18:35:01.379+01:00</inspire:dateAccepted>
		<skos:prefLabel xml:lang="en">NUTS region</skos:prefLabel>
		<skos:definition xml:lang="en">Territorial unit for statistics defined in the framework of the Regulation (EC) No 1059/2003 of the European Parliament and of the Council of 26 May 2003.</skos:definition>
		<dct:description xml:lang="en">NOTE 1 NUTS regions subdivide each Member State into a whole number of territorial units for statistic at NUTS1 level. Each of these is then subdivided into regions at NUTS2 level and these in turn into regions at NUTS3 level.
NOTE 2 This type is a candidate type to be considered by the spatial data theme Statistical units in Annex III to Directive 2007/2/EC.</dct:description>
		<skos:prefLabel xml:lang="el">SAMPLE ALTERNATIVE EXPRESSION - αναφορά</skos:prefLabel>
		<skos:definition xml:lang="el">Συστήματα συντεταγμένων</skos:definition>
		<dct:description xml:lang="el">Συστήματα για μονοσήμαντη αναφορά χωρικών πληροφοριών στον χώρο, ως σύνολο συντεταγμένων (x,y,z) ή/και γεωγραφικό πλάτος και μήκος και ύψος, με βάση γεωδαιτικό οριζόντιο και κατακόρυφο σύστημα αναφοράς (datum).</dct:description>
		<skos:inScheme rdf:resource="http://inspire-registry.jrc.ec.europa.eu/registers/FCD/items"/>
	</inspire:SpatialObjectType>
	<inspire:SpatialObjectType rdf:about="http://inspire-registry.jrc.ec.europa.eu/registers/FCD/items/272">
		<inspire:itemStatus>valid</inspire:itemStatus>
		<inspire:dateAccepted>2010-01-12T18:35:01.605+01:00</inspire:dateAccepted>
		<skos:prefLabel xml:lang="en">Condominium</skos:prefLabel>
		<skos:definition xml:lang="en">An administrative area established independently to any national administrative division of territory and administered by two or more countries.</skos:definition>
		<dct:description xml:lang="en">NOTE Condominium is not a part of any national administrative hierarchy of territory division in Member State.</dct:description>
		<skos:prefLabel xml:lang="el">SAMPLE ALTERNATIVE EXPRESSION - αναφορά</skos:prefLabel>
		<skos:definition xml:lang="el">Συστήματα συντεταγμένων</skos:definition>
		<dct:description xml:lang="el">Συστήματα για μονοσήμαντη αναφορά χωρικών πληροφοριών στον χώρο, ως σύνολο συντεταγμένων (x,y,z) ή/και γεωγραφικό πλάτος και μήκος και ύψος, με βάση γεωδαιτικό οριζόντιο και κατακόρυφο σύστημα αναφοράς (datum).</dct:description>
		<skos:inScheme rdf:resource="http://inspire-registry.jrc.ec.europa.eu/registers/FCD/items"/>
	</inspire:SpatialObjectType>
	<inspire:SpatialObjectType rdf:about="http://inspire-registry.jrc.ec.europa.eu/registers/FCD/items/273">
		<inspire:itemStatus>valid</inspire:itemStatus>
		<inspire:dateAccepted>2010-01-12T18:40:32.343+01:00</inspire:dateAccepted>
		<skos:prefLabel xml:lang="en">Basic Property Unit</skos:prefLabel>
		<skos:definition xml:lang="en">The basic unit of ownership that is recorded in the land books, land registers or equivalent. It is defined by unique ownership and homogeneous real property rights, and may consist of one or more adjacent or geographically separate parcels.</skos:definition>
		<dct:description xml:lang="en">SOURCE Adapted from UN ECE 2004.
NOTE 1 In the INSPIRE context, basic property units are to be made available by Member States where unique cadastral references are given only for basic property units and not for parcels.
NOTE 2 In many (but not all) countries, the area of the basic property unit corresponds to the cadastral parcel itself.
NOTE 3 Some countries, such as Finland, may also register officially basic property units without any area. These basic property units are considered out of the INSPIRE scope.
NOTE 4 Some countries, such as Norway, may have parcels which belong to several basic property units.</dct:description>
		<skos:prefLabel xml:lang="el">SAMPLE ALTERNATIVE EXPRESSION - αναφορά</skos:prefLabel>
		<skos:definition xml:lang="el">Συστήματα συντεταγμένων</skos:definition>
		<dct:description xml:lang="el">Συστήματα για μονοσήμαντη αναφορά χωρικών πληροφοριών στον χώρο, ως σύνολο συντεταγμένων (x,y,z) ή/και γεωγραφικό πλάτος και μήκος και ύψος, με βάση γεωδαιτικό οριζόντιο και κατακόρυφο σύστημα αναφοράς (datum).</dct:description>
		<skos:inScheme rdf:resource="http://inspire-registry.jrc.ec.europa.eu/registers/FCD/items"/>
	</inspire:SpatialObjectType>
	<inspire:SpatialObjectType rdf:about="http://inspire-registry.jrc.ec.europa.eu/registers/FCD/items/274">
		<inspire:itemStatus>valid</inspire:itemStatus>
		<inspire:dateAccepted>2010-01-12T18:40:32.635+01:00</inspire:dateAccepted>
		<skos:prefLabel xml:lang="en">Cadastral Boundary</skos:prefLabel>
		<skos:definition xml:lang="en">Part of the outline of a cadastral parcel. One cadastral boundary may be shared by two neighbouring cadastral parcels.</skos:definition>
		<dct:description xml:lang="en">NOTE In the INSPIRE context, cadastral boundaries are to be made available by Member States where absolute positional accuracy information is recorded for the cadastral boundary (attribute estimated accuracy).</dct:description>
		<skos:prefLabel xml:lang="el">SAMPLE ALTERNATIVE EXPRESSION - αναφορά</skos:prefLabel>
		<skos:definition xml:lang="el">Συστήματα συντεταγμένων</skos:definition>
		<dct:description xml:lang="el">Συστήματα για μονοσήμαντη αναφορά χωρικών πληροφοριών στον χώρο, ως σύνολο συντεταγμένων (x,y,z) ή/και γεωγραφικό πλάτος και μήκος και ύψος, με βάση γεωδαιτικό οριζόντιο και κατακόρυφο σύστημα αναφοράς (datum).</dct:description>
		<skos:inScheme rdf:resource="http://inspire-registry.jrc.ec.europa.eu/registers/FCD/items"/>
	</inspire:SpatialObjectType>
	<inspire:SpatialObjectType rdf:about="http://inspire-registry.jrc.ec.europa.eu/registers/FCD/items/275">
		<inspire:itemStatus>valid</inspire:itemStatus>
		<inspire:dateAccepted>2010-01-12T18:40:37.571+01:00</inspire:dateAccepted>
		<skos:prefLabel xml:lang="en">Cadastral Parcel</skos:prefLabel>
		<skos:definition xml:lang="en">Areas defined by cadastral registers or equivalent.</skos:definition>
		<dct:description xml:lang="en">SOURCE [INSPIRE Directive:2007].
NOTE As much as possible, in the INSPIRE context, cadastral parcels should be forming a partition of national territory. Cadastral parcel should be considered as a single area of Earth surface (land and/or water), under homogeneous real property rights and unique ownership, real property rights and ownership being defined by national law (adapted from UN ECE 2004 and WG-CPI, 2006). By unique ownership is meant that the ownership is held by one or several joint owners for the whole parcel.</dct:description>
		<skos:prefLabel xml:lang="el">SAMPLE ALTERNATIVE EXPRESSION - αναφορά</skos:prefLabel>
		<skos:definition xml:lang="el">Συστήματα συντεταγμένων</skos:definition>
		<dct:description xml:lang="el">Συστήματα για μονοσήμαντη αναφορά χωρικών πληροφοριών στον χώρο, ως σύνολο συντεταγμένων (x,y,z) ή/και γεωγραφικό πλάτος και μήκος και ύψος, με βάση γεωδαιτικό οριζόντιο και κατακόρυφο σύστημα αναφοράς (datum).</dct:description>
		<skos:inScheme rdf:resource="http://inspire-registry.jrc.ec.europa.eu/registers/FCD/items"/>
	</inspire:SpatialObjectType>
	<inspire:SpatialObjectType rdf:about="http://inspire-registry.jrc.ec.europa.eu/registers/FCD/items/276">
		<inspire:itemStatus>valid</inspire:itemStatus>
		<inspire:dateAccepted>2010-01-12T18:40:37.793+01:00</inspire:dateAccepted>
		<skos:prefLabel xml:lang="en">Cadastral Zoning</skos:prefLabel>
		<skos:definition xml:lang="en">Intermediary areas used in order to divide national territory into cadastral parcels.</skos:definition>
		<dct:description xml:lang="en">NOTE 1 In the INSPIRE context, cadastral zonings are to be used to carry metadata information and to facilitate portrayal and search of data.
NOTE 2 Cadastral zonings have generally been defined when cadastral maps were created for the first time.
EXAMPLE Municipality, section, parish, district, block.</dct:description>
		<skos:prefLabel xml:lang="el">SAMPLE ALTERNATIVE EXPRESSION - αναφορά</skos:prefLabel>
		<skos:definition xml:lang="el">Συστήματα συντεταγμένων</skos:definition>
		<dct:description xml:lang="el">Συστήματα για μονοσήμαντη αναφορά χωρικών πληροφοριών στον χώρο, ως σύνολο συντεταγμένων (x,y,z) ή/και γεωγραφικό πλάτος και μήκος και ύψος, με βάση γεωδαιτικό οριζόντιο και κατακόρυφο σύστημα αναφοράς (datum).</dct:description>
		<skos:inScheme rdf:resource="http://inspire-registry.jrc.ec.europa.eu/registers/FCD/items"/>
	</inspire:SpatialObjectType>
	<inspire:SpatialObjectType rdf:about="http://inspire-registry.jrc.ec.europa.eu/registers/FCD/items/278">
		<inspire:itemStatus>valid</inspire:itemStatus>
		<inspire:dateAccepted>2010-01-13T16:54:33.244+01:00</inspire:dateAccepted>
		<skos:prefLabel xml:lang="en">Responsible Agency (Protected Sites)</skos:prefLabel>
		<skos:definition xml:lang="en">The agency, organisation or body responsible for selecting, describing and designating the protected site.</skos:definition>
		<dct:description xml:lang="en">NOTE Responsibility for establishing a protected site allows all interested parties to know who to liaise with over queries or requests for more detailed information on each Area. The responsible body will vary according to the basis of establishment with national governments ultimately responsible for Natura2000 sites, down to voluntary bodies responsible for local designations or quasi-legislative protected sites.
Supporting code lists will need to be flexible to accommodate types of responsible bodies.</dct:description>
		<skos:prefLabel xml:lang="el">SAMPLE ALTERNATIVE EXPRESSION - αναφορά</skos:prefLabel>
		<skos:definition xml:lang="el">Συστήματα συντεταγμένων</skos:definition>
		<dct:description xml:lang="el">Συστήματα για μονοσήμαντη αναφορά χωρικών πληροφοριών στον χώρο, ως σύνολο συντεταγμένων (x,y,z) ή/και γεωγραφικό πλάτος και μήκος και ύψος, με βάση γεωδαιτικό οριζόντιο και κατακόρυφο σύστημα αναφοράς (datum).</dct:description>
		<skos:inScheme rdf:resource="http://inspire-registry.jrc.ec.europa.eu/registers/FCD/items"/>
	</inspire:SpatialObjectType>
	<inspire:SpatialObjectType rdf:about="http://inspire-registry.jrc.ec.europa.eu/registers/FCD/items/279">
		<inspire:itemStatus>valid</inspire:itemStatus>
		<inspire:dateAccepted>2010-01-13T16:54:34.145+01:00</inspire:dateAccepted>
		<skos:prefLabel xml:lang="en">Protected Site</skos:prefLabel>
		<skos:definition xml:lang="en">An area designated or managed within a framework of international, Union and Member States' legislation to achieve specific conservation objectives.</skos:definition>
		<dct:description xml:lang="en">Each protected site has a boundary defined through formal, legal or administrative agreements or decisions. The establishment of a protected site is normally underpinned by legislation and thus given weight in decisions about land use change and spatial planning. Each Site is normally selected as a representative example of a wider resource and selected through a formal criterion based approach. A protected site can be a contiguous extent of land/sea or a collection of discrete areas that together represent a single formal Protected Site. This class has the attributes, constraints and associations that are part of the Simple application schema.</dct:description>
		<skos:prefLabel xml:lang="el">SAMPLE ALTERNATIVE EXPRESSION - αναφορά</skos:prefLabel>
		<skos:definition xml:lang="el">Συστήματα συντεταγμένων</skos:definition>
		<dct:description xml:lang="el">Συστήματα για μονοσήμαντη αναφορά χωρικών πληροφοριών στον χώρο, ως σύνολο συντεταγμένων (x,y,z) ή/και γεωγραφικό πλάτος και μήκος και ύψος, με βάση γεωδαιτικό οριζόντιο και κατακόρυφο σύστημα αναφοράς (datum).</dct:description>
		<skos:inScheme rdf:resource="http://inspire-registry.jrc.ec.europa.eu/registers/FCD/items"/>
	</inspire:SpatialObjectType>
	<inspire:SpatialObjectType rdf:about="http://inspire-registry.jrc.ec.europa.eu/registers/FCD/items/280">
		<inspire:itemStatus>valid</inspire:itemStatus>
		<inspire:dateAccepted>2010-01-13T16:54:35.182+01:00</inspire:dateAccepted>
		<skos:prefLabel xml:lang="en">Bio-geographic Regions (Bio-geographic Regions)</skos:prefLabel>
		<skos:definition xml:lang="en">An area of relatively homogeneous ecological conditions with common characteristics.</skos:definition>
		<dct:description xml:lang="en">Bio-geographical Regions [Candidate type that might be extended in Annex II/III INSPIRE data specification].</dct:description>
		<skos:prefLabel xml:lang="el">SAMPLE ALTERNATIVE EXPRESSION - αναφορά</skos:prefLabel>
		<skos:definition xml:lang="el">Συστήματα συντεταγμένων</skos:definition>
		<dct:description xml:lang="el">Συστήματα για μονοσήμαντη αναφορά χωρικών πληροφοριών στον χώρο, ως σύνολο συντεταγμένων (x,y,z) ή/και γεωγραφικό πλάτος και μήκος και ύψος, με βάση γεωδαιτικό οριζόντιο και κατακόρυφο σύστημα αναφοράς (datum).</dct:description>
		<skos:inScheme rdf:resource="http://inspire-registry.jrc.ec.europa.eu/registers/FCD/items"/>
	</inspire:SpatialObjectType>
	<inspire:SpatialObjectType rdf:about="http://inspire-registry.jrc.ec.europa.eu/registers/FCD/items/281">
		<inspire:itemStatus>valid</inspire:itemStatus>
		<inspire:dateAccepted>2010-01-13T17:18:38.692+01:00</inspire:dateAccepted>
		<skos:prefLabel xml:lang="en">Transport Area</skos:prefLabel>
		<skos:definition xml:lang="en">Surface that represents the spatial extent of an element of a transport network.</skos:definition>
		<skos:prefLabel xml:lang="el">SAMPLE ALTERNATIVE EXPRESSION - αναφορά</skos:prefLabel>
		<skos:definition xml:lang="el">Συστήματα συντεταγμένων</skos:definition>
		<dct:description xml:lang="el">Συστήματα για μονοσήμαντη αναφορά χωρικών πληροφοριών στον χώρο, ως σύνολο συντεταγμένων (x,y,z) ή/και γεωγραφικό πλάτος και μήκος και ύψος, με βάση γεωδαιτικό οριζόντιο και κατακόρυφο σύστημα αναφοράς (datum).</dct:description>
		<skos:inScheme rdf:resource="http://inspire-registry.jrc.ec.europa.eu/registers/FCD/items"/>
	</inspire:SpatialObjectType>
	<inspire:SpatialObjectType rdf:about="http://inspire-registry.jrc.ec.europa.eu/registers/FCD/items/282">
		<inspire:itemStatus>valid</inspire:itemStatus>
		<inspire:dateAccepted>2010-01-13T17:18:39.234+01:00</inspire:dateAccepted>
		<skos:prefLabel xml:lang="en">Transport Link</skos:prefLabel>
		<skos:definition xml:lang="en">A linear spatial object that describes the geometry and connectivity of a transport network between two points in the network.</skos:definition>
		<skos:prefLabel xml:lang="el">SAMPLE ALTERNATIVE EXPRESSION - αναφορά</skos:prefLabel>
		<skos:definition xml:lang="el">Συστήματα συντεταγμένων</skos:definition>
		<dct:description xml:lang="el">Συστήματα για μονοσήμαντη αναφορά χωρικών πληροφοριών στον χώρο, ως σύνολο συντεταγμένων (x,y,z) ή/και γεωγραφικό πλάτος και μήκος και ύψος, με βάση γεωδαιτικό οριζόντιο και κατακόρυφο σύστημα αναφοράς (datum).</dct:description>
		<skos:inScheme rdf:resource="http://inspire-registry.jrc.ec.europa.eu/registers/FCD/items"/>
	</inspire:SpatialObjectType>
	<inspire:SpatialObjectType rdf:about="http://inspire-registry.jrc.ec.europa.eu/registers/FCD/items/283">
		<inspire:itemStatus>valid</inspire:itemStatus>
		<inspire:dateAccepted>2010-01-13T17:18:39.728+01:00</inspire:dateAccepted>
		<skos:prefLabel xml:lang="en">Transport Node</skos:prefLabel>
		<skos:definition xml:lang="en">A point spatial object which is used for connectivity.</skos:definition>
		<dct:description xml:lang="en">Nodes are found at either end of the TransportLink.</dct:description>
		<skos:prefLabel xml:lang="el">SAMPLE ALTERNATIVE EXPRESSION - αναφορά</skos:prefLabel>
		<skos:definition xml:lang="el">Συστήματα συντεταγμένων</skos:definition>
		<dct:description xml:lang="el">Συστήματα για μονοσήμαντη αναφορά χωρικών πληροφοριών στον χώρο, ως σύνολο συντεταγμένων (x,y,z) ή/και γεωγραφικό πλάτος και μήκος και ύψος, με βάση γεωδαιτικό οριζόντιο και κατακόρυφο σύστημα αναφοράς (datum).</dct:description>
		<skos:inScheme rdf:resource="http://inspire-registry.jrc.ec.europa.eu/registers/FCD/items"/>
	</inspire:SpatialObjectType>
	<inspire:SpatialObjectType rdf:about="http://inspire-registry.jrc.ec.europa.eu/registers/FCD/items/284">
		<inspire:itemStatus>valid</inspire:itemStatus>
		<inspire:dateAccepted>2010-01-13T17:18:40.368+01:00</inspire:dateAccepted>
		<skos:prefLabel xml:lang="en">Functional Road Class</skos:prefLabel>
		<skos:definition xml:lang="en">A classification based on the importance of the role that the road performs in the road network.</skos:definition>
		<dct:description xml:lang="en">SOURCE Adapted from [GDF, EuroRoadS].</dct:description>
		<skos:prefLabel xml:lang="el">SAMPLE ALTERNATIVE EXPRESSION - αναφορά</skos:prefLabel>
		<skos:definition xml:lang="el">Συστήματα συντεταγμένων</skos:definition>
		<dct:description xml:lang="el">Συστήματα για μονοσήμαντη αναφορά χωρικών πληροφοριών στον χώρο, ως σύνολο συντεταγμένων (x,y,z) ή/και γεωγραφικό πλάτος και μήκος και ύψος, με βάση γεωδαιτικό οριζόντιο και κατακόρυφο σύστημα αναφοράς (datum).</dct:description>
		<skos:inScheme rdf:resource="http://inspire-registry.jrc.ec.europa.eu/registers/FCD/items"/>
	</inspire:SpatialObjectType>
	<inspire:SpatialObjectType rdf:about="http://inspire-registry.jrc.ec.europa.eu/registers/FCD/items/285">
		<inspire:itemStatus>valid</inspire:itemStatus>
		<inspire:dateAccepted>2010-01-13T17:18:41.057+01:00</inspire:dateAccepted>
		<skos:prefLabel xml:lang="en">Road</skos:prefLabel>
		<skos:definition xml:lang="en">A collection of road link sequences and/or individual road links that are characterized by one or more thematic identifiers and/or properties.</skos:definition>
		<dct:description xml:lang="en">EXAMPLE Examples are roads characterized by a specific identification code, used by road management authorities or tourist routes, identified by a specific name.</dct:description>
		<skos:prefLabel xml:lang="el">SAMPLE ALTERNATIVE EXPRESSION - αναφορά</skos:prefLabel>
		<skos:definition xml:lang="el">Συστήματα συντεταγμένων</skos:definition>
		<dct:description xml:lang="el">Συστήματα για μονοσήμαντη αναφορά χωρικών πληροφοριών στον χώρο, ως σύνολο συντεταγμένων (x,y,z) ή/και γεωγραφικό πλάτος και μήκος και ύψος, με βάση γεωδαιτικό οριζόντιο και κατακόρυφο σύστημα αναφοράς (datum).</dct:description>
		<skos:inScheme rdf:resource="http://inspire-registry.jrc.ec.europa.eu/registers/FCD/items"/>
	</inspire:SpatialObjectType>
	<inspire:SpatialObjectType rdf:about="http://inspire-registry.jrc.ec.europa.eu/registers/FCD/items/286">
		<inspire:itemStatus>valid</inspire:itemStatus>
		<inspire:dateAccepted>2010-01-13T17:18:41.595+01:00</inspire:dateAccepted>
		<skos:prefLabel xml:lang="en">Road Area</skos:prefLabel>
		<skos:definition xml:lang="en">Surface which extends to the limits of a road, including vehicular areas and other parts of it.</skos:definition>
		<dct:description xml:lang="en">EXAMPLE Pedestrian areas.</dct:description>
		<skos:prefLabel xml:lang="el">SAMPLE ALTERNATIVE EXPRESSION - αναφορά</skos:prefLabel>
		<skos:definition xml:lang="el">Συστήματα συντεταγμένων</skos:definition>
		<dct:description xml:lang="el">Συστήματα για μονοσήμαντη αναφορά χωρικών πληροφοριών στον χώρο, ως σύνολο συντεταγμένων (x,y,z) ή/και γεωγραφικό πλάτος και μήκος και ύψος, με βάση γεωδαιτικό οριζόντιο και κατακόρυφο σύστημα αναφοράς (datum).</dct:description>
		<skos:inScheme rdf:resource="http://inspire-registry.jrc.ec.europa.eu/registers/FCD/items"/>
	</inspire:SpatialObjectType>
	<inspire:SpatialObjectType rdf:about="http://inspire-registry.jrc.ec.europa.eu/registers/FCD/items/287">
		<inspire:itemStatus>valid</inspire:itemStatus>
		<inspire:dateAccepted>2010-01-13T17:18:42.091+01:00</inspire:dateAccepted>
		<skos:prefLabel xml:lang="en">Road Link</skos:prefLabel>
		<skos:definition xml:lang="en">A linear spatial object that describes the geometry and connectivity of a road network between two points in the network. Road links can represent paths, bicycle roads, single carriageways, multiple carriageway roads and even fictitious trajectories across traffic squares.</skos:definition>
		<skos:prefLabel xml:lang="el">SAMPLE ALTERNATIVE EXPRESSION - αναφορά</skos:prefLabel>
		<skos:definition xml:lang="el">Συστήματα συντεταγμένων</skos:definition>
		<dct:description xml:lang="el">Συστήματα για μονοσήμαντη αναφορά χωρικών πληροφοριών στον χώρο, ως σύνολο συντεταγμένων (x,y,z) ή/και γεωγραφικό πλάτος και μήκος και ύψος, με βάση γεωδαιτικό οριζόντιο και κατακόρυφο σύστημα αναφοράς (datum).</dct:description>
		<skos:inScheme rdf:resource="http://inspire-registry.jrc.ec.europa.eu/registers/FCD/items"/>
	</inspire:SpatialObjectType>
	<inspire:SpatialObjectType rdf:about="http://inspire-registry.jrc.ec.europa.eu/registers/FCD/items/288">
		<inspire:itemStatus>valid</inspire:itemStatus>
		<inspire:dateAccepted>2010-01-13T17:18:42.602+01:00</inspire:dateAccepted>
		<skos:prefLabel xml:lang="en">Road Node</skos:prefLabel>
		<skos:definition xml:lang="en">A point spatial object that is used to either represent connectivity between two road links or to represent a significant spatial object such as a services station or roundabout.</skos:definition>
		<skos:prefLabel xml:lang="el">SAMPLE ALTERNATIVE EXPRESSION - αναφορά</skos:prefLabel>
		<skos:definition xml:lang="el">Συστήματα συντεταγμένων</skos:definition>
		<dct:description xml:lang="el">Συστήματα για μονοσήμαντη αναφορά χωρικών πληροφοριών στον χώρο, ως σύνολο συντεταγμένων (x,y,z) ή/και γεωγραφικό πλάτος και μήκος και ύψος, με βάση γεωδαιτικό οριζόντιο και κατακόρυφο σύστημα αναφοράς (datum).</dct:description>
		<skos:inScheme rdf:resource="http://inspire-registry.jrc.ec.europa.eu/registers/FCD/items"/>
	</inspire:SpatialObjectType>
	<inspire:SpatialObjectType rdf:about="http://inspire-registry.jrc.ec.europa.eu/registers/FCD/items/289">
		<inspire:itemStatus>valid</inspire:itemStatus>
		<inspire:dateAccepted>2010-01-13T17:18:43.108+01:00</inspire:dateAccepted>
		<skos:prefLabel xml:lang="en">Road Service Area</skos:prefLabel>
		<skos:definition xml:lang="en">Surface annexed to a road and devoted to offer particular services for it.</skos:definition>
		<dct:description xml:lang="en">EXAMPLES Gas station, rest area, toll area.</dct:description>
		<skos:prefLabel xml:lang="el">SAMPLE ALTERNATIVE EXPRESSION - αναφορά</skos:prefLabel>
		<skos:definition xml:lang="el">Συστήματα συντεταγμένων</skos:definition>
		<dct:description xml:lang="el">Συστήματα για μονοσήμαντη αναφορά χωρικών πληροφοριών στον χώρο, ως σύνολο συντεταγμένων (x,y,z) ή/και γεωγραφικό πλάτος και μήκος και ύψος, με βάση γεωδαιτικό οριζόντιο και κατακόρυφο σύστημα αναφοράς (datum).</dct:description>
		<skos:inScheme rdf:resource="http://inspire-registry.jrc.ec.europa.eu/registers/FCD/items"/>
	</inspire:SpatialObjectType>
	<inspire:SpatialObjectType rdf:about="http://inspire-registry.jrc.ec.europa.eu/registers/FCD/items/290">
		<inspire:itemStatus>valid</inspire:itemStatus>
		<inspire:dateAccepted>2010-01-13T17:18:43.659+01:00</inspire:dateAccepted>
		<skos:prefLabel xml:lang="en">Road Surface Category</skos:prefLabel>
		<skos:definition xml:lang="en">Specification of the state of the surface of the associated Road Element. Indicates whether a road is paved or unpaved.</skos:definition>
		<dct:description xml:lang="en">SOURCE [GDF3, Euroroads].</dct:description>
		<skos:prefLabel xml:lang="el">SAMPLE ALTERNATIVE EXPRESSION - αναφορά</skos:prefLabel>
		<skos:definition xml:lang="el">Συστήματα συντεταγμένων</skos:definition>
		<dct:description xml:lang="el">Συστήματα για μονοσήμαντη αναφορά χωρικών πληροφοριών στον χώρο, ως σύνολο συντεταγμένων (x,y,z) ή/και γεωγραφικό πλάτος και μήκος και ύψος, με βάση γεωδαιτικό οριζόντιο και κατακόρυφο σύστημα αναφοράς (datum).</dct:description>
		<skos:inScheme rdf:resource="http://inspire-registry.jrc.ec.europa.eu/registers/FCD/items"/>
	</inspire:SpatialObjectType>
	<inspire:SpatialObjectType rdf:about="http://inspire-registry.jrc.ec.europa.eu/registers/FCD/items/291">
		<inspire:itemStatus>valid</inspire:itemStatus>
		<inspire:dateAccepted>2010-01-13T17:18:44.152+01:00</inspire:dateAccepted>
		<skos:prefLabel xml:lang="en">Road Width</skos:prefLabel>
		<skos:definition xml:lang="en">The width of the road, measured as an average value.</skos:definition>
		<dct:description xml:lang="en">SOURCE [Euroroads].</dct:description>
		<skos:prefLabel xml:lang="el">SAMPLE ALTERNATIVE EXPRESSION - αναφορά</skos:prefLabel>
		<skos:definition xml:lang="el">Συστήματα συντεταγμένων</skos:definition>
		<dct:description xml:lang="el">Συστήματα για μονοσήμαντη αναφορά χωρικών πληροφοριών στον χώρο, ως σύνολο συντεταγμένων (x,y,z) ή/και γεωγραφικό πλάτος και μήκος και ύψος, με βάση γεωδαιτικό οριζόντιο και κατακόρυφο σύστημα αναφοράς (datum).</dct:description>
		<skos:inScheme rdf:resource="http://inspire-registry.jrc.ec.europa.eu/registers/FCD/items"/>
	</inspire:SpatialObjectType>
	<inspire:SpatialObjectType rdf:about="http://inspire-registry.jrc.ec.europa.eu/registers/FCD/items/292">
		<inspire:itemStatus>valid</inspire:itemStatus>
		<inspire:dateAccepted>2010-01-13T17:18:44.757+01:00</inspire:dateAccepted>
		<skos:prefLabel xml:lang="en">Traffic Flow Direction</skos:prefLabel>
		<skos:definition xml:lang="en">Indicates the direction of the flow of traffic in relation to the direction of the transport link vector.</skos:definition>
		<skos:prefLabel xml:lang="el">SAMPLE ALTERNATIVE EXPRESSION - αναφορά</skos:prefLabel>
		<skos:definition xml:lang="el">Συστήματα συντεταγμένων</skos:definition>
		<dct:description xml:lang="el">Συστήματα για μονοσήμαντη αναφορά χωρικών πληροφοριών στον χώρο, ως σύνολο συντεταγμένων (x,y,z) ή/και γεωγραφικό πλάτος και μήκος και ύψος, με βάση γεωδαιτικό οριζόντιο και κατακόρυφο σύστημα αναφοράς (datum).</dct:description>
		<skos:inScheme rdf:resource="http://inspire-registry.jrc.ec.europa.eu/registers/FCD/items"/>
	</inspire:SpatialObjectType>
	<inspire:SpatialObjectType rdf:about="http://inspire-registry.jrc.ec.europa.eu/registers/FCD/items/293">
		<inspire:itemStatus>valid</inspire:itemStatus>
		<inspire:dateAccepted>2010-01-13T17:18:45.261+01:00</inspire:dateAccepted>
		<skos:prefLabel xml:lang="en">Vehicle Traffic Area</skos:prefLabel>
		<skos:definition xml:lang="en">Surface that represents the part of a road which is used for the normal traffic of vehicles.</skos:definition>
		<skos:prefLabel xml:lang="el">SAMPLE ALTERNATIVE EXPRESSION - αναφορά</skos:prefLabel>
		<skos:definition xml:lang="el">Συστήματα συντεταγμένων</skos:definition>
		<dct:description xml:lang="el">Συστήματα για μονοσήμαντη αναφορά χωρικών πληροφοριών στον χώρο, ως σύνολο συντεταγμένων (x,y,z) ή/και γεωγραφικό πλάτος και μήκος και ύψος, με βάση γεωδαιτικό οριζόντιο και κατακόρυφο σύστημα αναφοράς (datum).</dct:description>
		<skos:inScheme rdf:resource="http://inspire-registry.jrc.ec.europa.eu/registers/FCD/items"/>
	</inspire:SpatialObjectType>
	<inspire:SpatialObjectType rdf:about="http://inspire-registry.jrc.ec.europa.eu/registers/FCD/items/294">
		<inspire:itemStatus>valid</inspire:itemStatus>
		<inspire:dateAccepted>2010-01-13T17:18:45.701+01:00</inspire:dateAccepted>
		<skos:prefLabel xml:lang="en">Cableway Link</skos:prefLabel>
		<skos:definition xml:lang="en">Linear spatial object that describes the geometry and connectivity of a cable network between two points in a cableway transport network.</skos:definition>
		<dct:description xml:lang="en">NOTE Cableway transport is a form of transport based on a cable suspended normally from a set of consecutive towers.</dct:description>
		<skos:prefLabel xml:lang="el">SAMPLE ALTERNATIVE EXPRESSION - αναφορά</skos:prefLabel>
		<skos:definition xml:lang="el">Συστήματα συντεταγμένων</skos:definition>
		<dct:description xml:lang="el">Συστήματα για μονοσήμαντη αναφορά χωρικών πληροφοριών στον χώρο, ως σύνολο συντεταγμένων (x,y,z) ή/και γεωγραφικό πλάτος και μήκος και ύψος, με βάση γεωδαιτικό οριζόντιο και κατακόρυφο σύστημα αναφοράς (datum).</dct:description>
		<skos:inScheme rdf:resource="http://inspire-registry.jrc.ec.europa.eu/registers/FCD/items"/>
	</inspire:SpatialObjectType>
	<inspire:SpatialObjectType rdf:about="http://inspire-registry.jrc.ec.europa.eu/registers/FCD/items/295">
		<inspire:itemStatus>valid</inspire:itemStatus>
		<inspire:dateAccepted>2010-01-13T17:18:46.150+01:00</inspire:dateAccepted>
		<skos:prefLabel xml:lang="en">Cableway Node</skos:prefLabel>
		<skos:definition xml:lang="en">A point spatial object that is used to represent connectivity between two consecutive cableway links.</skos:definition>
		<skos:prefLabel xml:lang="el">SAMPLE ALTERNATIVE EXPRESSION - αναφορά</skos:prefLabel>
		<skos:definition xml:lang="el">Συστήματα συντεταγμένων</skos:definition>
		<dct:description xml:lang="el">Συστήματα για μονοσήμαντη αναφορά χωρικών πληροφοριών στον χώρο, ως σύνολο συντεταγμένων (x,y,z) ή/και γεωγραφικό πλάτος και μήκος και ύψος, με βάση γεωδαιτικό οριζόντιο και κατακόρυφο σύστημα αναφοράς (datum).</dct:description>
		<skos:inScheme rdf:resource="http://inspire-registry.jrc.ec.europa.eu/registers/FCD/items"/>
	</inspire:SpatialObjectType>
	<inspire:SpatialObjectType rdf:about="http://inspire-registry.jrc.ec.europa.eu/registers/FCD/items/296">
		<inspire:itemStatus>valid</inspire:itemStatus>
		<inspire:dateAccepted>2010-01-13T17:18:46.674+01:00</inspire:dateAccepted>
		<skos:prefLabel xml:lang="en">Railway Line</skos:prefLabel>
		<skos:definition xml:lang="en">A collection of railway link sequences and or individual railway links that are characterized by one or more thematical identifiers and/or properties.</skos:definition>
		<dct:description xml:lang="en">EXAMPLE Railway lines characterized by a specific identification code, used by railroad companies or tourist railways, identified by a specific name.</dct:description>
		<skos:prefLabel xml:lang="el">SAMPLE ALTERNATIVE EXPRESSION - αναφορά</skos:prefLabel>
		<skos:definition xml:lang="el">Συστήματα συντεταγμένων</skos:definition>
		<dct:description xml:lang="el">Συστήματα για μονοσήμαντη αναφορά χωρικών πληροφοριών στον χώρο, ως σύνολο συντεταγμένων (x,y,z) ή/και γεωγραφικό πλάτος και μήκος και ύψος, με βάση γεωδαιτικό οριζόντιο και κατακόρυφο σύστημα αναφοράς (datum).</dct:description>
		<skos:inScheme rdf:resource="http://inspire-registry.jrc.ec.europa.eu/registers/FCD/items"/>
	</inspire:SpatialObjectType>
	<inspire:SpatialObjectType rdf:about="http://inspire-registry.jrc.ec.europa.eu/registers/FCD/items/297">
		<inspire:itemStatus>valid</inspire:itemStatus>
		<inspire:dateAccepted>2010-01-13T17:18:47.203+01:00</inspire:dateAccepted>
		<skos:prefLabel xml:lang="en">Railway Link</skos:prefLabel>
		<skos:definition xml:lang="en">A linear spatial object that describes the geometry and connectivity of a railway network between two points in the network.</skos:definition>
		<dct:description xml:lang="en">NOTE Railway links can be used to represent stretches of railway with one or multiple tracks.</dct:description>
		<skos:prefLabel xml:lang="el">SAMPLE ALTERNATIVE EXPRESSION - αναφορά</skos:prefLabel>
		<skos:definition xml:lang="el">Συστήματα συντεταγμένων</skos:definition>
		<dct:description xml:lang="el">Συστήματα για μονοσήμαντη αναφορά χωρικών πληροφοριών στον χώρο, ως σύνολο συντεταγμένων (x,y,z) ή/και γεωγραφικό πλάτος και μήκος και ύψος, με βάση γεωδαιτικό οριζόντιο και κατακόρυφο σύστημα αναφοράς (datum).</dct:description>
		<skos:inScheme rdf:resource="http://inspire-registry.jrc.ec.europa.eu/registers/FCD/items"/>
	</inspire:SpatialObjectType>
	<inspire:SpatialObjectType rdf:about="http://inspire-registry.jrc.ec.europa.eu/registers/FCD/items/298">
		<inspire:itemStatus>valid</inspire:itemStatus>
		<inspire:dateAccepted>2010-01-13T17:18:47.582+01:00</inspire:dateAccepted>
		<skos:prefLabel xml:lang="en">Railway Node</skos:prefLabel>
		<skos:definition xml:lang="en">A point spatial object which represents a significant point along the railway network or defines an intersection of railway tracks used to describe its connectivity.</skos:definition>
		<skos:prefLabel xml:lang="el">SAMPLE ALTERNATIVE EXPRESSION - αναφορά</skos:prefLabel>
		<skos:definition xml:lang="el">Συστήματα συντεταγμένων</skos:definition>
		<dct:description xml:lang="el">Συστήματα για μονοσήμαντη αναφορά χωρικών πληροφοριών στον χώρο, ως σύνολο συντεταγμένων (x,y,z) ή/και γεωγραφικό πλάτος και μήκος και ύψος, με βάση γεωδαιτικό οριζόντιο και κατακόρυφο σύστημα αναφοράς (datum).</dct:description>
		<skos:inScheme rdf:resource="http://inspire-registry.jrc.ec.europa.eu/registers/FCD/items"/>
	</inspire:SpatialObjectType>
	<inspire:SpatialObjectType rdf:about="http://inspire-registry.jrc.ec.europa.eu/registers/FCD/items/299">
		<inspire:itemStatus>valid</inspire:itemStatus>
		<inspire:dateAccepted>2010-01-13T17:18:48.053+01:00</inspire:dateAccepted>
		<skos:prefLabel xml:lang="en">Railway Station Area</skos:prefLabel>
		<skos:definition xml:lang="en">An area spatial object which is used to represent the topographical limits of the facilities of a railway station (buildings, railway yards, installations and equipment) devoted to carry out railway station operations.</skos:definition>
		<skos:prefLabel xml:lang="el">SAMPLE ALTERNATIVE EXPRESSION - αναφορά</skos:prefLabel>
		<skos:definition xml:lang="el">Συστήματα συντεταγμένων</skos:definition>
		<dct:description xml:lang="el">Συστήματα για μονοσήμαντη αναφορά χωρικών πληροφοριών στον χώρο, ως σύνολο συντεταγμένων (x,y,z) ή/και γεωγραφικό πλάτος και μήκος και ύψος, με βάση γεωδαιτικό οριζόντιο και κατακόρυφο σύστημα αναφοράς (datum).</dct:description>
		<skos:inScheme rdf:resource="http://inspire-registry.jrc.ec.europa.eu/registers/FCD/items"/>
	</inspire:SpatialObjectType>
	<inspire:SpatialObjectType rdf:about="http://inspire-registry.jrc.ec.europa.eu/registers/FCD/items/300">
		<inspire:itemStatus>valid</inspire:itemStatus>
		<inspire:dateAccepted>2010-01-13T17:18:48.576+01:00</inspire:dateAccepted>
		<skos:prefLabel xml:lang="en">Railway Use</skos:prefLabel>
		<skos:definition xml:lang="en">The current use of the railway.</skos:definition>
		<skos:prefLabel xml:lang="el">SAMPLE ALTERNATIVE EXPRESSION - αναφορά</skos:prefLabel>
		<skos:definition xml:lang="el">Συστήματα συντεταγμένων</skos:definition>
		<dct:description xml:lang="el">Συστήματα για μονοσήμαντη αναφορά χωρικών πληροφοριών στον χώρο, ως σύνολο συντεταγμένων (x,y,z) ή/και γεωγραφικό πλάτος και μήκος και ύψος, με βάση γεωδαιτικό οριζόντιο και κατακόρυφο σύστημα αναφοράς (datum).</dct:description>
		<skos:inScheme rdf:resource="http://inspire-registry.jrc.ec.europa.eu/registers/FCD/items"/>
	</inspire:SpatialObjectType>
	<inspire:SpatialObjectType rdf:about="http://inspire-registry.jrc.ec.europa.eu/registers/FCD/items/301">
		<inspire:itemStatus>valid</inspire:itemStatus>
		<inspire:dateAccepted>2010-01-13T17:18:48.962+01:00</inspire:dateAccepted>
		<skos:prefLabel xml:lang="en">Railway Yard Area</skos:prefLabel>
		<skos:definition xml:lang="en">An area spatial object which is used to represent the topographical limits of a railway yard.</skos:definition>
		<dct:description xml:lang="en">DEFINITION Railway yard: An area crossed by a number of parallel railway tracks (usually more than two) interconnected between them, which are used to stop trains in order to load / unload freight without interrupting the traffic of a main railway line.</dct:description>
		<skos:prefLabel xml:lang="el">SAMPLE ALTERNATIVE EXPRESSION - αναφορά</skos:prefLabel>
		<skos:definition xml:lang="el">Συστήματα συντεταγμένων</skos:definition>
		<dct:description xml:lang="el">Συστήματα για μονοσήμαντη αναφορά χωρικών πληροφοριών στον χώρο, ως σύνολο συντεταγμένων (x,y,z) ή/και γεωγραφικό πλάτος και μήκος και ύψος, με βάση γεωδαιτικό οριζόντιο και κατακόρυφο σύστημα αναφοράς (datum).</dct:description>
		<skos:inScheme rdf:resource="http://inspire-registry.jrc.ec.europa.eu/registers/FCD/items"/>
	</inspire:SpatialObjectType>
	<inspire:SpatialObjectType rdf:about="http://inspire-registry.jrc.ec.europa.eu/registers/FCD/items/302">
		<inspire:itemStatus>valid</inspire:itemStatus>
		<inspire:dateAccepted>2010-01-13T17:18:49.429+01:00</inspire:dateAccepted>
		<skos:prefLabel xml:lang="en">Railway Yard Node</skos:prefLabel>
		<skos:definition xml:lang="en">A railway node which occurs within a railway yard area.</skos:definition>
		<dct:description xml:lang="en">DEFINTION Railway yard: An area crossed by a number of parallel railway tracks (usually more than two) interconnected between them, which are used to stop trains in order to load / unload freight without interrupting the traffic of a main railway line.</dct:description>
		<skos:prefLabel xml:lang="el">SAMPLE ALTERNATIVE EXPRESSION - αναφορά</skos:prefLabel>
		<skos:definition xml:lang="el">Συστήματα συντεταγμένων</skos:definition>
		<dct:description xml:lang="el">Συστήματα για μονοσήμαντη αναφορά χωρικών πληροφοριών στον χώρο, ως σύνολο συντεταγμένων (x,y,z) ή/και γεωγραφικό πλάτος και μήκος και ύψος, με βάση γεωδαιτικό οριζόντιο και κατακόρυφο σύστημα αναφοράς (datum).</dct:description>
		<skos:inScheme rdf:resource="http://inspire-registry.jrc.ec.europa.eu/registers/FCD/items"/>
	</inspire:SpatialObjectType>
	<inspire:SpatialObjectType rdf:about="http://inspire-registry.jrc.ec.europa.eu/registers/FCD/items/303">
		<inspire:itemStatus>valid</inspire:itemStatus>
		<inspire:dateAccepted>2010-01-13T17:18:49.820+01:00</inspire:dateAccepted>
		<skos:prefLabel xml:lang="en">Ferry Crossing</skos:prefLabel>
		<skos:definition xml:lang="en">A special waterway aimed at supporting the transport of passengers, vehicles or other cargo/freight across a water body, and which is normally used as a connection linking two or more nodes of a land based transport network.</skos:definition>
		<skos:prefLabel xml:lang="el">SAMPLE ALTERNATIVE EXPRESSION - αναφορά</skos:prefLabel>
		<skos:definition xml:lang="el">Συστήματα συντεταγμένων</skos:definition>
		<dct:description xml:lang="el">Συστήματα για μονοσήμαντη αναφορά χωρικών πληροφοριών στον χώρο, ως σύνολο συντεταγμένων (x,y,z) ή/και γεωγραφικό πλάτος και μήκος και ύψος, με βάση γεωδαιτικό οριζόντιο και κατακόρυφο σύστημα αναφοράς (datum).</dct:description>
		<skos:inScheme rdf:resource="http://inspire-registry.jrc.ec.europa.eu/registers/FCD/items"/>
	</inspire:SpatialObjectType>
	<inspire:SpatialObjectType rdf:about="http://inspire-registry.jrc.ec.europa.eu/registers/FCD/items/304">
		<inspire:itemStatus>valid</inspire:itemStatus>
		<inspire:dateAccepted>2010-01-13T17:18:50.213+01:00</inspire:dateAccepted>
		<skos:prefLabel xml:lang="en">Port Area</skos:prefLabel>
		<skos:definition xml:lang="en">An area spatial object which is used to represent the physical limits of all the facilities which constitute the terrestrial zone of a sea or inland port.</skos:definition>
		<skos:prefLabel xml:lang="el">SAMPLE ALTERNATIVE EXPRESSION - αναφορά</skos:prefLabel>
		<skos:definition xml:lang="el">Συστήματα συντεταγμένων</skos:definition>
		<dct:description xml:lang="el">Συστήματα για μονοσήμαντη αναφορά χωρικών πληροφοριών στον χώρο, ως σύνολο συντεταγμένων (x,y,z) ή/και γεωγραφικό πλάτος και μήκος και ύψος, με βάση γεωδαιτικό οριζόντιο και κατακόρυφο σύστημα αναφοράς (datum).</dct:description>
		<skos:inScheme rdf:resource="http://inspire-registry.jrc.ec.europa.eu/registers/FCD/items"/>
	</inspire:SpatialObjectType>
	<inspire:SpatialObjectType rdf:about="http://inspire-registry.jrc.ec.europa.eu/registers/FCD/items/305">
		<inspire:itemStatus>valid</inspire:itemStatus>
		<inspire:dateAccepted>2010-01-13T17:18:50.566+01:00</inspire:dateAccepted>
		<skos:prefLabel xml:lang="en">Port Node</skos:prefLabel>
		<skos:definition xml:lang="en">A point spatial object which is used to represent a sea or inland port in a simplified way, aproximately located at the bank of the waterbody where the port is placed.</skos:definition>
		<dct:description xml:lang="en">NOTE It is used to connect the port with the rest of the water transport network, by means of the different waterway links which arrive to / depart from it.</dct:description>
		<skos:prefLabel xml:lang="el">SAMPLE ALTERNATIVE EXPRESSION - αναφορά</skos:prefLabel>
		<skos:definition xml:lang="el">Συστήματα συντεταγμένων</skos:definition>
		<dct:description xml:lang="el">Συστήματα για μονοσήμαντη αναφορά χωρικών πληροφοριών στον χώρο, ως σύνολο συντεταγμένων (x,y,z) ή/και γεωγραφικό πλάτος και μήκος και ύψος, με βάση γεωδαιτικό οριζόντιο και κατακόρυφο σύστημα αναφοράς (datum).</dct:description>
		<skos:inScheme rdf:resource="http://inspire-registry.jrc.ec.europa.eu/registers/FCD/items"/>
	</inspire:SpatialObjectType>
	<inspire:SpatialObjectType rdf:about="http://inspire-registry.jrc.ec.europa.eu/registers/FCD/items/306">
		<inspire:itemStatus>valid</inspire:itemStatus>
		<inspire:dateAccepted>2010-01-13T17:18:50.947+01:00</inspire:dateAccepted>
		<skos:prefLabel xml:lang="en">Water Node</skos:prefLabel>
		<skos:definition xml:lang="en">A point spatial object which is used to represent the connectivity between two different waterway links, or between a waterway link and a watercourse link, in the water transport network.</skos:definition>
		<dct:description xml:lang="en">NOTE It is also used to represent a significant feature in the network, such as a port.</dct:description>
		<skos:prefLabel xml:lang="el">SAMPLE ALTERNATIVE EXPRESSION - αναφορά</skos:prefLabel>
		<skos:definition xml:lang="el">Συστήματα συντεταγμένων</skos:definition>
		<dct:description xml:lang="el">Συστήματα για μονοσήμαντη αναφορά χωρικών πληροφοριών στον χώρο, ως σύνολο συντεταγμένων (x,y,z) ή/και γεωγραφικό πλάτος και μήκος και ύψος, με βάση γεωδαιτικό οριζόντιο και κατακόρυφο σύστημα αναφοράς (datum).</dct:description>
		<skos:inScheme rdf:resource="http://inspire-registry.jrc.ec.europa.eu/registers/FCD/items"/>
	</inspire:SpatialObjectType>
	<inspire:SpatialObjectType rdf:about="http://inspire-registry.jrc.ec.europa.eu/registers/FCD/items/307">
		<inspire:itemStatus>valid</inspire:itemStatus>
		<inspire:dateAccepted>2010-01-13T17:18:51.402+01:00</inspire:dateAccepted>
		<skos:prefLabel xml:lang="en">Waterway</skos:prefLabel>
		<skos:definition xml:lang="en">A collection of water link sequences and or individual waterway and/or watercourse links (as necessary) that are characterized by one or more thematical identifiers and/or properties, which perform a navigable route within a water body (oceans, seas, rivers, lakes, channels or canals).</skos:definition>
		<skos:prefLabel xml:lang="el">SAMPLE ALTERNATIVE EXPRESSION - αναφορά</skos:prefLabel>
		<skos:definition xml:lang="el">Συστήματα συντεταγμένων</skos:definition>
		<dct:description xml:lang="el">Συστήματα για μονοσήμαντη αναφορά χωρικών πληροφοριών στον χώρο, ως σύνολο συντεταγμένων (x,y,z) ή/και γεωγραφικό πλάτος και μήκος και ύψος, με βάση γεωδαιτικό οριζόντιο και κατακόρυφο σύστημα αναφοράς (datum).</dct:description>
		<skos:inScheme rdf:resource="http://inspire-registry.jrc.ec.europa.eu/registers/FCD/items"/>
	</inspire:SpatialObjectType>
	<inspire:SpatialObjectType rdf:about="http://inspire-registry.jrc.ec.europa.eu/registers/FCD/items/308">
		<inspire:itemStatus>valid</inspire:itemStatus>
		<inspire:dateAccepted>2010-01-13T17:18:51.850+01:00</inspire:dateAccepted>
		<skos:prefLabel xml:lang="en">Waterway Link</skos:prefLabel>
		<skos:definition xml:lang="en">A linear spatial object that describes the geometry or connectivity of the water transport network between two consecutive waterway or watercourse nodes. It represents a linear section across a body of water which is used for shipping.</skos:definition>
		<dct:description xml:lang="en">NOTE Water Transport Networks will use the WatercourseLink class - provided by the INSPIRE Hydrography Data Specification - wherever possible.</dct:description>
		<skos:prefLabel xml:lang="el">SAMPLE ALTERNATIVE EXPRESSION - αναφορά</skos:prefLabel>
		<skos:definition xml:lang="el">Συστήματα συντεταγμένων</skos:definition>
		<dct:description xml:lang="el">Συστήματα για μονοσήμαντη αναφορά χωρικών πληροφοριών στον χώρο, ως σύνολο συντεταγμένων (x,y,z) ή/και γεωγραφικό πλάτος και μήκος και ύψος, με βάση γεωδαιτικό οριζόντιο και κατακόρυφο σύστημα αναφοράς (datum).</dct:description>
		<skos:inScheme rdf:resource="http://inspire-registry.jrc.ec.europa.eu/registers/FCD/items"/>
	</inspire:SpatialObjectType>
	<inspire:SpatialObjectType rdf:about="http://inspire-registry.jrc.ec.europa.eu/registers/FCD/items/309">
		<inspire:itemStatus>valid</inspire:itemStatus>
		<inspire:dateAccepted>2010-01-13T17:18:52.285+01:00</inspire:dateAccepted>
		<skos:prefLabel xml:lang="en">Waterway Node</skos:prefLabel>
		<skos:definition xml:lang="en">A point spatial object which is used to represent the connectivity between two different waterway links, or between a waterway link and a watercourse link, in the water transport network.</skos:definition>
		<skos:prefLabel xml:lang="el">SAMPLE ALTERNATIVE EXPRESSION - αναφορά</skos:prefLabel>
		<skos:definition xml:lang="el">Συστήματα συντεταγμένων</skos:definition>
		<dct:description xml:lang="el">Συστήματα για μονοσήμαντη αναφορά χωρικών πληροφοριών στον χώρο, ως σύνολο συντεταγμένων (x,y,z) ή/και γεωγραφικό πλάτος και μήκος και ύψος, με βάση γεωδαιτικό οριζόντιο και κατακόρυφο σύστημα αναφοράς (datum).</dct:description>
		<skos:inScheme rdf:resource="http://inspire-registry.jrc.ec.europa.eu/registers/FCD/items"/>
	</inspire:SpatialObjectType>
	<inspire:SpatialObjectType rdf:about="http://inspire-registry.jrc.ec.europa.eu/registers/FCD/items/310">
		<inspire:itemStatus>valid</inspire:itemStatus>
		<inspire:dateAccepted>2010-01-13T17:18:52.798+01:00</inspire:dateAccepted>
		<skos:prefLabel xml:lang="en">Aerodrome Area</skos:prefLabel>
		<skos:definition xml:lang="en">A defined area on land or water (including any buildings, installations and equipment) intended to be used either wholly or in part for the arrival, departure and surface movement of aircraft and/or helicopters.</skos:definition>
		<dct:description xml:lang="en">SOURCE [AIXM5.0].
NOTE An area spatial object which is used to represent the physical limits of all the facilities which form part of an inland aerodrome.</dct:description>
		<skos:prefLabel xml:lang="el">SAMPLE ALTERNATIVE EXPRESSION - αναφορά</skos:prefLabel>
		<skos:definition xml:lang="el">Συστήματα συντεταγμένων</skos:definition>
		<dct:description xml:lang="el">Συστήματα για μονοσήμαντη αναφορά χωρικών πληροφοριών στον χώρο, ως σύνολο συντεταγμένων (x,y,z) ή/και γεωγραφικό πλάτος και μήκος και ύψος, με βάση γεωδαιτικό οριζόντιο και κατακόρυφο σύστημα αναφοράς (datum).</dct:description>
		<skos:inScheme rdf:resource="http://inspire-registry.jrc.ec.europa.eu/registers/FCD/items"/>
	</inspire:SpatialObjectType>
	<inspire:SpatialObjectType rdf:about="http://inspire-registry.jrc.ec.europa.eu/registers/FCD/items/311">
		<inspire:itemStatus>valid</inspire:itemStatus>
		<inspire:dateAccepted>2010-01-13T17:18:53.233+01:00</inspire:dateAccepted>
		<skos:prefLabel xml:lang="en">Aerodrome Node</skos:prefLabel>
		<skos:definition xml:lang="en">Node located at the aerodrome reference point of an airport/heliport, which is used to represent it in a simplified way.</skos:definition>
		<dct:description xml:lang="en">DEFINITION Aerodrome Reference Point (ARP): The designated geographical location of an aerodrome, located near the initial or planned geometric centre of the aerodrome and normally remaining where originally established [AIXM3.3]. DEFINITION Airport/heliport: A defined area on land or water (including any buildings, installations and equipment) intended to be used either wholly or in part for the arrival, departure and surface movement of aircraft/helicopters [AIXM5.0].
SOURCE [AIXM5.0].</dct:description>
		<skos:prefLabel xml:lang="el">SAMPLE ALTERNATIVE EXPRESSION - αναφορά</skos:prefLabel>
		<skos:definition xml:lang="el">Συστήματα συντεταγμένων</skos:definition>
		<dct:description xml:lang="el">Συστήματα για μονοσήμαντη αναφορά χωρικών πληροφοριών στον χώρο, ως σύνολο συντεταγμένων (x,y,z) ή/και γεωγραφικό πλάτος και μήκος και ύψος, με βάση γεωδαιτικό οριζόντιο και κατακόρυφο σύστημα αναφοράς (datum).</dct:description>
		<skos:inScheme rdf:resource="http://inspire-registry.jrc.ec.europa.eu/registers/FCD/items"/>
	</inspire:SpatialObjectType>
	<inspire:SpatialObjectType rdf:about="http://inspire-registry.jrc.ec.europa.eu/registers/FCD/items/312">
		<inspire:itemStatus>valid</inspire:itemStatus>
		<inspire:dateAccepted>2010-01-13T17:18:53.626+01:00</inspire:dateAccepted>
		<skos:prefLabel xml:lang="en">Air Node</skos:prefLabel>
		<skos:definition xml:lang="en">A node which occurs in a air network.</skos:definition>
		<skos:prefLabel xml:lang="el">SAMPLE ALTERNATIVE EXPRESSION - αναφορά</skos:prefLabel>
		<skos:definition xml:lang="el">Συστήματα συντεταγμένων</skos:definition>
		<dct:description xml:lang="el">Συστήματα για μονοσήμαντη αναφορά χωρικών πληροφοριών στον χώρο, ως σύνολο συντεταγμένων (x,y,z) ή/και γεωγραφικό πλάτος και μήκος και ύψος, με βάση γεωδαιτικό οριζόντιο και κατακόρυφο σύστημα αναφοράς (datum).</dct:description>
		<skos:inScheme rdf:resource="http://inspire-registry.jrc.ec.europa.eu/registers/FCD/items"/>
	</inspire:SpatialObjectType>
	<inspire:SpatialObjectType rdf:about="http://inspire-registry.jrc.ec.europa.eu/registers/FCD/items/313">
		<inspire:itemStatus>valid</inspire:itemStatus>
		<inspire:dateAccepted>2010-01-13T17:18:54.134+01:00</inspire:dateAccepted>
		<skos:prefLabel xml:lang="en">Air Route</skos:prefLabel>
		<skos:definition xml:lang="en">A specified route designed for channelling the flow of traffic as necessary for the provision of air traffic services, from the end of the take-off and initial climb phase to the commencement of the approach and landing phase.</skos:definition>
		<dct:description xml:lang="en">SOURCE [Route - AIXM5.0].
NOTE A collection of air link sequences and or individual air links that are characterized by one or more thematic identifiers and /or properties, which perform a Route.</dct:description>
		<skos:prefLabel xml:lang="el">SAMPLE ALTERNATIVE EXPRESSION - αναφορά</skos:prefLabel>
		<skos:definition xml:lang="el">Συστήματα συντεταγμένων</skos:definition>
		<dct:description xml:lang="el">Συστήματα για μονοσήμαντη αναφορά χωρικών πληροφοριών στον χώρο, ως σύνολο συντεταγμένων (x,y,z) ή/και γεωγραφικό πλάτος και μήκος και ύψος, με βάση γεωδαιτικό οριζόντιο και κατακόρυφο σύστημα αναφοράς (datum).</dct:description>
		<skos:inScheme rdf:resource="http://inspire-registry.jrc.ec.europa.eu/registers/FCD/items"/>
	</inspire:SpatialObjectType>
	<inspire:SpatialObjectType rdf:about="http://inspire-registry.jrc.ec.europa.eu/registers/FCD/items/314">
		<inspire:itemStatus>valid</inspire:itemStatus>
		<inspire:dateAccepted>2010-01-13T17:18:54.317+01:00</inspire:dateAccepted>
		<skos:prefLabel xml:lang="en">Airspace Area</skos:prefLabel>
		<skos:definition xml:lang="en">A defined volume in the air, described as horizontal projection with vertical limits.</skos:definition>
		<dct:description xml:lang="en">SOURCE [AirspaceVolume - AIXM5.0].
NOTE 1 Definition of Airspace: A defined three dimensional region of space relevant to air traffic [AIXM5.0].
NOTE 2 Airspace regions are managed by air traffic control systems to provide a safe IFR (Instrument Flight Rules) navigation for air traffic services and aircrafts.</dct:description>
		<skos:prefLabel xml:lang="el">SAMPLE ALTERNATIVE EXPRESSION - αναφορά</skos:prefLabel>
		<skos:definition xml:lang="el">Συστήματα συντεταγμένων</skos:definition>
		<dct:description xml:lang="el">Συστήματα για μονοσήμαντη αναφορά χωρικών πληροφοριών στον χώρο, ως σύνολο συντεταγμένων (x,y,z) ή/και γεωγραφικό πλάτος και μήκος και ύψος, με βάση γεωδαιτικό οριζόντιο και κατακόρυφο σύστημα αναφοράς (datum).</dct:description>
		<skos:inScheme rdf:resource="http://inspire-registry.jrc.ec.europa.eu/registers/FCD/items"/>
	</inspire:SpatialObjectType>
	<inspire:SpatialObjectType rdf:about="http://inspire-registry.jrc.ec.europa.eu/registers/FCD/items/315">
		<inspire:itemStatus>valid</inspire:itemStatus>
		<inspire:dateAccepted>2010-01-13T17:18:54.751+01:00</inspire:dateAccepted>
		<skos:prefLabel xml:lang="en">Designated Point</skos:prefLabel>
		<skos:definition xml:lang="en">A geographical location not marked by the site of a radio navigation aid, used in defining an ATS route, the flight path of an aircraft or for other navigation or ATS purposes.</skos:definition>
		<dct:description xml:lang="en">SOURCE [AIXM5.0].
NOTE Examples of Designated points are compulsory and non-compulsory reporting points.</dct:description>
		<skos:prefLabel xml:lang="el">SAMPLE ALTERNATIVE EXPRESSION - αναφορά</skos:prefLabel>
		<skos:definition xml:lang="el">Συστήματα συντεταγμένων</skos:definition>
		<dct:description xml:lang="el">Συστήματα για μονοσήμαντη αναφορά χωρικών πληροφοριών στον χώρο, ως σύνολο συντεταγμένων (x,y,z) ή/και γεωγραφικό πλάτος και μήκος και ύψος, με βάση γεωδαιτικό οριζόντιο και κατακόρυφο σύστημα αναφοράς (datum).</dct:description>
		<skos:inScheme rdf:resource="http://inspire-registry.jrc.ec.europa.eu/registers/FCD/items"/>
	</inspire:SpatialObjectType>
	<inspire:SpatialObjectType rdf:about="http://inspire-registry.jrc.ec.europa.eu/registers/FCD/items/316">
		<inspire:itemStatus>valid</inspire:itemStatus>
		<inspire:dateAccepted>2010-01-13T17:18:55.262+01:00</inspire:dateAccepted>
		<skos:prefLabel xml:lang="en">Runway Area</skos:prefLabel>
		<skos:definition xml:lang="en">A defined rectangular area on a land aerodrome/heliport prepared for the landing and take-off of aircraft.</skos:definition>
		<dct:description xml:lang="en">SOURCE [Runway - AIXM5.0].
NOTE 1 This includes the concept of Final Approach and Take-Off Area (FATO) for helicopters [Runway - AIXM5.0].
NOTE 2 The runway strip is a defined area including the runway and stopway, if provided, intended : a) to reduce the risk of damage to aircraft running off a runway; and b) to protect aircraft flying over it during take-off or landing operations [ICAO].</dct:description>
		<skos:prefLabel xml:lang="el">SAMPLE ALTERNATIVE EXPRESSION - αναφορά</skos:prefLabel>
		<skos:definition xml:lang="el">Συστήματα συντεταγμένων</skos:definition>
		<dct:description xml:lang="el">Συστήματα για μονοσήμαντη αναφορά χωρικών πληροφοριών στον χώρο, ως σύνολο συντεταγμένων (x,y,z) ή/και γεωγραφικό πλάτος και μήκος και ύψος, με βάση γεωδαιτικό οριζόντιο και κατακόρυφο σύστημα αναφοράς (datum).</dct:description>
		<skos:inScheme rdf:resource="http://inspire-registry.jrc.ec.europa.eu/registers/FCD/items"/>
	</inspire:SpatialObjectType>
	<inspire:SpatialObjectType rdf:about="http://inspire-registry.jrc.ec.europa.eu/registers/FCD/items/317">
		<inspire:itemStatus>valid</inspire:itemStatus>
		<inspire:dateAccepted>2010-01-13T17:18:55.755+01:00</inspire:dateAccepted>
		<skos:prefLabel xml:lang="en">Standard Instrument Departure</skos:prefLabel>
		<skos:definition xml:lang="en">A designated instrument flight rule (IFR) departure route linking the aerodrome or a specific runway of the aerodrome with a specified significant point, normally on a designated ATS route, at which the en-route phase of a flight commences.</skos:definition>
		<dct:description xml:lang="en">SOURCE [AIXM5.0].
NOTE 1 Acronym: SID.
NOTE 2 It corresponds to the take-off phase. Each airport/heliport could have various SID linking the different runways to one or various significant points, usually connected to air routes.</dct:description>
		<skos:prefLabel xml:lang="el">SAMPLE ALTERNATIVE EXPRESSION - αναφορά</skos:prefLabel>
		<skos:definition xml:lang="el">Συστήματα συντεταγμένων</skos:definition>
		<dct:description xml:lang="el">Συστήματα για μονοσήμαντη αναφορά χωρικών πληροφοριών στον χώρο, ως σύνολο συντεταγμένων (x,y,z) ή/και γεωγραφικό πλάτος και μήκος και ύψος, με βάση γεωδαιτικό οριζόντιο και κατακόρυφο σύστημα αναφοράς (datum).</dct:description>
		<skos:inScheme rdf:resource="http://inspire-registry.jrc.ec.europa.eu/registers/FCD/items"/>
	</inspire:SpatialObjectType>
	<inspire:SpatialObjectType rdf:about="http://inspire-registry.jrc.ec.europa.eu/registers/FCD/items/318">
		<inspire:itemStatus>valid</inspire:itemStatus>
		<inspire:dateAccepted>2010-01-13T17:18:55.896+01:00</inspire:dateAccepted>
		<skos:prefLabel xml:lang="en">Marker Post</skos:prefLabel>
		<skos:definition xml:lang="en">Reference marker placed along a route in a transport network, mostly at regular intervals, indicating the distance from the beginning of the route, or some other reference point, to the point where the marker is located.</skos:definition>
		<dct:description xml:lang="en">EXAMPLE Examples of routes along which marker posts can be found are roads, railway lines and navigable waterways.</dct:description>
		<skos:prefLabel xml:lang="el">SAMPLE ALTERNATIVE EXPRESSION - αναφορά</skos:prefLabel>
		<skos:definition xml:lang="el">Συστήματα συντεταγμένων</skos:definition>
		<dct:description xml:lang="el">Συστήματα για μονοσήμαντη αναφορά χωρικών πληροφοριών στον χώρο, ως σύνολο συντεταγμένων (x,y,z) ή/και γεωγραφικό πλάτος και μήκος και ύψος, με βάση γεωδαιτικό οριζόντιο και κατακόρυφο σύστημα αναφοράς (datum).</dct:description>
		<skos:inScheme rdf:resource="http://inspire-registry.jrc.ec.europa.eu/registers/FCD/items"/>
	</inspire:SpatialObjectType>
	<inspire:SpatialObjectType rdf:about="http://inspire-registry.jrc.ec.europa.eu/registers/FCD/items/319">
		<inspire:itemStatus>valid</inspire:itemStatus>
		<inspire:dateAccepted>2010-01-13T17:18:56.020+01:00</inspire:dateAccepted>
		<skos:prefLabel xml:lang="en">Transport Link Sequence</skos:prefLabel>
		<skos:definition xml:lang="en">A linear spatial object, composed of an ordered collection of transport links, which represents a continuous path in the transport network without any branches. The element has a defined beginning and end and every position on the transport link sequence is identifiable with one single parameter such as length. It describes an element of the transport network, characterized by one or more thematical identifiers and/or properties.</skos:definition>
		<skos:prefLabel xml:lang="el">SAMPLE ALTERNATIVE EXPRESSION - αναφορά</skos:prefLabel>
		<skos:definition xml:lang="el">Συστήματα συντεταγμένων</skos:definition>
		<dct:description xml:lang="el">Συστήματα για μονοσήμαντη αναφορά χωρικών πληροφοριών στον χώρο, ως σύνολο συντεταγμένων (x,y,z) ή/και γεωγραφικό πλάτος και μήκος και ύψος, με βάση γεωδαιτικό οριζόντιο και κατακόρυφο σύστημα αναφοράς (datum).</dct:description>
		<skos:inScheme rdf:resource="http://inspire-registry.jrc.ec.europa.eu/registers/FCD/items"/>
	</inspire:SpatialObjectType>
	<inspire:SpatialObjectType rdf:about="http://inspire-registry.jrc.ec.europa.eu/registers/FCD/items/320">
		<inspire:itemStatus>valid</inspire:itemStatus>
		<inspire:dateAccepted>2010-01-13T17:18:56.121+01:00</inspire:dateAccepted>
		<skos:prefLabel xml:lang="en">Transport Link Set</skos:prefLabel>
		<skos:definition xml:lang="en">A collection of transport link sequences and or individual transport links that has a specific function or siginificance in a transport network.</skos:definition>
		<dct:description xml:lang="en">NOTE This spatial object type supports the aggregation of links to form objects with branches, loops, parallel sequences of links, gaps, etc.
EXAMPLE A dual carriageway road, as a collection of the two link sequences that represent each carriageway.</dct:description>
		<skos:prefLabel xml:lang="el">SAMPLE ALTERNATIVE EXPRESSION - αναφορά</skos:prefLabel>
		<skos:definition xml:lang="el">Συστήματα συντεταγμένων</skos:definition>
		<dct:description xml:lang="el">Συστήματα για μονοσήμαντη αναφορά χωρικών πληροφοριών στον χώρο, ως σύνολο συντεταγμένων (x,y,z) ή/και γεωγραφικό πλάτος και μήκος και ύψος, με βάση γεωδαιτικό οριζόντιο και κατακόρυφο σύστημα αναφοράς (datum).</dct:description>
		<skos:inScheme rdf:resource="http://inspire-registry.jrc.ec.europa.eu/registers/FCD/items"/>
	</inspire:SpatialObjectType>
	<inspire:SpatialObjectType rdf:about="http://inspire-registry.jrc.ec.europa.eu/registers/FCD/items/321">
		<inspire:itemStatus>valid</inspire:itemStatus>
		<inspire:dateAccepted>2010-01-13T17:18:56.246+01:00</inspire:dateAccepted>
		<skos:prefLabel xml:lang="en">Transport Network</skos:prefLabel>
		<skos:definition xml:lang="en">Collection of network elements that belong to a single mode of transport.</skos:definition>
		<dct:description xml:lang="en">NOTE Road, rail, water and air transport are always considered separate transport modes. Even within these four categories, multiple modes of transport can be defined, based on infrastructure, vehicle types, propulsion system,
operation and/or other defining characteristics.
EXAMPLE All road transport can be considered one mode of transport for some applications. For other applications, it might be necessary to distinguish between different public road transport networks. Within water transport, marine and
inland water transport can be considered to be separate modes of transport for some applications, as they use different types of ships.</dct:description>
		<skos:prefLabel xml:lang="el">SAMPLE ALTERNATIVE EXPRESSION - αναφορά</skos:prefLabel>
		<skos:definition xml:lang="el">Συστήματα συντεταγμένων</skos:definition>
		<dct:description xml:lang="el">Συστήματα για μονοσήμαντη αναφορά χωρικών πληροφοριών στον χώρο, ως σύνολο συντεταγμένων (x,y,z) ή/και γεωγραφικό πλάτος και μήκος και ύψος, με βάση γεωδαιτικό οριζόντιο και κατακόρυφο σύστημα αναφοράς (datum).</dct:description>
		<skos:inScheme rdf:resource="http://inspire-registry.jrc.ec.europa.eu/registers/FCD/items"/>
	</inspire:SpatialObjectType>
	<inspire:SpatialObjectType rdf:about="http://inspire-registry.jrc.ec.europa.eu/registers/FCD/items/322">
		<inspire:itemStatus>valid</inspire:itemStatus>
		<inspire:dateAccepted>2010-01-13T17:18:56.363+01:00</inspire:dateAccepted>
		<skos:prefLabel xml:lang="en">Transport Object</skos:prefLabel>
		<skos:definition xml:lang="en">An identity base for transport network objects in the real world.</skos:definition>
		<dct:description xml:lang="en">NOTE Derived 'views' of real-world transport objects are represented through specialisations in other application schemas; all representations of the same real-world object share a common geographic name.</dct:description>
		<skos:prefLabel xml:lang="el">SAMPLE ALTERNATIVE EXPRESSION - αναφορά</skos:prefLabel>
		<skos:definition xml:lang="el">Συστήματα συντεταγμένων</skos:definition>
		<dct:description xml:lang="el">Συστήματα για μονοσήμαντη αναφορά χωρικών πληροφοριών στον χώρο, ως σύνολο συντεταγμένων (x,y,z) ή/και γεωγραφικό πλάτος και μήκος και ύψος, με βάση γεωδαιτικό οριζόντιο και κατακόρυφο σύστημα αναφοράς (datum).</dct:description>
		<skos:inScheme rdf:resource="http://inspire-registry.jrc.ec.europa.eu/registers/FCD/items"/>
	</inspire:SpatialObjectType>
	<inspire:SpatialObjectType rdf:about="http://inspire-registry.jrc.ec.europa.eu/registers/FCD/items/323">
		<inspire:itemStatus>valid</inspire:itemStatus>
		<inspire:dateAccepted>2010-01-13T17:18:56.485+01:00</inspire:dateAccepted>
		<skos:prefLabel xml:lang="en">Transport Point</skos:prefLabel>
		<skos:definition xml:lang="en">A point spatial object - which is not a node - that represents the position of an element of a transport network.</skos:definition>
		<skos:prefLabel xml:lang="el">SAMPLE ALTERNATIVE EXPRESSION - αναφορά</skos:prefLabel>
		<skos:definition xml:lang="el">Συστήματα συντεταγμένων</skos:definition>
		<dct:description xml:lang="el">Συστήματα για μονοσήμαντη αναφορά χωρικών πληροφοριών στον χώρο, ως σύνολο συντεταγμένων (x,y,z) ή/και γεωγραφικό πλάτος και μήκος και ύψος, με βάση γεωδαιτικό οριζόντιο και κατακόρυφο σύστημα αναφοράς (datum).</dct:description>
		<skos:inScheme rdf:resource="http://inspire-registry.jrc.ec.europa.eu/registers/FCD/items"/>
	</inspire:SpatialObjectType>
	<inspire:SpatialObjectType rdf:about="http://inspire-registry.jrc.ec.europa.eu/registers/FCD/items/324">
		<inspire:itemStatus>valid</inspire:itemStatus>
		<inspire:dateAccepted>2010-01-13T17:18:56.652+01:00</inspire:dateAccepted>
		<skos:prefLabel xml:lang="en">Vertical Position</skos:prefLabel>
		<skos:definition xml:lang="en">Vertical level relative to other transport network elements.</skos:definition>
		<skos:prefLabel xml:lang="el">SAMPLE ALTERNATIVE EXPRESSION - αναφορά</skos:prefLabel>
		<skos:definition xml:lang="el">Συστήματα συντεταγμένων</skos:definition>
		<dct:description xml:lang="el">Συστήματα για μονοσήμαντη αναφορά χωρικών πληροφοριών στον χώρο, ως σύνολο συντεταγμένων (x,y,z) ή/και γεωγραφικό πλάτος και μήκος και ύψος, με βάση γεωδαιτικό οριζόντιο και κατακόρυφο σύστημα αναφοράς (datum).</dct:description>
		<skos:inScheme rdf:resource="http://inspire-registry.jrc.ec.europa.eu/registers/FCD/items"/>
	</inspire:SpatialObjectType>
	<inspire:SpatialObjectType rdf:about="http://inspire-registry.jrc.ec.europa.eu/registers/FCD/items/325">
		<inspire:itemStatus>valid</inspire:itemStatus>
		<inspire:dateAccepted>2010-01-13T17:18:56.782+01:00</inspire:dateAccepted>
		<skos:prefLabel xml:lang="en">E-road</skos:prefLabel>
		<skos:definition xml:lang="en">A collection of road link sequences and or individual road links that represents a route that is part of the international E-road network, characterized by its European route number.</skos:definition>
		<dct:description xml:lang="en">EXAMPLE E40.</dct:description>
		<skos:prefLabel xml:lang="el">SAMPLE ALTERNATIVE EXPRESSION - αναφορά</skos:prefLabel>
		<skos:definition xml:lang="el">Συστήματα συντεταγμένων</skos:definition>
		<dct:description xml:lang="el">Συστήματα για μονοσήμαντη αναφορά χωρικών πληροφοριών στον χώρο, ως σύνολο συντεταγμένων (x,y,z) ή/και γεωγραφικό πλάτος και μήκος και ύψος, με βάση γεωδαιτικό οριζόντιο και κατακόρυφο σύστημα αναφοράς (datum).</dct:description>
		<skos:inScheme rdf:resource="http://inspire-registry.jrc.ec.europa.eu/registers/FCD/items"/>
	</inspire:SpatialObjectType>
	<inspire:SpatialObjectType rdf:about="http://inspire-registry.jrc.ec.europa.eu/registers/FCD/items/326">
		<inspire:itemStatus>valid</inspire:itemStatus>
		<inspire:dateAccepted>2010-01-13T17:18:56.909+01:00</inspire:dateAccepted>
		<skos:prefLabel xml:lang="en">Road Link Sequence</skos:prefLabel>
		<skos:definition xml:lang="en">A linear spatial object, composed of an ordered collection of road links, which represents a continuous path in a road network without any branches. The element has a defined beginning and end and every position on the road link sequence is identifiable with one single parameter such as length. It describes an element of the road network, characterized by one or more thematic identifiers and/or properties.</skos:definition>
		<skos:prefLabel xml:lang="el">SAMPLE ALTERNATIVE EXPRESSION - αναφορά</skos:prefLabel>
		<skos:definition xml:lang="el">Συστήματα συντεταγμένων</skos:definition>
		<dct:description xml:lang="el">Συστήματα για μονοσήμαντη αναφορά χωρικών πληροφοριών στον χώρο, ως σύνολο συντεταγμένων (x,y,z) ή/και γεωγραφικό πλάτος και μήκος και ύψος, με βάση γεωδαιτικό οριζόντιο και κατακόρυφο σύστημα αναφοράς (datum).</dct:description>
		<skos:inScheme rdf:resource="http://inspire-registry.jrc.ec.europa.eu/registers/FCD/items"/>
	</inspire:SpatialObjectType>
	<inspire:SpatialObjectType rdf:about="http://inspire-registry.jrc.ec.europa.eu/registers/FCD/items/327">
		<inspire:itemStatus>valid</inspire:itemStatus>
		<inspire:dateAccepted>2010-01-13T17:18:57.022+01:00</inspire:dateAccepted>
		<skos:prefLabel xml:lang="en">Road Name</skos:prefLabel>
		<skos:definition xml:lang="en">Name of a road, as assigned by the responsible authority.</skos:definition>
		<skos:prefLabel xml:lang="el">SAMPLE ALTERNATIVE EXPRESSION - αναφορά</skos:prefLabel>
		<skos:definition xml:lang="el">Συστήματα συντεταγμένων</skos:definition>
		<dct:description xml:lang="el">Συστήματα για μονοσήμαντη αναφορά χωρικών πληροφοριών στον χώρο, ως σύνολο συντεταγμένων (x,y,z) ή/και γεωγραφικό πλάτος και μήκος και ύψος, με βάση γεωδαιτικό οριζόντιο και κατακόρυφο σύστημα αναφοράς (datum).</dct:description>
		<skos:inScheme rdf:resource="http://inspire-registry.jrc.ec.europa.eu/registers/FCD/items"/>
	</inspire:SpatialObjectType>
	<inspire:SpatialObjectType rdf:about="http://inspire-registry.jrc.ec.europa.eu/registers/FCD/items/328">
		<inspire:itemStatus>valid</inspire:itemStatus>
		<inspire:dateAccepted>2010-01-13T17:18:57.148+01:00</inspire:dateAccepted>
		<skos:prefLabel xml:lang="en">Road Service Type</skos:prefLabel>
		<skos:definition xml:lang="en">Description of the type of road service area and the available facilities.</skos:definition>
		<skos:prefLabel xml:lang="el">SAMPLE ALTERNATIVE EXPRESSION - αναφορά</skos:prefLabel>
		<skos:definition xml:lang="el">Συστήματα συντεταγμένων</skos:definition>
		<dct:description xml:lang="el">Συστήματα για μονοσήμαντη αναφορά χωρικών πληροφοριών στον χώρο, ως σύνολο συντεταγμένων (x,y,z) ή/και γεωγραφικό πλάτος και μήκος και ύψος, με βάση γεωδαιτικό οριζόντιο και κατακόρυφο σύστημα αναφοράς (datum).</dct:description>
		<skos:inScheme rdf:resource="http://inspire-registry.jrc.ec.europa.eu/registers/FCD/items"/>
	</inspire:SpatialObjectType>
	<inspire:SpatialObjectType rdf:about="http://inspire-registry.jrc.ec.europa.eu/registers/FCD/items/329">
		<inspire:itemStatus>valid</inspire:itemStatus>
		<inspire:dateAccepted>2010-01-13T17:18:57.287+01:00</inspire:dateAccepted>
		<skos:prefLabel xml:lang="en">Design Speed</skos:prefLabel>
		<skos:definition xml:lang="en">The specification of the maximum speed to which a railway line is designed for.</skos:definition>
		<skos:prefLabel xml:lang="el">SAMPLE ALTERNATIVE EXPRESSION - αναφορά</skos:prefLabel>
		<skos:definition xml:lang="el">Συστήματα συντεταγμένων</skos:definition>
		<dct:description xml:lang="el">Συστήματα για μονοσήμαντη αναφορά χωρικών πληροφοριών στον χώρο, ως σύνολο συντεταγμένων (x,y,z) ή/και γεωγραφικό πλάτος και μήκος και ύψος, με βάση γεωδαιτικό οριζόντιο και κατακόρυφο σύστημα αναφοράς (datum).</dct:description>
		<skos:inScheme rdf:resource="http://inspire-registry.jrc.ec.europa.eu/registers/FCD/items"/>
	</inspire:SpatialObjectType>
	<inspire:SpatialObjectType rdf:about="http://inspire-registry.jrc.ec.europa.eu/registers/FCD/items/330">
		<inspire:itemStatus>valid</inspire:itemStatus>
		<inspire:dateAccepted>2010-01-13T17:18:57.424+01:00</inspire:dateAccepted>
		<skos:prefLabel xml:lang="en">Number of Tracks</skos:prefLabel>
		<skos:definition xml:lang="en">The number of tracks for a railway stretch.</skos:definition>
		<dct:description xml:lang="en">This is dependent on the resolution of the data.</dct:description>
		<skos:prefLabel xml:lang="el">SAMPLE ALTERNATIVE EXPRESSION - αναφορά</skos:prefLabel>
		<skos:definition xml:lang="el">Συστήματα συντεταγμένων</skos:definition>
		<dct:description xml:lang="el">Συστήματα για μονοσήμαντη αναφορά χωρικών πληροφοριών στον χώρο, ως σύνολο συντεταγμένων (x,y,z) ή/και γεωγραφικό πλάτος και μήκος και ύψος, με βάση γεωδαιτικό οριζόντιο και κατακόρυφο σύστημα αναφοράς (datum).</dct:description>
		<skos:inScheme rdf:resource="http://inspire-registry.jrc.ec.europa.eu/registers/FCD/items"/>
	</inspire:SpatialObjectType>
	<inspire:SpatialObjectType rdf:about="http://inspire-registry.jrc.ec.europa.eu/registers/FCD/items/331">
		<inspire:itemStatus>valid</inspire:itemStatus>
		<inspire:dateAccepted>2010-01-13T17:18:57.596+01:00</inspire:dateAccepted>
		<skos:prefLabel xml:lang="en">Railway Area</skos:prefLabel>
		<skos:definition xml:lang="en">Surface occupied by a railway track, including ballast.</skos:definition>
		<skos:prefLabel xml:lang="el">SAMPLE ALTERNATIVE EXPRESSION - αναφορά</skos:prefLabel>
		<skos:definition xml:lang="el">Συστήματα συντεταγμένων</skos:definition>
		<dct:description xml:lang="el">Συστήματα για μονοσήμαντη αναφορά χωρικών πληροφοριών στον χώρο, ως σύνολο συντεταγμένων (x,y,z) ή/και γεωγραφικό πλάτος και μήκος και ύψος, με βάση γεωδαιτικό οριζόντιο και κατακόρυφο σύστημα αναφοράς (datum).</dct:description>
		<skos:inScheme rdf:resource="http://inspire-registry.jrc.ec.europa.eu/registers/FCD/items"/>
	</inspire:SpatialObjectType>
	<inspire:SpatialObjectType rdf:about="http://inspire-registry.jrc.ec.europa.eu/registers/FCD/items/332">
		<inspire:itemStatus>valid</inspire:itemStatus>
		<inspire:dateAccepted>2010-01-13T17:18:57.726+01:00</inspire:dateAccepted>
		<skos:prefLabel xml:lang="en">Railway Electrification</skos:prefLabel>
		<skos:definition xml:lang="en">Indication whether the railway is provided with an electric system to power vehicles moving along it.</skos:definition>
		<skos:prefLabel xml:lang="el">SAMPLE ALTERNATIVE EXPRESSION - αναφορά</skos:prefLabel>
		<skos:definition xml:lang="el">Συστήματα συντεταγμένων</skos:definition>
		<dct:description xml:lang="el">Συστήματα για μονοσήμαντη αναφορά χωρικών πληροφοριών στον χώρο, ως σύνολο συντεταγμένων (x,y,z) ή/και γεωγραφικό πλάτος και μήκος και ύψος, με βάση γεωδαιτικό οριζόντιο και κατακόρυφο σύστημα αναφοράς (datum).</dct:description>
		<skos:inScheme rdf:resource="http://inspire-registry.jrc.ec.europa.eu/registers/FCD/items"/>
	</inspire:SpatialObjectType>
	<inspire:SpatialObjectType rdf:about="http://inspire-registry.jrc.ec.europa.eu/registers/FCD/items/333">
		<inspire:itemStatus>valid</inspire:itemStatus>
		<inspire:dateAccepted>2010-01-13T17:18:57.848+01:00</inspire:dateAccepted>
		<skos:prefLabel xml:lang="en">Railway Link Sequence</skos:prefLabel>
		<skos:definition xml:lang="en">A linear spatial object, composed of an ordered collection of railway links, which represents a continuous path in a railway network without any branches. The element has a defined beginning and end and every position on the railway link sequence is identifiable with one single parameter such as length. It describes an element of the railway network, characterized by one or more thematical identifiers and/or properties.</skos:definition>
		<skos:prefLabel xml:lang="el">SAMPLE ALTERNATIVE EXPRESSION - αναφορά</skos:prefLabel>
		<skos:definition xml:lang="el">Συστήματα συντεταγμένων</skos:definition>
		<dct:description xml:lang="el">Συστήματα για μονοσήμαντη αναφορά χωρικών πληροφοριών στον χώρο, ως σύνολο συντεταγμένων (x,y,z) ή/και γεωγραφικό πλάτος και μήκος και ύψος, με βάση γεωδαιτικό οριζόντιο και κατακόρυφο σύστημα αναφοράς (datum).</dct:description>
		<skos:inScheme rdf:resource="http://inspire-registry.jrc.ec.europa.eu/registers/FCD/items"/>
	</inspire:SpatialObjectType>
	<inspire:SpatialObjectType rdf:about="http://inspire-registry.jrc.ec.europa.eu/registers/FCD/items/334">
		<inspire:itemStatus>valid</inspire:itemStatus>
		<inspire:dateAccepted>2010-01-13T17:18:57.974+01:00</inspire:dateAccepted>
		<skos:prefLabel xml:lang="en">Railway Type</skos:prefLabel>
		<skos:definition xml:lang="en">The type of railway transport the line is designed for.</skos:definition>
		<skos:prefLabel xml:lang="el">SAMPLE ALTERNATIVE EXPRESSION - αναφορά</skos:prefLabel>
		<skos:definition xml:lang="el">Συστήματα συντεταγμένων</skos:definition>
		<dct:description xml:lang="el">Συστήματα για μονοσήμαντη αναφορά χωρικών πληροφοριών στον χώρο, ως σύνολο συντεταγμένων (x,y,z) ή/και γεωγραφικό πλάτος και μήκος και ύψος, με βάση γεωδαιτικό οριζόντιο και κατακόρυφο σύστημα αναφοράς (datum).</dct:description>
		<skos:inScheme rdf:resource="http://inspire-registry.jrc.ec.europa.eu/registers/FCD/items"/>
	</inspire:SpatialObjectType>
	<inspire:SpatialObjectType rdf:about="http://inspire-registry.jrc.ec.europa.eu/registers/FCD/items/335">
		<inspire:itemStatus>valid</inspire:itemStatus>
		<inspire:dateAccepted>2010-01-13T17:18:58.088+01:00</inspire:dateAccepted>
		<skos:prefLabel xml:lang="en">Cableway Link Sequence</skos:prefLabel>
		<skos:definition xml:lang="en">An ordered collection of cableway links that are characterized by one or more thematic identifiers and/or properties.</skos:definition>
		<skos:prefLabel xml:lang="el">SAMPLE ALTERNATIVE EXPRESSION - αναφορά</skos:prefLabel>
		<skos:definition xml:lang="el">Συστήματα συντεταγμένων</skos:definition>
		<dct:description xml:lang="el">Συστήματα για μονοσήμαντη αναφορά χωρικών πληροφοριών στον χώρο, ως σύνολο συντεταγμένων (x,y,z) ή/και γεωγραφικό πλάτος και μήκος και ύψος, με βάση γεωδαιτικό οριζόντιο και κατακόρυφο σύστημα αναφοράς (datum).</dct:description>
		<skos:inScheme rdf:resource="http://inspire-registry.jrc.ec.europa.eu/registers/FCD/items"/>
	</inspire:SpatialObjectType>
	<inspire:SpatialObjectType rdf:about="http://inspire-registry.jrc.ec.europa.eu/registers/FCD/items/336">
		<inspire:itemStatus>valid</inspire:itemStatus>
		<inspire:dateAccepted>2010-01-13T17:18:58.221+01:00</inspire:dateAccepted>
		<skos:prefLabel xml:lang="en">Cableway Link Set</skos:prefLabel>
		<skos:definition xml:lang="en">A collection of cableway link sequences and or individual cableway links that has a specific function or significance in a cable transport network.</skos:definition>
		<skos:prefLabel xml:lang="el">SAMPLE ALTERNATIVE EXPRESSION - αναφορά</skos:prefLabel>
		<skos:definition xml:lang="el">Συστήματα συντεταγμένων</skos:definition>
		<dct:description xml:lang="el">Συστήματα για μονοσήμαντη αναφορά χωρικών πληροφοριών στον χώρο, ως σύνολο συντεταγμένων (x,y,z) ή/και γεωγραφικό πλάτος και μήκος και ύψος, με βάση γεωδαιτικό οριζόντιο και κατακόρυφο σύστημα αναφοράς (datum).</dct:description>
		<skos:inScheme rdf:resource="http://inspire-registry.jrc.ec.europa.eu/registers/FCD/items"/>
	</inspire:SpatialObjectType>
	<inspire:SpatialObjectType rdf:about="http://inspire-registry.jrc.ec.europa.eu/registers/FCD/items/337">
		<inspire:itemStatus>valid</inspire:itemStatus>
		<inspire:dateAccepted>2010-01-13T17:18:58.391+01:00</inspire:dateAccepted>
		<skos:prefLabel xml:lang="en">Beacon</skos:prefLabel>
		<skos:definition xml:lang="en">A prominent specially constructed object forming a conspicuous mark as a fixed aid to navigation, or for use in hydrographic survey.</skos:definition>
		<dct:description xml:lang="en">SOURCE [S-32 - IHO International Hydrographic Dictionary].</dct:description>
		<skos:prefLabel xml:lang="el">SAMPLE ALTERNATIVE EXPRESSION - αναφορά</skos:prefLabel>
		<skos:definition xml:lang="el">Συστήματα συντεταγμένων</skos:definition>
		<dct:description xml:lang="el">Συστήματα για μονοσήμαντη αναφορά χωρικών πληροφοριών στον χώρο, ως σύνολο συντεταγμένων (x,y,z) ή/και γεωγραφικό πλάτος και μήκος και ύψος, με βάση γεωδαιτικό οριζόντιο και κατακόρυφο σύστημα αναφοράς (datum).</dct:description>
		<skos:inScheme rdf:resource="http://inspire-registry.jrc.ec.europa.eu/registers/FCD/items"/>
	</inspire:SpatialObjectType>
	<inspire:SpatialObjectType rdf:about="http://inspire-registry.jrc.ec.europa.eu/registers/FCD/items/338">
		<inspire:itemStatus>valid</inspire:itemStatus>
		<inspire:dateAccepted>2010-01-13T17:18:58.580+01:00</inspire:dateAccepted>
		<skos:prefLabel xml:lang="en">Buoy</skos:prefLabel>
		<skos:definition xml:lang="en">A floating object moored to the bottom in a particular (charted) place, as an aid to navigation or for other specific purposes.</skos:definition>
		<dct:description xml:lang="en">SOURCE [S-32 - IHO International Hydrographic Dictionary]
NOTE Navigational buoys may be classified according to: (a) their shape, appearance, or construction, such as barrel, can, cask, conical, cylindrical, dan, keg, nun, pillar, spar, spherical, or topmark buoy; (b) their colour, such as black, chequered, green, red buoy; (c) their location, such as bifurcation, fairway, junction, mid-channel, middle-ground, or turning buoy; (d) the various kinds of hazards or dangers to navigation which they mark, such as bar, isolated danger, fish trap, obstruction, spoil ground, telegraph or wreck buoy; (e) their particular purpose or use, such as anchor, anchorage, compass adjustment, dredging, farewell (or landfall), marker, quarantine, station (or watch), or warping buoy. [S-32 - IHO International Hydrographic Dictionary].</dct:description>
		<skos:prefLabel xml:lang="el">SAMPLE ALTERNATIVE EXPRESSION - αναφορά</skos:prefLabel>
		<skos:definition xml:lang="el">Συστήματα συντεταγμένων</skos:definition>
		<dct:description xml:lang="el">Συστήματα για μονοσήμαντη αναφορά χωρικών πληροφοριών στον χώρο, ως σύνολο συντεταγμένων (x,y,z) ή/και γεωγραφικό πλάτος και μήκος και ύψος, με βάση γεωδαιτικό οριζόντιο και κατακόρυφο σύστημα αναφοράς (datum).</dct:description>
		<skos:inScheme rdf:resource="http://inspire-registry.jrc.ec.europa.eu/registers/FCD/items"/>
	</inspire:SpatialObjectType>
	<inspire:SpatialObjectType rdf:about="http://inspire-registry.jrc.ec.europa.eu/registers/FCD/items/339">
		<inspire:itemStatus>valid</inspire:itemStatus>
		<inspire:dateAccepted>2010-01-13T17:18:58.722+01:00</inspire:dateAccepted>
		<skos:prefLabel xml:lang="en">CEMT Class</skos:prefLabel>
		<skos:definition xml:lang="en">Classification of an inland waterway according to CEMT (European Conference of Ministers of Transport).</skos:definition>
		<skos:prefLabel xml:lang="el">SAMPLE ALTERNATIVE EXPRESSION - αναφορά</skos:prefLabel>
		<skos:definition xml:lang="el">Συστήματα συντεταγμένων</skos:definition>
		<dct:description xml:lang="el">Συστήματα για μονοσήμαντη αναφορά χωρικών πληροφοριών στον χώρο, ως σύνολο συντεταγμένων (x,y,z) ή/και γεωγραφικό πλάτος και μήκος και ύψος, με βάση γεωδαιτικό οριζόντιο και κατακόρυφο σύστημα αναφοράς (datum).</dct:description>
		<skos:inScheme rdf:resource="http://inspire-registry.jrc.ec.europa.eu/registers/FCD/items"/>
	</inspire:SpatialObjectType>
	<inspire:SpatialObjectType rdf:about="http://inspire-registry.jrc.ec.europa.eu/registers/FCD/items/340">
		<inspire:itemStatus>valid</inspire:itemStatus>
		<inspire:dateAccepted>2010-01-13T17:18:58.858+01:00</inspire:dateAccepted>
		<skos:prefLabel xml:lang="en">Condition of Water Facility</skos:prefLabel>
		<skos:definition xml:lang="en">State of a water transport network element with regards to its completion and use.</skos:definition>
		<skos:prefLabel xml:lang="el">SAMPLE ALTERNATIVE EXPRESSION - αναφορά</skos:prefLabel>
		<skos:definition xml:lang="el">Συστήματα συντεταγμένων</skos:definition>
		<dct:description xml:lang="el">Συστήματα για μονοσήμαντη αναφορά χωρικών πληροφοριών στον χώρο, ως σύνολο συντεταγμένων (x,y,z) ή/και γεωγραφικό πλάτος και μήκος και ύψος, με βάση γεωδαιτικό οριζόντιο και κατακόρυφο σύστημα αναφοράς (datum).</dct:description>
		<skos:inScheme rdf:resource="http://inspire-registry.jrc.ec.europa.eu/registers/FCD/items"/>
	</inspire:SpatialObjectType>
	<inspire:SpatialObjectType rdf:about="http://inspire-registry.jrc.ec.europa.eu/registers/FCD/items/341">
		<inspire:itemStatus>valid</inspire:itemStatus>
		<inspire:dateAccepted>2010-01-13T17:18:59.025+01:00</inspire:dateAccepted>
		<skos:prefLabel xml:lang="en">Fairway Area</skos:prefLabel>
		<skos:definition xml:lang="en">The main travelled part of a waterway.</skos:definition>
		<dct:description xml:lang="en">SOURCE [International Hydrographic Dictionary].
NOTE That part of a river, harbour and so on, where the main navigable channel for vessels of larger size lies. It is also the usual course followed by vessels entering or leaving harbours, called 'ship channel' [IHO Hidrographic Registry].</dct:description>
		<skos:prefLabel xml:lang="el">SAMPLE ALTERNATIVE EXPRESSION - αναφορά</skos:prefLabel>
		<skos:definition xml:lang="el">Συστήματα συντεταγμένων</skos:definition>
		<dct:description xml:lang="el">Συστήματα για μονοσήμαντη αναφορά χωρικών πληροφοριών στον χώρο, ως σύνολο συντεταγμένων (x,y,z) ή/και γεωγραφικό πλάτος και μήκος και ύψος, με βάση γεωδαιτικό οριζόντιο και κατακόρυφο σύστημα αναφοράς (datum).</dct:description>
		<skos:inScheme rdf:resource="http://inspire-registry.jrc.ec.europa.eu/registers/FCD/items"/>
	</inspire:SpatialObjectType>
	<inspire:SpatialObjectType rdf:about="http://inspire-registry.jrc.ec.europa.eu/registers/FCD/items/342">
		<inspire:itemStatus>valid</inspire:itemStatus>
		<inspire:dateAccepted>2010-01-13T17:18:59.171+01:00</inspire:dateAccepted>
		<skos:prefLabel xml:lang="en">Ferry Use</skos:prefLabel>
		<skos:definition xml:lang="en">The type of transport carried out by a ferry crossing.</skos:definition>
		<skos:prefLabel xml:lang="el">SAMPLE ALTERNATIVE EXPRESSION - αναφορά</skos:prefLabel>
		<skos:definition xml:lang="el">Συστήματα συντεταγμένων</skos:definition>
		<dct:description xml:lang="el">Συστήματα για μονοσήμαντη αναφορά χωρικών πληροφοριών στον χώρο, ως σύνολο συντεταγμένων (x,y,z) ή/και γεωγραφικό πλάτος και μήκος και ύψος, με βάση γεωδαιτικό οριζόντιο και κατακόρυφο σύστημα αναφοράς (datum).</dct:description>
		<skos:inScheme rdf:resource="http://inspire-registry.jrc.ec.europa.eu/registers/FCD/items"/>
	</inspire:SpatialObjectType>
	<inspire:SpatialObjectType rdf:about="http://inspire-registry.jrc.ec.europa.eu/registers/FCD/items/343">
		<inspire:itemStatus>valid</inspire:itemStatus>
		<inspire:dateAccepted>2010-01-13T17:18:59.306+01:00</inspire:dateAccepted>
		<skos:prefLabel xml:lang="en">Inland Waterway</skos:prefLabel>
		<skos:definition xml:lang="en">Waterway which is defined at inland continental waters.</skos:definition>
		<dct:description xml:lang="en">EXAMPLE The inland waterways classified by the CEMT (European Conference of Ministers of Transport).</dct:description>
		<skos:prefLabel xml:lang="el">SAMPLE ALTERNATIVE EXPRESSION - αναφορά</skos:prefLabel>
		<skos:definition xml:lang="el">Συστήματα συντεταγμένων</skos:definition>
		<dct:description xml:lang="el">Συστήματα για μονοσήμαντη αναφορά χωρικών πληροφοριών στον χώρο, ως σύνολο συντεταγμένων (x,y,z) ή/και γεωγραφικό πλάτος και μήκος και ύψος, με βάση γεωδαιτικό οριζόντιο και κατακόρυφο σύστημα αναφοράς (datum).</dct:description>
		<skos:inScheme rdf:resource="http://inspire-registry.jrc.ec.europa.eu/registers/FCD/items"/>
	</inspire:SpatialObjectType>
	<inspire:SpatialObjectType rdf:about="http://inspire-registry.jrc.ec.europa.eu/registers/FCD/items/344">
		<inspire:itemStatus>valid</inspire:itemStatus>
		<inspire:dateAccepted>2010-01-13T17:18:59.441+01:00</inspire:dateAccepted>
		<skos:prefLabel xml:lang="en">Marine Waterway</skos:prefLabel>
		<skos:definition xml:lang="en">Waterway which is defined at sea waters.</skos:definition>
		<skos:prefLabel xml:lang="el">SAMPLE ALTERNATIVE EXPRESSION - αναφορά</skos:prefLabel>
		<skos:definition xml:lang="el">Συστήματα συντεταγμένων</skos:definition>
		<dct:description xml:lang="el">Συστήματα για μονοσήμαντη αναφορά χωρικών πληροφοριών στον χώρο, ως σύνολο συντεταγμένων (x,y,z) ή/και γεωγραφικό πλάτος και μήκος και ύψος, με βάση γεωδαιτικό οριζόντιο και κατακόρυφο σύστημα αναφοράς (datum).</dct:description>
		<skos:inScheme rdf:resource="http://inspire-registry.jrc.ec.europa.eu/registers/FCD/items"/>
	</inspire:SpatialObjectType>
	<inspire:SpatialObjectType rdf:about="http://inspire-registry.jrc.ec.europa.eu/registers/FCD/items/345">
		<inspire:itemStatus>valid</inspire:itemStatus>
		<inspire:dateAccepted>2010-01-13T17:18:59.570+01:00</inspire:dateAccepted>
		<skos:prefLabel xml:lang="en">Restriction for Water Vehicles</skos:prefLabel>
		<skos:definition xml:lang="en">Restriction on vehicles on a water transport element.</skos:definition>
		<skos:prefLabel xml:lang="el">SAMPLE ALTERNATIVE EXPRESSION - αναφορά</skos:prefLabel>
		<skos:definition xml:lang="el">Συστήματα συντεταγμένων</skos:definition>
		<dct:description xml:lang="el">Συστήματα για μονοσήμαντη αναφορά χωρικών πληροφοριών στον χώρο, ως σύνολο συντεταγμένων (x,y,z) ή/και γεωγραφικό πλάτος και μήκος και ύψος, με βάση γεωδαιτικό οριζόντιο και κατακόρυφο σύστημα αναφοράς (datum).</dct:description>
		<skos:inScheme rdf:resource="http://inspire-registry.jrc.ec.europa.eu/registers/FCD/items"/>
	</inspire:SpatialObjectType>
	<inspire:SpatialObjectType rdf:about="http://inspire-registry.jrc.ec.europa.eu/registers/FCD/items/346">
		<inspire:itemStatus>valid</inspire:itemStatus>
		<inspire:dateAccepted>2010-01-13T17:18:59.723+01:00</inspire:dateAccepted>
		<skos:prefLabel xml:lang="en">Traffic Separation Scheme</skos:prefLabel>
		<skos:definition xml:lang="en">A scheme which aims at reducing the risk of collision in congested and/or converging areas by separating traffic moving in opposite, or nearly opposite, directions.</skos:definition>
		<dct:description xml:lang="en">SOURCE [S-32 - IHO International Hydrographic Dictionary]
NOTE 1 Acronym: TSS.
NOTE 2 TSSs constitute main components of maritime routing measures for hydrographic transport.</dct:description>
		<skos:prefLabel xml:lang="el">SAMPLE ALTERNATIVE EXPRESSION - αναφορά</skos:prefLabel>
		<skos:definition xml:lang="el">Συστήματα συντεταγμένων</skos:definition>
		<dct:description xml:lang="el">Συστήματα για μονοσήμαντη αναφορά χωρικών πληροφοριών στον χώρο, ως σύνολο συντεταγμένων (x,y,z) ή/και γεωγραφικό πλάτος και μήκος και ύψος, με βάση γεωδαιτικό οριζόντιο και κατακόρυφο σύστημα αναφοράς (datum).</dct:description>
		<skos:inScheme rdf:resource="http://inspire-registry.jrc.ec.europa.eu/registers/FCD/items"/>
	</inspire:SpatialObjectType>
	<inspire:SpatialObjectType rdf:about="http://inspire-registry.jrc.ec.europa.eu/registers/FCD/items/347">
		<inspire:itemStatus>valid</inspire:itemStatus>
		<inspire:dateAccepted>2010-01-13T17:18:59.842+01:00</inspire:dateAccepted>
		<skos:prefLabel xml:lang="en">Traffic Separation Scheme Area</skos:prefLabel>
		<skos:definition xml:lang="en">An area spatial object forming part of a traffic seperation scheme.</skos:definition>
		<skos:prefLabel xml:lang="el">SAMPLE ALTERNATIVE EXPRESSION - αναφορά</skos:prefLabel>
		<skos:definition xml:lang="el">Συστήματα συντεταγμένων</skos:definition>
		<dct:description xml:lang="el">Συστήματα για μονοσήμαντη αναφορά χωρικών πληροφοριών στον χώρο, ως σύνολο συντεταγμένων (x,y,z) ή/και γεωγραφικό πλάτος και μήκος και ύψος, με βάση γεωδαιτικό οριζόντιο και κατακόρυφο σύστημα αναφοράς (datum).</dct:description>
		<skos:inScheme rdf:resource="http://inspire-registry.jrc.ec.europa.eu/registers/FCD/items"/>
	</inspire:SpatialObjectType>
	<inspire:SpatialObjectType rdf:about="http://inspire-registry.jrc.ec.europa.eu/registers/FCD/items/348">
		<inspire:itemStatus>valid</inspire:itemStatus>
		<inspire:dateAccepted>2010-01-13T17:18:59.988+01:00</inspire:dateAccepted>
		<skos:prefLabel xml:lang="en">Traffic Separation Scheme Crossing</skos:prefLabel>
		<skos:definition xml:lang="en">A defined area where traffic lanes cross.</skos:definition>
		<dct:description xml:lang="en">SOURCE [IHO Hydrographic Registry].</dct:description>
		<skos:prefLabel xml:lang="el">SAMPLE ALTERNATIVE EXPRESSION - αναφορά</skos:prefLabel>
		<skos:definition xml:lang="el">Συστήματα συντεταγμένων</skos:definition>
		<dct:description xml:lang="el">Συστήματα για μονοσήμαντη αναφορά χωρικών πληροφοριών στον χώρο, ως σύνολο συντεταγμένων (x,y,z) ή/και γεωγραφικό πλάτος και μήκος και ύψος, με βάση γεωδαιτικό οριζόντιο και κατακόρυφο σύστημα αναφοράς (datum).</dct:description>
		<skos:inScheme rdf:resource="http://inspire-registry.jrc.ec.europa.eu/registers/FCD/items"/>
	</inspire:SpatialObjectType>
	<inspire:SpatialObjectType rdf:about="http://inspire-registry.jrc.ec.europa.eu/registers/FCD/items/349">
		<inspire:itemStatus>valid</inspire:itemStatus>
		<inspire:dateAccepted>2010-01-13T17:19:00.159+01:00</inspire:dateAccepted>
		<skos:prefLabel xml:lang="en">Traffic Separation Scheme Lane</skos:prefLabel>
		<skos:definition xml:lang="en">An area within defined limits in which one-way traffic flow is established.</skos:definition>
		<dct:description xml:lang="en">SOURCE [IMO Ships Routeing, 6th Edition], [IHO Hydrographic Registry].</dct:description>
		<skos:prefLabel xml:lang="el">SAMPLE ALTERNATIVE EXPRESSION - αναφορά</skos:prefLabel>
		<skos:definition xml:lang="el">Συστήματα συντεταγμένων</skos:definition>
		<dct:description xml:lang="el">Συστήματα για μονοσήμαντη αναφορά χωρικών πληροφοριών στον χώρο, ως σύνολο συντεταγμένων (x,y,z) ή/και γεωγραφικό πλάτος και μήκος και ύψος, με βάση γεωδαιτικό οριζόντιο και κατακόρυφο σύστημα αναφοράς (datum).</dct:description>
		<skos:inScheme rdf:resource="http://inspire-registry.jrc.ec.europa.eu/registers/FCD/items"/>
	</inspire:SpatialObjectType>
	<inspire:SpatialObjectType rdf:about="http://inspire-registry.jrc.ec.europa.eu/registers/FCD/items/350">
		<inspire:itemStatus>valid</inspire:itemStatus>
		<inspire:dateAccepted>2010-01-13T17:19:00.348+01:00</inspire:dateAccepted>
		<skos:prefLabel xml:lang="en">Traffic Separation Scheme Roundabout</skos:prefLabel>
		<skos:definition xml:lang="en">A traffic separation scheme in which traffic moves in a counter-clockwise direction around a specified point or zone.</skos:definition>
		<dct:description xml:lang="en">SOURCE [IHO Hydrographic Registry].</dct:description>
		<skos:prefLabel xml:lang="el">SAMPLE ALTERNATIVE EXPRESSION - αναφορά</skos:prefLabel>
		<skos:definition xml:lang="el">Συστήματα συντεταγμένων</skos:definition>
		<dct:description xml:lang="el">Συστήματα για μονοσήμαντη αναφορά χωρικών πληροφοριών στον χώρο, ως σύνολο συντεταγμένων (x,y,z) ή/και γεωγραφικό πλάτος και μήκος και ύψος, με βάση γεωδαιτικό οριζόντιο και κατακόρυφο σύστημα αναφοράς (datum).</dct:description>
		<skos:inScheme rdf:resource="http://inspire-registry.jrc.ec.europa.eu/registers/FCD/items"/>
	</inspire:SpatialObjectType>
	<inspire:SpatialObjectType rdf:about="http://inspire-registry.jrc.ec.europa.eu/registers/FCD/items/351">
		<inspire:itemStatus>valid</inspire:itemStatus>
		<inspire:dateAccepted>2010-01-13T17:19:00.514+01:00</inspire:dateAccepted>
		<skos:prefLabel xml:lang="en">Traffic Separation Scheme Separator</skos:prefLabel>
		<skos:definition xml:lang="en">A zone separating the lanes in which ships are proceeding in opposite or nearly opposite directions; or separating traffic lanes designated for particular classes of ships proceeding in the same direction.</skos:definition>
		<dct:description xml:lang="en">SOURCE [IHO Hydrographic Registry].</dct:description>
		<skos:prefLabel xml:lang="el">SAMPLE ALTERNATIVE EXPRESSION - αναφορά</skos:prefLabel>
		<skos:definition xml:lang="el">Συστήματα συντεταγμένων</skos:definition>
		<dct:description xml:lang="el">Συστήματα για μονοσήμαντη αναφορά χωρικών πληροφοριών στον χώρο, ως σύνολο συντεταγμένων (x,y,z) ή/και γεωγραφικό πλάτος και μήκος και ύψος, με βάση γεωδαιτικό οριζόντιο και κατακόρυφο σύστημα αναφοράς (datum).</dct:description>
		<skos:inScheme rdf:resource="http://inspire-registry.jrc.ec.europa.eu/registers/FCD/items"/>
	</inspire:SpatialObjectType>
	<inspire:SpatialObjectType rdf:about="http://inspire-registry.jrc.ec.europa.eu/registers/FCD/items/352">
		<inspire:itemStatus>valid</inspire:itemStatus>
		<inspire:dateAccepted>2010-01-13T17:19:00.627+01:00</inspire:dateAccepted>
		<skos:prefLabel xml:lang="en">Water Link Sequence</skos:prefLabel>
		<skos:definition xml:lang="en">A linear spatial object, composed of an ordered collection of waterway and/or watercourse links (as necessary), which represents a continuous path in the water network without any branches.</skos:definition>
		<dct:description xml:lang="en">NOTE The element has a defined beginning and end and every position on the water link sequence is identifiable with one single parameter such as length. It describes a element of the water network, which is a navigable path within a water body (oceans, seas, rivers, lakes, channels or canals) and could be characterized by one or more thematical identifiers and/or properties.</dct:description>
		<skos:prefLabel xml:lang="el">SAMPLE ALTERNATIVE EXPRESSION - αναφορά</skos:prefLabel>
		<skos:definition xml:lang="el">Συστήματα συντεταγμένων</skos:definition>
		<dct:description xml:lang="el">Συστήματα για μονοσήμαντη αναφορά χωρικών πληροφοριών στον χώρο, ως σύνολο συντεταγμένων (x,y,z) ή/και γεωγραφικό πλάτος και μήκος και ύψος, με βάση γεωδαιτικό οριζόντιο και κατακόρυφο σύστημα αναφοράς (datum).</dct:description>
		<skos:inScheme rdf:resource="http://inspire-registry.jrc.ec.europa.eu/registers/FCD/items"/>
	</inspire:SpatialObjectType>
	<inspire:SpatialObjectType rdf:about="http://inspire-registry.jrc.ec.europa.eu/registers/FCD/items/353">
		<inspire:itemStatus>valid</inspire:itemStatus>
		<inspire:dateAccepted>2010-01-13T17:19:00.746+01:00</inspire:dateAccepted>
		<skos:prefLabel xml:lang="en">Water Traffic Flow Direction</skos:prefLabel>
		<skos:definition xml:lang="en">Indicates the direction of the flow of water transport traffic in relation to the direction of the water transport link vector.</skos:definition>
		<skos:prefLabel xml:lang="el">SAMPLE ALTERNATIVE EXPRESSION - αναφορά</skos:prefLabel>
		<skos:definition xml:lang="el">Συστήματα συντεταγμένων</skos:definition>
		<dct:description xml:lang="el">Συστήματα για μονοσήμαντη αναφορά χωρικών πληροφοριών στον χώρο, ως σύνολο συντεταγμένων (x,y,z) ή/και γεωγραφικό πλάτος και μήκος και ύψος, με βάση γεωδαιτικό οριζόντιο και κατακόρυφο σύστημα αναφοράς (datum).</dct:description>
		<skos:inScheme rdf:resource="http://inspire-registry.jrc.ec.europa.eu/registers/FCD/items"/>
	</inspire:SpatialObjectType>
	<inspire:SpatialObjectType rdf:about="http://inspire-registry.jrc.ec.europa.eu/registers/FCD/items/354">
		<inspire:itemStatus>valid</inspire:itemStatus>
		<inspire:dateAccepted>2010-01-13T17:19:00.877+01:00</inspire:dateAccepted>
		<skos:prefLabel xml:lang="en">Aerodrome Category</skos:prefLabel>
		<skos:definition xml:lang="en">Aerodrome category concerning the scope and importance of the air traffic services offered from and to it.</skos:definition>
		<skos:prefLabel xml:lang="el">SAMPLE ALTERNATIVE EXPRESSION - αναφορά</skos:prefLabel>
		<skos:definition xml:lang="el">Συστήματα συντεταγμένων</skos:definition>
		<dct:description xml:lang="el">Συστήματα για μονοσήμαντη αναφορά χωρικών πληροφοριών στον χώρο, ως σύνολο συντεταγμένων (x,y,z) ή/και γεωγραφικό πλάτος και μήκος και ύψος, με βάση γεωδαιτικό οριζόντιο και κατακόρυφο σύστημα αναφοράς (datum).</dct:description>
		<skos:inScheme rdf:resource="http://inspire-registry.jrc.ec.europa.eu/registers/FCD/items"/>
	</inspire:SpatialObjectType>
	<inspire:SpatialObjectType rdf:about="http://inspire-registry.jrc.ec.europa.eu/registers/FCD/items/355">
		<inspire:itemStatus>valid</inspire:itemStatus>
		<inspire:dateAccepted>2010-01-13T17:19:01.037+01:00</inspire:dateAccepted>
		<skos:prefLabel xml:lang="en">Aerodrome Type</skos:prefLabel>
		<skos:definition xml:lang="en">A code specifying the type of aerodrome.</skos:definition>
		<dct:description xml:lang="en">SOURCE [AIXM5.0].
EXAMPLE Aerodrome only, combined aerodrome/heliport or simple landing site.</dct:description>
		<skos:prefLabel xml:lang="el">SAMPLE ALTERNATIVE EXPRESSION - αναφορά</skos:prefLabel>
		<skos:definition xml:lang="el">Συστήματα συντεταγμένων</skos:definition>
		<dct:description xml:lang="el">Συστήματα για μονοσήμαντη αναφορά χωρικών πληροφοριών στον χώρο, ως σύνολο συντεταγμένων (x,y,z) ή/και γεωγραφικό πλάτος και μήκος και ύψος, με βάση γεωδαιτικό οριζόντιο και κατακόρυφο σύστημα αναφοράς (datum).</dct:description>
		<skos:inScheme rdf:resource="http://inspire-registry.jrc.ec.europa.eu/registers/FCD/items"/>
	</inspire:SpatialObjectType>
	<inspire:SpatialObjectType rdf:about="http://inspire-registry.jrc.ec.europa.eu/registers/FCD/items/356">
		<inspire:itemStatus>valid</inspire:itemStatus>
		<inspire:dateAccepted>2010-01-13T17:19:01.176+01:00</inspire:dateAccepted>
		<skos:prefLabel xml:lang="en">Air Link</skos:prefLabel>
		<skos:definition xml:lang="en">A linear spatial object that describes the geometry and connectivity of the air network between two points in the network.</skos:definition>
		<skos:prefLabel xml:lang="el">SAMPLE ALTERNATIVE EXPRESSION - αναφορά</skos:prefLabel>
		<skos:definition xml:lang="el">Συστήματα συντεταγμένων</skos:definition>
		<dct:description xml:lang="el">Συστήματα για μονοσήμαντη αναφορά χωρικών πληροφοριών στον χώρο, ως σύνολο συντεταγμένων (x,y,z) ή/και γεωγραφικό πλάτος και μήκος και ύψος, με βάση γεωδαιτικό οριζόντιο και κατακόρυφο σύστημα αναφοράς (datum).</dct:description>
		<skos:inScheme rdf:resource="http://inspire-registry.jrc.ec.europa.eu/registers/FCD/items"/>
	</inspire:SpatialObjectType>
	<inspire:SpatialObjectType rdf:about="http://inspire-registry.jrc.ec.europa.eu/registers/FCD/items/357">
		<inspire:itemStatus>valid</inspire:itemStatus>
		<inspire:dateAccepted>2010-01-13T17:19:01.414+01:00</inspire:dateAccepted>
		<skos:prefLabel xml:lang="en">Air Link Sequence</skos:prefLabel>
		<skos:definition xml:lang="en">A linear spatial object, composed of an ordered collection of air links, which represents a continuous path in the air network without any branches.</skos:definition>
		<dct:description xml:lang="en">NOTE 1 The element has a defined beginning and end and every position on the air link sequence is identifiable with one single parameter such as length. It describes an element of the air network, which could be characterized by one or more thematical identifiers and/or properties.
NOTE 2 This collection of air links is equivalent to RoutePortion feature in AIXM5.0. RoutePortion: A group of two or more consecutive segments of the same route, which have the usage and/or the same flight restrictions [AIXM5.0].</dct:description>
		<skos:prefLabel xml:lang="el">SAMPLE ALTERNATIVE EXPRESSION - αναφορά</skos:prefLabel>
		<skos:definition xml:lang="el">Συστήματα συντεταγμένων</skos:definition>
		<dct:description xml:lang="el">Συστήματα για μονοσήμαντη αναφορά χωρικών πληροφοριών στον χώρο, ως σύνολο συντεταγμένων (x,y,z) ή/και γεωγραφικό πλάτος και μήκος και ύψος, με βάση γεωδαιτικό οριζόντιο και κατακόρυφο σύστημα αναφοράς (datum).</dct:description>
		<skos:inScheme rdf:resource="http://inspire-registry.jrc.ec.europa.eu/registers/FCD/items"/>
	</inspire:SpatialObjectType>
	<inspire:SpatialObjectType rdf:about="http://inspire-registry.jrc.ec.europa.eu/registers/FCD/items/358">
		<inspire:itemStatus>valid</inspire:itemStatus>
		<inspire:dateAccepted>2010-01-13T17:19:01.685+01:00</inspire:dateAccepted>
		<skos:prefLabel xml:lang="en">Air Route Link</skos:prefLabel>
		<skos:definition xml:lang="en">A portion of a route to be flown usually without an intermediate stop, as defined by two consecutive significant points.</skos:definition>
		<dct:description xml:lang="en">SOURCE [AirRouteSegment - AIXM5.0].
NOTE The presence of air nodes (normally defining Significant Points) is not mandated.</dct:description>
		<skos:prefLabel xml:lang="el">SAMPLE ALTERNATIVE EXPRESSION - αναφορά</skos:prefLabel>
		<skos:definition xml:lang="el">Συστήματα συντεταγμένων</skos:definition>
		<dct:description xml:lang="el">Συστήματα για μονοσήμαντη αναφορά χωρικών πληροφοριών στον χώρο, ως σύνολο συντεταγμένων (x,y,z) ή/και γεωγραφικό πλάτος και μήκος και ύψος, με βάση γεωδαιτικό οριζόντιο και κατακόρυφο σύστημα αναφοράς (datum).</dct:description>
		<skos:inScheme rdf:resource="http://inspire-registry.jrc.ec.europa.eu/registers/FCD/items"/>
	</inspire:SpatialObjectType>
	<inspire:SpatialObjectType rdf:about="http://inspire-registry.jrc.ec.europa.eu/registers/FCD/items/359">
		<inspire:itemStatus>valid</inspire:itemStatus>
		<inspire:dateAccepted>2010-01-13T17:19:01.955+01:00</inspire:dateAccepted>
		<skos:prefLabel xml:lang="en">Apron Area</skos:prefLabel>
		<skos:definition xml:lang="en">A defined area, on a land aerodrome/heliport, intended to accommodate aircraft/helicopters for purposes of loading and unloading passengers, mail or cargo, and for fuelling, parking or maintenance.</skos:definition>
		<dct:description xml:lang="en">SOURCE [Apron - AIXM5.0].</dct:description>
		<skos:prefLabel xml:lang="el">SAMPLE ALTERNATIVE EXPRESSION - αναφορά</skos:prefLabel>
		<skos:definition xml:lang="el">Συστήματα συντεταγμένων</skos:definition>
		<dct:description xml:lang="el">Συστήματα για μονοσήμαντη αναφορά χωρικών πληροφοριών στον χώρο, ως σύνολο συντεταγμένων (x,y,z) ή/και γεωγραφικό πλάτος και μήκος και ύψος, με βάση γεωδαιτικό οριζόντιο και κατακόρυφο σύστημα αναφοράς (datum).</dct:description>
		<skos:inScheme rdf:resource="http://inspire-registry.jrc.ec.europa.eu/registers/FCD/items"/>
	</inspire:SpatialObjectType>
	<inspire:SpatialObjectType rdf:about="http://inspire-registry.jrc.ec.europa.eu/registers/FCD/items/360">
		<inspire:itemStatus>valid</inspire:itemStatus>
		<inspire:dateAccepted>2010-01-13T17:19:02.163+01:00</inspire:dateAccepted>
		<skos:prefLabel xml:lang="en">Condition of Air Facility</skos:prefLabel>
		<skos:definition xml:lang="en">State of an air transport network element with regards to its completion and use.</skos:definition>
		<skos:prefLabel xml:lang="el">SAMPLE ALTERNATIVE EXPRESSION - αναφορά</skos:prefLabel>
		<skos:definition xml:lang="el">Συστήματα συντεταγμένων</skos:definition>
		<dct:description xml:lang="el">Συστήματα για μονοσήμαντη αναφορά χωρικών πληροφοριών στον χώρο, ως σύνολο συντεταγμένων (x,y,z) ή/και γεωγραφικό πλάτος και μήκος και ύψος, με βάση γεωδαιτικό οριζόντιο και κατακόρυφο σύστημα αναφοράς (datum).</dct:description>
		<skos:inScheme rdf:resource="http://inspire-registry.jrc.ec.europa.eu/registers/FCD/items"/>
	</inspire:SpatialObjectType>
	<inspire:SpatialObjectType rdf:about="http://inspire-registry.jrc.ec.europa.eu/registers/FCD/items/361">
		<inspire:itemStatus>valid</inspire:itemStatus>
		<inspire:dateAccepted>2010-01-13T17:19:02.354+01:00</inspire:dateAccepted>
		<skos:prefLabel xml:lang="en">Element Length</skos:prefLabel>
		<skos:definition xml:lang="en">The physical length of the element.</skos:definition>
		<skos:prefLabel xml:lang="el">SAMPLE ALTERNATIVE EXPRESSION - αναφορά</skos:prefLabel>
		<skos:definition xml:lang="el">Συστήματα συντεταγμένων</skos:definition>
		<dct:description xml:lang="el">Συστήματα για μονοσήμαντη αναφορά χωρικών πληροφοριών στον χώρο, ως σύνολο συντεταγμένων (x,y,z) ή/και γεωγραφικό πλάτος και μήκος και ύψος, με βάση γεωδαιτικό οριζόντιο και κατακόρυφο σύστημα αναφοράς (datum).</dct:description>
		<skos:inScheme rdf:resource="http://inspire-registry.jrc.ec.europa.eu/registers/FCD/items"/>
	</inspire:SpatialObjectType>
	<inspire:SpatialObjectType rdf:about="http://inspire-registry.jrc.ec.europa.eu/registers/FCD/items/362">
		<inspire:itemStatus>valid</inspire:itemStatus>
		<inspire:dateAccepted>2010-01-13T17:19:02.523+01:00</inspire:dateAccepted>
		<skos:prefLabel xml:lang="en">Element Width</skos:prefLabel>
		<skos:definition xml:lang="en">The physical width of the element.</skos:definition>
		<skos:prefLabel xml:lang="el">SAMPLE ALTERNATIVE EXPRESSION - αναφορά</skos:prefLabel>
		<skos:definition xml:lang="el">Συστήματα συντεταγμένων</skos:definition>
		<dct:description xml:lang="el">Συστήματα για μονοσήμαντη αναφορά χωρικών πληροφοριών στον χώρο, ως σύνολο συντεταγμένων (x,y,z) ή/και γεωγραφικό πλάτος και μήκος και ύψος, με βάση γεωδαιτικό οριζόντιο και κατακόρυφο σύστημα αναφοράς (datum).</dct:description>
		<skos:inScheme rdf:resource="http://inspire-registry.jrc.ec.europa.eu/registers/FCD/items"/>
	</inspire:SpatialObjectType>
	<inspire:SpatialObjectType rdf:about="http://inspire-registry.jrc.ec.europa.eu/registers/FCD/items/363">
		<inspire:itemStatus>valid</inspire:itemStatus>
		<inspire:dateAccepted>2010-01-13T17:19:02.727+01:00</inspire:dateAccepted>
		<skos:prefLabel xml:lang="en">Field Elevation</skos:prefLabel>
		<skos:definition xml:lang="en">The aerodrome elevation as the vertical distance between the highest point of the landing area of an aerodrome and mean sea level.</skos:definition>
		<dct:description xml:lang="en">SOURCE [AIXM5.0].
NOTE This might be different from the elevation of the Aerodrome Reference Point.</dct:description>
		<skos:prefLabel xml:lang="el">SAMPLE ALTERNATIVE EXPRESSION - αναφορά</skos:prefLabel>
		<skos:definition xml:lang="el">Συστήματα συντεταγμένων</skos:definition>
		<dct:description xml:lang="el">Συστήματα για μονοσήμαντη αναφορά χωρικών πληροφοριών στον χώρο, ως σύνολο συντεταγμένων (x,y,z) ή/και γεωγραφικό πλάτος και μήκος και ύψος, με βάση γεωδαιτικό οριζόντιο και κατακόρυφο σύστημα αναφοράς (datum).</dct:description>
		<skos:inScheme rdf:resource="http://inspire-registry.jrc.ec.europa.eu/registers/FCD/items"/>
	</inspire:SpatialObjectType>
	<inspire:SpatialObjectType rdf:about="http://inspire-registry.jrc.ec.europa.eu/registers/FCD/items/364">
		<inspire:itemStatus>valid</inspire:itemStatus>
		<inspire:dateAccepted>2010-01-13T17:19:02.967+01:00</inspire:dateAccepted>
		<skos:prefLabel xml:lang="en">Instrument Approach Procedure</skos:prefLabel>
		<skos:definition xml:lang="en">A series of predetermined manoeuvres by reference to flight instruments with specified protection from obstacles from the initial approach fix, or where applicable, from the beginning of a defined arrival route to a point from which a landing can be completed and thereafter, if a landing is not completed, to a position at which holding or en route obstacle clearance criteria apply.</skos:definition>
		<dct:description xml:lang="en">SOURCE [AIXM5.0].
NOTE 1 Acronym: IAP.
NOTE 2 It corresponds to the final approach and arrival during the landing phase.
NOTE 3 A specific runway of an airport/heliport usually has more than one IAP, depending on the landing direction on it.</dct:description>
		<skos:prefLabel xml:lang="el">SAMPLE ALTERNATIVE EXPRESSION - αναφορά</skos:prefLabel>
		<skos:definition xml:lang="el">Συστήματα συντεταγμένων</skos:definition>
		<dct:description xml:lang="el">Συστήματα για μονοσήμαντη αναφορά χωρικών πληροφοριών στον χώρο, ως σύνολο συντεταγμένων (x,y,z) ή/και γεωγραφικό πλάτος και μήκος και ύψος, με βάση γεωδαιτικό οριζόντιο και κατακόρυφο σύστημα αναφοράς (datum).</dct:description>
		<skos:inScheme rdf:resource="http://inspire-registry.jrc.ec.europa.eu/registers/FCD/items"/>
	</inspire:SpatialObjectType>
	<inspire:SpatialObjectType rdf:about="http://inspire-registry.jrc.ec.europa.eu/registers/FCD/items/365">
		<inspire:itemStatus>valid</inspire:itemStatus>
		<inspire:dateAccepted>2010-01-13T17:19:03.163+01:00</inspire:dateAccepted>
		<skos:prefLabel xml:lang="en">Lower Altitude Limit</skos:prefLabel>
		<skos:definition xml:lang="en">Altitude that defines the lower limit of an air transport network object.</skos:definition>
		<dct:description xml:lang="en">NOTE When applied to an AirRouteLink it corresponds to the Lowest Safe Altitude, which is defined in order to provide safety for navigation.</dct:description>
		<skos:prefLabel xml:lang="el">SAMPLE ALTERNATIVE EXPRESSION - αναφορά</skos:prefLabel>
		<skos:definition xml:lang="el">Συστήματα συντεταγμένων</skos:definition>
		<dct:description xml:lang="el">Συστήματα για μονοσήμαντη αναφορά χωρικών πληροφοριών στον χώρο, ως σύνολο συντεταγμένων (x,y,z) ή/και γεωγραφικό πλάτος και μήκος και ύψος, με βάση γεωδαιτικό οριζόντιο και κατακόρυφο σύστημα αναφοράς (datum).</dct:description>
		<skos:inScheme rdf:resource="http://inspire-registry.jrc.ec.europa.eu/registers/FCD/items"/>
	</inspire:SpatialObjectType>
	<inspire:SpatialObjectType rdf:about="http://inspire-registry.jrc.ec.europa.eu/registers/FCD/items/366">
		<inspire:itemStatus>valid</inspire:itemStatus>
		<inspire:dateAccepted>2010-01-13T17:19:03.370+01:00</inspire:dateAccepted>
		<skos:prefLabel xml:lang="en">Navaid</skos:prefLabel>
		<skos:definition xml:lang="en">One or more Navaid Equipments providing navigation services.</skos:definition>
		<dct:description xml:lang="en">DEFINITION Navaid equipment: A physical navaid equipment like VOR, DME, localizer, TACAN or etc.
SOURCE [AIXM5.0].
NOTE 1 The Navaid Equipment share business rules like paired frequencies [AIXM5.0].</dct:description>
		<skos:prefLabel xml:lang="el">SAMPLE ALTERNATIVE EXPRESSION - αναφορά</skos:prefLabel>
		<skos:definition xml:lang="el">Συστήματα συντεταγμένων</skos:definition>
		<dct:description xml:lang="el">Συστήματα για μονοσήμαντη αναφορά χωρικών πληροφοριών στον χώρο, ως σύνολο συντεταγμένων (x,y,z) ή/και γεωγραφικό πλάτος και μήκος και ύψος, με βάση γεωδαιτικό οριζόντιο και κατακόρυφο σύστημα αναφοράς (datum).</dct:description>
		<skos:inScheme rdf:resource="http://inspire-registry.jrc.ec.europa.eu/registers/FCD/items"/>
	</inspire:SpatialObjectType>
	<inspire:SpatialObjectType rdf:about="http://inspire-registry.jrc.ec.europa.eu/registers/FCD/items/367">
		<inspire:itemStatus>valid</inspire:itemStatus>
		<inspire:dateAccepted>2010-01-13T17:19:03.586+01:00</inspire:dateAccepted>
		<skos:prefLabel xml:lang="en">Procedure Link</skos:prefLabel>
		<skos:definition xml:lang="en">A series of predetermined manoeuvres with specified protection from obstacles.</skos:definition>
		<dct:description xml:lang="en">SOURCE [Procedure - AIXM5.0].
NOTE 1 A defined airway connector designed for channelling the flow of traffic as necessary for the provision of air traffic services during the take-off or landing phase, which links an airport/heliport to a significant point, usually connected to one or more air routes.
NOTE 2 When a airport/heliport is not connected with a standardized airway connector to the rest of the air network, this object can be used as a fictitious connector between the airport/heliport and a significant point on one or more ATS routes - for example for VFR (Visual Flight Rules) flights.
NOTE 3 Nevertheless, three main types of standardized Procedures are usually defined for IFR (Instrument Flight Rules) flights:
- Standard Instrument Departure (SID), corresponding to the take-off phase.
- Standard Instrument Arrival (STAR), corresponding to the initial approach during the landing phase.
- Instrument Approach Procedure (IAP), corresponding to the final approach and arrival during the landing phase.</dct:description>
		<skos:prefLabel xml:lang="el">SAMPLE ALTERNATIVE EXPRESSION - αναφορά</skos:prefLabel>
		<skos:definition xml:lang="el">Συστήματα συντεταγμένων</skos:definition>
		<dct:description xml:lang="el">Συστήματα για μονοσήμαντη αναφορά χωρικών πληροφοριών στον χώρο, ως σύνολο συντεταγμένων (x,y,z) ή/και γεωγραφικό πλάτος και μήκος και ύψος, με βάση γεωδαιτικό οριζόντιο και κατακόρυφο σύστημα αναφοράς (datum).</dct:description>
		<skos:inScheme rdf:resource="http://inspire-registry.jrc.ec.europa.eu/registers/FCD/items"/>
	</inspire:SpatialObjectType>
	<inspire:SpatialObjectType rdf:about="http://inspire-registry.jrc.ec.europa.eu/registers/FCD/items/368">
		<inspire:itemStatus>valid</inspire:itemStatus>
		<inspire:dateAccepted>2010-01-13T17:19:03.794+01:00</inspire:dateAccepted>
		<skos:prefLabel xml:lang="en">Runway Centreline Point</skos:prefLabel>
		<skos:definition xml:lang="en">An operationally significant position on the center line of a runway direction.</skos:definition>
		<dct:description xml:lang="en">SOURCE [AIXM5.0].
NOTE 1 The role of the point along the runway direction centreline is indicated within the pointRole attribute.
NOTE 2 Runway centreline points are used to connect the Procedure Links that connect an airport/heliport to the rest of the air network.
EXAMPLE A typical example is the runway threshold [AIXM5.0].</dct:description>
		<skos:prefLabel xml:lang="el">SAMPLE ALTERNATIVE EXPRESSION - αναφορά</skos:prefLabel>
		<skos:definition xml:lang="el">Συστήματα συντεταγμένων</skos:definition>
		<dct:description xml:lang="el">Συστήματα για μονοσήμαντη αναφορά χωρικών πληροφοριών στον χώρο, ως σύνολο συντεταγμένων (x,y,z) ή/και γεωγραφικό πλάτος και μήκος και ύψος, με βάση γεωδαιτικό οριζόντιο και κατακόρυφο σύστημα αναφοράς (datum).</dct:description>
		<skos:inScheme rdf:resource="http://inspire-registry.jrc.ec.europa.eu/registers/FCD/items"/>
	</inspire:SpatialObjectType>
	<inspire:SpatialObjectType rdf:about="http://inspire-registry.jrc.ec.europa.eu/registers/FCD/items/369">
		<inspire:itemStatus>valid</inspire:itemStatus>
		<inspire:dateAccepted>2010-01-13T17:19:04.056+01:00</inspire:dateAccepted>
		<skos:prefLabel xml:lang="en">Standard Instrument Arrival</skos:prefLabel>
		<skos:definition xml:lang="en">A designated instrument flight rule (IFR) arrival route linking a significant point, normally on an ATS route, with a point from which a published instrument approach procedure can be commenced.</skos:definition>
		<dct:description xml:lang="en">SOURCE [AIXM5.0].
NOTE 1 Acronym: STAR.
NOTE 2 It corresponds to the initial approach during the landing phase. Each airport/heliport could have various STAR linking significant points (usually connected to air routes) to the points designated to start the landing on a specific runway.</dct:description>
		<skos:prefLabel xml:lang="el">SAMPLE ALTERNATIVE EXPRESSION - αναφορά</skos:prefLabel>
		<skos:definition xml:lang="el">Συστήματα συντεταγμένων</skos:definition>
		<dct:description xml:lang="el">Συστήματα για μονοσήμαντη αναφορά χωρικών πληροφοριών στον χώρο, ως σύνολο συντεταγμένων (x,y,z) ή/και γεωγραφικό πλάτος και μήκος και ύψος, με βάση γεωδαιτικό οριζόντιο και κατακόρυφο σύστημα αναφοράς (datum).</dct:description>
		<skos:inScheme rdf:resource="http://inspire-registry.jrc.ec.europa.eu/registers/FCD/items"/>
	</inspire:SpatialObjectType>
	<inspire:SpatialObjectType rdf:about="http://inspire-registry.jrc.ec.europa.eu/registers/FCD/items/370">
		<inspire:itemStatus>valid</inspire:itemStatus>
		<inspire:dateAccepted>2010-01-13T17:19:04.207+01:00</inspire:dateAccepted>
		<skos:prefLabel xml:lang="en">Surface Composition</skos:prefLabel>
		<skos:definition xml:lang="en">The composition of an aerodrome/heliport related surface.</skos:definition>
		<skos:prefLabel xml:lang="el">SAMPLE ALTERNATIVE EXPRESSION - αναφορά</skos:prefLabel>
		<skos:definition xml:lang="el">Συστήματα συντεταγμένων</skos:definition>
		<dct:description xml:lang="el">Συστήματα για μονοσήμαντη αναφορά χωρικών πληροφοριών στον χώρο, ως σύνολο συντεταγμένων (x,y,z) ή/και γεωγραφικό πλάτος και μήκος και ύψος, με βάση γεωδαιτικό οριζόντιο και κατακόρυφο σύστημα αναφοράς (datum).</dct:description>
		<skos:inScheme rdf:resource="http://inspire-registry.jrc.ec.europa.eu/registers/FCD/items"/>
	</inspire:SpatialObjectType>
	<inspire:SpatialObjectType rdf:about="http://inspire-registry.jrc.ec.europa.eu/registers/FCD/items/371">
		<inspire:itemStatus>valid</inspire:itemStatus>
		<inspire:dateAccepted>2010-01-13T17:19:04.388+01:00</inspire:dateAccepted>
		<skos:prefLabel xml:lang="en">Taxiway Area</skos:prefLabel>
		<skos:definition xml:lang="en">A defined path at an aerodrome/heliport established for the taxiing of aircraft/helicopters and intended to provide a link between one part of the aerodrome and another.</skos:definition>
		<dct:description xml:lang="en">SOURCE [Taxiway - AIXM5.0].
NOTE This includes aircraft/helicopter stand taxilines, apron taxiways, rapid exit taxiways, air taxiways etc.</dct:description>
		<skos:prefLabel xml:lang="el">SAMPLE ALTERNATIVE EXPRESSION - αναφορά</skos:prefLabel>
		<skos:definition xml:lang="el">Συστήματα συντεταγμένων</skos:definition>
		<dct:description xml:lang="el">Συστήματα για μονοσήμαντη αναφορά χωρικών πληροφοριών στον χώρο, ως σύνολο συντεταγμένων (x,y,z) ή/και γεωγραφικό πλάτος και μήκος και ύψος, με βάση γεωδαιτικό οριζόντιο και κατακόρυφο σύστημα αναφοράς (datum).</dct:description>
		<skos:inScheme rdf:resource="http://inspire-registry.jrc.ec.europa.eu/registers/FCD/items"/>
	</inspire:SpatialObjectType>
	<inspire:SpatialObjectType rdf:about="http://inspire-registry.jrc.ec.europa.eu/registers/FCD/items/372">
		<inspire:itemStatus>valid</inspire:itemStatus>
		<inspire:dateAccepted>2010-01-13T17:19:04.576+01:00</inspire:dateAccepted>
		<skos:prefLabel xml:lang="en">Touch Down Lift Off</skos:prefLabel>
		<skos:definition xml:lang="en">A load bearing area on which a helicopter may touch down or lift-off.</skos:definition>
		<dct:description xml:lang="en">SOURCE [AIXM5.0].</dct:description>
		<skos:prefLabel xml:lang="el">SAMPLE ALTERNATIVE EXPRESSION - αναφορά</skos:prefLabel>
		<skos:definition xml:lang="el">Συστήματα συντεταγμένων</skos:definition>
		<dct:description xml:lang="el">Συστήματα για μονοσήμαντη αναφορά χωρικών πληροφοριών στον χώρο, ως σύνολο συντεταγμένων (x,y,z) ή/και γεωγραφικό πλάτος και μήκος και ύψος, με βάση γεωδαιτικό οριζόντιο και κατακόρυφο σύστημα αναφοράς (datum).</dct:description>
		<skos:inScheme rdf:resource="http://inspire-registry.jrc.ec.europa.eu/registers/FCD/items"/>
	</inspire:SpatialObjectType>
	<inspire:SpatialObjectType rdf:about="http://inspire-registry.jrc.ec.europa.eu/registers/FCD/items/373">
		<inspire:itemStatus>valid</inspire:itemStatus>
		<inspire:dateAccepted>2010-01-13T17:19:04.761+01:00</inspire:dateAccepted>
		<skos:prefLabel xml:lang="en">Upper Altitude Limit</skos:prefLabel>
		<skos:definition xml:lang="en">Altitude that defines the upper limit of an air transport network object.</skos:definition>
		<skos:prefLabel xml:lang="el">SAMPLE ALTERNATIVE EXPRESSION - αναφορά</skos:prefLabel>
		<skos:definition xml:lang="el">Συστήματα συντεταγμένων</skos:definition>
		<dct:description xml:lang="el">Συστήματα για μονοσήμαντη αναφορά χωρικών πληροφοριών στον χώρο, ως σύνολο συντεταγμένων (x,y,z) ή/και γεωγραφικό πλάτος και μήκος και ύψος, με βάση γεωδαιτικό οριζόντιο και κατακόρυφο σύστημα αναφοράς (datum).</dct:description>
		<skos:inScheme rdf:resource="http://inspire-registry.jrc.ec.europa.eu/registers/FCD/items"/>
	</inspire:SpatialObjectType>
	<inspire:SpatialObjectType rdf:about="http://inspire-registry.jrc.ec.europa.eu/registers/FCD/items/374">
		<inspire:itemStatus>valid</inspire:itemStatus>
		<inspire:dateAccepted>2010-01-13T17:19:04.874+01:00</inspire:dateAccepted>
		<skos:prefLabel xml:lang="en">Use Restriction</skos:prefLabel>
		<skos:definition xml:lang="en">The restrictions to the use of an air network object.</skos:definition>
		<skos:prefLabel xml:lang="el">SAMPLE ALTERNATIVE EXPRESSION - αναφορά</skos:prefLabel>
		<skos:definition xml:lang="el">Συστήματα συντεταγμένων</skos:definition>
		<dct:description xml:lang="el">Συστήματα για μονοσήμαντη αναφορά χωρικών πληροφοριών στον χώρο, ως σύνολο συντεταγμένων (x,y,z) ή/και γεωγραφικό πλάτος και μήκος και ύψος, με βάση γεωδαιτικό οριζόντιο και κατακόρυφο σύστημα αναφοράς (datum).</dct:description>
		<skos:inScheme rdf:resource="http://inspire-registry.jrc.ec.europa.eu/registers/FCD/items"/>
	</inspire:SpatialObjectType>
	<inspire:SpatialObjectType rdf:about="http://inspire-registry.jrc.ec.europa.eu/registers/FCD/items/375">
		<inspire:itemStatus>valid</inspire:itemStatus>
		<inspire:dateAccepted>2010-01-13T17:19:05.019+01:00</inspire:dateAccepted>
		<skos:prefLabel xml:lang="en">Nominal Track Gauge</skos:prefLabel>
		<skos:definition xml:lang="en">The nominal distance between the two outer rails (gauge) of a railway track.</skos:definition>
		<skos:prefLabel xml:lang="el">SAMPLE ALTERNATIVE EXPRESSION - αναφορά</skos:prefLabel>
		<skos:definition xml:lang="el">Συστήματα συντεταγμένων</skos:definition>
		<dct:description xml:lang="el">Συστήματα για μονοσήμαντη αναφορά χωρικών πληροφοριών στον χώρο, ως σύνολο συντεταγμένων (x,y,z) ή/και γεωγραφικό πλάτος και μήκος και ύψος, με βάση γεωδαιτικό οριζόντιο και κατακόρυφο σύστημα αναφοράς (datum).</dct:description>
		<skos:inScheme rdf:resource="http://inspire-registry.jrc.ec.europa.eu/registers/FCD/items"/>
	</inspire:SpatialObjectType>
	<inspire:SpatialObjectType rdf:about="http://inspire-registry.jrc.ec.europa.eu/registers/FCD/items/376">
		<inspire:itemStatus>valid</inspire:itemStatus>
		<inspire:dateAccepted>2010-01-13T17:19:05.152+01:00</inspire:dateAccepted>
		<skos:prefLabel xml:lang="en">Railway Station Code</skos:prefLabel>
		<skos:definition xml:lang="en">The unique code assigned to a railway station.</skos:definition>
		<skos:prefLabel xml:lang="el">SAMPLE ALTERNATIVE EXPRESSION - αναφορά</skos:prefLabel>
		<skos:definition xml:lang="el">Συστήματα συντεταγμένων</skos:definition>
		<dct:description xml:lang="el">Συστήματα για μονοσήμαντη αναφορά χωρικών πληροφοριών στον χώρο, ως σύνολο συντεταγμένων (x,y,z) ή/και γεωγραφικό πλάτος και μήκος και ύψος, με βάση γεωδαιτικό οριζόντιο και κατακόρυφο σύστημα αναφοράς (datum).</dct:description>
		<skos:inScheme rdf:resource="http://inspire-registry.jrc.ec.europa.eu/registers/FCD/items"/>
	</inspire:SpatialObjectType>
	<inspire:SpatialObjectType rdf:about="http://inspire-registry.jrc.ec.europa.eu/registers/FCD/items/377">
		<inspire:itemStatus>valid</inspire:itemStatus>
		<inspire:dateAccepted>2010-01-13T17:29:04.787+01:00</inspire:dateAccepted>
		<skos:prefLabel xml:lang="en">Location Type</skos:prefLabel>
		<skos:definition xml:lang="en">classification scheme for location instances</skos:definition>
		<skos:prefLabel xml:lang="el">SAMPLE ALTERNATIVE EXPRESSION - αναφορά</skos:prefLabel>
		<skos:definition xml:lang="el">Συστήματα συντεταγμένων</skos:definition>
		<dct:description xml:lang="el">Συστήματα για μονοσήμαντη αναφορά χωρικών πληροφοριών στον χώρο, ως σύνολο συντεταγμένων (x,y,z) ή/και γεωγραφικό πλάτος και μήκος και ύψος, με βάση γεωδαιτικό οριζόντιο και κατακόρυφο σύστημα αναφοράς (datum).</dct:description>
		<skos:inScheme rdf:resource="http://inspire-registry.jrc.ec.europa.eu/registers/FCD/items"/>
	</inspire:SpatialObjectType>
	<inspire:SpatialObjectType rdf:about="http://inspire-registry.jrc.ec.europa.eu/registers/FCD/items/378">
		<inspire:itemStatus>valid</inspire:itemStatus>
		<inspire:dateAccepted>2010-01-13T17:29:05.002+01:00</inspire:dateAccepted>
		<skos:prefLabel xml:lang="en">Network Area</skos:prefLabel>
		<skos:definition xml:lang="en">A 2-dimensional element in a network.</skos:definition>
		<skos:prefLabel xml:lang="el">SAMPLE ALTERNATIVE EXPRESSION - αναφορά</skos:prefLabel>
		<skos:definition xml:lang="el">Συστήματα συντεταγμένων</skos:definition>
		<dct:description xml:lang="el">Συστήματα για μονοσήμαντη αναφορά χωρικών πληροφοριών στον χώρο, ως σύνολο συντεταγμένων (x,y,z) ή/και γεωγραφικό πλάτος και μήκος και ύψος, με βάση γεωδαιτικό οριζόντιο και κατακόρυφο σύστημα αναφοράς (datum).</dct:description>
		<skos:inScheme rdf:resource="http://inspire-registry.jrc.ec.europa.eu/registers/FCD/items"/>
	</inspire:SpatialObjectType>
	<inspire:SpatialObjectType rdf:about="http://inspire-registry.jrc.ec.europa.eu/registers/FCD/items/379">
		<inspire:itemStatus>valid</inspire:itemStatus>
		<inspire:dateAccepted>2010-01-13T17:29:11.168+01:00</inspire:dateAccepted>
		<skos:prefLabel xml:lang="en">Grade Separated Crossing</skos:prefLabel>
		<skos:definition xml:lang="en">Indicator which of two or more intersecting elements is/are above and which is/are below, to be used if elevation coordinates are not present or cannot be trusted.</skos:definition>
		<dct:description xml:lang="en">NOTE 1 In most cases, the number of elements will be two.
NOTE 2 In the normal case this is when elements intersect in the x/y-plane when the z coordinate is not present or is not accurate enough.</dct:description>
		<skos:prefLabel xml:lang="el">SAMPLE ALTERNATIVE EXPRESSION - αναφορά</skos:prefLabel>
		<skos:definition xml:lang="el">Συστήματα συντεταγμένων</skos:definition>
		<dct:description xml:lang="el">Συστήματα για μονοσήμαντη αναφορά χωρικών πληροφοριών στον χώρο, ως σύνολο συντεταγμένων (x,y,z) ή/και γεωγραφικό πλάτος και μήκος και ύψος, με βάση γεωδαιτικό οριζόντιο και κατακόρυφο σύστημα αναφοράς (datum).</dct:description>
		<skos:inScheme rdf:resource="http://inspire-registry.jrc.ec.europa.eu/registers/FCD/items"/>
	</inspire:SpatialObjectType>
	<inspire:SpatialObjectType rdf:about="http://inspire-registry.jrc.ec.europa.eu/registers/FCD/items/380">
		<inspire:itemStatus>valid</inspire:itemStatus>
		<inspire:dateAccepted>2010-01-13T17:29:11.661+01:00</inspire:dateAccepted>
		<skos:prefLabel xml:lang="en">Link</skos:prefLabel>
		<skos:definition xml:lang="en">Curvilinear network element that connects two positions and represents a homogeneous path in the network. The connected positions may be represented as nodes.</skos:definition>
		<skos:prefLabel xml:lang="el">SAMPLE ALTERNATIVE EXPRESSION - αναφορά</skos:prefLabel>
		<skos:definition xml:lang="el">Συστήματα συντεταγμένων</skos:definition>
		<dct:description xml:lang="el">Συστήματα για μονοσήμαντη αναφορά χωρικών πληροφοριών στον χώρο, ως σύνολο συντεταγμένων (x,y,z) ή/και γεωγραφικό πλάτος και μήκος και ύψος, με βάση γεωδαιτικό οριζόντιο και κατακόρυφο σύστημα αναφοράς (datum).</dct:description>
		<skos:inScheme rdf:resource="http://inspire-registry.jrc.ec.europa.eu/registers/FCD/items"/>
	</inspire:SpatialObjectType>
	<inspire:SpatialObjectType rdf:about="http://inspire-registry.jrc.ec.europa.eu/registers/FCD/items/381">
		<inspire:itemStatus>valid</inspire:itemStatus>
		<inspire:dateAccepted>2010-01-13T17:29:12.288+01:00</inspire:dateAccepted>
		<skos:prefLabel xml:lang="en">Network Connection</skos:prefLabel>
		<skos:definition xml:lang="en">Represents a logical connection between two or more network elements in different networks.</skos:definition>
		<dct:description xml:lang="en">In the case where the networks are in different spatial data sets, a network connection object may exist in both data sets.</dct:description>
		<skos:prefLabel xml:lang="el">SAMPLE ALTERNATIVE EXPRESSION - αναφορά</skos:prefLabel>
		<skos:definition xml:lang="el">Συστήματα συντεταγμένων</skos:definition>
		<dct:description xml:lang="el">Συστήματα για μονοσήμαντη αναφορά χωρικών πληροφοριών στον χώρο, ως σύνολο συντεταγμένων (x,y,z) ή/και γεωγραφικό πλάτος και μήκος και ύψος, με βάση γεωδαιτικό οριζόντιο και κατακόρυφο σύστημα αναφοράς (datum).</dct:description>
		<skos:inScheme rdf:resource="http://inspire-registry.jrc.ec.europa.eu/registers/FCD/items"/>
	</inspire:SpatialObjectType>
	<inspire:SpatialObjectType rdf:about="http://inspire-registry.jrc.ec.europa.eu/registers/FCD/items/382">
		<inspire:itemStatus>valid</inspire:itemStatus>
		<inspire:dateAccepted>2010-01-13T17:29:12.779+01:00</inspire:dateAccepted>
		<skos:prefLabel xml:lang="en">Network Element</skos:prefLabel>
		<skos:definition xml:lang="en">Abstract base type representing an element in a network. Every element in a network provides some function that is of interest in the network.</skos:definition>
		<dct:description xml:lang="en">n/a</dct:description>
		<skos:prefLabel xml:lang="el">SAMPLE ALTERNATIVE EXPRESSION - αναφορά</skos:prefLabel>
		<skos:definition xml:lang="el">Συστήματα συντεταγμένων</skos:definition>
		<dct:description xml:lang="el">Συστήματα για μονοσήμαντη αναφορά χωρικών πληροφοριών στον χώρο, ως σύνολο συντεταγμένων (x,y,z) ή/και γεωγραφικό πλάτος και μήκος και ύψος, με βάση γεωδαιτικό οριζόντιο και κατακόρυφο σύστημα αναφοράς (datum).</dct:description>
		<skos:inScheme rdf:resource="http://inspire-registry.jrc.ec.europa.eu/registers/FCD/items"/>
	</inspire:SpatialObjectType>
	<inspire:SpatialObjectType rdf:about="http://inspire-registry.jrc.ec.europa.eu/registers/FCD/items/383">
		<inspire:itemStatus>valid</inspire:itemStatus>
		<inspire:dateAccepted>2010-01-13T17:29:13.295+01:00</inspire:dateAccepted>
		<skos:prefLabel xml:lang="en">Network Property</skos:prefLabel>
		<skos:definition xml:lang="en">Abstract base type representing phenomena located at or along a network element. This base type provides general properties to associate the network-related phenomena (network properties) with the network elements.</skos:definition>
		<dct:description xml:lang="en">In the simplest case (NetworkReference), the network property applies to the whole network element. In the case of a Link, the spatial reference may be restricted to part of the Link by using a linear reference. ISO/TC 211 is currently in the early stages of developing a standard for Linear Referencing (ISO 19148). A simple mechanism to express linear references is provided in this version of the network model; it is expected that the model will be extended once ISO 19148 is stable. The current simple model requires for all linear references two expressions representing a distance from the start of the Link along its curve geometry. The network property applies to the part of the Link between fromPosition and toPosition.</dct:description>
		<skos:prefLabel xml:lang="el">SAMPLE ALTERNATIVE EXPRESSION - αναφορά</skos:prefLabel>
		<skos:definition xml:lang="el">Συστήματα συντεταγμένων</skos:definition>
		<dct:description xml:lang="el">Συστήματα για μονοσήμαντη αναφορά χωρικών πληροφοριών στον χώρο, ως σύνολο συντεταγμένων (x,y,z) ή/και γεωγραφικό πλάτος και μήκος και ύψος, με βάση γεωδαιτικό οριζόντιο και κατακόρυφο σύστημα αναφοράς (datum).</dct:description>
		<skos:inScheme rdf:resource="http://inspire-registry.jrc.ec.europa.eu/registers/FCD/items"/>
	</inspire:SpatialObjectType>
	<inspire:SpatialObjectType rdf:about="http://inspire-registry.jrc.ec.europa.eu/registers/FCD/items/384">
		<inspire:itemStatus>valid</inspire:itemStatus>
		<inspire:dateAccepted>2010-01-13T17:29:13.765+01:00</inspire:dateAccepted>
		<skos:prefLabel xml:lang="en">Node</skos:prefLabel>
		<skos:definition xml:lang="en">Represents a significant position in the network that always occurs at the
beginning or the end of a link.</skos:definition>
		<dct:description xml:lang="en">NOTE if a topological representation of the network is used the road node is either a topological connection between two or more links or the termination of a link. If a geometric representation of the network is used road nodes are represented by points or alternatively another geometric shape. [EuroRoadS]</dct:description>
		<skos:prefLabel xml:lang="el">SAMPLE ALTERNATIVE EXPRESSION - αναφορά</skos:prefLabel>
		<skos:definition xml:lang="el">Συστήματα συντεταγμένων</skos:definition>
		<dct:description xml:lang="el">Συστήματα για μονοσήμαντη αναφορά χωρικών πληροφοριών στον χώρο, ως σύνολο συντεταγμένων (x,y,z) ή/και γεωγραφικό πλάτος και μήκος και ύψος, με βάση γεωδαιτικό οριζόντιο και κατακόρυφο σύστημα αναφοράς (datum).</dct:description>
		<skos:inScheme rdf:resource="http://inspire-registry.jrc.ec.europa.eu/registers/FCD/items"/>
	</inspire:SpatialObjectType>
	<inspire:SpatialObjectType rdf:about="http://inspire-registry.jrc.ec.europa.eu/registers/FCD/items/385">
		<inspire:itemStatus>valid</inspire:itemStatus>
		<inspire:dateAccepted>2010-01-13T17:29:13.986+01:00</inspire:dateAccepted>
		<skos:prefLabel xml:lang="en">Cross Reference</skos:prefLabel>
		<skos:definition xml:lang="en">Represents a cross reference between two elements in the same network.</skos:definition>
		<dct:description xml:lang="en">The cross reference may represent the case where two elements are different representations of the same spatial object.</dct:description>
		<skos:prefLabel xml:lang="el">SAMPLE ALTERNATIVE EXPRESSION - αναφορά</skos:prefLabel>
		<skos:definition xml:lang="el">Συστήματα συντεταγμένων</skos:definition>
		<dct:description xml:lang="el">Συστήματα για μονοσήμαντη αναφορά χωρικών πληροφοριών στον χώρο, ως σύνολο συντεταγμένων (x,y,z) ή/και γεωγραφικό πλάτος και μήκος και ύψος, με βάση γεωδαιτικό οριζόντιο και κατακόρυφο σύστημα αναφοράς (datum).</dct:description>
		<skos:inScheme rdf:resource="http://inspire-registry.jrc.ec.europa.eu/registers/FCD/items"/>
	</inspire:SpatialObjectType>
	<inspire:SpatialObjectType rdf:about="http://inspire-registry.jrc.ec.europa.eu/registers/FCD/items/386">
		<inspire:itemStatus>valid</inspire:itemStatus>
		<inspire:dateAccepted>2010-01-13T17:29:14.214+01:00</inspire:dateAccepted>
		<skos:prefLabel xml:lang="en">Generalised Link</skos:prefLabel>
		<skos:definition xml:lang="en">Abstract base type representing a linear network element that may be used as a target in linear referencing.</skos:definition>
		<skos:prefLabel xml:lang="el">SAMPLE ALTERNATIVE EXPRESSION - αναφορά</skos:prefLabel>
		<skos:definition xml:lang="el">Συστήματα συντεταγμένων</skos:definition>
		<dct:description xml:lang="el">Συστήματα για μονοσήμαντη αναφορά χωρικών πληροφοριών στον χώρο, ως σύνολο συντεταγμένων (x,y,z) ή/και γεωγραφικό πλάτος και μήκος και ύψος, με βάση γεωδαιτικό οριζόντιο και κατακόρυφο σύστημα αναφοράς (datum).</dct:description>
		<skos:inScheme rdf:resource="http://inspire-registry.jrc.ec.europa.eu/registers/FCD/items"/>
	</inspire:SpatialObjectType>
	<inspire:SpatialObjectType rdf:about="http://inspire-registry.jrc.ec.europa.eu/registers/FCD/items/387">
		<inspire:itemStatus>valid</inspire:itemStatus>
		<inspire:dateAccepted>2010-01-13T17:29:14.483+01:00</inspire:dateAccepted>
		<skos:prefLabel xml:lang="en">Link Sequence</skos:prefLabel>
		<skos:definition xml:lang="en">A network element which represents a continuous path in the network without any branches. The element has a defined beginning and end and every position on the link sequence is identifiable with one single parameter such as length.</skos:definition>
		<dct:description xml:lang="en">EXAMPLE A link sequence may represent a route.</dct:description>
		<skos:prefLabel xml:lang="el">SAMPLE ALTERNATIVE EXPRESSION - αναφορά</skos:prefLabel>
		<skos:definition xml:lang="el">Συστήματα συντεταγμένων</skos:definition>
		<dct:description xml:lang="el">Συστήματα για μονοσήμαντη αναφορά χωρικών πληροφοριών στον χώρο, ως σύνολο συντεταγμένων (x,y,z) ή/και γεωγραφικό πλάτος και μήκος και ύψος, με βάση γεωδαιτικό οριζόντιο και κατακόρυφο σύστημα αναφοράς (datum).</dct:description>
		<skos:inScheme rdf:resource="http://inspire-registry.jrc.ec.europa.eu/registers/FCD/items"/>
	</inspire:SpatialObjectType>
	<inspire:SpatialObjectType rdf:about="http://inspire-registry.jrc.ec.europa.eu/registers/FCD/items/388">
		<inspire:itemStatus>valid</inspire:itemStatus>
		<inspire:dateAccepted>2010-01-13T17:29:14.704+01:00</inspire:dateAccepted>
		<skos:prefLabel xml:lang="en">Link Set</skos:prefLabel>
		<skos:definition xml:lang="en">A collection of link sequences and/or individual links that has a specific function or significance in a network.</skos:definition>
		<dct:description xml:lang="en">NOTE This spatial object type supports the aggregation of links to form objects with branches, loops, parallel sequences of links, gaps, etc.
EXAMPLE A dual carriageway road, as a collection of the two link sequences that represent each carriageway.</dct:description>
		<skos:prefLabel xml:lang="el">SAMPLE ALTERNATIVE EXPRESSION - αναφορά</skos:prefLabel>
		<skos:definition xml:lang="el">Συστήματα συντεταγμένων</skos:definition>
		<dct:description xml:lang="el">Συστήματα για μονοσήμαντη αναφορά χωρικών πληροφοριών στον χώρο, ως σύνολο συντεταγμένων (x,y,z) ή/και γεωγραφικό πλάτος και μήκος και ύψος, με βάση γεωδαιτικό οριζόντιο και κατακόρυφο σύστημα αναφοράς (datum).</dct:description>
		<skos:inScheme rdf:resource="http://inspire-registry.jrc.ec.europa.eu/registers/FCD/items"/>
	</inspire:SpatialObjectType>
	<inspire:SpatialObjectType rdf:about="http://inspire-registry.jrc.ec.europa.eu/registers/FCD/items/392">
		<inspire:itemStatus>valid</inspire:itemStatus>
		<inspire:dateAccepted>2010-01-19T16:18:29.552+01:00</inspire:dateAccepted>
		<skos:prefLabel xml:lang="en">Crossing</skos:prefLabel>
		<skos:definition xml:lang="en">A man-made object allowing the passage of water above or below an obstacle.</skos:definition>
		<dct:description xml:lang="en">EXAMPLE Aqueduct, bridge, culvert, siphon.</dct:description>
		<skos:prefLabel xml:lang="el">SAMPLE ALTERNATIVE EXPRESSION - αναφορά</skos:prefLabel>
		<skos:definition xml:lang="el">Συστήματα συντεταγμένων</skos:definition>
		<dct:description xml:lang="el">Συστήματα για μονοσήμαντη αναφορά χωρικών πληροφοριών στον χώρο, ως σύνολο συντεταγμένων (x,y,z) ή/και γεωγραφικό πλάτος και μήκος και ύψος, με βάση γεωδαιτικό οριζόντιο και κατακόρυφο σύστημα αναφοράς (datum).</dct:description>
		<skos:inScheme rdf:resource="http://inspire-registry.jrc.ec.europa.eu/registers/FCD/items"/>
	</inspire:SpatialObjectType>
	<inspire:SpatialObjectType rdf:about="http://inspire-registry.jrc.ec.europa.eu/registers/FCD/items/393">
		<inspire:itemStatus>valid</inspire:itemStatus>
		<inspire:dateAccepted>2010-01-19T16:18:30.227+01:00</inspire:dateAccepted>
		<skos:prefLabel xml:lang="en">Dam or weir</skos:prefLabel>
		<skos:definition xml:lang="en">A permanent barrier across a watercourse used to impound water or to control its flow</skos:definition>
		<skos:prefLabel xml:lang="el">SAMPLE ALTERNATIVE EXPRESSION - αναφορά</skos:prefLabel>
		<skos:definition xml:lang="el">Συστήματα συντεταγμένων</skos:definition>
		<dct:description xml:lang="el">Συστήματα για μονοσήμαντη αναφορά χωρικών πληροφοριών στον χώρο, ως σύνολο συντεταγμένων (x,y,z) ή/και γεωγραφικό πλάτος και μήκος και ύψος, με βάση γεωδαιτικό οριζόντιο και κατακόρυφο σύστημα αναφοράς (datum).</dct:description>
		<skos:inScheme rdf:resource="http://inspire-registry.jrc.ec.europa.eu/registers/FCD/items"/>
	</inspire:SpatialObjectType>
	<inspire:SpatialObjectType rdf:about="http://inspire-registry.jrc.ec.europa.eu/registers/FCD/items/394">
		<inspire:itemStatus>valid</inspire:itemStatus>
		<inspire:dateAccepted>2010-01-19T16:18:30.441+01:00</inspire:dateAccepted>
		<skos:prefLabel xml:lang="en">Drainage Basin</skos:prefLabel>
		<skos:definition xml:lang="en">Area having a common outlet for its surface runoff.</skos:definition>
		<dct:description xml:lang="en">SOURCE [UNESCO/WMO International Glossary of Hydrology].
NOTE 1 Regarding the different classifications of drainage basins, no distinction is made between drainage basins / sub-basins since this will vary with application. It is possible to build basins from other basins.
NOTE 2 The outlet of a drainage basin may be a canal or a lake.
NOTE 3 Synonyms for drainage basin include: catchment; catchment area; drainage area; river basin; watershed.</dct:description>
		<skos:prefLabel xml:lang="el">SAMPLE ALTERNATIVE EXPRESSION - αναφορά</skos:prefLabel>
		<skos:definition xml:lang="el">Συστήματα συντεταγμένων</skos:definition>
		<dct:description xml:lang="el">Συστήματα για μονοσήμαντη αναφορά χωρικών πληροφοριών στον χώρο, ως σύνολο συντεταγμένων (x,y,z) ή/και γεωγραφικό πλάτος και μήκος και ύψος, με βάση γεωδαιτικό οριζόντιο και κατακόρυφο σύστημα αναφοράς (datum).</dct:description>
		<skos:inScheme rdf:resource="http://inspire-registry.jrc.ec.europa.eu/registers/FCD/items"/>
	</inspire:SpatialObjectType>
	<inspire:SpatialObjectType rdf:about="http://inspire-registry.jrc.ec.europa.eu/registers/FCD/items/395">
		<inspire:itemStatus>valid</inspire:itemStatus>
		<inspire:dateAccepted>2010-01-19T16:18:31.044+01:00</inspire:dateAccepted>
		<skos:prefLabel xml:lang="en">Embankment</skos:prefLabel>
		<skos:definition xml:lang="en">A man-made raised long mound of earth or other material.</skos:definition>
		<dct:description xml:lang="en">SOURCE [DFDD].
NOTE 1 Includes retaining walls, harbours, dikes.
NOTE 2 Regarded as a candidate spatial object in Annex III theme 'Natural risk zones' due to its role in limiting flooding.
This type is a candidate type to be considered by the spatial data theme Natural risk zones in Annex III to Directive 2007/2/EC.</dct:description>
		<skos:prefLabel xml:lang="el">SAMPLE ALTERNATIVE EXPRESSION - αναφορά</skos:prefLabel>
		<skos:definition xml:lang="el">Συστήματα συντεταγμένων</skos:definition>
		<dct:description xml:lang="el">Συστήματα για μονοσήμαντη αναφορά χωρικών πληροφοριών στον χώρο, ως σύνολο συντεταγμένων (x,y,z) ή/και γεωγραφικό πλάτος και μήκος και ύψος, με βάση γεωδαιτικό οριζόντιο και κατακόρυφο σύστημα αναφοράς (datum).</dct:description>
		<skos:inScheme rdf:resource="http://inspire-registry.jrc.ec.europa.eu/registers/FCD/items"/>
	</inspire:SpatialObjectType>
	<inspire:SpatialObjectType rdf:about="http://inspire-registry.jrc.ec.europa.eu/registers/FCD/items/396">
		<inspire:itemStatus>valid</inspire:itemStatus>
		<inspire:dateAccepted>2010-01-19T16:18:31.580+01:00</inspire:dateAccepted>
		<skos:prefLabel xml:lang="en">Falls</skos:prefLabel>
		<skos:definition xml:lang="en">A vertically descending part of a watercourse where it falls from a height.</skos:definition>
		<skos:prefLabel xml:lang="el">SAMPLE ALTERNATIVE EXPRESSION - αναφορά</skos:prefLabel>
		<skos:definition xml:lang="el">Συστήματα συντεταγμένων</skos:definition>
		<dct:description xml:lang="el">Συστήματα για μονοσήμαντη αναφορά χωρικών πληροφοριών στον χώρο, ως σύνολο συντεταγμένων (x,y,z) ή/και γεωγραφικό πλάτος και μήκος και ύψος, με βάση γεωδαιτικό οριζόντιο και κατακόρυφο σύστημα αναφοράς (datum).</dct:description>
		<skos:inScheme rdf:resource="http://inspire-registry.jrc.ec.europa.eu/registers/FCD/items"/>
	</inspire:SpatialObjectType>
	<inspire:SpatialObjectType rdf:about="http://inspire-registry.jrc.ec.europa.eu/registers/FCD/items/397">
		<inspire:itemStatus>valid</inspire:itemStatus>
		<inspire:dateAccepted>2010-01-19T16:18:32.050+01:00</inspire:dateAccepted>
		<skos:prefLabel xml:lang="en">Fluvial point</skos:prefLabel>
		<skos:definition xml:lang="en">A hydro point of interest that affects the flow of a watercourse.</skos:definition>
		<skos:prefLabel xml:lang="el">SAMPLE ALTERNATIVE EXPRESSION - αναφορά</skos:prefLabel>
		<skos:definition xml:lang="el">Συστήματα συντεταγμένων</skos:definition>
		<dct:description xml:lang="el">Συστήματα για μονοσήμαντη αναφορά χωρικών πληροφοριών στον χώρο, ως σύνολο συντεταγμένων (x,y,z) ή/και γεωγραφικό πλάτος και μήκος και ύψος, με βάση γεωδαιτικό οριζόντιο και κατακόρυφο σύστημα αναφοράς (datum).</dct:description>
		<skos:inScheme rdf:resource="http://inspire-registry.jrc.ec.europa.eu/registers/FCD/items"/>
	</inspire:SpatialObjectType>
	<inspire:SpatialObjectType rdf:about="http://inspire-registry.jrc.ec.europa.eu/registers/FCD/items/398">
		<inspire:itemStatus>valid</inspire:itemStatus>
		<inspire:dateAccepted>2010-01-19T16:18:32.530+01:00</inspire:dateAccepted>
		<skos:prefLabel xml:lang="en">Ford</skos:prefLabel>
		<skos:definition xml:lang="en">A shallow part of a watercourse used as a road crossing.</skos:definition>
		<skos:prefLabel xml:lang="el">SAMPLE ALTERNATIVE EXPRESSION - αναφορά</skos:prefLabel>
		<skos:definition xml:lang="el">Συστήματα συντεταγμένων</skos:definition>
		<dct:description xml:lang="el">Συστήματα για μονοσήμαντη αναφορά χωρικών πληροφοριών στον χώρο, ως σύνολο συντεταγμένων (x,y,z) ή/και γεωγραφικό πλάτος και μήκος και ύψος, με βάση γεωδαιτικό οριζόντιο και κατακόρυφο σύστημα αναφοράς (datum).</dct:description>
		<skos:inScheme rdf:resource="http://inspire-registry.jrc.ec.europa.eu/registers/FCD/items"/>
	</inspire:SpatialObjectType>
	<inspire:SpatialObjectType rdf:about="http://inspire-registry.jrc.ec.europa.eu/registers/FCD/items/399">
		<inspire:itemStatus>valid</inspire:itemStatus>
		<inspire:dateAccepted>2010-01-19T16:18:32.697+01:00</inspire:dateAccepted>
		<skos:prefLabel xml:lang="en">Hydro Node</skos:prefLabel>
		<skos:definition xml:lang="en">A node within the hydrographic network.</skos:definition>
		<dct:description xml:lang="en">NOTE May represent a physical confluence, bifurcation/confluence/vanishing point etc, or it may be associated with a hydrographic point of interest or facility.</dct:description>
		<skos:prefLabel xml:lang="el">SAMPLE ALTERNATIVE EXPRESSION - αναφορά</skos:prefLabel>
		<skos:definition xml:lang="el">Συστήματα συντεταγμένων</skos:definition>
		<dct:description xml:lang="el">Συστήματα για μονοσήμαντη αναφορά χωρικών πληροφοριών στον χώρο, ως σύνολο συντεταγμένων (x,y,z) ή/και γεωγραφικό πλάτος και μήκος και ύψος, με βάση γεωδαιτικό οριζόντιο και κατακόρυφο σύστημα αναφοράς (datum).</dct:description>
		<skos:inScheme rdf:resource="http://inspire-registry.jrc.ec.europa.eu/registers/FCD/items"/>
	</inspire:SpatialObjectType>
	<inspire:SpatialObjectType rdf:about="http://inspire-registry.jrc.ec.europa.eu/registers/FCD/items/400">
		<inspire:itemStatus>valid</inspire:itemStatus>
		<inspire:dateAccepted>2010-01-19T16:18:32.859+01:00</inspire:dateAccepted>
		<skos:prefLabel xml:lang="en">Hydro Object</skos:prefLabel>
		<skos:definition xml:lang="en">An identity base for hydrographic (including man-made) objects in the real world.</skos:definition>
		<dct:description xml:lang="en">NOTE Derived 'views' of real-world hydrographic objects are represented through specialisations in other application schemas; all representations of the same real-world object share a common geographic name or hydrographic identifier.</dct:description>
		<skos:prefLabel xml:lang="el">SAMPLE ALTERNATIVE EXPRESSION - αναφορά</skos:prefLabel>
		<skos:definition xml:lang="el">Συστήματα συντεταγμένων</skos:definition>
		<dct:description xml:lang="el">Συστήματα για μονοσήμαντη αναφορά χωρικών πληροφοριών στον χώρο, ως σύνολο συντεταγμένων (x,y,z) ή/και γεωγραφικό πλάτος και μήκος και ύψος, με βάση γεωδαιτικό οριζόντιο και κατακόρυφο σύστημα αναφοράς (datum).</dct:description>
		<skos:inScheme rdf:resource="http://inspire-registry.jrc.ec.europa.eu/registers/FCD/items"/>
	</inspire:SpatialObjectType>
	<inspire:SpatialObjectType rdf:about="http://inspire-registry.jrc.ec.europa.eu/registers/FCD/items/401">
		<inspire:itemStatus>valid</inspire:itemStatus>
		<inspire:dateAccepted>2010-01-19T16:18:33.030+01:00</inspire:dateAccepted>
		<skos:prefLabel xml:lang="en">Hydro Point of Interest</skos:prefLabel>
		<skos:definition xml:lang="en">A natural place where water appears, disappears or changes its flow.</skos:definition>
		<dct:description xml:lang="en">EXAMPLE Fluvial points (waterfall, cascade, rapids, breaker), spring/water hole (spring, source, geyser, thermal spring, natural fountain, well, also fumarole, artesian), sinkhole (sinkhole, drainage loss).
NOTE A hydro point of interest may create a flow constriction in the network.</dct:description>
		<skos:prefLabel xml:lang="el">SAMPLE ALTERNATIVE EXPRESSION - αναφορά</skos:prefLabel>
		<skos:definition xml:lang="el">Συστήματα συντεταγμένων</skos:definition>
		<dct:description xml:lang="el">Συστήματα για μονοσήμαντη αναφορά χωρικών πληροφοριών στον χώρο, ως σύνολο συντεταγμένων (x,y,z) ή/και γεωγραφικό πλάτος και μήκος και ύψος, με βάση γεωδαιτικό οριζόντιο και κατακόρυφο σύστημα αναφοράς (datum).</dct:description>
		<skos:inScheme rdf:resource="http://inspire-registry.jrc.ec.europa.eu/registers/FCD/items"/>
	</inspire:SpatialObjectType>
	<inspire:SpatialObjectType rdf:about="http://inspire-registry.jrc.ec.europa.eu/registers/FCD/items/402">
		<inspire:itemStatus>valid</inspire:itemStatus>
		<inspire:dateAccepted>2010-01-19T16:18:33.272+01:00</inspire:dateAccepted>
		<skos:prefLabel xml:lang="en">Hydro-Power Plant</skos:prefLabel>
		<skos:definition xml:lang="en">A facility for the generation of power from moving water.</skos:definition>
		<dct:description xml:lang="en">NOTE Regarded as a candidate spatial object in Annex III theme 'Energy resources' due to its primary energy-production role.
This type is a candidate type to be considered by the spatial data theme Energy resources in Annex III to Directive 2007/2/EC.</dct:description>
		<skos:prefLabel xml:lang="el">SAMPLE ALTERNATIVE EXPRESSION - αναφορά</skos:prefLabel>
		<skos:definition xml:lang="el">Συστήματα συντεταγμένων</skos:definition>
		<dct:description xml:lang="el">Συστήματα για μονοσήμαντη αναφορά χωρικών πληροφοριών στον χώρο, ως σύνολο συντεταγμένων (x,y,z) ή/και γεωγραφικό πλάτος και μήκος και ύψος, με βάση γεωδαιτικό οριζόντιο και κατακόρυφο σύστημα αναφοράς (datum).</dct:description>
		<skos:inScheme rdf:resource="http://inspire-registry.jrc.ec.europa.eu/registers/FCD/items"/>
	</inspire:SpatialObjectType>
	<inspire:SpatialObjectType rdf:about="http://inspire-registry.jrc.ec.europa.eu/registers/FCD/items/403">
		<inspire:itemStatus>valid</inspire:itemStatus>
		<inspire:dateAccepted>2010-01-19T16:18:33.438+01:00</inspire:dateAccepted>
		<skos:prefLabel xml:lang="en">Inundated Land</skos:prefLabel>
		<skos:definition xml:lang="en">A tract periodically covered by flood water, excluding tidal waters.</skos:definition>
		<dct:description xml:lang="en">SOURCE [DFDD].
NOTE 1 It may be caused by either uncontrolled inundation (for example:flooding due to a river overflowing its banks or low-lying regions accumulating standing water following severe rainfall) or controlled inundation (for example: flooded by the regulation of the level of a reservoir). [DFDD].
NOTE 2 Inundation for irrigation purposes is excluded. 
NOTE 3 Regarded as a candidate spatial object in Annex III theme 'Natural risk zones' due to the relationship (by definition) with flooding.
This type is a candidate type to be considered by the spatial data theme Natural risk zones in Annex III to Directive 2007/2/EC.</dct:description>
		<skos:prefLabel xml:lang="el">SAMPLE ALTERNATIVE EXPRESSION - αναφορά</skos:prefLabel>
		<skos:definition xml:lang="el">Συστήματα συντεταγμένων</skos:definition>
		<dct:description xml:lang="el">Συστήματα για μονοσήμαντη αναφορά χωρικών πληροφοριών στον χώρο, ως σύνολο συντεταγμένων (x,y,z) ή/και γεωγραφικό πλάτος και μήκος και ύψος, με βάση γεωδαιτικό οριζόντιο και κατακόρυφο σύστημα αναφοράς (datum).</dct:description>
		<skos:inScheme rdf:resource="http://inspire-registry.jrc.ec.europa.eu/registers/FCD/items"/>
	</inspire:SpatialObjectType>
	<inspire:SpatialObjectType rdf:about="http://inspire-registry.jrc.ec.europa.eu/registers/FCD/items/404">
		<inspire:itemStatus>valid</inspire:itemStatus>
		<inspire:dateAccepted>2010-01-19T16:18:33.991+01:00</inspire:dateAccepted>
		<skos:prefLabel xml:lang="en">Land-Water boundary</skos:prefLabel>
		<skos:definition xml:lang="en">The line where a land mass is in contact with a body of water.</skos:definition>
		<dct:description xml:lang="en">SOURCE [DFDD].
NOTE The plane of reference for the land-water boundary should be a high water datum, such as 'Mean High Water Springs', 'High Water' or 'Mean Higher High Water'. Where there is little appreciable change in waterlevels / tide at the adjacent shore, then 'Mean Sea Level' or 'Local Datum' may be used.</dct:description>
		<skos:prefLabel xml:lang="el">SAMPLE ALTERNATIVE EXPRESSION - αναφορά</skos:prefLabel>
		<skos:definition xml:lang="el">Συστήματα συντεταγμένων</skos:definition>
		<dct:description xml:lang="el">Συστήματα για μονοσήμαντη αναφορά χωρικών πληροφοριών στον χώρο, ως σύνολο συντεταγμένων (x,y,z) ή/και γεωγραφικό πλάτος και μήκος και ύψος, με βάση γεωδαιτικό οριζόντιο και κατακόρυφο σύστημα αναφοράς (datum).</dct:description>
		<skos:inScheme rdf:resource="http://inspire-registry.jrc.ec.europa.eu/registers/FCD/items"/>
	</inspire:SpatialObjectType>
	<inspire:SpatialObjectType rdf:about="http://inspire-registry.jrc.ec.europa.eu/registers/FCD/items/405">
		<inspire:itemStatus>valid</inspire:itemStatus>
		<inspire:dateAccepted>2010-01-19T16:18:34.173+01:00</inspire:dateAccepted>
		<skos:prefLabel xml:lang="en">Man-made object</skos:prefLabel>
		<skos:definition xml:lang="en">An artificial object which lies inside a body of water and has one of the following types of function: 
- Retains the water; - Regulates the quantity of water; - Alters the course of the water; - Allows watercourses to cross each other.</skos:definition>
		<skos:prefLabel xml:lang="el">SAMPLE ALTERNATIVE EXPRESSION - αναφορά</skos:prefLabel>
		<skos:definition xml:lang="el">Συστήματα συντεταγμένων</skos:definition>
		<dct:description xml:lang="el">Συστήματα για μονοσήμαντη αναφορά χωρικών πληροφοριών στον χώρο, ως σύνολο συντεταγμένων (x,y,z) ή/και γεωγραφικό πλάτος και μήκος και ύψος, με βάση γεωδαιτικό οριζόντιο και κατακόρυφο σύστημα αναφοράς (datum).</dct:description>
		<skos:inScheme rdf:resource="http://inspire-registry.jrc.ec.europa.eu/registers/FCD/items"/>
	</inspire:SpatialObjectType>
	<inspire:SpatialObjectType rdf:about="http://inspire-registry.jrc.ec.europa.eu/registers/FCD/items/406">
		<inspire:itemStatus>valid</inspire:itemStatus>
		<inspire:dateAccepted>2010-01-19T16:18:34.375+01:00</inspire:dateAccepted>
		<skos:prefLabel xml:lang="en">Ocean Region</skos:prefLabel>
		<skos:definition xml:lang="en">One of the three large regions of the world-wide ocean, each with associated sub- and marginal areas and subject to an independent flow-regime.</skos:definition>
		<dct:description xml:lang="en">SOURCE [DFDD].
NOTE Regarded as a candidate spatial object in Annex II theme 'Sea Regions' due to the close fit to the definition in 2007/2/EC Ann III. 16.
This type is a candidate type to be considered by the spatial data theme Sea regions in Annex III to Directive 2007/2/EC.</dct:description>
		<skos:prefLabel xml:lang="el">SAMPLE ALTERNATIVE EXPRESSION - αναφορά</skos:prefLabel>
		<skos:definition xml:lang="el">Συστήματα συντεταγμένων</skos:definition>
		<dct:description xml:lang="el">Συστήματα για μονοσήμαντη αναφορά χωρικών πληροφοριών στον χώρο, ως σύνολο συντεταγμένων (x,y,z) ή/και γεωγραφικό πλάτος και μήκος και ύψος, με βάση γεωδαιτικό οριζόντιο και κατακόρυφο σύστημα αναφοράς (datum).</dct:description>
		<skos:inScheme rdf:resource="http://inspire-registry.jrc.ec.europa.eu/registers/FCD/items"/>
	</inspire:SpatialObjectType>
	<inspire:SpatialObjectType rdf:about="http://inspire-registry.jrc.ec.europa.eu/registers/FCD/items/407">
		<inspire:itemStatus>valid</inspire:itemStatus>
		<inspire:dateAccepted>2010-01-19T16:18:34.801+01:00</inspire:dateAccepted>
		<skos:prefLabel xml:lang="en">PumpingStation</skos:prefLabel>
		<skos:definition xml:lang="en">A facility to move solids, liquids or gases by means of pressure or suction.</skos:definition>
		<dct:description xml:lang="en">SOURCE [EuroRegionalMap].
NOTE Regarded as a candidate spatial object in Annex III theme 'Utility and governmental services' due to its role in water supply/waste management/etc., which are mentioned in the definition 2007/2/EC Ann III. 6.
This type is a candidate type to be considered by the spatial data theme Utility and governmental services in Annex III to Directive 2007/2/EC.</dct:description>
		<skos:prefLabel xml:lang="el">SAMPLE ALTERNATIVE EXPRESSION - αναφορά</skos:prefLabel>
		<skos:definition xml:lang="el">Συστήματα συντεταγμένων</skos:definition>
		<dct:description xml:lang="el">Συστήματα για μονοσήμαντη αναφορά χωρικών πληροφοριών στον χώρο, ως σύνολο συντεταγμένων (x,y,z) ή/και γεωγραφικό πλάτος και μήκος και ύψος, με βάση γεωδαιτικό οριζόντιο και κατακόρυφο σύστημα αναφοράς (datum).</dct:description>
		<skos:inScheme rdf:resource="http://inspire-registry.jrc.ec.europa.eu/registers/FCD/items"/>
	</inspire:SpatialObjectType>
	<inspire:SpatialObjectType rdf:about="http://inspire-registry.jrc.ec.europa.eu/registers/FCD/items/408">
		<inspire:itemStatus>valid</inspire:itemStatus>
		<inspire:dateAccepted>2010-01-19T16:18:35.293+01:00</inspire:dateAccepted>
		<skos:prefLabel xml:lang="en">Rapids</skos:prefLabel>
		<skos:definition xml:lang="en">Portions of a stream with accelerated current where it descends rapidly but without a break in the slope of the bed sufficient to form a waterfall.</skos:definition>
		<dct:description xml:lang="en">SOURCE [DFDD].</dct:description>
		<skos:prefLabel xml:lang="el">SAMPLE ALTERNATIVE EXPRESSION - αναφορά</skos:prefLabel>
		<skos:definition xml:lang="el">Συστήματα συντεταγμένων</skos:definition>
		<dct:description xml:lang="el">Συστήματα για μονοσήμαντη αναφορά χωρικών πληροφοριών στον χώρο, ως σύνολο συντεταγμένων (x,y,z) ή/και γεωγραφικό πλάτος και μήκος και ύψος, με βάση γεωδαιτικό οριζόντιο και κατακόρυφο σύστημα αναφοράς (datum).</dct:description>
		<skos:inScheme rdf:resource="http://inspire-registry.jrc.ec.europa.eu/registers/FCD/items"/>
	</inspire:SpatialObjectType>
	<inspire:SpatialObjectType rdf:about="http://inspire-registry.jrc.ec.europa.eu/registers/FCD/items/409">
		<inspire:itemStatus>valid</inspire:itemStatus>
		<inspire:dateAccepted>2010-01-19T16:18:35.486+01:00</inspire:dateAccepted>
		<skos:prefLabel xml:lang="en">River Basin</skos:prefLabel>
		<skos:definition xml:lang="en">The area of land from which all surface run-off flows through a sequence of streams, rivers and, possibly, lakes into the sea at a single river mouth, estuary or delta.</skos:definition>
		<dct:description xml:lang="en">SOURCE [2000/60/EC Art. 2(13)].</dct:description>
		<skos:prefLabel xml:lang="el">SAMPLE ALTERNATIVE EXPRESSION - αναφορά</skos:prefLabel>
		<skos:definition xml:lang="el">Συστήματα συντεταγμένων</skos:definition>
		<dct:description xml:lang="el">Συστήματα για μονοσήμαντη αναφορά χωρικών πληροφοριών στον χώρο, ως σύνολο συντεταγμένων (x,y,z) ή/και γεωγραφικό πλάτος και μήκος και ύψος, με βάση γεωδαιτικό οριζόντιο και κατακόρυφο σύστημα αναφοράς (datum).</dct:description>
		<skos:inScheme rdf:resource="http://inspire-registry.jrc.ec.europa.eu/registers/FCD/items"/>
	</inspire:SpatialObjectType>
	<inspire:SpatialObjectType rdf:about="http://inspire-registry.jrc.ec.europa.eu/registers/FCD/items/410">
		<inspire:itemStatus>valid</inspire:itemStatus>
		<inspire:dateAccepted>2010-01-19T16:18:35.699+01:00</inspire:dateAccepted>
		<skos:prefLabel xml:lang="en">Shore</skos:prefLabel>
		<skos:definition xml:lang="en">The narrow strip of land in immediate contact with any body of water including the area between high and low water lines.</skos:definition>
		<dct:description xml:lang="en">SOURCE [IHO S-32].
NOTE Regarded as a candidate spatial object in Annex II theme 'Land cover' due to unconsolidated shore inclusion in coastal land-cover classificaction schemes.
This type is a candidate type to be considered by the spatial data theme Land cover in Annex II to Directive 2007/2/EC.</dct:description>
		<skos:prefLabel xml:lang="el">SAMPLE ALTERNATIVE EXPRESSION - αναφορά</skos:prefLabel>
		<skos:definition xml:lang="el">Συστήματα συντεταγμένων</skos:definition>
		<dct:description xml:lang="el">Συστήματα για μονοσήμαντη αναφορά χωρικών πληροφοριών στον χώρο, ως σύνολο συντεταγμένων (x,y,z) ή/και γεωγραφικό πλάτος και μήκος και ύψος, με βάση γεωδαιτικό οριζόντιο και κατακόρυφο σύστημα αναφοράς (datum).</dct:description>
		<skos:inScheme rdf:resource="http://inspire-registry.jrc.ec.europa.eu/registers/FCD/items"/>
	</inspire:SpatialObjectType>
	<inspire:SpatialObjectType rdf:about="http://inspire-registry.jrc.ec.europa.eu/registers/FCD/items/411">
		<inspire:itemStatus>valid</inspire:itemStatus>
		<inspire:dateAccepted>2010-01-19T16:18:36.228+01:00</inspire:dateAccepted>
		<skos:prefLabel xml:lang="en">Shoreline construction</skos:prefLabel>
		<skos:definition xml:lang="en">An artificial structure attached to land bordering a body of water and fixed in position.</skos:definition>
		<dct:description xml:lang="en">SOURCE [DFDD].
NOTE 1 It is usually fixed to the waterbody bottom (for example: a mole) but may occasionally be fixed in position (for example: attached to the shore at one end and held between pilings at the other) but floating. Shoreline constructions are normally used for berthing and/or protection.
NOTE 2 Includes breakwater/groyne/wharf; but has more flexibility - also applies to inland waters.</dct:description>
		<skos:prefLabel xml:lang="el">SAMPLE ALTERNATIVE EXPRESSION - αναφορά</skos:prefLabel>
		<skos:definition xml:lang="el">Συστήματα συντεταγμένων</skos:definition>
		<dct:description xml:lang="el">Συστήματα για μονοσήμαντη αναφορά χωρικών πληροφοριών στον χώρο, ως σύνολο συντεταγμένων (x,y,z) ή/και γεωγραφικό πλάτος και μήκος και ύψος, με βάση γεωδαιτικό οριζόντιο και κατακόρυφο σύστημα αναφοράς (datum).</dct:description>
		<skos:inScheme rdf:resource="http://inspire-registry.jrc.ec.europa.eu/registers/FCD/items"/>
	</inspire:SpatialObjectType>
	<inspire:SpatialObjectType rdf:about="http://inspire-registry.jrc.ec.europa.eu/registers/FCD/items/412">
		<inspire:itemStatus>valid</inspire:itemStatus>
		<inspire:dateAccepted>2010-01-19T16:18:36.772+01:00</inspire:dateAccepted>
		<skos:prefLabel xml:lang="en">Standing water</skos:prefLabel>
		<skos:definition xml:lang="en">A body of water that is entirely surrounded by land.</skos:definition>
		<dct:description xml:lang="en">SOURCE [DFDD].
NOTE It may occur in a natural terrain depression in which water collects, or may be impounded by a dam, or formed by its bed being hollowed out of the soil, or formed by embanking and/or damming up a natural hollow (for example: by a beaver dam). It may be connected to inflowing / outflowing watercourses or other standing waters.</dct:description>
		<skos:prefLabel xml:lang="el">SAMPLE ALTERNATIVE EXPRESSION - αναφορά</skos:prefLabel>
		<skos:definition xml:lang="el">Συστήματα συντεταγμένων</skos:definition>
		<dct:description xml:lang="el">Συστήματα για μονοσήμαντη αναφορά χωρικών πληροφοριών στον χώρο, ως σύνολο συντεταγμένων (x,y,z) ή/και γεωγραφικό πλάτος και μήκος και ύψος, με βάση γεωδαιτικό οριζόντιο και κατακόρυφο σύστημα αναφοράς (datum).</dct:description>
		<skos:inScheme rdf:resource="http://inspire-registry.jrc.ec.europa.eu/registers/FCD/items"/>
	</inspire:SpatialObjectType>
	<inspire:SpatialObjectType rdf:about="http://inspire-registry.jrc.ec.europa.eu/registers/FCD/items/413">
		<inspire:itemStatus>valid</inspire:itemStatus>
		<inspire:dateAccepted>2010-01-19T16:18:37.339+01:00</inspire:dateAccepted>
		<skos:prefLabel xml:lang="en">Surface water</skos:prefLabel>
		<skos:definition xml:lang="en">Any known inland waterway body.</skos:definition>
		<dct:description xml:lang="en">SOURCE [Based on DFDD].
EXAMPLE Lake/pond, reservoir, river/stream, etc.
NOTE May include islands, represented as 'holes' in its geometry. Islands may be surrounded by a shore and / or land-ware boundary.</dct:description>
		<skos:prefLabel xml:lang="el">SAMPLE ALTERNATIVE EXPRESSION - αναφορά</skos:prefLabel>
		<skos:definition xml:lang="el">Συστήματα συντεταγμένων</skos:definition>
		<dct:description xml:lang="el">Συστήματα για μονοσήμαντη αναφορά χωρικών πληροφοριών στον χώρο, ως σύνολο συντεταγμένων (x,y,z) ή/και γεωγραφικό πλάτος και μήκος και ύψος, με βάση γεωδαιτικό οριζόντιο και κατακόρυφο σύστημα αναφοράς (datum).</dct:description>
		<skos:inScheme rdf:resource="http://inspire-registry.jrc.ec.europa.eu/registers/FCD/items"/>
	</inspire:SpatialObjectType>
	<inspire:SpatialObjectType rdf:about="http://inspire-registry.jrc.ec.europa.eu/registers/FCD/items/414">
		<inspire:itemStatus>valid</inspire:itemStatus>
		<inspire:dateAccepted>2010-01-19T16:18:37.783+01:00</inspire:dateAccepted>
		<skos:prefLabel xml:lang="en">Watercourse Link</skos:prefLabel>
		<skos:definition xml:lang="en">A segment of a watercourse within a hydrographic network.</skos:definition>
		<dct:description xml:lang="en">NOTE A watercourse link may be fictitious, with no direct correspondence to a real-world object and included only to ensure a closed network.
EXAMPLE Fictitious examples:
- virtual network segment in coastal water area
- virtual network segment in lake area
- virtual network segment in river to connect tributary
- virtual network segment in transitional water area</dct:description>
		<skos:prefLabel xml:lang="el">SAMPLE ALTERNATIVE EXPRESSION - αναφορά</skos:prefLabel>
		<skos:definition xml:lang="el">Συστήματα συντεταγμένων</skos:definition>
		<dct:description xml:lang="el">Συστήματα για μονοσήμαντη αναφορά χωρικών πληροφοριών στον χώρο, ως σύνολο συντεταγμένων (x,y,z) ή/και γεωγραφικό πλάτος και μήκος και ύψος, με βάση γεωδαιτικό οριζόντιο και κατακόρυφο σύστημα αναφοράς (datum).</dct:description>
		<skos:inScheme rdf:resource="http://inspire-registry.jrc.ec.europa.eu/registers/FCD/items"/>
	</inspire:SpatialObjectType>
	<inspire:SpatialObjectType rdf:about="http://inspire-registry.jrc.ec.europa.eu/registers/FCD/items/415">
		<inspire:itemStatus>valid</inspire:itemStatus>
		<inspire:dateAccepted>2010-01-19T16:18:37.931+01:00</inspire:dateAccepted>
		<skos:prefLabel xml:lang="en">Watercourse Link Sequence</skos:prefLabel>
		<skos:definition xml:lang="en">A sequence of watercourse links representing a non-branching path through a hydrographic network.</skos:definition>
		<skos:prefLabel xml:lang="el">SAMPLE ALTERNATIVE EXPRESSION - αναφορά</skos:prefLabel>
		<skos:definition xml:lang="el">Συστήματα συντεταγμένων</skos:definition>
		<dct:description xml:lang="el">Συστήματα για μονοσήμαντη αναφορά χωρικών πληροφοριών στον χώρο, ως σύνολο συντεταγμένων (x,y,z) ή/και γεωγραφικό πλάτος και μήκος και ύψος, με βάση γεωδαιτικό οριζόντιο και κατακόρυφο σύστημα αναφοράς (datum).</dct:description>
		<skos:inScheme rdf:resource="http://inspire-registry.jrc.ec.europa.eu/registers/FCD/items"/>
	</inspire:SpatialObjectType>
	<inspire:SpatialObjectType rdf:about="http://inspire-registry.jrc.ec.europa.eu/registers/FCD/items/416">
		<inspire:itemStatus>valid</inspire:itemStatus>
		<inspire:dateAccepted>2010-01-19T16:18:38.386+01:00</inspire:dateAccepted>
		<skos:prefLabel xml:lang="en">Watercourse Separated Crossing</skos:prefLabel>
		<skos:definition xml:lang="en">An element in the hydrographic network used to indicate non-interacting crossing of watercourse links separated by level.</skos:definition>
		<dct:description xml:lang="en">NOTE The crossing may legitimately break a no-intersection quality rule.</dct:description>
		<skos:prefLabel xml:lang="el">SAMPLE ALTERNATIVE EXPRESSION - αναφορά</skos:prefLabel>
		<skos:definition xml:lang="el">Συστήματα συντεταγμένων</skos:definition>
		<dct:description xml:lang="el">Συστήματα για μονοσήμαντη αναφορά χωρικών πληροφοριών στον χώρο, ως σύνολο συντεταγμένων (x,y,z) ή/και γεωγραφικό πλάτος και μήκος και ύψος, με βάση γεωδαιτικό οριζόντιο και κατακόρυφο σύστημα αναφοράς (datum).</dct:description>
		<skos:inScheme rdf:resource="http://inspire-registry.jrc.ec.europa.eu/registers/FCD/items"/>
	</inspire:SpatialObjectType>
	<inspire:SpatialObjectType rdf:about="http://inspire-registry.jrc.ec.europa.eu/registers/FCD/items/417">
		<inspire:itemStatus>valid</inspire:itemStatus>
		<inspire:dateAccepted>2010-01-19T16:18:38.857+01:00</inspire:dateAccepted>
		<skos:prefLabel xml:lang="en">Wetland</skos:prefLabel>
		<skos:definition xml:lang="en">A poorly drained or periodically flooded area where the soil is saturated with water, and vegetation is supported.</skos:definition>
		<dct:description xml:lang="en">SOURCE [EuroRegionalMap].
EXAMPLE Marsh/swamp, bog/moor.
NOTE Regarded as a candidate spatial object in Annex II theme 'Land cover' due to explicit mention in 2007/2/EC Ann. II 2.
This type is a candidate type to be considered by the spatial data theme Land cover in Annex II to Directive 2007/2/EC.</dct:description>
		<skos:prefLabel xml:lang="el">SAMPLE ALTERNATIVE EXPRESSION - αναφορά</skos:prefLabel>
		<skos:definition xml:lang="el">Συστήματα συντεταγμένων</skos:definition>
		<dct:description xml:lang="el">Συστήματα για μονοσήμαντη αναφορά χωρικών πληροφοριών στον χώρο, ως σύνολο συντεταγμένων (x,y,z) ή/και γεωγραφικό πλάτος και μήκος και ύψος, με βάση γεωδαιτικό οριζόντιο και κατακόρυφο σύστημα αναφοράς (datum).</dct:description>
		<skos:inScheme rdf:resource="http://inspire-registry.jrc.ec.europa.eu/registers/FCD/items"/>
	</inspire:SpatialObjectType>
	<inspire:SpatialObjectType rdf:about="http://inspire-registry.jrc.ec.europa.eu/registers/FCD/items/418">
		<inspire:itemStatus>valid</inspire:itemStatus>
		<inspire:dateAccepted>2010-01-19T16:18:39.078+01:00</inspire:dateAccepted>
		<skos:prefLabel xml:lang="en">WFD Coastal Water</skos:prefLabel>
		<skos:definition xml:lang="en">Surface water on the landward side of a line, every point of which is at a distance of one nautical mile on the seaward side from the nearest point of the baseline from which the breadth of territorial waters is measured, extending where appropriate up to the outer limit of transitional waters.</skos:definition>
		<dct:description xml:lang="en">SOURCE [2000/60/EC Art. 2(7)]. 
NOTE All WFD spatial object types are regarded as candidate spatial objects in Annex III theme 'Area management/restriction/regulation zones and reporting units' due to their primary function for reporting under Directive 2000/60/EC. 
This type is a candidate type to be considered by the spatial data theme Area management/restriction/regulation zones and reporting units in Annex III to Directive 2007/2/EC.</dct:description>
		<skos:prefLabel xml:lang="el">SAMPLE ALTERNATIVE EXPRESSION - αναφορά</skos:prefLabel>
		<skos:definition xml:lang="el">Συστήματα συντεταγμένων</skos:definition>
		<dct:description xml:lang="el">Συστήματα για μονοσήμαντη αναφορά χωρικών πληροφοριών στον χώρο, ως σύνολο συντεταγμένων (x,y,z) ή/και γεωγραφικό πλάτος και μήκος και ύψος, με βάση γεωδαιτικό οριζόντιο και κατακόρυφο σύστημα αναφοράς (datum).</dct:description>
		<skos:inScheme rdf:resource="http://inspire-registry.jrc.ec.europa.eu/registers/FCD/items"/>
	</inspire:SpatialObjectType>
	<inspire:SpatialObjectType rdf:about="http://inspire-registry.jrc.ec.europa.eu/registers/FCD/items/419">
		<inspire:itemStatus>valid</inspire:itemStatus>
		<inspire:dateAccepted>2010-01-19T16:18:39.272+01:00</inspire:dateAccepted>
		<skos:prefLabel xml:lang="en">WFD Ground Water Body</skos:prefLabel>
		<skos:definition xml:lang="en">A distinct volume of groundwater within an aquifer or aquifers.</skos:definition>
		<dct:description xml:lang="en">SOURCE [2000/60/EC Art. 2(12)].
NOTE All WFD spatial object types are regarded as candidate spatial objects in Annex III theme 'Area management/restriction/regulation zones and reporting units' due to their primary function for reporting under Directive 2000/60/EC.
This type is a candidate type to be considered by the spatial data theme Area management/restriction/regulation zones and reporting units in Annex III to Directive 2007/2/EC.</dct:description>
		<skos:prefLabel xml:lang="el">SAMPLE ALTERNATIVE EXPRESSION - αναφορά</skos:prefLabel>
		<skos:definition xml:lang="el">Συστήματα συντεταγμένων</skos:definition>
		<dct:description xml:lang="el">Συστήματα για μονοσήμαντη αναφορά χωρικών πληροφοριών στον χώρο, ως σύνολο συντεταγμένων (x,y,z) ή/και γεωγραφικό πλάτος και μήκος και ύψος, με βάση γεωδαιτικό οριζόντιο και κατακόρυφο σύστημα αναφοράς (datum).</dct:description>
		<skos:inScheme rdf:resource="http://inspire-registry.jrc.ec.europa.eu/registers/FCD/items"/>
	</inspire:SpatialObjectType>
	<inspire:SpatialObjectType rdf:about="http://inspire-registry.jrc.ec.europa.eu/registers/FCD/items/420">
		<inspire:itemStatus>valid</inspire:itemStatus>
		<inspire:dateAccepted>2010-01-19T16:18:39.465+01:00</inspire:dateAccepted>
		<skos:prefLabel xml:lang="en">WFD Lake</skos:prefLabel>
		<skos:definition xml:lang="en">A body of standing inland surface water.</skos:definition>
		<dct:description xml:lang="en">SOURCE [2000/60/EC Art. 2(5)].
NOTE All WFD spatial object types are regarded as candidate spatial objects in Annex III theme 'Area management/restriction/regulation zones and reporting units' due to their primary function for reporting under Directive 2000/60/EC.
This type is a candidate type to be considered by the spatial data theme Area management/restriction/regulation zones and reporting units in Annex III to Directive 2007/2/EC.</dct:description>
		<skos:prefLabel xml:lang="el">SAMPLE ALTERNATIVE EXPRESSION - αναφορά</skos:prefLabel>
		<skos:definition xml:lang="el">Συστήματα συντεταγμένων</skos:definition>
		<dct:description xml:lang="el">Συστήματα για μονοσήμαντη αναφορά χωρικών πληροφοριών στον χώρο, ως σύνολο συντεταγμένων (x,y,z) ή/και γεωγραφικό πλάτος και μήκος και ύψος, με βάση γεωδαιτικό οριζόντιο και κατακόρυφο σύστημα αναφοράς (datum).</dct:description>
		<skos:inScheme rdf:resource="http://inspire-registry.jrc.ec.europa.eu/registers/FCD/items"/>
	</inspire:SpatialObjectType>
	<inspire:SpatialObjectType rdf:about="http://inspire-registry.jrc.ec.europa.eu/registers/FCD/items/421">
		<inspire:itemStatus>valid</inspire:itemStatus>
		<inspire:dateAccepted>2010-01-19T16:18:39.682+01:00</inspire:dateAccepted>
		<skos:prefLabel xml:lang="en">WFD River</skos:prefLabel>
		<skos:definition xml:lang="en">A body of inland water flowing for the most part on the surface of the land but which may flow underground for part of its course.</skos:definition>
		<dct:description xml:lang="en">SOURCE [2000/60/EC Art. 2(4)].
NOTE All WFD spatial object types are regarded as candidate spatial objects in Annex III theme 'Area management/restriction/regulation zones and reporting units' due to their primary function for reporting under Directive 2000/60/EC.
This type is a candidate type to be considered by the spatial data theme Area management/restriction/regulation zones and reporting units in Annex III to Directive 2007/2/EC.</dct:description>
		<skos:prefLabel xml:lang="el">SAMPLE ALTERNATIVE EXPRESSION - αναφορά</skos:prefLabel>
		<skos:definition xml:lang="el">Συστήματα συντεταγμένων</skos:definition>
		<dct:description xml:lang="el">Συστήματα για μονοσήμαντη αναφορά χωρικών πληροφοριών στον χώρο, ως σύνολο συντεταγμένων (x,y,z) ή/και γεωγραφικό πλάτος και μήκος και ύψος, με βάση γεωδαιτικό οριζόντιο και κατακόρυφο σύστημα αναφοράς (datum).</dct:description>
		<skos:inScheme rdf:resource="http://inspire-registry.jrc.ec.europa.eu/registers/FCD/items"/>
	</inspire:SpatialObjectType>
	<inspire:SpatialObjectType rdf:about="http://inspire-registry.jrc.ec.europa.eu/registers/FCD/items/422">
		<inspire:itemStatus>valid</inspire:itemStatus>
		<inspire:dateAccepted>2010-01-19T16:18:39.853+01:00</inspire:dateAccepted>
		<skos:prefLabel xml:lang="en">WFD River or Lake</skos:prefLabel>
		<skos:definition xml:lang="en">Abstract class containing common attributes for WFD River or Lake.</skos:definition>
		<dct:description xml:lang="en">NOTE All WFD spatial object types are regarded as candidate spatial objects in Annex III theme 'Area management/restriction/regulation zones and reporting units' due to their primary function for reporting under Directive 2000/60/EC.
This type is a candidate type to be considered by the spatial data theme Area management/restriction/regulation zones and reporting units in Annex III to Directive 2007/2/EC.</dct:description>
		<skos:prefLabel xml:lang="el">SAMPLE ALTERNATIVE EXPRESSION - αναφορά</skos:prefLabel>
		<skos:definition xml:lang="el">Συστήματα συντεταγμένων</skos:definition>
		<dct:description xml:lang="el">Συστήματα για μονοσήμαντη αναφορά χωρικών πληροφοριών στον χώρο, ως σύνολο συντεταγμένων (x,y,z) ή/και γεωγραφικό πλάτος και μήκος και ύψος, με βάση γεωδαιτικό οριζόντιο και κατακόρυφο σύστημα αναφοράς (datum).</dct:description>
		<skos:inScheme rdf:resource="http://inspire-registry.jrc.ec.europa.eu/registers/FCD/items"/>
	</inspire:SpatialObjectType>
	<inspire:SpatialObjectType rdf:about="http://inspire-registry.jrc.ec.europa.eu/registers/FCD/items/423">
		<inspire:itemStatus>valid</inspire:itemStatus>
		<inspire:dateAccepted>2010-01-19T16:18:40.034+01:00</inspire:dateAccepted>
		<skos:prefLabel xml:lang="en">WFD Surface Water Body</skos:prefLabel>
		<skos:definition xml:lang="en">A discrete and significant element of surface water.</skos:definition>
		<dct:description xml:lang="en">SOURCE [2000/60/EC Art. 2(10)].
Such as: a lake, a reservoir, a stream, river or canal, part of a stream, river or canal, a transitional water or a stretch of coastal water.
NOTE 1 The surface water bodies shall be identified as falling within either one of the following surface water categories - rivers, lakes, transitional waters or coastal waters - or as artificial surface water bodies or heavily modified surface water bodies. [2000/60/EC Ann. II 1.1(ii)]
NOTE 2 All WFD spatial object types are regarded as candidate spatial objects in Annex III theme 'Area management/restriction/regulation zones and reporting units' due to their primary function for reporting under Directive 2000/60/EC.
This type is a candidate type to be considered by the spatial data theme Area management/restriction/regulation zones and reporting units in Annex III to Directive 2007/2/EC.</dct:description>
		<skos:prefLabel xml:lang="el">SAMPLE ALTERNATIVE EXPRESSION - αναφορά</skos:prefLabel>
		<skos:definition xml:lang="el">Συστήματα συντεταγμένων</skos:definition>
		<dct:description xml:lang="el">Συστήματα για μονοσήμαντη αναφορά χωρικών πληροφοριών στον χώρο, ως σύνολο συντεταγμένων (x,y,z) ή/και γεωγραφικό πλάτος και μήκος και ύψος, με βάση γεωδαιτικό οριζόντιο και κατακόρυφο σύστημα αναφοράς (datum).</dct:description>
		<skos:inScheme rdf:resource="http://inspire-registry.jrc.ec.europa.eu/registers/FCD/items"/>
	</inspire:SpatialObjectType>
	<inspire:SpatialObjectType rdf:about="http://inspire-registry.jrc.ec.europa.eu/registers/FCD/items/424">
		<inspire:itemStatus>valid</inspire:itemStatus>
		<inspire:dateAccepted>2010-01-19T16:18:40.245+01:00</inspire:dateAccepted>
		<skos:prefLabel xml:lang="en">WFD Transitional Water</skos:prefLabel>
		<skos:definition xml:lang="en">Bodies of surface water in the vicinity of river mouths which are partly saline in character as a result of their proximity to coastal waters but which are substantially influenced by freshwater flows.</skos:definition>
		<dct:description xml:lang="en">SOURCE [2000/60/EC Art. 2(6)].
NOTE All WFD spatial object types are regarded as candidate spatial objects in Annex III theme 'Area management/restriction/regulation zones and reporting units' due to their primary function for reporting under Directive 2000/60/EC.
This type is a candidate type to be considered by the spatial data theme Area management/restriction/regulation zones and reporting units in Annex III to Directive 2007/2/EC.</dct:description>
		<skos:prefLabel xml:lang="el">SAMPLE ALTERNATIVE EXPRESSION - αναφορά</skos:prefLabel>
		<skos:definition xml:lang="el">Συστήματα συντεταγμένων</skos:definition>
		<dct:description xml:lang="el">Συστήματα για μονοσήμαντη αναφορά χωρικών πληροφοριών στον χώρο, ως σύνολο συντεταγμένων (x,y,z) ή/και γεωγραφικό πλάτος και μήκος και ύψος, με βάση γεωδαιτικό οριζόντιο και κατακόρυφο σύστημα αναφοράς (datum).</dct:description>
		<skos:inScheme rdf:resource="http://inspire-registry.jrc.ec.europa.eu/registers/FCD/items"/>
	</inspire:SpatialObjectType>
	<inspire:SpatialObjectType rdf:about="http://inspire-registry.jrc.ec.europa.eu/registers/FCD/items/425">
		<inspire:itemStatus>valid</inspire:itemStatus>
		<inspire:dateAccepted>2010-01-19T16:18:40.412+01:00</inspire:dateAccepted>
		<skos:prefLabel xml:lang="en">WFD Water Body</skos:prefLabel>
		<skos:definition xml:lang="en">Abstract class representing a WFD body of surface water or body of groundwater.</skos:definition>
		<dct:description xml:lang="en">NOTE All WFD spatial object types are regarded as candidate spatial objects in Annex III theme 'Area management/restriction/regulation zones and reporting units' due to their primary function for reporting under Directive 2000/60/EC.
This type is a candidate type to be considered by the spatial data theme Area management/restriction/regulation zones and reporting units in Annex III to Directive 2007/2/EC.</dct:description>
		<skos:prefLabel xml:lang="el">SAMPLE ALTERNATIVE EXPRESSION - αναφορά</skos:prefLabel>
		<skos:definition xml:lang="el">Συστήματα συντεταγμένων</skos:definition>
		<dct:description xml:lang="el">Συστήματα για μονοσήμαντη αναφορά χωρικών πληροφοριών στον χώρο, ως σύνολο συντεταγμένων (x,y,z) ή/και γεωγραφικό πλάτος και μήκος και ύψος, με βάση γεωδαιτικό οριζόντιο και κατακόρυφο σύστημα αναφοράς (datum).</dct:description>
		<skos:inScheme rdf:resource="http://inspire-registry.jrc.ec.europa.eu/registers/FCD/items"/>
	</inspire:SpatialObjectType>
</rdf:RDF>
